@prefix actionStat: <https://purl.org/ctdl/vocabs/actionStat/> .
@prefix agentSector: <https://purl.org/ctdl/vocabs/agentSector/> .
@prefix array: <https://purl.org/ctdl/vocabs/array/> .
@prefix asn: <http://purl.org/ASN/schema/core/> .
@prefix assessMethod: <https://purl.org/ctdl/vocabs/assessMethod/> .
@prefix assessUse: <https://purl.org/ctdl/vocabs/assessUse/> .
@prefix audience: <https://purl.org/ctdl/vocabs/audience/> .
@prefix audLevel: <https://purl.org/ctdl/vocabs/audLevel/> .
@prefix case: <https://purl.imsglobal.org/spec/case/> .
@prefix ceasn: <https://purl.org/ctdlasn/terms/> .
@prefix ceds: <https://ceds.ed.gov/element/> .
@prefix ceterms: <https://purl.org/ctdl/terms/> .
@prefix claimType: <https://purl.org/ctdl/vocabs/claimType/> .
@prefix collectionCategory: <https://purl.org/ctdl/vocabs/collectionCategory/> .
@prefix compare: <https://purl.org/ctdl/vocabs/compare/> .
@prefix costType: <https://purl.org/ctdl/vocabs/costType/> .
@prefix credentialStat: <https://purl.org/ctdl/vocabs/credentialStat/> .
@prefix creditUnit: <https://purl.org/ctdl/vocabs/creditUnit/> .
@prefix cs: <http://vocab.org/changeset/schema#> .
@prefix dc: <http://purl.org/dc/elements/1.1/> .
@prefix dct: <http://purl.org/dc/terms/> .
@prefix deliveryType: <https://purl.org/ctdl/vocabs/deliveryType/> .
@prefix financialAid: <https://purl.org/ctdl/vocabs/financialAid/> .
@prefix foaf: <http://xmlns.com/foaf/0.1/> .
@prefix gemq: <http://purl.org/gem/qualifiers/> .
@prefix inputType: <https://purl.org/ctdl/vocabs/inputType/> .
@prefix learnMethod: <https://purl.org/ctdl/vocabs/learnMethod/> .
@prefix lifeCycle: <https://purl.org/ctdl/vocabs/lifeCycle/> .
@prefix logic: <https://purl.org/ctdl/vocabs/logic/> .
@prefix lrmi: <http://purl.org/dcx/lrmi-terms/> .
@prefix meta: <http://credreg.net/meta/terms/> .
@prefix obi: <https://w3id.org/openbadges#> .
@prefix odrl2: <https://www.w3.org/ns/odrl/2/> .
@prefix orgType: <https://purl.org/ctdl/vocabs/orgType/> .
@prefix owl: <http://www.w3.org/2002/07/owl#> .
@prefix qdata: <https://credreg.net/qdata/terms/> .
@prefix rdf: <http://www.w3.org/1999/02/22-rdf-syntax-ns#> .
@prefix rdfs: <http://www.w3.org/2000/01/rdf-schema#> .
@prefix residency: <https://purl.org/ctdl/vocabs/residency/> .
@prefix scheduleFrequency: <https://purl.org/ctdl/vocabs/scheduleFrequency/> .
@prefix scheduleTiming: <https://purl.org/ctdl/vocabs/scheduleTiming/> .
@prefix schema: <https://schema.org/> .
@prefix score: <https://purl.org/ctdl/vocabs/score/> .
@prefix serviceType: <https://purl.org/ctdl/vocabs/serviceType/> .
@prefix skos: <http://www.w3.org/2004/02/skos/core#> .
@prefix vann: <http://purl.org/vocab/vann/> .
@prefix vs: <https://www.w3.org/2003/06/sw-vocab-status/ns#> .
@prefix xsd: <http://www.w3.org/2001/XMLSchema#> .

#====================
# CLASSES
#====================
ceterms:AccreditAction a rdfs:Class ;
	rdfs:label "Accredit Action"@en-US ;
	rdfs:comment "Action by an independent, neutral, and authoritative agent that certifies an entity as meeting a prescribed set of standards."@en-US ;
	dct:description "Since an instance of ceterms:CredentialingAction is a claim that a certain agent has taken the action being described, creation of such a ceterms:CredentialingAction should be reserved to the agent of that action."@en-US ;
	vs:term_status vs:stable ;
	meta:changeHistory <http://credreg.net/ctdl/termhistory/ceterms/AccreditAction/json> ;
	rdfs:subClassOf ceterms:CredentialingAction ;
	meta:domainFor ceterms:actingAgent, ceterms:actionStatusType, ceterms:description, ceterms:endDate, ceterms:evidenceOfAction, ceterms:instrument, ceterms:object, ceterms:participant, ceterms:resultingAward, ceterms:startDate .

ceterms:AdvancedStandingAction a rdfs:Class ;
	rdfs:label "Advanced Standing Action"@en-US ;
	rdfs:comment "Claim by an agent asserting that the object credential of the action provides advanced standing for a credential under the asserting agent's authority."@en-US ;
	dct:description "Since an instance of ceterms:CredentialingAction is a claim that a certain agent has taken the action being described, creation of such a ceterms:CredentialingAction should be reserved to the agent of that action."@en-US ;
	vs:term_status vs:stable ;
	meta:changeHistory <http://credreg.net/ctdl/termhistory/ceterms/AdvancedStandingAction/json> ;
	rdfs:subClassOf ceterms:CredentialingAction ;
	meta:domainFor ceterms:actingAgent, ceterms:actionStatusType, ceterms:description, ceterms:endDate, ceterms:evidenceOfAction, ceterms:instrument, ceterms:object, ceterms:participant, ceterms:startDate .

ceterms:Agent a rdfs:Class ;
	rdfs:label "Agent"@en-US ;
	rdfs:comment "Organization or person that acts or has the power to act."@en-US ;
	dct:description "Broad type that includes both organizations and people who play roles in the lifecycle of a resource."@en-US ;
	vs:term_status vs:stable ;
	meta:changeHistory <http://credreg.net/ctdl/termhistory/ceterms/Agent/json> ;
	owl:equivalentClass dct:Agent .

ceterms:AggregateDataProfile a rdfs:Class ;
	rdfs:label "Aggregate Data Profile"@en-US ;
	rdfs:comment "Resource containing summary statistical data."@en-US ;
	vann:usageNote "To express more complex data, use qdata:DataSetProfile."@en-US ;
	vs:term_status vs:stable ;
	meta:changeHistory <http://credreg.net/ctdl/termhistory/ceterms/AggregateDataProfile/json> ;
	meta:domainFor ceterms:currency, ceterms:dateEffective, ceterms:demographicInformation, ceterms:description, ceterms:expirationDate, ceterms:highEarnings, ceterms:jobsObtained, ceterms:jurisdiction, ceterms:lowEarnings, ceterms:medianEarnings, ceterms:name, ceterms:numberAwarded, ceterms:postReceiptMonths, ceterms:source, qdata:relevantDataSet .

ceterms:AlignmentMap a rdfs:Class ;
	rdfs:label "Alignment Map"@en-US ;
	rdfs:comment "An entity comprised of a set of alignment or mapping assertions between two existing entities such as mapping a certificate providing advanced standing to a degree."@en-US ;
	dct:description "Alignment maps provide the means for parties to assert sets of alignments between already existing entities created by themselves or other parties--e.g., a 3rd party mapping of a learning resource owned by one party to a credential owned by another; or, mapping a military occupational experience or Military Occupational Specialty (MOS code) as advanced standing to a course or credential."@en-US ;
	vs:term_status vs:stable ;
	meta:changeHistory <http://credreg.net/ctdl/termhistory/ceterms/AlignmentMap/json> ;
	meta:domainFor ceterms:hasStatement .

ceterms:ApprenticeshipCertificate a rdfs:Class ;
	rdfs:label "Apprenticeship Certificate"@en-US ;
	rdfs:comment "Credential earned through work-based learning and earn-and-learn models that meet standards and are applicable to industry trades and professions."@en-US ;
	vs:term_status vs:stable ;
	meta:changeHistory <http://credreg.net/ctdl/termhistory/ceterms/ApprenticeshipCertificate/json> ;
	rdfs:subClassOf ceterms:Certificate ;
	meta:domainFor ceterms:accreditedBy, ceterms:accreditedIn, ceterms:administrationProcess, ceterms:advancedStandingFrom, ceterms:aggregateData, ceterms:alternateName, ceterms:appealProcess, ceterms:approvedBy, ceterms:approvedIn, ceterms:assessmentDeliveryType, ceterms:audienceLevelType, ceterms:audienceType, ceterms:availabilityListing, ceterms:availableAt, ceterms:availableOnlineAt, ceterms:broadAlignment, ceterms:commonConditions, ceterms:commonCosts, ceterms:complaintProcess, ceterms:copyrightHolder, ceterms:corequisite, ceterms:credentialId, ceterms:credentialStatusType, ceterms:ctid, ceterms:dateEffective, ceterms:description, ceterms:developmentProcess, ceterms:earnings, ceterms:employmentOutcome, ceterms:estimatedCost, ceterms:estimatedDuration, ceterms:exactAlignment, ceterms:expirationDate, ceterms:financialAssistance, ceterms:hasPart, ceterms:hasProxy, ceterms:holders, ceterms:identifier, ceterms:image, ceterms:industryType, ceterms:inLanguage, ceterms:instructionalProgramType, ceterms:isAdvancedStandingFor, ceterms:isicV4, ceterms:isPartOf, ceterms:isPreparationFor, ceterms:isRecommendedFor, ceterms:isRequiredFor, ceterms:jurisdiction, ceterms:keyword, ceterms:latestVersion, ceterms:learningDeliveryType, ceterms:maintenanceProcess, ceterms:majorAlignment, ceterms:minorAlignment, ceterms:naics, ceterms:name, ceterms:narrowAlignment, ceterms:nextVersion, ceterms:occupationType, ceterms:offeredBy, ceterms:offeredIn, ceterms:ownedBy, ceterms:preparationFrom, ceterms:previousVersion, ceterms:processStandards, ceterms:processStandardsDescription, ceterms:recognizedBy, ceterms:recognizedIn, ceterms:recommends, ceterms:region, ceterms:regulatedBy, ceterms:regulatedIn, ceterms:relatedAction, ceterms:renewal, ceterms:renewalFrequency, ceterms:renewedBy, ceterms:renewedIn, ceterms:requires, ceterms:reviewProcess, ceterms:revocation, ceterms:revocationProcess, ceterms:revokedBy, ceterms:revokedIn, ceterms:sameAs, ceterms:subject, ceterms:subjectWebpage, ceterms:supersededBy, ceterms:supersedes, ceterms:targetPathway, ceterms:versionIdentifier .

ceterms:ApproveAction a rdfs:Class ;
	rdfs:label "Approve Action"@en-US ;
	rdfs:comment "Action by an independent, neutral, and authoritative agent that pronounces a favorable judgment of a credential."@en-US ;
	dct:description "Since an instance of ceterms:CredentialingAction is a claim that a certain agent has taken the action being described, creation of such a ceterms:CredentialingAction should be reserved to the agent of that action."@en-US ;
	vs:term_status vs:unstable ;
	meta:changeHistory <http://credreg.net/ctdl/termhistory/ceterms/ApproveAction/json> ;
	rdfs:subClassOf ceterms:CredentialingAction ;
	meta:domainFor ceterms:actingAgent, ceterms:actionStatusType, ceterms:description, ceterms:endDate, ceterms:evidenceOfAction, ceterms:instrument, ceterms:object, ceterms:participant, ceterms:startDate .

ceterms:Assessment a rdfs:Class ;
	rdfs:label "Assessment"@en-US ;
	rdfs:comment "Direct, indirect, formative, and summative evaluation or estimation of the nature, ability, or quality of an entity, performance, or outcome of an action."@en-US ;
	vs:term_status vs:stable ;
	meta:changeHistory <http://credreg.net/ctdl/termhistory/ceterms/Assessment/json> .

ceterms:AssessmentComponent a rdfs:Class ;
	rdfs:label "Assessment Component"@en-US ;
	rdfs:comment "Resource that identifies a direct, indirect, formative, and summative evaluation or estimation of the nature, ability, or quality of a resource, performance, or outcome of an action."@en-US ;
	dct:description "Instances act as proxies or stand-ins for other resources in the context of a particular pathway so that relationships between them as components of that pathway can be stated without implying that the those relationships are true of the resources in other contexts."@en-US ;
	vs:term_status vs:stable ;
	meta:changeHistory <http://credreg.net/ctdl/termhistory/ceterms/AssessmentComponent/json> ;
	rdfs:subClassOf ceterms:PathwayComponent ;
	meta:domainFor ceasn:hasChild, ceasn:isChildOf, ceterms:componentDesignation, ceterms:ctid, ceterms:description, ceterms:hasCondition, ceterms:identifier, ceterms:isDestinationComponentOf, ceterms:isPartOf, ceterms:name, ceterms:pointValue, ceterms:precededBy, ceterms:precedes, ceterms:proxyFor, ceterms:sourceData, ceterms:subjectWebpage .

ceterms:AssessmentProfile a rdfs:Class ;
	rdfs:label "Assessment Profile"@en-US ;
	rdfs:comment "Entity that describes the key characteristics of an assessment for a credential."@en-US ;
	dct:description "Characteristics described include, but are not limited to, processes for assessment development, maintenance, selection and evaluation as well as assessment examples."@en-US ;
	vann:usageNote "The ceterms:AssessmentProfile is intended for use in describing stand-alone assessments. Assessments that are a part of a learning opportunity associated with a credential should be described as part the ceterms:LearningOpportunityProfile for that learning opportunity."@en-US ;
	vs:term_status vs:stable ;
	meta:changeHistory <http://credreg.net/ctdl/termhistory/ceterms/AssessmentProfile/json> ;
	rdfs:subClassOf schema:CreativeWork ;
	meta:domainFor ceterms:accreditedBy, ceterms:accreditedIn, ceterms:administrationProcess, ceterms:advancedStandingFrom, ceterms:approvedBy, ceterms:approvedIn, ceterms:assesses, ceterms:assessmentExample, ceterms:assessmentExampleDescription, ceterms:assessmentMethodDescription, ceterms:assessmentMethodType, ceterms:assessmentOutput, ceterms:assessmentUseType, ceterms:audienceLevelType, ceterms:audienceType, ceterms:availabilityListing, ceterms:availableAt, ceterms:availableOnlineAt, ceterms:commonConditions, ceterms:commonCosts, ceterms:corequisite, ceterms:creditUnitTypeDescription, ceterms:creditValue, ceterms:ctid, ceterms:dateEffective, ceterms:deliveryType, ceterms:deliveryTypeDescription, ceterms:description, ceterms:developmentProcess, ceterms:entryCondition, ceterms:estimatedCost, ceterms:estimatedDuration, ceterms:expirationDate, ceterms:externalResearch, ceterms:financialAssistance, ceterms:hasGroupEvaluation, ceterms:hasGroupParticipation, ceterms:hasOffering, ceterms:hasProxy, ceterms:identifier, ceterms:industryType, ceterms:inLanguage, ceterms:instructionalProgramType, ceterms:isAdvancedStandingFor, ceterms:isNonCredit, ceterms:isPreparationFor, ceterms:isProctored, ceterms:isRecommendedFor, ceterms:isRequiredFor, ceterms:jurisdiction, ceterms:keyword, ceterms:learningMethodDescription, ceterms:lifeCycleStatusType, ceterms:maintenanceProcess, ceterms:name, ceterms:occupationType, ceterms:offeredBy, ceterms:offeredIn, ceterms:offerFrequencyType, ceterms:ownedBy, ceterms:preparationFrom, ceterms:processStandards, ceterms:processStandardsDescription, ceterms:recognizedBy, ceterms:recognizedIn, ceterms:recommends, ceterms:region, ceterms:regulatedBy, ceterms:regulatedIn, ceterms:requires, ceterms:sameAs, ceterms:scheduleFrequencyType, ceterms:scheduleTimingType, ceterms:scoringMethodDescription, ceterms:scoringMethodExample, ceterms:scoringMethodExampleDescription, ceterms:scoringMethodType, ceterms:subject, ceterms:subjectWebpage, ceterms:supersededBy, ceterms:supersedes, ceterms:targetAssessment, ceterms:targetLearningResource, ceterms:targetPathway, ceterms:versionIdentifier .

ceterms:AssociateDegree a rdfs:Class ;
	rdfs:label "Associate Degree"@en-US ;
	rdfs:comment "College/university award for students typically completing the first one to two years of post secondary school education."@en-US ;
	dct:description "Equivalent to an award at UNESCO ISCED 2011, Level 5."@en-US ;
	vs:term_status vs:stable ;
	meta:changeHistory <http://credreg.net/ctdl/termhistory/ceterms/AssociateDegree/json> ;
	rdfs:subClassOf ceterms:Degree ;
	meta:domainFor ceterms:accreditedBy, ceterms:accreditedIn, ceterms:administrationProcess, ceterms:advancedStandingFrom, ceterms:aggregateData, ceterms:alternateName, ceterms:appealProcess, ceterms:approvedBy, ceterms:approvedIn, ceterms:assessmentDeliveryType, ceterms:audienceLevelType, ceterms:audienceType, ceterms:availabilityListing, ceterms:availableAt, ceterms:availableOnlineAt, ceterms:broadAlignment, ceterms:commonConditions, ceterms:commonCosts, ceterms:complaintProcess, ceterms:copyrightHolder, ceterms:corequisite, ceterms:credentialId, ceterms:credentialStatusType, ceterms:ctid, ceterms:dateEffective, ceterms:degreeConcentration, ceterms:degreeMajor, ceterms:degreeMinor, ceterms:description, ceterms:developmentProcess, ceterms:earnings, ceterms:employmentOutcome, ceterms:estimatedCost, ceterms:estimatedDuration, ceterms:exactAlignment, ceterms:expirationDate, ceterms:financialAssistance, ceterms:hasPart, ceterms:hasProxy, ceterms:holders, ceterms:identifier, ceterms:image, ceterms:industryType, ceterms:inLanguage, ceterms:instructionalProgramType, ceterms:isAdvancedStandingFor, ceterms:isicV4, ceterms:isPartOf, ceterms:isPreparationFor, ceterms:isRecommendedFor, ceterms:isRequiredFor, ceterms:jurisdiction, ceterms:keyword, ceterms:latestVersion, ceterms:learningDeliveryType, ceterms:maintenanceProcess, ceterms:majorAlignment, ceterms:minorAlignment, ceterms:naics, ceterms:name, ceterms:narrowAlignment, ceterms:nextVersion, ceterms:occupationType, ceterms:offeredBy, ceterms:offeredIn, ceterms:ownedBy, ceterms:preparationFrom, ceterms:previousVersion, ceterms:processStandards, ceterms:processStandardsDescription, ceterms:recognizedBy, ceterms:recognizedIn, ceterms:recommends, ceterms:region, ceterms:regulatedBy, ceterms:regulatedIn, ceterms:relatedAction, ceterms:renewal, ceterms:renewalFrequency, ceterms:renewedBy, ceterms:renewedIn, ceterms:requires, ceterms:reviewProcess, ceterms:revocation, ceterms:revocationProcess, ceterms:revokedBy, ceterms:revokedIn, ceterms:sameAs, ceterms:subject, ceterms:subjectWebpage, ceterms:supersededBy, ceterms:supersedes, ceterms:targetPathway, ceterms:versionIdentifier .

ceterms:BachelorDegree a rdfs:Class ;
	rdfs:label "Bachelor's Degree"@en-US ;
	rdfs:comment "College/university award for students typically completing three to five years of education where course work and activities advance skills beyond those of the first one to two years of college/university study."@en-US ;
	dct:description "Equivalent to an award at UNESCO ISCED 2011, Level 6."@en-US ;
	vann:usageNote "Use for 5-year cooperative (work-study) programs. A cooperative plan provides for alternate class attendance and employment in business, industry, or governmentÍ¾ thus, it allows students to combine actual work experience with their college studies. Also includes bachelor's degrees in which the normal 4 years of work are completed in 3 years."@en-US ;
	vs:term_status vs:stable ;
	meta:changeHistory <http://credreg.net/ctdl/termhistory/ceterms/BachelorDegree/json> ;
	rdfs:subClassOf ceterms:Degree ;
	meta:domainFor ceterms:accreditedBy, ceterms:accreditedIn, ceterms:administrationProcess, ceterms:advancedStandingFrom, ceterms:aggregateData, ceterms:alternateName, ceterms:appealProcess, ceterms:approvedBy, ceterms:approvedIn, ceterms:assessmentDeliveryType, ceterms:audienceLevelType, ceterms:audienceType, ceterms:availabilityListing, ceterms:availableAt, ceterms:availableOnlineAt, ceterms:broadAlignment, ceterms:commonConditions, ceterms:commonCosts, ceterms:complaintProcess, ceterms:copyrightHolder, ceterms:corequisite, ceterms:credentialId, ceterms:credentialStatusType, ceterms:ctid, ceterms:dateEffective, ceterms:degreeConcentration, ceterms:degreeMajor, ceterms:degreeMinor, ceterms:description, ceterms:developmentProcess, ceterms:earnings, ceterms:employmentOutcome, ceterms:estimatedCost, ceterms:estimatedDuration, ceterms:exactAlignment, ceterms:expirationDate, ceterms:financialAssistance, ceterms:hasPart, ceterms:hasProxy, ceterms:holders, ceterms:identifier, ceterms:image, ceterms:industryType, ceterms:inLanguage, ceterms:instructionalProgramType, ceterms:isAdvancedStandingFor, ceterms:isicV4, ceterms:isPartOf, ceterms:isPreparationFor, ceterms:isRecommendedFor, ceterms:isRequiredFor, ceterms:jurisdiction, ceterms:keyword, ceterms:latestVersion, ceterms:learningDeliveryType, ceterms:maintenanceProcess, ceterms:majorAlignment, ceterms:minorAlignment, ceterms:naics, ceterms:name, ceterms:narrowAlignment, ceterms:nextVersion, ceterms:occupationType, ceterms:offeredBy, ceterms:offeredIn, ceterms:ownedBy, ceterms:preparationFrom, ceterms:previousVersion, ceterms:processStandards, ceterms:processStandardsDescription, ceterms:recognizedBy, ceterms:recognizedIn, ceterms:recommends, ceterms:region, ceterms:regulatedBy, ceterms:regulatedIn, ceterms:relatedAction, ceterms:renewal, ceterms:renewalFrequency, ceterms:renewedBy, ceterms:renewedIn, ceterms:requires, ceterms:reviewProcess, ceterms:revocation, ceterms:revocationProcess, ceterms:revokedBy, ceterms:revokedIn, ceterms:sameAs, ceterms:subject, ceterms:subjectWebpage, ceterms:supersededBy, ceterms:supersedes, ceterms:targetPathway, ceterms:versionIdentifier .

ceterms:Badge a rdfs:Class ;
	rdfs:label "Badge"@en-US ;
	rdfs:comment "Recognition designed to be displayed as a marker of accomplishment, activity, achievement, skill, interest, association, or identity."@en-US ;
	vs:term_status vs:stable ;
	meta:changeHistory <http://credreg.net/ctdl/termhistory/ceterms/Badge/json> ;
	rdfs:subClassOf ceterms:Credential ;
	meta:domainFor ceterms:accreditedBy, ceterms:accreditedIn, ceterms:administrationProcess, ceterms:advancedStandingFrom, ceterms:aggregateData, ceterms:alternateName, ceterms:appealProcess, ceterms:approvedBy, ceterms:approvedIn, ceterms:assessmentDeliveryType, ceterms:audienceLevelType, ceterms:audienceType, ceterms:availabilityListing, ceterms:availableAt, ceterms:availableOnlineAt, ceterms:broadAlignment, ceterms:commonConditions, ceterms:commonCosts, ceterms:complaintProcess, ceterms:copyrightHolder, ceterms:corequisite, ceterms:credentialId, ceterms:credentialStatusType, ceterms:ctid, ceterms:dateEffective, ceterms:description, ceterms:developmentProcess, ceterms:earnings, ceterms:employmentOutcome, ceterms:estimatedCost, ceterms:estimatedDuration, ceterms:exactAlignment, ceterms:expirationDate, ceterms:financialAssistance, ceterms:hasPart, ceterms:hasProxy, ceterms:holders, ceterms:identifier, ceterms:image, ceterms:industryType, ceterms:inLanguage, ceterms:instructionalProgramType, ceterms:isAdvancedStandingFor, ceterms:isicV4, ceterms:isPartOf, ceterms:isPreparationFor, ceterms:isRecommendedFor, ceterms:isRequiredFor, ceterms:jurisdiction, ceterms:keyword, ceterms:latestVersion, ceterms:learningDeliveryType, ceterms:maintenanceProcess, ceterms:majorAlignment, ceterms:minorAlignment, ceterms:naics, ceterms:name, ceterms:narrowAlignment, ceterms:nextVersion, ceterms:occupationType, ceterms:offeredBy, ceterms:offeredIn, ceterms:ownedBy, ceterms:preparationFrom, ceterms:previousVersion, ceterms:processStandards, ceterms:processStandardsDescription, ceterms:recognizedBy, ceterms:recognizedIn, ceterms:recommends, ceterms:region, ceterms:regulatedBy, ceterms:regulatedIn, ceterms:relatedAction, ceterms:renewal, ceterms:renewalFrequency, ceterms:renewedBy, ceterms:renewedIn, ceterms:requires, ceterms:reviewProcess, ceterms:revocation, ceterms:revocationProcess, ceterms:revokedBy, ceterms:revokedIn, ceterms:sameAs, ceterms:subject, ceterms:subjectWebpage, ceterms:supersededBy, ceterms:supersedes, ceterms:targetPathway, ceterms:versionIdentifier .

ceterms:BasicComponent a rdfs:Class ;
	rdfs:label "Basic Component"@en-US ;
	rdfs:comment "Resource that identifies a resource not otherwise covered by the enumerated PathwayComponent subclasses."@en-US ;
	dct:description "Instances act as proxies or stand-ins for other resources in the context of a particular pathway so that relationships between them as components of that pathway can be stated without implying that the those relationships are true of the resources in other contexts."@en-US ;
	vs:term_status vs:stable ;
	meta:changeHistory <http://credreg.net/ctdl/termhistory/ceterms/BasicComponent/json> ;
	rdfs:subClassOf ceterms:PathwayComponent ;
	meta:domainFor ceasn:hasChild, ceasn:isChildOf, ceterms:componentCategory, ceterms:componentDesignation, ceterms:ctid, ceterms:description, ceterms:hasCondition, ceterms:identifier, ceterms:isDestinationComponentOf, ceterms:isPartOf, ceterms:name, ceterms:pointValue, ceterms:precededBy, ceterms:precedes, ceterms:proxyFor, ceterms:sourceData, ceterms:subjectWebpage .

ceterms:Certificate a rdfs:Class ;
	rdfs:label "Certificate"@en-US ;
	rdfs:comment "Credential that designates requisite knowledge and skills of an occupation, profession, or academic program."@en-US ;
	vs:term_status vs:stable ;
	meta:changeHistory <http://credreg.net/ctdl/termhistory/ceterms/Certificate/json> ;
	rdfs:subClassOf ceterms:Credential ;
	meta:domainFor ceterms:accreditedBy, ceterms:accreditedIn, ceterms:administrationProcess, ceterms:advancedStandingFrom, ceterms:aggregateData, ceterms:alternateName, ceterms:appealProcess, ceterms:approvedBy, ceterms:approvedIn, ceterms:assessmentDeliveryType, ceterms:audienceLevelType, ceterms:audienceType, ceterms:availabilityListing, ceterms:availableAt, ceterms:availableOnlineAt, ceterms:broadAlignment, ceterms:commonConditions, ceterms:commonCosts, ceterms:complaintProcess, ceterms:copyrightHolder, ceterms:corequisite, ceterms:credentialId, ceterms:credentialStatusType, ceterms:ctid, ceterms:dateEffective, ceterms:description, ceterms:developmentProcess, ceterms:earnings, ceterms:employmentOutcome, ceterms:estimatedCost, ceterms:estimatedDuration, ceterms:exactAlignment, ceterms:expirationDate, ceterms:financialAssistance, ceterms:hasPart, ceterms:hasProxy, ceterms:holders, ceterms:identifier, ceterms:image, ceterms:industryType, ceterms:inLanguage, ceterms:instructionalProgramType, ceterms:isAdvancedStandingFor, ceterms:isicV4, ceterms:isPartOf, ceterms:isPreparationFor, ceterms:isRecommendedFor, ceterms:isRequiredFor, ceterms:jurisdiction, ceterms:keyword, ceterms:latestVersion, ceterms:learningDeliveryType, ceterms:maintenanceProcess, ceterms:majorAlignment, ceterms:minorAlignment, ceterms:naics, ceterms:name, ceterms:narrowAlignment, ceterms:nextVersion, ceterms:occupationType, ceterms:offeredBy, ceterms:offeredIn, ceterms:ownedBy, ceterms:preparationFrom, ceterms:previousVersion, ceterms:processStandards, ceterms:processStandardsDescription, ceterms:recognizedBy, ceterms:recognizedIn, ceterms:recommends, ceterms:region, ceterms:regulatedBy, ceterms:regulatedIn, ceterms:relatedAction, ceterms:renewal, ceterms:renewalFrequency, ceterms:renewedBy, ceterms:renewedIn, ceterms:requires, ceterms:reviewProcess, ceterms:revocation, ceterms:revocationProcess, ceterms:revokedBy, ceterms:revokedIn, ceterms:sameAs, ceterms:subject, ceterms:subjectWebpage, ceterms:supersededBy, ceterms:supersedes, ceterms:targetPathway, ceterms:versionIdentifier .

ceterms:CertificateOfCompletion a rdfs:Class ;
	rdfs:label "Certificate of Completion"@en-US ;
	rdfs:comment "Credential that acknowledges completion of an assignment, training or other activity."@en-US ;
	dct:description "A record of the activity may or may not exist, and the credential may or may not be designed as preparation for another resource such as a credential, assessment, or learning opportunity."@en-US ;
	vs:term_status vs:stable ;
	meta:changeHistory <http://credreg.net/ctdl/termhistory/ceterms/CertificateOfCompletion/json> ;
	rdfs:subClassOf ceterms:Credential ;
	meta:domainFor ceterms:accreditedBy, ceterms:accreditedIn, ceterms:administrationProcess, ceterms:advancedStandingFrom, ceterms:aggregateData, ceterms:alternateName, ceterms:appealProcess, ceterms:approvedBy, ceterms:approvedIn, ceterms:assessmentDeliveryType, ceterms:audienceLevelType, ceterms:audienceType, ceterms:availabilityListing, ceterms:availableAt, ceterms:availableOnlineAt, ceterms:broadAlignment, ceterms:commonConditions, ceterms:commonCosts, ceterms:complaintProcess, ceterms:copyrightHolder, ceterms:corequisite, ceterms:credentialId, ceterms:credentialStatusType, ceterms:ctid, ceterms:dateEffective, ceterms:description, ceterms:developmentProcess, ceterms:earnings, ceterms:employmentOutcome, ceterms:estimatedCost, ceterms:estimatedDuration, ceterms:exactAlignment, ceterms:expirationDate, ceterms:financialAssistance, ceterms:hasPart, ceterms:hasProxy, ceterms:holders, ceterms:identifier, ceterms:image, ceterms:industryType, ceterms:inLanguage, ceterms:instructionalProgramType, ceterms:isAdvancedStandingFor, ceterms:isicV4, ceterms:isPartOf, ceterms:isPreparationFor, ceterms:isRecommendedFor, ceterms:isRequiredFor, ceterms:jurisdiction, ceterms:keyword, ceterms:latestVersion, ceterms:learningDeliveryType, ceterms:maintenanceProcess, ceterms:majorAlignment, ceterms:minorAlignment, ceterms:naics, ceterms:name, ceterms:narrowAlignment, ceterms:nextVersion, ceterms:occupationType, ceterms:offeredBy, ceterms:offeredIn, ceterms:ownedBy, ceterms:preparationFrom, ceterms:previousVersion, ceterms:processStandards, ceterms:processStandardsDescription, ceterms:recognizedBy, ceterms:recognizedIn, ceterms:recommends, ceterms:region, ceterms:regulatedBy, ceterms:regulatedIn, ceterms:relatedAction, ceterms:renewal, ceterms:renewalFrequency, ceterms:renewedBy, ceterms:renewedIn, ceterms:requires, ceterms:reviewProcess, ceterms:revocation, ceterms:revocationProcess, ceterms:revokedBy, ceterms:revokedIn, ceterms:sameAs, ceterms:subject, ceterms:subjectWebpage, ceterms:supersededBy, ceterms:supersedes, ceterms:targetPathway, ceterms:versionIdentifier .

ceterms:Certification a rdfs:Class ;
	rdfs:label "Certification"@en-US ;
	rdfs:comment "Time-limited, revocable, renewable credential awarded by an authoritative body for demonstrating the knowledge, skills, and abilities to perform specific tasks or an occupation."@en-US ;
	dct:description "Certifications can typically be revoked if not renewed, for a violation of a code of ethics (if applicable) or proven incompetence after due process. Description of revocation criteria for a specific Certification should be defined using Revocation Profile."@en-US ;
	vs:term_status vs:stable ;
	meta:changeHistory <http://credreg.net/ctdl/termhistory/ceterms/Certification/json> ;
	rdfs:subClassOf ceterms:Credential, ceterms:Credential ;
	meta:domainFor ceterms:accreditedBy, ceterms:accreditedIn, ceterms:administrationProcess, ceterms:advancedStandingFrom, ceterms:aggregateData, ceterms:alternateName, ceterms:appealProcess, ceterms:approvedBy, ceterms:approvedIn, ceterms:assessmentDeliveryType, ceterms:audienceLevelType, ceterms:audienceType, ceterms:availabilityListing, ceterms:availableAt, ceterms:availableOnlineAt, ceterms:broadAlignment, ceterms:commonConditions, ceterms:commonCosts, ceterms:complaintProcess, ceterms:copyrightHolder, ceterms:corequisite, ceterms:credentialId, ceterms:credentialStatusType, ceterms:ctid, ceterms:dateEffective, ceterms:description, ceterms:developmentProcess, ceterms:earnings, ceterms:employmentOutcome, ceterms:estimatedCost, ceterms:estimatedDuration, ceterms:exactAlignment, ceterms:expirationDate, ceterms:financialAssistance, ceterms:hasPart, ceterms:hasProxy, ceterms:holders, ceterms:identifier, ceterms:image, ceterms:industryType, ceterms:inLanguage, ceterms:instructionalProgramType, ceterms:isAdvancedStandingFor, ceterms:isicV4, ceterms:isPartOf, ceterms:isPreparationFor, ceterms:isRecommendedFor, ceterms:isRequiredFor, ceterms:jurisdiction, ceterms:keyword, ceterms:latestVersion, ceterms:learningDeliveryType, ceterms:maintenanceProcess, ceterms:majorAlignment, ceterms:minorAlignment, ceterms:naics, ceterms:name, ceterms:narrowAlignment, ceterms:nextVersion, ceterms:occupationType, ceterms:offeredBy, ceterms:offeredIn, ceterms:ownedBy, ceterms:preparationFrom, ceterms:previousVersion, ceterms:processStandards, ceterms:processStandardsDescription, ceterms:recognizedBy, ceterms:recognizedIn, ceterms:recommends, ceterms:region, ceterms:regulatedBy, ceterms:regulatedIn, ceterms:relatedAction, ceterms:renewal, ceterms:renewalFrequency, ceterms:renewedBy, ceterms:renewedIn, ceterms:requires, ceterms:reviewProcess, ceterms:revocation, ceterms:revocationProcess, ceterms:revokedBy, ceterms:revokedIn, ceterms:sameAs, ceterms:subject, ceterms:subjectWebpage, ceterms:supersededBy, ceterms:supersedes, ceterms:targetPathway, ceterms:versionIdentifier .

ceterms:CocurricularComponent a rdfs:Class ;
	rdfs:label "Cocurricular Component"@en-US ;
	rdfs:comment "Resource that identifies an activity, program, or informal learning experience such as a civic or service activity that supplements and complements the curriculum."@en-US ;
	dct:description "Instances act as proxies or stand-ins for other resources in the context of a particular pathway so that relationships between them as components of that pathway can be stated without implying that the those relationships are true of the resources in other contexts."@en-US ;
	vs:term_status vs:stable ;
	meta:changeHistory <http://credreg.net/ctdl/termhistory/ceterms/CocurricularComponent/json> ;
	rdfs:subClassOf ceterms:PathwayComponent ;
	meta:domainFor ceasn:hasChild, ceasn:isChildOf, ceterms:componentCategory, ceterms:componentDesignation, ceterms:ctid, ceterms:description, ceterms:hasCondition, ceterms:identifier, ceterms:isDestinationComponentOf, ceterms:isPartOf, ceterms:name, ceterms:pointValue, ceterms:precededBy, ceterms:precedes, ceterms:proxyFor, ceterms:sourceData, ceterms:subjectWebpage .

ceterms:Collection a rdfs:Class ;
	rdfs:label "Collection"@en-US ;
	rdfs:comment "Aggregation of related resources."@en-US ;
	vs:term_status vs:unstable ;
	meta:changeHistory <http://credreg.net/ctdl/termhistory/ceterms/Collection/json> ;
	meta:domainFor ceterms:classification, ceterms:codedNotation, ceterms:collectionType, ceterms:ctid, ceterms:dateEffective, ceterms:description, ceterms:expirationDate, ceterms:hasMember, ceterms:industryType, ceterms:inLanguage, ceterms:instructionalProgramType, ceterms:keyword, ceterms:lifeCycleStatusType, ceterms:membershipCondition, ceterms:name, ceterms:occupationType, ceterms:ownedBy, ceterms:subject, ceterms:subjectWebpage .

ceterms:CollectionMember a rdfs:Class ;
	rdfs:label "Collection Member"@en-US ;
	rdfs:comment "Provides information about the membership of a resource in a Collection."@en-US ;
	dct:description "Instances act as proxies or stand-ins for other resources in the context of a particular collection so that the relationships between them and the collection can be stated without implying that those relationships are true in other contexts."@en-US ;
	vann:usageNote "The data recorded for a Collection Member should refer to the membership of the resource in a Collection."@en-US ;
	vs:term_status vs:unstable ;
	meta:changeHistory <http://credreg.net/ctdl/termhistory/ceterms/CollectionMember/json> ;
	meta:domainFor ceterms:description, ceterms:endDate, ceterms:name, ceterms:proxyFor, ceterms:startDate .

ceterms:CompetencyComponent a rdfs:Class ;
	rdfs:label "Competency Component"@en-US ;
	rdfs:comment "Resource that identifies a measurable or observable knowledge, skill, or ability necessary to successful performance of a person in a given context."@en-US ;
	dct:description "Competency is broadly defined to include assertions of academic, professional, occupational, vocational and life goals, outcomes, and standards, however labeled. Instances act as proxies or stand-ins for other resources in the context of a particular pathway so that relationships between them as components of that pathway can be stated without implying that the those relationships are true of the resources in other contexts."@en-US ;
	vs:term_status vs:stable ;
	meta:changeHistory <http://credreg.net/ctdl/termhistory/ceterms/CompetencyComponent/json> ;
	rdfs:subClassOf ceterms:PathwayComponent ;
	meta:domainFor ceasn:hasChild, ceasn:isChildOf, ceterms:componentDesignation, ceterms:ctid, ceterms:description, ceterms:hasCondition, ceterms:identifier, ceterms:isDestinationComponentOf, ceterms:isPartOf, ceterms:name, ceterms:pointValue, ceterms:precededBy, ceterms:precedes, ceterms:proxyFor, ceterms:sourceData, ceterms:subjectWebpage .

ceterms:ComponentCondition a rdfs:Class ;
	rdfs:label "Component Condition"@en-US ;
	rdfs:comment "Resource that describes what must be done to complete a PathwayComponent, or part thereof, as determined by the issuer of the Pathway."@en-US ;
	dct:description "A ComponentCondition references a single RuleSet defining appropriate values fulfilling the condition."@en-US ;
	vs:term_status vs:stable ;
	meta:changeHistory <http://credreg.net/ctdl/termhistory/ceterms/ComponentCondition/json> ;
	meta:domainFor ceterms:description, ceterms:hasCondition, ceterms:hasConstraint, ceterms:logicalOperator, ceterms:name, ceterms:requiredNumber, ceterms:targetComponent .

ceterms:ConditionManifest a rdfs:Class ;
	rdfs:label "Condition Manifest"@en-US ;
	rdfs:comment "Set of constraints, prerequisites, entry conditions, or requirements maintained at the organizational and/or sub-organizational level."@en-US ;
	dct:description "These conditions are intended to be referenced by external entities such as individual credentials in order to facilitate the process of their description and to reduce unnecessary duplication of data applicable across an array of entities."@en-US ;
	vs:term_status vs:stable ;
	meta:changeHistory <http://credreg.net/ctdl/termhistory/ceterms/ConditionManifest/json> ;
	meta:domainFor ceterms:conditionManifestOf, ceterms:corequisite, ceterms:ctid, ceterms:description, ceterms:entryCondition, ceterms:name, ceterms:recommends, ceterms:renewal, ceterms:requires, ceterms:subjectWebpage .

ceterms:ConditionProfile a rdfs:Class ;
	rdfs:label "Condition Profile"@en-US ;
	rdfs:comment "Entity describing a constraint, prerequisite, entry condition, or requirement."@en-US ;
	dct:description "Constraints exist with credentials, learning opportunities, assessments and other entites to which they are subject during their lifecycles."@en-US ;
	vs:term_status vs:stable ;
	meta:changeHistory <http://credreg.net/ctdl/termhistory/ceterms/ConditionProfile/json> ;
	rdfs:subClassOf schema:CreativeWork ;
	meta:domainFor ceterms:alternativeCondition, ceterms:assertedBy, ceterms:audienceLevelType, ceterms:audienceType, ceterms:commonCosts, ceterms:condition, ceterms:creditUnitTypeDescription, ceterms:creditValue, ceterms:dateEffective, ceterms:description, ceterms:estimatedCost, ceterms:experience, ceterms:jurisdiction, ceterms:minimumAge, ceterms:name, ceterms:residentOf, ceterms:subjectWebpage, ceterms:submissionOf, ceterms:submissionOfDescription, ceterms:targetAssessment, ceterms:targetCompetency, ceterms:targetCredential, ceterms:targetLearningOpportunity, ceterms:weight, ceterms:yearsOfExperience .

ceterms:Constraint a rdfs:Class ;
	rdfs:label "Constraint"@en-US ;
	rdfs:comment "Resource that identifies the parameters defining a limitation or restriction applicable to candidate pathway components."@en-US ;
	vs:term_status vs:unstable ;
	meta:changeHistory <http://credreg.net/ctdl/termhistory/ceterms/Constraint/json> ;
	meta:domainFor ceterms:comparator, ceterms:description, ceterms:leftAction, ceterms:leftSource, ceterms:name, ceterms:rightAction, ceterms:rightSource .

ceterms:ConstraintRule a rdfs:Class ;
	rdfs:label "Constraint Rule"@en-US ;
	rdfs:comment "Abstract class of executable constraints."@en-US ;
	dct:description "An instance of the Constraint Rule class is a deployable machine solution for executing pathway constraints using specifications such as XPath, JSONPath, JsonLogic, ShEx, SHACL, BPMN, XPDL and BPEL."@en-US ;
	vs:term_status vs:unstable ;
	meta:changeHistory <http://credreg.net/ctdl/termhistory/ceterms/ConstraintRule/json> .

ceterms:ContactPoint a rdfs:Class ;
	rdfs:label "Contact Point"@en-US ;
	rdfs:comment "Means of contacting an organization or its representative."@en-US ;
	dct:description "For example, a public relations email address or phone number."@en-US ;
	vs:term_status vs:stable ;
	meta:changeHistory <http://credreg.net/ctdl/termhistory/ceterms/ContactPoint/json> ;
	owl:equivalentClass schema:ContactPoint ;
	meta:domainFor ceterms:contactType, ceterms:email, ceterms:faxNumber, ceterms:name, ceterms:socialMedia, ceterms:telephone .

ceterms:CostManifest a rdfs:Class ;
	rdfs:label "Cost Manifest"@en-US ;
	rdfs:comment "Entity that describes a set of costs maintained at, and applicable across the organizational and/or sub-organizational level."@en-US ;
	dct:description "Instances of these ceterms:CostManifest entities are intended to be referenced by other entities to augment the process of describing their costs."@en-US ;
	vs:term_status vs:stable ;
	meta:changeHistory <http://credreg.net/ctdl/termhistory/ceterms/CostManifest/json> ;
	meta:domainFor ceterms:costDetails, ceterms:costManifestOf, ceterms:ctid, ceterms:description, ceterms:endDate, ceterms:estimatedCost, ceterms:name, ceterms:startDate .

ceterms:CostProfile a rdfs:Class ;
	rdfs:label "Cost Profile"@en-US ;
	rdfs:comment "Entity that describes direct costs one would incur if one were to pursue a credential, assessment, learning opportunity, or aspects thereof."@en-US ;
	vs:term_status vs:stable ;
	meta:changeHistory <http://credreg.net/ctdl/termhistory/ceterms/CostProfile/json> ;
	rdfs:subClassOf schema:CreativeWork ;
	meta:domainFor ceterms:audienceType, ceterms:condition, ceterms:costDetails, ceterms:currency, ceterms:description, ceterms:directCostType, ceterms:endDate, ceterms:jurisdiction, ceterms:name, ceterms:paymentPattern, ceterms:price, ceterms:region, ceterms:residencyType, ceterms:startDate .

ceterms:Course a rdfs:Class ;
	rdfs:label "Course"@en-US ;
	rdfs:comment "Single structured sequence of one or more educational activities that aims to develop a prescribed set of competencies of learners."@en-US ;
	dct:description "Course is distinct from Program, which aggregates several courses."@en-US ;
	vs:term_status vs:stable ;
	meta:changeHistory <http://credreg.net/ctdl/termhistory/ceterms/Course/json> ;
	rdfs:subClassOf ceterms:LearningOpportunityProfile, schema:CreativeWork ;
	owl:equivalentClass schema:Course ;
	meta:domainFor ceterms:accreditedBy, ceterms:accreditedIn, ceterms:advancedStandingFrom, ceterms:approvedBy, ceterms:approvedIn, ceterms:assessmentMethodDescription, ceterms:assessmentMethodType, ceterms:audienceLevelType, ceterms:audienceType, ceterms:availabilityListing, ceterms:availableAt, ceterms:availableOnlineAt, ceterms:codedNotation, ceterms:commonConditions, ceterms:commonCosts, ceterms:corequisite, ceterms:creditUnitTypeDescription, ceterms:creditValue, ceterms:ctid, ceterms:dateEffective, ceterms:deliveryType, ceterms:deliveryTypeDescription, ceterms:description, ceterms:entryCondition, ceterms:estimatedCost, ceterms:estimatedDuration, ceterms:expirationDate, ceterms:financialAssistance, ceterms:hasOffering, ceterms:hasPart, ceterms:hasProxy, ceterms:identifier, ceterms:industryType, ceterms:inLanguage, ceterms:instructionalProgramType, ceterms:isAdvancedStandingFor, ceterms:isMemberOf, ceterms:isNonCredit, ceterms:isPartOf, ceterms:isPreparationFor, ceterms:isRecommendedFor, ceterms:isRequiredFor, ceterms:jurisdiction, ceterms:keyword, ceterms:learningMethodDescription, ceterms:learningMethodType, ceterms:lifeCycleStatusType, ceterms:name, ceterms:occupationType, ceterms:offeredBy, ceterms:offeredIn, ceterms:offerFrequencyType, ceterms:ownedBy, ceterms:preparationFrom, ceterms:recognizedBy, ceterms:recognizedIn, ceterms:recommends, ceterms:region, ceterms:regulatedBy, ceterms:regulatedIn, ceterms:requires, ceterms:sameAs, ceterms:sced, ceterms:scheduleFrequencyType, ceterms:scheduleTimingType, ceterms:subject, ceterms:subjectWebpage, ceterms:supersededBy, ceterms:supersedes, ceterms:targetAssessment, ceterms:targetLearningOpportunity, ceterms:targetLearningResource, ceterms:targetPathway, ceterms:teaches, ceterms:versionIdentifier .

ceterms:CourseComponent a rdfs:Class ;
	rdfs:label "Course Component"@en-US ;
	rdfs:comment "Resource that identifies a structured sequence of one or more learning activities that aims to develop a prescribed set of knowledge, skill, or ability of learners."@en-US ;
	dct:description "Instances act as proxies or stand-ins for other resources in the context of a particular pathway so that relationships between them as components of that pathway can be stated without implying that the those relationships are true of the resources in other contexts."@en-US ;
	vs:term_status vs:stable ;
	meta:changeHistory <http://credreg.net/ctdl/termhistory/ceterms/CourseComponent/json> ;
	rdfs:subClassOf ceterms:PathwayComponent ;
	meta:domainFor ceasn:hasChild, ceasn:isChildOf, ceterms:componentDesignation, ceterms:creditValue, ceterms:ctid, ceterms:description, ceterms:hasCondition, ceterms:identifier, ceterms:isDestinationComponentOf, ceterms:isPartOf, ceterms:name, ceterms:pointValue, ceterms:precededBy, ceterms:precedes, ceterms:programTerm, ceterms:proxyFor, ceterms:sourceData, ceterms:subjectWebpage .

ceterms:Credential a rdfs:Class ;
	rdfs:label "Credential"@en-US ;
	rdfs:comment "Qualification, achievement, personal or organizational quality, or aspect of an identity typically used to indicate suitability."@en-US ;
	dct:description "The ceterms:Credential class is broadly defined to encompass credentials used across domains and communities of practice. The class should be used only when speaking of credentials in general. Subclasses of ceterms:Credential as defined by Credential Engine (or other communities) should be used when referencing specific types of credentials."@en-US ;
	vs:term_status vs:stable ;
	meta:changeHistory <http://credreg.net/ctdl/termhistory/ceterms/Credential/json> ;
	rdfs:subClassOf schema:CreativeWork ;
	owl:equivalentClass obi:BadgeClass ;
	meta:domainFor ceterms:accreditedBy, ceterms:accreditedIn, ceterms:administrationProcess, ceterms:advancedStandingFrom, ceterms:aggregateData, ceterms:alternateName, ceterms:appealProcess, ceterms:approvedBy, ceterms:approvedIn, ceterms:assessmentDeliveryType, ceterms:audienceLevelType, ceterms:audienceType, ceterms:availabilityListing, ceterms:availableAt, ceterms:availableOnlineAt, ceterms:broadAlignment, ceterms:commonConditions, ceterms:commonCosts, ceterms:complaintProcess, ceterms:copyrightHolder, ceterms:corequisite, ceterms:credentialId, ceterms:credentialStatusType, ceterms:ctid, ceterms:dateEffective, ceterms:description, ceterms:developmentProcess, ceterms:earnings, ceterms:employmentOutcome, ceterms:estimatedCost, ceterms:estimatedDuration, ceterms:exactAlignment, ceterms:expirationDate, ceterms:financialAssistance, ceterms:hasPart, ceterms:hasProxy, ceterms:holders, ceterms:identifier, ceterms:image, ceterms:industryType, ceterms:inLanguage, ceterms:instructionalProgramType, ceterms:isAdvancedStandingFor, ceterms:isicV4, ceterms:isPartOf, ceterms:isPreparationFor, ceterms:isRecommendedFor, ceterms:isRequiredFor, ceterms:jurisdiction, ceterms:keyword, ceterms:latestVersion, ceterms:learningDeliveryType, ceterms:maintenanceProcess, ceterms:majorAlignment, ceterms:minorAlignment, ceterms:naics, ceterms:name, ceterms:narrowAlignment, ceterms:nextVersion, ceterms:occupationType, ceterms:offeredBy, ceterms:offeredIn, ceterms:ownedBy, ceterms:preparationFrom, ceterms:previousVersion, ceterms:processStandards, ceterms:processStandardsDescription, ceterms:recognizedBy, ceterms:recognizedIn, ceterms:recommends, ceterms:region, ceterms:regulatedBy, ceterms:regulatedIn, ceterms:relatedAction, ceterms:renewal, ceterms:renewalFrequency, ceterms:renewedBy, ceterms:renewedIn, ceterms:requires, ceterms:reviewProcess, ceterms:revocation, ceterms:revocationProcess, ceterms:revokedBy, ceterms:revokedIn, ceterms:sameAs, ceterms:subject, ceterms:subjectWebpage, ceterms:supersededBy, ceterms:supersedes, ceterms:targetPathway, ceterms:versionIdentifier .

ceterms:CredentialAlignmentObject a rdfs:Class ;
	rdfs:label "Credential Alignment Object"@en-US ;
	rdfs:comment "Entity describing an affiliation or association between an entity such as a credential, learning opportunity or assessment and another entity in a structured framework such as a concept scheme, enumerated list, or competency framework."@en-US ;
	vs:term_status vs:stable ;
	meta:changeHistory <http://credreg.net/ctdl/termhistory/ceterms/CredentialAlignmentObject/json> ;
	rdfs:subClassOf schema:AlignmentObject ;
	meta:domainFor ceterms:alignmentDate, ceterms:alignmentType, ceterms:codedNotation, ceterms:framework, ceterms:frameworkName, ceterms:targetNode, ceterms:targetNodeDescription, ceterms:targetNodeName, ceterms:weight .

ceterms:CredentialAssertion a rdfs:Class ;
	rdfs:label "Credential Assertion"@en-US ;
	rdfs:comment "Representation of a credential awarded to a person."@en-US ;
	vs:term_status vs:stable ;
	meta:changeHistory <http://credreg.net/ctdl/termhistory/ceterms/CredentialAssertion/json> ;
	owl:equivalentClass obi:Assertion .

ceterms:CredentialComponent a rdfs:Class ;
	rdfs:label "Credential Component"@en-US ;
	rdfs:comment "Resource that identifies another resource that describes qualification, achievement, personal or organizational quality, or aspect of an identity typically used to indicate suitability."@en-US ;
	dct:description "The ceterms:Credential class is broadly defined to encompass credentials used across domains and communities of practice. Subclasses of ceterms:Credential as defined by Credential Engine (or other communities) should be referenced. Instances act as proxies or stand-ins for other resources in the context of a particular pathway so that relationships between them as components of that pathway can be stated without implying that the those relationships are true of the resources in other contexts."@en-US ;
	vs:term_status vs:stable ;
	meta:changeHistory <http://credreg.net/ctdl/termhistory/ceterms/CredentialComponent/json> ;
	rdfs:subClassOf ceterms:PathwayComponent ;
	meta:domainFor ceasn:hasChild, ceasn:isChildOf, ceterms:componentDesignation, ceterms:credentialType, ceterms:ctid, ceterms:description, ceterms:hasCondition, ceterms:identifier, ceterms:isDestinationComponentOf, ceterms:isPartOf, ceterms:name, ceterms:pointValue, ceterms:precededBy, ceterms:precedes, ceterms:proxyFor, ceterms:sourceData, ceterms:subjectWebpage .

ceterms:CredentialFramework a rdfs:Class ;
	rdfs:label "Credential Framework"@en-US ;
	rdfs:comment "Class of all structured sets of conceptual entities intentionally designed for use as value vocabulary terms for description and classification in the credentialing context."@en-US ;
	dct:description "The class includes, but is not limited to, subclasses of specialized concept schemes describing industries, occupations, professions, learning contexts and jobs, as well as specialized subject concept schemes, assessment rubrics, proficiency scales, and competency frameworks."@en-US ;
	vs:term_status vs:stable ;
	meta:changeHistory <http://credreg.net/ctdl/termhistory/ceterms/CredentialFramework/json> ;
	owl:equivalentClass asn:EducationalFramework .

ceterms:CredentialingAction a rdfs:Class ;
	rdfs:label "Credentialing Action"@en-US ;
	rdfs:comment "Action taken by an agent affecting the status of an object entity."@en-US ;
	dct:description "Since an instance of ceterms:CredentialingAction is a claim that a certain agent has taken the action being described, creation of such a ceterms:CredentialingAction should be reserved to the agent of that action."@en-US ;
	vs:term_status vs:stable ;
	meta:changeHistory <http://credreg.net/ctdl/termhistory/ceterms/CredentialingAction/json> ;
	meta:domainFor ceterms:actingAgent, ceterms:actionStatusType, ceterms:description, ceterms:endDate, ceterms:evidenceOfAction, ceterms:instrument, ceterms:object, ceterms:participant, ceterms:startDate .

ceterms:CredentialOrganization a rdfs:Class ;
	rdfs:label "Credential Organization"@en-US ;
	rdfs:comment "Organization that plays one or more key roles in the lifecycle of a credential."@en-US ;
	vann:usageNote "For organizations that are not a Credential Organization or a QA Credential Organization, use ceterms:Organization."@en-US ;
	vs:term_status vs:stable ;
	meta:changeHistory <http://credreg.net/ctdl/termhistory/ceterms/CredentialOrganization/json> ;
	rdfs:subClassOf ceterms:Organization ;
	meta:domainFor ceterms:accreditedBy, ceterms:accreditedIn, ceterms:address, ceterms:administrationProcess, ceterms:agentPurpose, ceterms:agentPurposeDescription, ceterms:agentSectorType, ceterms:agentType, ceterms:alternateName, ceterms:appealProcess, ceterms:approvedBy, ceterms:approvedIn, ceterms:approves, ceterms:availabilityListing, ceterms:complaintProcess, ceterms:credentialingAction, ceterms:ctid, ceterms:department, ceterms:description, ceterms:developmentProcess, ceterms:duns, ceterms:email, ceterms:employee, ceterms:fein, ceterms:foundingDate, ceterms:hasAlignmentMap, ceterms:hasConditionManifest, ceterms:hasCostManifest, ceterms:hasVerificationService, ceterms:identifier, ceterms:image, ceterms:inDemandAction, ceterms:industryType, ceterms:ipedsID, ceterms:isicV4, ceterms:jurisdiction, ceterms:keyword, ceterms:leiCode, ceterms:lifeCycleStatusType, ceterms:maintenanceProcess, ceterms:missionAndGoalsStatement, ceterms:missionAndGoalsStatementDescription, ceterms:naics, ceterms:name, ceterms:ncesID, ceterms:offers, ceterms:opeID, ceterms:owns, ceterms:parentOrganization, ceterms:recognizedBy, ceterms:recognizedIn, ceterms:recognizes, ceterms:regulatedBy, ceterms:regulatedIn, ceterms:renews, ceterms:reviewProcess, ceterms:revocationProcess, ceterms:revokes, ceterms:sameAs, ceterms:serviceType, ceterms:socialMedia, ceterms:subjectWebpage, ceterms:subOrganization, ceterms:supersededBy, ceterms:supersedes, ceterms:transferValueStatement, ceterms:transferValueStatementDescription .

ceterms:CredentialPerson a rdfs:Class ;
	rdfs:label "CredentialPerson"@en-US ;
	rdfs:comment "Person who plays a role as primary agent in a credentialing action."@en-US ;
	dct:description "The ceterms:CredentialPerson class should be used to describe persons directly engaged as primary agent in credentialing actions such as approving, offering, recognizing, renewing and revoking credentials and should not include persons merely affiliated with, or employed by organizations that perform such actions."@en-US ;
	vs:term_status vs:stable ;
	meta:changeHistory <http://credreg.net/ctdl/termhistory/ceterms/CredentialPerson/json> ;
	rdfs:subClassOf ceterms:Agent, dct:Agent, schema:Person ;
	meta:domainFor ceterms:affiliation, ceterms:familyName, ceterms:givenName, ceterms:honorificSuffix, ceterms:targetContactPoint, ceterms:worksFor .

ceterms:Degree a rdfs:Class ;
	rdfs:label "Degree"@en-US ;
	rdfs:comment "Academic credential conferred upon completion of a program or course of study, typically over multiple years at a college or university."@en-US ;
	vs:term_status vs:stable ;
	meta:changeHistory <http://credreg.net/ctdl/termhistory/ceterms/Degree/json> ;
	rdfs:subClassOf ceterms:Credential ;
	meta:domainFor ceterms:accreditedBy, ceterms:accreditedIn, ceterms:administrationProcess, ceterms:advancedStandingFrom, ceterms:aggregateData, ceterms:alternateName, ceterms:appealProcess, ceterms:approvedBy, ceterms:approvedIn, ceterms:assessmentDeliveryType, ceterms:audienceLevelType, ceterms:audienceType, ceterms:availabilityListing, ceterms:availableAt, ceterms:availableOnlineAt, ceterms:broadAlignment, ceterms:commonConditions, ceterms:commonCosts, ceterms:complaintProcess, ceterms:copyrightHolder, ceterms:corequisite, ceterms:credentialId, ceterms:credentialStatusType, ceterms:ctid, ceterms:dateEffective, ceterms:degreeConcentration, ceterms:degreeMajor, ceterms:degreeMinor, ceterms:description, ceterms:developmentProcess, ceterms:earnings, ceterms:employmentOutcome, ceterms:estimatedCost, ceterms:estimatedDuration, ceterms:exactAlignment, ceterms:expirationDate, ceterms:financialAssistance, ceterms:hasPart, ceterms:hasProxy, ceterms:holders, ceterms:identifier, ceterms:image, ceterms:industryType, ceterms:inLanguage, ceterms:instructionalProgramType, ceterms:isAdvancedStandingFor, ceterms:isicV4, ceterms:isPartOf, ceterms:isPreparationFor, ceterms:isRecommendedFor, ceterms:isRequiredFor, ceterms:jurisdiction, ceterms:keyword, ceterms:latestVersion, ceterms:learningDeliveryType, ceterms:maintenanceProcess, ceterms:majorAlignment, ceterms:minorAlignment, ceterms:naics, ceterms:name, ceterms:narrowAlignment, ceterms:nextVersion, ceterms:occupationType, ceterms:offeredBy, ceterms:offeredIn, ceterms:ownedBy, ceterms:preparationFrom, ceterms:previousVersion, ceterms:processStandards, ceterms:processStandardsDescription, ceterms:recognizedBy, ceterms:recognizedIn, ceterms:recommends, ceterms:region, ceterms:regulatedBy, ceterms:regulatedIn, ceterms:relatedAction, ceterms:renewal, ceterms:renewalFrequency, ceterms:renewedBy, ceterms:renewedIn, ceterms:requires, ceterms:reviewProcess, ceterms:revocation, ceterms:revocationProcess, ceterms:revokedBy, ceterms:revokedIn, ceterms:sameAs, ceterms:subject, ceterms:subjectWebpage, ceterms:supersededBy, ceterms:supersedes, ceterms:targetPathway, ceterms:versionIdentifier .

ceterms:DigitalBadge a rdfs:Class ;
	rdfs:label "Digital Badge"@en-US ;
	rdfs:comment "Badge offered in digital form."@en-US ;
	vs:term_status vs:stable ;
	meta:changeHistory <http://credreg.net/ctdl/termhistory/ceterms/DigitalBadge/json> ;
	rdfs:subClassOf ceterms:Badge ;
	meta:domainFor ceterms:accreditedBy, ceterms:accreditedIn, ceterms:administrationProcess, ceterms:advancedStandingFrom, ceterms:aggregateData, ceterms:alternateName, ceterms:appealProcess, ceterms:approvedBy, ceterms:approvedIn, ceterms:assessmentDeliveryType, ceterms:audienceLevelType, ceterms:audienceType, ceterms:availabilityListing, ceterms:availableAt, ceterms:availableOnlineAt, ceterms:broadAlignment, ceterms:commonConditions, ceterms:commonCosts, ceterms:complaintProcess, ceterms:copyrightHolder, ceterms:corequisite, ceterms:credentialId, ceterms:credentialStatusType, ceterms:ctid, ceterms:dateEffective, ceterms:description, ceterms:developmentProcess, ceterms:earnings, ceterms:employmentOutcome, ceterms:estimatedCost, ceterms:estimatedDuration, ceterms:exactAlignment, ceterms:expirationDate, ceterms:financialAssistance, ceterms:hasPart, ceterms:hasProxy, ceterms:holders, ceterms:identifier, ceterms:image, ceterms:industryType, ceterms:inLanguage, ceterms:instructionalProgramType, ceterms:isAdvancedStandingFor, ceterms:isicV4, ceterms:isPartOf, ceterms:isPreparationFor, ceterms:isRecommendedFor, ceterms:isRequiredFor, ceterms:jurisdiction, ceterms:keyword, ceterms:latestVersion, ceterms:learningDeliveryType, ceterms:maintenanceProcess, ceterms:majorAlignment, ceterms:minorAlignment, ceterms:naics, ceterms:name, ceterms:narrowAlignment, ceterms:nextVersion, ceterms:occupationType, ceterms:offeredBy, ceterms:offeredIn, ceterms:ownedBy, ceterms:preparationFrom, ceterms:previousVersion, ceterms:processStandards, ceterms:processStandardsDescription, ceterms:recognizedBy, ceterms:recognizedIn, ceterms:recommends, ceterms:region, ceterms:regulatedBy, ceterms:regulatedIn, ceterms:relatedAction, ceterms:renewal, ceterms:renewalFrequency, ceterms:renewedBy, ceterms:renewedIn, ceterms:requires, ceterms:reviewProcess, ceterms:revocation, ceterms:revocationProcess, ceterms:revokedBy, ceterms:revokedIn, ceterms:sameAs, ceterms:subject, ceterms:subjectWebpage, ceterms:supersededBy, ceterms:supersedes, ceterms:targetPathway, ceterms:versionIdentifier .

ceterms:Diploma a rdfs:Class ;
	rdfs:label "Diploma"@en-US ;
	rdfs:comment "Credential awarded by educational institutions for successful completion of a course of study or its equivalent."@en-US ;
	vs:term_status vs:stable ;
	meta:changeHistory <http://credreg.net/ctdl/termhistory/ceterms/Diploma/json> ;
	rdfs:subClassOf ceterms:Credential ;
	meta:domainFor ceterms:accreditedBy, ceterms:accreditedIn, ceterms:administrationProcess, ceterms:advancedStandingFrom, ceterms:aggregateData, ceterms:alternateName, ceterms:appealProcess, ceterms:approvedBy, ceterms:approvedIn, ceterms:assessmentDeliveryType, ceterms:audienceLevelType, ceterms:audienceType, ceterms:availabilityListing, ceterms:availableAt, ceterms:availableOnlineAt, ceterms:broadAlignment, ceterms:commonConditions, ceterms:commonCosts, ceterms:complaintProcess, ceterms:copyrightHolder, ceterms:corequisite, ceterms:credentialId, ceterms:credentialStatusType, ceterms:ctid, ceterms:dateEffective, ceterms:description, ceterms:developmentProcess, ceterms:earnings, ceterms:employmentOutcome, ceterms:estimatedCost, ceterms:estimatedDuration, ceterms:exactAlignment, ceterms:expirationDate, ceterms:financialAssistance, ceterms:hasPart, ceterms:hasProxy, ceterms:holders, ceterms:identifier, ceterms:image, ceterms:industryType, ceterms:inLanguage, ceterms:instructionalProgramType, ceterms:isAdvancedStandingFor, ceterms:isicV4, ceterms:isPartOf, ceterms:isPreparationFor, ceterms:isRecommendedFor, ceterms:isRequiredFor, ceterms:jurisdiction, ceterms:keyword, ceterms:latestVersion, ceterms:learningDeliveryType, ceterms:maintenanceProcess, ceterms:majorAlignment, ceterms:minorAlignment, ceterms:naics, ceterms:name, ceterms:narrowAlignment, ceterms:nextVersion, ceterms:occupationType, ceterms:offeredBy, ceterms:offeredIn, ceterms:ownedBy, ceterms:preparationFrom, ceterms:previousVersion, ceterms:processStandards, ceterms:processStandardsDescription, ceterms:recognizedBy, ceterms:recognizedIn, ceterms:recommends, ceterms:region, ceterms:regulatedBy, ceterms:regulatedIn, ceterms:relatedAction, ceterms:renewal, ceterms:renewalFrequency, ceterms:renewedBy, ceterms:renewedIn, ceterms:requires, ceterms:reviewProcess, ceterms:revocation, ceterms:revocationProcess, ceterms:revokedBy, ceterms:revokedIn, ceterms:sameAs, ceterms:subject, ceterms:subjectWebpage, ceterms:supersededBy, ceterms:supersedes, ceterms:targetPathway, ceterms:versionIdentifier .

ceterms:DoctoralDegree a rdfs:Class ;
	rdfs:label "Doctoral Degree"@en-US ;
	rdfs:comment "Highest credential award for students who have completed both a bachelor's degree and a master's degree or their equivalent as well as independent research and/or a significant project or paper."@en-US ;
	dct:description "Equivalent to UNESCO ISCED, Level 8."@en-US ;
	vs:term_status vs:stable ;
	meta:changeHistory <http://credreg.net/ctdl/termhistory/ceterms/DoctoralDegree/json> ;
	rdfs:subClassOf ceterms:Degree ;
	meta:domainFor ceterms:accreditedBy, ceterms:accreditedIn, ceterms:administrationProcess, ceterms:advancedStandingFrom, ceterms:aggregateData, ceterms:alternateName, ceterms:appealProcess, ceterms:approvedBy, ceterms:approvedIn, ceterms:assessmentDeliveryType, ceterms:audienceLevelType, ceterms:audienceType, ceterms:availabilityListing, ceterms:availableAt, ceterms:availableOnlineAt, ceterms:broadAlignment, ceterms:commonConditions, ceterms:commonCosts, ceterms:complaintProcess, ceterms:copyrightHolder, ceterms:corequisite, ceterms:credentialId, ceterms:credentialStatusType, ceterms:ctid, ceterms:dateEffective, ceterms:degreeConcentration, ceterms:degreeMajor, ceterms:degreeMinor, ceterms:description, ceterms:developmentProcess, ceterms:earnings, ceterms:employmentOutcome, ceterms:estimatedCost, ceterms:estimatedDuration, ceterms:exactAlignment, ceterms:expirationDate, ceterms:financialAssistance, ceterms:hasPart, ceterms:hasProxy, ceterms:holders, ceterms:identifier, ceterms:image, ceterms:industryType, ceterms:inLanguage, ceterms:instructionalProgramType, ceterms:isAdvancedStandingFor, ceterms:isicV4, ceterms:isPartOf, ceterms:isPreparationFor, ceterms:isRecommendedFor, ceterms:isRequiredFor, ceterms:jurisdiction, ceterms:keyword, ceterms:latestVersion, ceterms:learningDeliveryType, ceterms:maintenanceProcess, ceterms:majorAlignment, ceterms:minorAlignment, ceterms:naics, ceterms:name, ceterms:narrowAlignment, ceterms:nextVersion, ceterms:occupationType, ceterms:offeredBy, ceterms:offeredIn, ceterms:ownedBy, ceterms:preparationFrom, ceterms:previousVersion, ceterms:processStandards, ceterms:processStandardsDescription, ceterms:recognizedBy, ceterms:recognizedIn, ceterms:recommends, ceterms:region, ceterms:regulatedBy, ceterms:regulatedIn, ceterms:relatedAction, ceterms:renewal, ceterms:renewalFrequency, ceterms:renewedBy, ceterms:renewedIn, ceterms:requires, ceterms:reviewProcess, ceterms:revocation, ceterms:revocationProcess, ceterms:revokedBy, ceterms:revokedIn, ceterms:sameAs, ceterms:subject, ceterms:subjectWebpage, ceterms:supersededBy, ceterms:supersedes, ceterms:targetPathway, ceterms:versionIdentifier .

ceterms:DurationProfile a rdfs:Class ;
	rdfs:label "Duration Profile"@en-US ;
	rdfs:comment "Entity describing the temporal aspects of a resource."@en-US ;
	dct:description "Temporal aspects include exact, minimum, and maximum timeframes of an activity."@en-US ;
	vs:term_status vs:stable ;
	meta:changeHistory <http://credreg.net/ctdl/termhistory/ceterms/DurationProfile/json> ;
	meta:domainFor ceterms:description, ceterms:exactDuration, ceterms:maximumDuration, ceterms:minimumDuration .

ceterms:EarningsProfile a rdfs:Class ;
	rdfs:label "Earnings Profile"@en-US ;
	rdfs:comment "Entity that describes earning and related statistical information for a given credential."@en-US ;
	vann:usageNote "The use of ceterms:AggregateDataProfile instead of this class is strongly recommended."@en-US ;
	vs:term_status vs:stable ;
	meta:changeHistory <http://credreg.net/ctdl/termhistory/ceterms/EarningsProfile/json> ;
	rdfs:subClassOf ceterms:AggregateDataProfile, schema:CreativeWork ;
	meta:domainFor ceterms:dateEffective, ceterms:highEarnings, ceterms:jurisdiction, ceterms:lowEarnings, ceterms:medianEarnings, ceterms:postReceiptMonths, ceterms:region, ceterms:source, qdata:relevantDataSet .

ceterms:EmploymentOutcomeProfile a rdfs:Class ;
	rdfs:label "Employment Outcome Profile"@en-US ;
	rdfs:comment "Entity that describes employment outcomes and related statistical information for a given credential."@en-US ;
	vann:usageNote "The use of ceterms:AggregateDataProfile instead of this class is strongly recommended."@en-US ;
	vs:term_status vs:stable ;
	meta:changeHistory <http://credreg.net/ctdl/termhistory/ceterms/EmploymentOutcomeProfile/json> ;
	rdfs:subClassOf ceterms:AggregateDataProfile, schema:CreativeWork ;
	meta:domainFor ceterms:dateEffective, ceterms:description, ceterms:jobsObtained, ceterms:jurisdiction, ceterms:source, qdata:relevantDataSet .

ceterms:ExtracurricularComponent a rdfs:Class ;
	rdfs:label "Extracurricular Component"@en-US ;
	rdfs:comment "Resource that identifies an activity, program, or informal learning experience that may be offered or provided by a school, college, or other organization that is not connected to a curriculum."@en-US ;
	dct:description "Instances act as proxies or stand-ins for other resources in the context of a particular pathway so that relationships between them as components of that pathway can be stated without implying that the those relationships are true of the resources in other contexts."@en-US ;
	vs:term_status vs:stable ;
	meta:changeHistory <http://credreg.net/ctdl/termhistory/ceterms/ExtracurricularComponent/json> ;
	rdfs:subClassOf ceterms:PathwayComponent ;
	meta:domainFor ceasn:hasChild, ceasn:isChildOf, ceterms:componentCategory, ceterms:componentDesignation, ceterms:ctid, ceterms:description, ceterms:hasCondition, ceterms:identifier, ceterms:isDestinationComponentOf, ceterms:isPartOf, ceterms:name, ceterms:pointValue, ceterms:precededBy, ceterms:precedes, ceterms:proxyFor, ceterms:sourceData, ceterms:subjectWebpage .

ceterms:FinancialAssistanceProfile a rdfs:Class ;
	rdfs:label "Financial Assistance Profile"@en-US ;
	rdfs:comment "Entity that describes financial assistance that is offered or available."@en-US ;
	vs:term_status vs:stable ;
	meta:changeHistory <http://credreg.net/ctdl/termhistory/ceterms/FinancialAssistanceProfile/json> ;
	meta:domainFor ceterms:description, ceterms:financialAssistanceType, ceterms:financialAssistanceValue, ceterms:name, ceterms:subjectWebpage .

ceterms:GeneralEducationDevelopment a rdfs:Class ;
	rdfs:label "General Education Development (GED)"@en-US ;
	rdfs:comment "Credential awarded by examination that demonstrates that an individual has acquired secondary school-level academic skills."@en-US ;
	dct:description "Equivalent to a secondary school diploma, based on passing a state- or province-selected examination such as GED, HiSET, or TASC; or to an award at UNESCO ISCED 2011 Levels 2 or 3."@en-US ;
	vs:term_status vs:stable ;
	meta:changeHistory <http://credreg.net/ctdl/termhistory/ceterms/GeneralEducationDevelopment/json> ;
	rdfs:subClassOf ceterms:Diploma ;
	meta:domainFor ceterms:accreditedBy, ceterms:accreditedIn, ceterms:administrationProcess, ceterms:advancedStandingFrom, ceterms:aggregateData, ceterms:alternateName, ceterms:appealProcess, ceterms:approvedBy, ceterms:approvedIn, ceterms:assessmentDeliveryType, ceterms:audienceLevelType, ceterms:audienceType, ceterms:availabilityListing, ceterms:availableAt, ceterms:availableOnlineAt, ceterms:broadAlignment, ceterms:commonConditions, ceterms:commonCosts, ceterms:complaintProcess, ceterms:copyrightHolder, ceterms:corequisite, ceterms:credentialId, ceterms:credentialStatusType, ceterms:ctid, ceterms:dateEffective, ceterms:description, ceterms:developmentProcess, ceterms:earnings, ceterms:employmentOutcome, ceterms:estimatedCost, ceterms:estimatedDuration, ceterms:exactAlignment, ceterms:expirationDate, ceterms:financialAssistance, ceterms:hasPart, ceterms:hasProxy, ceterms:holders, ceterms:identifier, ceterms:image, ceterms:industryType, ceterms:inLanguage, ceterms:instructionalProgramType, ceterms:isAdvancedStandingFor, ceterms:isicV4, ceterms:isPartOf, ceterms:isPreparationFor, ceterms:isRecommendedFor, ceterms:isRequiredFor, ceterms:jurisdiction, ceterms:keyword, ceterms:latestVersion, ceterms:learningDeliveryType, ceterms:maintenanceProcess, ceterms:majorAlignment, ceterms:minorAlignment, ceterms:naics, ceterms:name, ceterms:narrowAlignment, ceterms:nextVersion, ceterms:occupationType, ceterms:offeredBy, ceterms:offeredIn, ceterms:ownedBy, ceterms:preparationFrom, ceterms:previousVersion, ceterms:processStandards, ceterms:processStandardsDescription, ceterms:recognizedBy, ceterms:recognizedIn, ceterms:recommends, ceterms:region, ceterms:regulatedBy, ceterms:regulatedIn, ceterms:relatedAction, ceterms:renewal, ceterms:renewalFrequency, ceterms:renewedBy, ceterms:renewedIn, ceterms:requires, ceterms:reviewProcess, ceterms:revocation, ceterms:revocationProcess, ceterms:revokedBy, ceterms:revokedIn, ceterms:sameAs, ceterms:subject, ceterms:subjectWebpage, ceterms:supersededBy, ceterms:supersedes, ceterms:targetPathway, ceterms:versionIdentifier .

ceterms:GeoCoordinates a rdfs:Class ;
	rdfs:label "Geographic Coordinates"@en-US ;
	rdfs:comment "Geographic coordinates of a place or event including latitude and longitude as well as other locational information."@en-US ;
	vs:term_status vs:stable ;
	meta:changeHistory <http://credreg.net/ctdl/termhistory/ceterms/GeoCoordinates/json> ;
	rdfs:subClassOf schema:StructuredValue ;
	owl:equivalentClass schema:GeoCoordinates ;
	meta:domainFor ceterms:geoURI, ceterms:latitude, ceterms:longitude, ceterms:name .

ceterms:HoldersProfile a rdfs:Class ;
	rdfs:label "Holders Profile"@en-US ;
	rdfs:comment "Entity describing the count and related statistical information of holders of a given credential."@en-US ;
	vann:usageNote "The use of ceterms:AggregateDataProfile instead of this class is strongly recommended."@en-US ;
	vs:term_status vs:stable ;
	meta:changeHistory <http://credreg.net/ctdl/termhistory/ceterms/HoldersProfile/json> ;
	rdfs:subClassOf ceterms:AggregateDataProfile, schema:CreativeWork ;
	meta:domainFor ceterms:dateEffective, ceterms:demographicInformation, ceterms:description, ceterms:jurisdiction, ceterms:name, ceterms:numberAwarded, ceterms:region, ceterms:source, qdata:relevantDataSet .

ceterms:IdentifierValue a rdfs:Class ;
	rdfs:label "Identifier Value"@en-US ;
	rdfs:comment "Means of identifying a resource, typically consisting of an alphanumeric token and a context or scheme from which that token originates."@en-US ;
	vann:usageNote "Where a formal identification system exists for the identifier, recommended best practice is to use a string conforming to that system."@en-US ;
	vs:term_status vs:stable ;
	meta:changeHistory <http://credreg.net/ctdl/termhistory/ceterms/IdentifierValue/json> ;
	rdfs:subClassOf dct:identifier ;
	meta:domainFor ceterms:identifierType, ceterms:identifierTypeName, ceterms:identifierValueCode .

ceterms:IndustryClassification a rdfs:Class ;
	rdfs:label "Industry Classification"@en-US ;
	rdfs:comment "Class of of concept schemes defining industries such as NAICS in the U.S. and ESCO in the European Union."@en-US ;
	vs:term_status vs:stable ;
	meta:changeHistory <http://credreg.net/ctdl/termhistory/ceterms/IndustryClassification/json> ;
	rdfs:subClassOf ceterms:CredentialFramework .

ceterms:InstructionalProgramClassification a rdfs:Class ;
	rdfs:label "Instructional Program Classification"@en-US ;
	rdfs:comment "Class of concept schemes defining instructional program types such as the CIP codes in the U.S."@en-US ;
	vann:usageNote "Class of concept schemes defining types"@en-US ;
	vs:term_status vs:stable ;
	meta:changeHistory <http://credreg.net/ctdl/termhistory/ceterms/InstructionalProgramClassification/json> ;
	rdfs:subClassOf ceterms:CredentialFramework .

ceterms:Job a rdfs:Class ;
	rdfs:label "Job"@en-US ;
	rdfs:comment "Set of responsibilities based on work roles within an occupation as defined by an employer."@en-US ;
	dct:description "Job describes an abstraction or template that specific job postings or openings could be instances of."@en-US ;
	vs:term_status vs:stable ;
	meta:changeHistory <http://credreg.net/ctdl/termhistory/ceterms/Job/json> ;
	meta:domainFor ceasn:abilityEmbodied, ceasn:comment, ceasn:knowledgeEmbodied, ceasn:skillEmbodied, ceterms:classification, ceterms:codedNotation, ceterms:ctid, ceterms:description, ceterms:environmentalHazardType, ceterms:hasOccupation, ceterms:hasTask, ceterms:hasWorkRole, ceterms:identifier, ceterms:industryType, ceterms:isMemberOf, ceterms:keyword, ceterms:name, ceterms:occupationType, ceterms:offeredBy, ceterms:performanceLevelType, ceterms:physicalCapabilityType, ceterms:requires, ceterms:sameAs, ceterms:sensoryCapabilityType, ceterms:subjectWebpage, ceterms:versionIdentifier .

ceterms:JobComponent a rdfs:Class ;
	rdfs:label "Job Component"@en-US ;
	rdfs:comment "Resource that identifies a work position, employment, or occupation."@en-US ;
	dct:description "Instances act as proxies or stand-ins for other resources in the context of a particular pathway so that relationships between them as components of that pathway can be stated without implying that the those relationships are true of the resources in other contexts."@en-US ;
	vs:term_status vs:stable ;
	meta:changeHistory <http://credreg.net/ctdl/termhistory/ceterms/JobComponent/json> ;
	rdfs:subClassOf ceterms:PathwayComponent ;
	meta:domainFor ceasn:hasChild, ceasn:isChildOf, ceterms:componentDesignation, ceterms:ctid, ceterms:description, ceterms:hasCondition, ceterms:identifier, ceterms:industryType, ceterms:isDestinationComponentOf, ceterms:isPartOf, ceterms:name, ceterms:occupationType, ceterms:pointValue, ceterms:precededBy, ceterms:precedes, ceterms:proxyFor, ceterms:sourceData, ceterms:subjectWebpage .

ceterms:JourneymanCertificate a rdfs:Class ;
	rdfs:label "Journeyman Certificate"@en-US ;
	rdfs:comment "Credential awarded to skilled workers on successful completion of an apprenticeship in industry trades and professions."@en-US ;
	vs:term_status vs:stable ;
	meta:changeHistory <http://credreg.net/ctdl/termhistory/ceterms/JourneymanCertificate/json> ;
	rdfs:subClassOf ceterms:Certificate ;
	meta:domainFor ceterms:accreditedBy, ceterms:accreditedIn, ceterms:administrationProcess, ceterms:advancedStandingFrom, ceterms:aggregateData, ceterms:alternateName, ceterms:appealProcess, ceterms:approvedBy, ceterms:approvedIn, ceterms:assessmentDeliveryType, ceterms:audienceLevelType, ceterms:audienceType, ceterms:availabilityListing, ceterms:availableAt, ceterms:availableOnlineAt, ceterms:broadAlignment, ceterms:commonConditions, ceterms:commonCosts, ceterms:complaintProcess, ceterms:copyrightHolder, ceterms:corequisite, ceterms:credentialId, ceterms:credentialStatusType, ceterms:ctid, ceterms:dateEffective, ceterms:description, ceterms:developmentProcess, ceterms:earnings, ceterms:employmentOutcome, ceterms:estimatedCost, ceterms:estimatedDuration, ceterms:exactAlignment, ceterms:expirationDate, ceterms:financialAssistance, ceterms:hasPart, ceterms:hasProxy, ceterms:holders, ceterms:identifier, ceterms:image, ceterms:industryType, ceterms:inLanguage, ceterms:instructionalProgramType, ceterms:isAdvancedStandingFor, ceterms:isicV4, ceterms:isPartOf, ceterms:isPreparationFor, ceterms:isRecommendedFor, ceterms:isRequiredFor, ceterms:jurisdiction, ceterms:keyword, ceterms:latestVersion, ceterms:learningDeliveryType, ceterms:maintenanceProcess, ceterms:majorAlignment, ceterms:minorAlignment, ceterms:naics, ceterms:name, ceterms:narrowAlignment, ceterms:nextVersion, ceterms:occupationType, ceterms:offeredBy, ceterms:offeredIn, ceterms:ownedBy, ceterms:preparationFrom, ceterms:previousVersion, ceterms:processStandards, ceterms:processStandardsDescription, ceterms:recognizedBy, ceterms:recognizedIn, ceterms:recommends, ceterms:region, ceterms:regulatedBy, ceterms:regulatedIn, ceterms:relatedAction, ceterms:renewal, ceterms:renewalFrequency, ceterms:renewedBy, ceterms:renewedIn, ceterms:requires, ceterms:reviewProcess, ceterms:revocation, ceterms:revocationProcess, ceterms:revokedBy, ceterms:revokedIn, ceterms:sameAs, ceterms:subject, ceterms:subjectWebpage, ceterms:supersededBy, ceterms:supersedes, ceterms:targetPathway, ceterms:versionIdentifier .

ceterms:JurisdictionProfile a rdfs:Class ;
	rdfs:label "Jurisdiction Profile"@en-US ;
	rdfs:comment "Geo-political information about applicable geographic areas and their exceptions."@en-US ;
	vs:term_status vs:stable ;
	meta:changeHistory <http://credreg.net/ctdl/termhistory/ceterms/JurisdictionProfile/json> ;
	rdfs:subClassOf schema:CreativeWork ;
	meta:domainFor ceterms:assertedBy, ceterms:description, ceterms:globalJurisdiction, ceterms:jurisdictionException, ceterms:mainJurisdiction .

ceterms:LearningOpportunity a rdfs:Class ;
	rdfs:label "Learning Opportunity"@en-US ;
	rdfs:comment "Structured and unstructured learning and development opportunities based in direct experience, formal and informal study, observation, and involvement in discourse and practice."@en-US ;
	dct:description "Examples of learning opportunities include education and training programs and classes, courses of study, apprenticeship or work experience programs, or other structured experiences intended to serve as educational or training events."@en-US ;
	vann:usageNote "Classes of learning opportunities defined in other namespaces such as schema.org/Course may be declared as equivaleny or subclasses of ceterms:LearningOpportunity to support their discovery through applications processing CTDL data."@en-US ;
	vs:term_status vs:stable ;
	meta:changeHistory <http://credreg.net/ctdl/termhistory/ceterms/LearningOpportunity/json> .

ceterms:LearningOpportunityProfile a rdfs:Class ;
	rdfs:label "Learning Opportunity Profile"@en-US ;
	rdfs:comment "Entity describing an educational or training opportunity."@en-US ;
	dct:description "Opportunities include formal and informal educational training programs and classes, apprenticeship or work experience programs, or other structured or unstructured experiences that serve as educational or training activities."@en-US ;
	vs:term_status vs:stable ;
	meta:changeHistory <http://credreg.net/ctdl/termhistory/ceterms/LearningOpportunityProfile/json> ;
	rdfs:subClassOf schema:CreativeWork ;
	meta:domainFor ceterms:accreditedBy, ceterms:accreditedIn, ceterms:advancedStandingFrom, ceterms:approvedBy, ceterms:approvedIn, ceterms:assessmentMethodDescription, ceterms:assessmentMethodType, ceterms:audienceLevelType, ceterms:audienceType, ceterms:availabilityListing, ceterms:availableAt, ceterms:availableOnlineAt, ceterms:codedNotation, ceterms:commonConditions, ceterms:commonCosts, ceterms:corequisite, ceterms:creditUnitTypeDescription, ceterms:creditValue, ceterms:ctid, ceterms:dateEffective, ceterms:deliveryType, ceterms:deliveryTypeDescription, ceterms:description, ceterms:entryCondition, ceterms:estimatedCost, ceterms:estimatedDuration, ceterms:expirationDate, ceterms:financialAssistance, ceterms:hasOffering, ceterms:hasPart, ceterms:hasProxy, ceterms:identifier, ceterms:industryType, ceterms:inLanguage, ceterms:instructionalProgramType, ceterms:isAdvancedStandingFor, ceterms:isMemberOf, ceterms:isNonCredit, ceterms:isPartOf, ceterms:isPreparationFor, ceterms:isRecommendedFor, ceterms:isRequiredFor, ceterms:jurisdiction, ceterms:keyword, ceterms:learningMethodDescription, ceterms:learningMethodType, ceterms:lifeCycleStatusType, ceterms:name, ceterms:occupationType, ceterms:offeredBy, ceterms:offeredIn, ceterms:offerFrequencyType, ceterms:ownedBy, ceterms:preparationFrom, ceterms:recognizedBy, ceterms:recognizedIn, ceterms:recommends, ceterms:region, ceterms:regulatedBy, ceterms:regulatedIn, ceterms:requires, ceterms:sameAs, ceterms:scheduleFrequencyType, ceterms:scheduleTimingType, ceterms:subject, ceterms:subjectWebpage, ceterms:supersededBy, ceterms:supersedes, ceterms:targetAssessment, ceterms:targetLearningOpportunity, ceterms:targetLearningResource, ceterms:targetPathway, ceterms:teaches, ceterms:versionIdentifier .

ceterms:LearningProgram a rdfs:Class ;
	rdfs:label "Learning Program"@en-US ;
	rdfs:comment "Set of learning opportunities that leads to an outcome, usually a credential like a degree or certificate."@en-US ;
	vs:term_status vs:unstable ;
	meta:changeHistory <http://credreg.net/ctdl/termhistory/ceterms/LearningProgram/json> ;
	rdfs:subClassOf ceterms:LearningOpportunityProfile, schema:EducationalOccupationalProgram ;
	meta:domainFor ceterms:accreditedBy, ceterms:accreditedIn, ceterms:advancedStandingFrom, ceterms:approvedBy, ceterms:approvedIn, ceterms:assessmentMethodDescription, ceterms:assessmentMethodType, ceterms:audienceLevelType, ceterms:audienceType, ceterms:availabilityListing, ceterms:availableAt, ceterms:availableOnlineAt, ceterms:codedNotation, ceterms:commonConditions, ceterms:commonCosts, ceterms:corequisite, ceterms:creditUnitTypeDescription, ceterms:creditValue, ceterms:ctid, ceterms:dateEffective, ceterms:deliveryType, ceterms:deliveryTypeDescription, ceterms:description, ceterms:entryCondition, ceterms:estimatedCost, ceterms:estimatedDuration, ceterms:expirationDate, ceterms:financialAssistance, ceterms:hasOffering, ceterms:hasPart, ceterms:hasProxy, ceterms:identifier, ceterms:industryType, ceterms:inLanguage, ceterms:instructionalProgramType, ceterms:isAdvancedStandingFor, ceterms:isMemberOf, ceterms:isNonCredit, ceterms:isPartOf, ceterms:isPreparationFor, ceterms:isRecommendedFor, ceterms:isRequiredFor, ceterms:jurisdiction, ceterms:keyword, ceterms:learningMethodDescription, ceterms:learningMethodType, ceterms:lifeCycleStatusType, ceterms:name, ceterms:occupationType, ceterms:offeredBy, ceterms:offeredIn, ceterms:offerFrequencyType, ceterms:ownedBy, ceterms:preparationFrom, ceterms:recognizedBy, ceterms:recognizedIn, ceterms:recommends, ceterms:region, ceterms:regulatedBy, ceterms:regulatedIn, ceterms:requires, ceterms:sameAs, ceterms:scheduleFrequencyType, ceterms:scheduleTimingType, ceterms:subject, ceterms:subjectWebpage, ceterms:supersededBy, ceterms:supersedes, ceterms:targetAssessment, ceterms:targetLearningOpportunity, ceterms:targetLearningResource, ceterms:targetPathway, ceterms:teaches, ceterms:versionIdentifier .

ceterms:LearningResource a rdfs:Class ;
	rdfs:label "Learning Resource"@en-US ;
	rdfs:comment "Entity that is used as part of an learning activity (e.g. a textbook) or that describes (e.g. a lesson plan) or records the educational activity (e.g. an audio- or video-recording of a lesson)."@en-US ;
	vs:term_status vs:stable ;
	meta:changeHistory <http://credreg.net/ctdl/termhistory/ceterms/LearningResource/json> ;
	rdfs:subClassOf schema:CreativeWork ;
	owl:equivalentClass asn:LearningResource .

ceterms:License a rdfs:Class ;
	rdfs:label "License"@en-US ;
	rdfs:comment "Credential awarded by a government agency or other authorized organization that constitutes legal authority to do a specific job and/or utilize a specific item, system or infrastructure and are typically earned through some combination of degree or certificate attainment, certifications, assessments, work experience, and/or fees, and are time-limited and must be renewed periodically."@en-US ;
	vs:term_status vs:stable ;
	meta:changeHistory <http://credreg.net/ctdl/termhistory/ceterms/License/json> ;
	rdfs:subClassOf ceterms:Credential ;
	meta:domainFor ceterms:accreditedBy, ceterms:accreditedIn, ceterms:administrationProcess, ceterms:advancedStandingFrom, ceterms:aggregateData, ceterms:alternateName, ceterms:appealProcess, ceterms:approvedBy, ceterms:approvedIn, ceterms:assessmentDeliveryType, ceterms:audienceLevelType, ceterms:audienceType, ceterms:availabilityListing, ceterms:availableAt, ceterms:availableOnlineAt, ceterms:broadAlignment, ceterms:commonConditions, ceterms:commonCosts, ceterms:complaintProcess, ceterms:copyrightHolder, ceterms:corequisite, ceterms:credentialId, ceterms:credentialStatusType, ceterms:ctid, ceterms:dateEffective, ceterms:description, ceterms:developmentProcess, ceterms:earnings, ceterms:employmentOutcome, ceterms:estimatedCost, ceterms:estimatedDuration, ceterms:exactAlignment, ceterms:expirationDate, ceterms:financialAssistance, ceterms:hasPart, ceterms:hasProxy, ceterms:holders, ceterms:identifier, ceterms:image, ceterms:industryType, ceterms:inLanguage, ceterms:instructionalProgramType, ceterms:isAdvancedStandingFor, ceterms:isicV4, ceterms:isPartOf, ceterms:isPreparationFor, ceterms:isRecommendedFor, ceterms:isRequiredFor, ceterms:jurisdiction, ceterms:keyword, ceterms:latestVersion, ceterms:learningDeliveryType, ceterms:maintenanceProcess, ceterms:majorAlignment, ceterms:minorAlignment, ceterms:naics, ceterms:name, ceterms:narrowAlignment, ceterms:nextVersion, ceterms:occupationType, ceterms:offeredBy, ceterms:offeredIn, ceterms:ownedBy, ceterms:preparationFrom, ceterms:previousVersion, ceterms:processStandards, ceterms:processStandardsDescription, ceterms:recognizedBy, ceterms:recognizedIn, ceterms:recommends, ceterms:region, ceterms:regulatedBy, ceterms:regulatedIn, ceterms:relatedAction, ceterms:renewal, ceterms:renewalFrequency, ceterms:renewedBy, ceterms:renewedIn, ceterms:requires, ceterms:reviewProcess, ceterms:revocation, ceterms:revocationProcess, ceterms:revokedBy, ceterms:revokedIn, ceterms:sameAs, ceterms:subject, ceterms:subjectWebpage, ceterms:supersededBy, ceterms:supersedes, ceterms:targetPathway, ceterms:versionIdentifier .

ceterms:MasterCertificate a rdfs:Class ;
	rdfs:label "Master Certificate"@en-US ;
	rdfs:comment "Credential awarded upon demonstration through apprenticeship of the highest level of skills and performance in industry trades and professions."@en-US ;
	vs:term_status vs:stable ;
	meta:changeHistory <http://credreg.net/ctdl/termhistory/ceterms/MasterCertificate/json> ;
	rdfs:subClassOf ceterms:Certificate ;
	meta:domainFor ceterms:accreditedBy, ceterms:accreditedIn, ceterms:administrationProcess, ceterms:advancedStandingFrom, ceterms:aggregateData, ceterms:alternateName, ceterms:appealProcess, ceterms:approvedBy, ceterms:approvedIn, ceterms:assessmentDeliveryType, ceterms:audienceLevelType, ceterms:audienceType, ceterms:availabilityListing, ceterms:availableAt, ceterms:availableOnlineAt, ceterms:broadAlignment, ceterms:commonConditions, ceterms:commonCosts, ceterms:complaintProcess, ceterms:copyrightHolder, ceterms:corequisite, ceterms:credentialId, ceterms:credentialStatusType, ceterms:ctid, ceterms:dateEffective, ceterms:description, ceterms:developmentProcess, ceterms:earnings, ceterms:employmentOutcome, ceterms:estimatedCost, ceterms:estimatedDuration, ceterms:exactAlignment, ceterms:expirationDate, ceterms:financialAssistance, ceterms:hasPart, ceterms:hasProxy, ceterms:holders, ceterms:identifier, ceterms:image, ceterms:industryType, ceterms:inLanguage, ceterms:instructionalProgramType, ceterms:isAdvancedStandingFor, ceterms:isicV4, ceterms:isPartOf, ceterms:isPreparationFor, ceterms:isRecommendedFor, ceterms:isRequiredFor, ceterms:jurisdiction, ceterms:keyword, ceterms:latestVersion, ceterms:learningDeliveryType, ceterms:maintenanceProcess, ceterms:majorAlignment, ceterms:minorAlignment, ceterms:naics, ceterms:name, ceterms:narrowAlignment, ceterms:nextVersion, ceterms:occupationType, ceterms:offeredBy, ceterms:offeredIn, ceterms:ownedBy, ceterms:preparationFrom, ceterms:previousVersion, ceterms:processStandards, ceterms:processStandardsDescription, ceterms:recognizedBy, ceterms:recognizedIn, ceterms:recommends, ceterms:region, ceterms:regulatedBy, ceterms:regulatedIn, ceterms:relatedAction, ceterms:renewal, ceterms:renewalFrequency, ceterms:renewedBy, ceterms:renewedIn, ceterms:requires, ceterms:reviewProcess, ceterms:revocation, ceterms:revocationProcess, ceterms:revokedBy, ceterms:revokedIn, ceterms:sameAs, ceterms:subject, ceterms:subjectWebpage, ceterms:supersededBy, ceterms:supersedes, ceterms:targetPathway, ceterms:versionIdentifier .

ceterms:MasterDegree a rdfs:Class ;
	rdfs:label "Master's Degree"@en-US ;
	rdfs:comment "Credential awarded for a graduate level course of study where course work and activities advance skills beyond those of the bachelor's degree or its equivalent."@en-US ;
	dct:description "Equivalent to an award at UNESCO ISCED 2011, Level 7."@en-US ;
	vs:term_status vs:stable ;
	meta:changeHistory <http://credreg.net/ctdl/termhistory/ceterms/MasterDegree/json> ;
	rdfs:subClassOf ceterms:Degree ;
	meta:domainFor ceterms:accreditedBy, ceterms:accreditedIn, ceterms:administrationProcess, ceterms:advancedStandingFrom, ceterms:aggregateData, ceterms:alternateName, ceterms:appealProcess, ceterms:approvedBy, ceterms:approvedIn, ceterms:assessmentDeliveryType, ceterms:audienceLevelType, ceterms:audienceType, ceterms:availabilityListing, ceterms:availableAt, ceterms:availableOnlineAt, ceterms:broadAlignment, ceterms:commonConditions, ceterms:commonCosts, ceterms:complaintProcess, ceterms:copyrightHolder, ceterms:corequisite, ceterms:credentialId, ceterms:credentialStatusType, ceterms:ctid, ceterms:dateEffective, ceterms:degreeConcentration, ceterms:degreeMajor, ceterms:degreeMinor, ceterms:description, ceterms:developmentProcess, ceterms:earnings, ceterms:employmentOutcome, ceterms:estimatedCost, ceterms:estimatedDuration, ceterms:exactAlignment, ceterms:expirationDate, ceterms:financialAssistance, ceterms:hasPart, ceterms:hasProxy, ceterms:holders, ceterms:identifier, ceterms:image, ceterms:industryType, ceterms:inLanguage, ceterms:instructionalProgramType, ceterms:isAdvancedStandingFor, ceterms:isicV4, ceterms:isPartOf, ceterms:isPreparationFor, ceterms:isRecommendedFor, ceterms:isRequiredFor, ceterms:jurisdiction, ceterms:keyword, ceterms:latestVersion, ceterms:learningDeliveryType, ceterms:maintenanceProcess, ceterms:majorAlignment, ceterms:minorAlignment, ceterms:naics, ceterms:name, ceterms:narrowAlignment, ceterms:nextVersion, ceterms:occupationType, ceterms:offeredBy, ceterms:offeredIn, ceterms:ownedBy, ceterms:preparationFrom, ceterms:previousVersion, ceterms:processStandards, ceterms:processStandardsDescription, ceterms:recognizedBy, ceterms:recognizedIn, ceterms:recommends, ceterms:region, ceterms:regulatedBy, ceterms:regulatedIn, ceterms:relatedAction, ceterms:renewal, ceterms:renewalFrequency, ceterms:renewedBy, ceterms:renewedIn, ceterms:requires, ceterms:reviewProcess, ceterms:revocation, ceterms:revocationProcess, ceterms:revokedBy, ceterms:revokedIn, ceterms:sameAs, ceterms:subject, ceterms:subjectWebpage, ceterms:supersededBy, ceterms:supersedes, ceterms:targetPathway, ceterms:versionIdentifier .

ceterms:MicroCredential a rdfs:Class ;
	rdfs:label "Micro-Credential"@en-US ;
	rdfs:comment "Credential that addresses a subset of field-specific knowledge, skills, or competencies; often developmental with relationships to other micro-credentials and field credentials."@en-US ;
	vs:term_status vs:stable ;
	meta:changeHistory <http://credreg.net/ctdl/termhistory/ceterms/MicroCredential/json> ;
	rdfs:subClassOf ceterms:Credential ;
	meta:domainFor ceterms:accreditedBy, ceterms:accreditedIn, ceterms:administrationProcess, ceterms:advancedStandingFrom, ceterms:aggregateData, ceterms:alternateName, ceterms:appealProcess, ceterms:approvedBy, ceterms:approvedIn, ceterms:assessmentDeliveryType, ceterms:audienceLevelType, ceterms:audienceType, ceterms:availabilityListing, ceterms:availableAt, ceterms:availableOnlineAt, ceterms:broadAlignment, ceterms:commonConditions, ceterms:commonCosts, ceterms:complaintProcess, ceterms:copyrightHolder, ceterms:corequisite, ceterms:credentialId, ceterms:credentialStatusType, ceterms:ctid, ceterms:dateEffective, ceterms:description, ceterms:developmentProcess, ceterms:earnings, ceterms:employmentOutcome, ceterms:estimatedCost, ceterms:estimatedDuration, ceterms:exactAlignment, ceterms:expirationDate, ceterms:financialAssistance, ceterms:hasPart, ceterms:hasProxy, ceterms:holders, ceterms:identifier, ceterms:image, ceterms:industryType, ceterms:inLanguage, ceterms:instructionalProgramType, ceterms:isAdvancedStandingFor, ceterms:isicV4, ceterms:isPartOf, ceterms:isPreparationFor, ceterms:isRecommendedFor, ceterms:isRequiredFor, ceterms:jurisdiction, ceterms:keyword, ceterms:latestVersion, ceterms:learningDeliveryType, ceterms:maintenanceProcess, ceterms:majorAlignment, ceterms:minorAlignment, ceterms:naics, ceterms:name, ceterms:narrowAlignment, ceterms:nextVersion, ceterms:occupationType, ceterms:offeredBy, ceterms:offeredIn, ceterms:ownedBy, ceterms:preparationFrom, ceterms:previousVersion, ceterms:processStandards, ceterms:processStandardsDescription, ceterms:recognizedBy, ceterms:recognizedIn, ceterms:recommends, ceterms:region, ceterms:regulatedBy, ceterms:regulatedIn, ceterms:relatedAction, ceterms:renewal, ceterms:renewalFrequency, ceterms:renewedBy, ceterms:renewedIn, ceterms:requires, ceterms:reviewProcess, ceterms:revocation, ceterms:revocationProcess, ceterms:revokedBy, ceterms:revokedIn, ceterms:sameAs, ceterms:subject, ceterms:subjectWebpage, ceterms:supersededBy, ceterms:supersedes, ceterms:targetPathway, ceterms:versionIdentifier .

ceterms:Occupation a rdfs:Class ;
	rdfs:label "Occupation"@en-US ;
	rdfs:comment "Profession, trade, or career field that may involve training and/or a formal qualification."@en-US ;
	vs:term_status vs:stable ;
	meta:changeHistory <http://credreg.net/ctdl/termhistory/ceterms/Occupation/json> ;
	meta:domainFor ceasn:abilityEmbodied, ceasn:comment, ceasn:knowledgeEmbodied, ceasn:skillEmbodied, ceterms:classification, ceterms:codedNotation, ceterms:ctid, ceterms:description, ceterms:hasJob, ceterms:hasSpecialization, ceterms:hasWorkforceDemand, ceterms:hasWorkRole, ceterms:identifier, ceterms:industryType, ceterms:isSpecializationOf, ceterms:keyword, ceterms:name, ceterms:occupationType, ceterms:requires, ceterms:sameAs, ceterms:subjectWebpage, ceterms:versionIdentifier .

ceterms:OccupationClassification a rdfs:Class ;
	rdfs:label "Occupation Classification"@en-US ;
	rdfs:comment "Class of concept schemes identifying occupations such as the Standard Occupational Classification (SOC) system in the U.S. and the European Skills/Competences, Qualifications and Occupations (ESCO)."@en-US ;
	vs:term_status vs:stable ;
	meta:changeHistory <http://credreg.net/ctdl/termhistory/ceterms/OccupationClassification/json> ;
	rdfs:subClassOf ceterms:CredentialFramework .

ceterms:OfferAction a rdfs:Class ;
	rdfs:label "Offer Action"@en-US ;
	rdfs:comment "Action by an authoritative agent offering access to a entity such as a credential, learning opportunity or assessment."@en-US ;
	dct:description "Since an instance of ceterms:CredentialingAction is a claim that a certain agent has taken the action being described, creation of such a ceterms:CredentialingAction should be reserved to the agent of that action."@en-US ;
	vs:term_status vs:stable ;
	meta:changeHistory <http://credreg.net/ctdl/termhistory/ceterms/OfferAction/json> ;
	rdfs:subClassOf ceterms:CredentialingAction ;
	meta:domainFor ceterms:actingAgent, ceterms:actionStatusType, ceterms:description, ceterms:endDate, ceterms:evidenceOfAction, ceterms:instrument, ceterms:object, ceterms:participant, ceterms:startDate .

ceterms:OpenBadge a rdfs:Class ;
	rdfs:label "Open Badge"@en-US ;
	rdfs:comment "Visual symbol containing verifiable claims in accordance with the Open Badges specification and delivered digitally."@en-US ;
	vs:term_status vs:stable ;
	meta:changeHistory <http://credreg.net/ctdl/termhistory/ceterms/OpenBadge/json> ;
	rdfs:subClassOf ceterms:Badge ;
	meta:domainFor ceterms:accreditedBy, ceterms:accreditedIn, ceterms:administrationProcess, ceterms:advancedStandingFrom, ceterms:aggregateData, ceterms:alternateName, ceterms:appealProcess, ceterms:approvedBy, ceterms:approvedIn, ceterms:assessmentDeliveryType, ceterms:audienceLevelType, ceterms:audienceType, ceterms:availabilityListing, ceterms:availableAt, ceterms:availableOnlineAt, ceterms:broadAlignment, ceterms:commonConditions, ceterms:commonCosts, ceterms:complaintProcess, ceterms:copyrightHolder, ceterms:corequisite, ceterms:credentialId, ceterms:credentialStatusType, ceterms:ctid, ceterms:dateEffective, ceterms:description, ceterms:developmentProcess, ceterms:earnings, ceterms:employmentOutcome, ceterms:estimatedCost, ceterms:estimatedDuration, ceterms:exactAlignment, ceterms:expirationDate, ceterms:financialAssistance, ceterms:hasPart, ceterms:hasProxy, ceterms:holders, ceterms:identifier, ceterms:image, ceterms:industryType, ceterms:inLanguage, ceterms:instructionalProgramType, ceterms:isAdvancedStandingFor, ceterms:isicV4, ceterms:isPartOf, ceterms:isPreparationFor, ceterms:isRecommendedFor, ceterms:isRequiredFor, ceterms:jurisdiction, ceterms:keyword, ceterms:latestVersion, ceterms:learningDeliveryType, ceterms:maintenanceProcess, ceterms:majorAlignment, ceterms:minorAlignment, ceterms:naics, ceterms:name, ceterms:narrowAlignment, ceterms:nextVersion, ceterms:occupationType, ceterms:offeredBy, ceterms:offeredIn, ceterms:ownedBy, ceterms:preparationFrom, ceterms:previousVersion, ceterms:processStandards, ceterms:processStandardsDescription, ceterms:recognizedBy, ceterms:recognizedIn, ceterms:recommends, ceterms:region, ceterms:regulatedBy, ceterms:regulatedIn, ceterms:relatedAction, ceterms:renewal, ceterms:renewalFrequency, ceterms:renewedBy, ceterms:renewedIn, ceterms:requires, ceterms:reviewProcess, ceterms:revocation, ceterms:revocationProcess, ceterms:revokedBy, ceterms:revokedIn, ceterms:sameAs, ceterms:subject, ceterms:subjectWebpage, ceterms:supersededBy, ceterms:supersedes, ceterms:targetPathway, ceterms:versionIdentifier .

ceterms:Organization a rdfs:Class ;
	rdfs:label "Organization"@en-US ;
	rdfs:comment "An entity such as an association, company, corporation, club, co-operative, labor union etc."@en-US ;
	vann:usageNote "Use for organizations that are not a Credential Organization or a QACredential Organization."@en-US ;
	vs:term_status vs:stable ;
	meta:changeHistory <http://credreg.net/ctdl/termhistory/ceterms/Organization/json> ;
	rdfs:subClassOf ceterms:Agent, dct:Agent ;
	owl:equivalentClass schema:Organization ;
	meta:domainFor ceterms:accreditedBy, ceterms:accreditedIn, ceterms:accredits, ceterms:address, ceterms:administrationProcess, ceterms:agentPurpose, ceterms:agentPurposeDescription, ceterms:agentSectorType, ceterms:agentType, ceterms:alternateName, ceterms:appealProcess, ceterms:approvedBy, ceterms:approvedIn, ceterms:approves, ceterms:availabilityListing, ceterms:complaintProcess, ceterms:credentialingAction, ceterms:ctid, ceterms:department, ceterms:description, ceterms:developmentProcess, ceterms:duns, ceterms:email, ceterms:employee, ceterms:fein, ceterms:foundingDate, ceterms:hasAlignmentMap, ceterms:hasConditionManifest, ceterms:hasCostManifest, ceterms:hasVerificationService, ceterms:identifier, ceterms:image, ceterms:inDemandAction, ceterms:industryType, ceterms:ipedsID, ceterms:isicV4, ceterms:jurisdiction, ceterms:keyword, ceterms:leiCode, ceterms:lifeCycleStatusType, ceterms:maintenanceProcess, ceterms:missionAndGoalsStatement, ceterms:missionAndGoalsStatementDescription, ceterms:naics, ceterms:name, ceterms:offers, ceterms:opeID, ceterms:owns, ceterms:parentOrganization, ceterms:qualityAssuranceTargetType, ceterms:recognizedBy, ceterms:recognizedIn, ceterms:recognizes, ceterms:regulatedBy, ceterms:regulatedIn, ceterms:regulates, ceterms:renews, ceterms:reviewProcess, ceterms:revocationProcess, ceterms:revokes, ceterms:sameAs, ceterms:serviceType, ceterms:socialMedia, ceterms:subjectWebpage, ceterms:subOrganization, ceterms:supersededBy, ceterms:supersedes, ceterms:transferValueStatement, ceterms:transferValueStatementDescription .

ceterms:Pathway a rdfs:Class ;
	rdfs:label "Pathway"@en-US ;
	rdfs:comment "Resource composed of a structured set of PathwayComponents defining points along a route to fulfillment of a goal or objective."@en-US ;
	vs:term_status vs:stable ;
	meta:changeHistory <http://credreg.net/ctdl/termhistory/ceterms/Pathway/json> ;
	meta:domainFor ceterms:ctid, ceterms:description, ceterms:hasDestinationComponent, ceterms:hasPart, ceterms:industryType, ceterms:instructionalProgramType, ceterms:keyword, ceterms:name, ceterms:occupationType, ceterms:offeredBy, ceterms:ownedBy, ceterms:subject, ceterms:subjectWebpage .

ceterms:PathwayComponent a rdfs:Class ;
	rdfs:label "Pathway Component"@en-US ;
	rdfs:comment "Resource that serves as a defined point along the route of a Pathway which describes an objective and its completion requirements through reference to one or more instances of ComponentCondition."@en-US ;
	dct:description "An instance of PathwayComponent may serve as the goal or destination node of a Pathway."@en-US ;
	vann:usageNote "PathwayComponent is a super-type that represents a family of more precise sub-types. In pathway descriptions, always use the sub-type of PathwayComponent appropriate to your circumstances, e.g., AssessmentComponent, CocurricularComponent, CompetencyComponent, CourseComponent, CredentialComponent, ExtracurricularComponent, JobComponent, and WorkExperienceComponent. Use BasicComponent for types of entities not covered by the current set of sub-types."@en-US ;
	vs:term_status vs:stable ;
	meta:changeHistory <http://credreg.net/ctdl/termhistory/ceterms/PathwayComponent/json> .

ceterms:PathwaySet a rdfs:Class ;
	rdfs:label "Pathway Set"@en-US ;
	rdfs:comment "A roadmap of multiple related pathways that lead to one or more destinations."@en-US ;
	vs:term_status vs:stable ;
	meta:changeHistory <http://credreg.net/ctdl/termhistory/ceterms/PathwaySet/json> ;
	rdfs:subClassOf ceterms:Collection ;
	meta:domainFor ceterms:ctid, ceterms:description, ceterms:hasPathway, ceterms:name, ceterms:offeredBy, ceterms:ownedBy, ceterms:subjectWebpage .

ceterms:Place a rdfs:Class ;
	rdfs:label "Place"@en-US ;
	rdfs:comment "Entity describing a physical location or geospatial area."@en-US ;
	vs:term_status vs:stable ;
	meta:changeHistory <http://credreg.net/ctdl/termhistory/ceterms/Place/json> ;
	owl:equivalentClass schema:Place ;
	meta:domainFor ceterms:addressCountry, ceterms:addressLocality, ceterms:addressRegion, ceterms:description, ceterms:geoURI, ceterms:identifier, ceterms:latitude, ceterms:longitude, ceterms:name, ceterms:postalCode, ceterms:postOfficeBoxNumber, ceterms:streetAddress, ceterms:targetContactPoint .

ceterms:PostalAddress a rdfs:Class ;
	rdfs:label "Postal Address"@en-US ;
	rdfs:comment "Entity describing a mailing address."@en-US ;
	vs:term_status vs:stable ;
	meta:changeHistory <http://credreg.net/ctdl/termhistory/ceterms/PostalAddress/json> ;
	rdfs:subClassOf ceterms:ContactPoint ;
	owl:equivalentClass schema:PostalAddress ;
	meta:domainFor ceterms:addressCountry, ceterms:addressLocality, ceterms:addressRegion, ceterms:name, ceterms:postalCode, ceterms:postOfficeBoxNumber, ceterms:streetAddress .

ceterms:ProcessProfile a rdfs:Class ;
	rdfs:label "Process Profile"@en-US ;
	rdfs:comment "Entity describing the type, nature, and other relevant information about a process related to a credential."@en-US ;
	vs:term_status vs:stable ;
	meta:changeHistory <http://credreg.net/ctdl/termhistory/ceterms/ProcessProfile/json> ;
	rdfs:subClassOf schema:CreativeWork ;
	meta:domainFor ceterms:dateEffective, ceterms:description, ceterms:externalInputType, ceterms:jurisdiction, ceterms:processFrequency, ceterms:processingAgent, ceterms:processMethod, ceterms:processMethodDescription, ceterms:processStandards, ceterms:processStandardsDescription, ceterms:region, ceterms:scoringMethodDescription, ceterms:scoringMethodExample, ceterms:scoringMethodExampleDescription, ceterms:subjectWebpage, ceterms:targetAssessment, ceterms:targetCompetencyFramework, ceterms:targetCredential, ceterms:targetLearningOpportunity, ceterms:verificationMethodDescription, qdata:dataCollectionMethodType .

ceterms:ProfessionalDoctorate a rdfs:Class ;
	rdfs:label "Professional Doctorate"@en-US ;
	rdfs:comment "Doctoral degree conferred upon completion of a program providing the knowledge and skills for the recognition, credential, or license required for professional practice."@en-US ;
	dct:description "Equivalent to an award at UNESCO ISCED 2011, Level 8."@en-US ;
	vs:term_status vs:stable ;
	meta:changeHistory <http://credreg.net/ctdl/termhistory/ceterms/ProfessionalDoctorate/json> ;
	rdfs:subClassOf ceterms:DoctoralDegree ;
	meta:domainFor ceterms:accreditedBy, ceterms:accreditedIn, ceterms:administrationProcess, ceterms:advancedStandingFrom, ceterms:aggregateData, ceterms:alternateName, ceterms:appealProcess, ceterms:approvedBy, ceterms:approvedIn, ceterms:assessmentDeliveryType, ceterms:audienceLevelType, ceterms:audienceType, ceterms:availabilityListing, ceterms:availableAt, ceterms:availableOnlineAt, ceterms:broadAlignment, ceterms:commonConditions, ceterms:commonCosts, ceterms:complaintProcess, ceterms:copyrightHolder, ceterms:corequisite, ceterms:credentialId, ceterms:credentialStatusType, ceterms:ctid, ceterms:dateEffective, ceterms:description, ceterms:developmentProcess, ceterms:earnings, ceterms:employmentOutcome, ceterms:estimatedCost, ceterms:estimatedDuration, ceterms:exactAlignment, ceterms:expirationDate, ceterms:financialAssistance, ceterms:hasPart, ceterms:hasProxy, ceterms:holders, ceterms:identifier, ceterms:image, ceterms:industryType, ceterms:inLanguage, ceterms:instructionalProgramType, ceterms:isAdvancedStandingFor, ceterms:isicV4, ceterms:isPartOf, ceterms:isPreparationFor, ceterms:isRecommendedFor, ceterms:isRequiredFor, ceterms:jurisdiction, ceterms:keyword, ceterms:latestVersion, ceterms:learningDeliveryType, ceterms:maintenanceProcess, ceterms:majorAlignment, ceterms:minorAlignment, ceterms:naics, ceterms:name, ceterms:narrowAlignment, ceterms:nextVersion, ceterms:occupationType, ceterms:offeredBy, ceterms:offeredIn, ceterms:ownedBy, ceterms:preparationFrom, ceterms:previousVersion, ceterms:processStandards, ceterms:processStandardsDescription, ceterms:recognizedBy, ceterms:recognizedIn, ceterms:recommends, ceterms:region, ceterms:regulatedBy, ceterms:regulatedIn, ceterms:relatedAction, ceterms:renewal, ceterms:renewalFrequency, ceterms:renewedBy, ceterms:renewedIn, ceterms:requires, ceterms:reviewProcess, ceterms:revocation, ceterms:revocationProcess, ceterms:revokedBy, ceterms:revokedIn, ceterms:sameAs, ceterms:subject, ceterms:subjectWebpage, ceterms:supersededBy, ceterms:supersedes, ceterms:targetPathway, ceterms:versionIdentifier .

ceterms:QACredentialOrganization a rdfs:Class ;
	rdfs:label "QA Credential Organization"@en-US ;
	rdfs:comment "Quality assurance organization that plays one or more key roles in the lifecycle of a credential, learning program, or assessment."@en-US ;
	vann:usageNote "For organizations that are not a QA Credential Organization or a Credential Organization, use ceterms:Organization."@en-US ;
	vs:term_status vs:stable ;
	meta:changeHistory <http://credreg.net/ctdl/termhistory/ceterms/QACredentialOrganization/json> ;
	rdfs:subClassOf ceterms:Organization ;
	meta:domainFor ceterms:accreditedBy, ceterms:accreditedIn, ceterms:accredits, ceterms:address, ceterms:administrationProcess, ceterms:agentPurpose, ceterms:agentPurposeDescription, ceterms:agentSectorType, ceterms:agentType, ceterms:alternateName, ceterms:appealProcess, ceterms:approvedBy, ceterms:approvedIn, ceterms:approves, ceterms:availabilityListing, ceterms:complaintProcess, ceterms:credentialingAction, ceterms:ctid, ceterms:department, ceterms:description, ceterms:developmentProcess, ceterms:duns, ceterms:email, ceterms:employee, ceterms:fein, ceterms:foundingDate, ceterms:hasAlignmentMap, ceterms:hasConditionManifest, ceterms:hasCostManifest, ceterms:hasVerificationService, ceterms:identifier, ceterms:image, ceterms:inDemandAction, ceterms:industryType, ceterms:ipedsID, ceterms:isicV4, ceterms:jurisdiction, ceterms:keyword, ceterms:leiCode, ceterms:lifeCycleStatusType, ceterms:maintenanceProcess, ceterms:missionAndGoalsStatement, ceterms:missionAndGoalsStatementDescription, ceterms:naics, ceterms:name, ceterms:offers, ceterms:opeID, ceterms:owns, ceterms:parentOrganization, ceterms:qualityAssuranceTargetType, ceterms:recognizedBy, ceterms:recognizedIn, ceterms:recognizes, ceterms:regulatedBy, ceterms:regulatedIn, ceterms:regulates, ceterms:renews, ceterms:reviewProcess, ceterms:revocationProcess, ceterms:revokes, ceterms:sameAs, ceterms:serviceType, ceterms:socialMedia, ceterms:subjectWebpage, ceterms:subOrganization, ceterms:supersededBy, ceterms:supersedes, ceterms:transferValueStatement, ceterms:transferValueStatementDescription .

ceterms:QualityAssuranceCredential a rdfs:Class ;
	rdfs:label "Quality Assurance Credential"@en-US ;
	rdfs:comment "Credential assuring that an organization, program, or awarded credential meets prescribed requirements and may include development and administration of qualifying examinations."@en-US ;
	vs:term_status vs:stable ;
	meta:changeHistory <http://credreg.net/ctdl/termhistory/ceterms/QualityAssuranceCredential/json> ;
	rdfs:subClassOf ceterms:Credential ;
	meta:domainFor ceterms:accreditedBy, ceterms:accreditedIn, ceterms:administrationProcess, ceterms:advancedStandingFrom, ceterms:aggregateData, ceterms:alternateName, ceterms:appealProcess, ceterms:approvedBy, ceterms:approvedIn, ceterms:assessmentDeliveryType, ceterms:audienceLevelType, ceterms:audienceType, ceterms:availabilityListing, ceterms:availableAt, ceterms:availableOnlineAt, ceterms:broadAlignment, ceterms:commonConditions, ceterms:commonCosts, ceterms:complaintProcess, ceterms:copyrightHolder, ceterms:corequisite, ceterms:credentialId, ceterms:credentialStatusType, ceterms:ctid, ceterms:dateEffective, ceterms:description, ceterms:developmentProcess, ceterms:earnings, ceterms:employmentOutcome, ceterms:estimatedCost, ceterms:estimatedDuration, ceterms:exactAlignment, ceterms:expirationDate, ceterms:financialAssistance, ceterms:hasPart, ceterms:hasProxy, ceterms:holders, ceterms:identifier, ceterms:image, ceterms:industryType, ceterms:inLanguage, ceterms:instructionalProgramType, ceterms:isAdvancedStandingFor, ceterms:isicV4, ceterms:isPartOf, ceterms:isPreparationFor, ceterms:isRecommendedFor, ceterms:isRequiredFor, ceterms:jurisdiction, ceterms:keyword, ceterms:latestVersion, ceterms:learningDeliveryType, ceterms:maintenanceProcess, ceterms:majorAlignment, ceterms:minorAlignment, ceterms:naics, ceterms:name, ceterms:narrowAlignment, ceterms:nextVersion, ceterms:occupationType, ceterms:offeredBy, ceterms:offeredIn, ceterms:ownedBy, ceterms:preparationFrom, ceterms:previousVersion, ceterms:processStandards, ceterms:processStandardsDescription, ceterms:recognizedBy, ceterms:recognizedIn, ceterms:recommends, ceterms:region, ceterms:regulatedBy, ceterms:regulatedIn, ceterms:relatedAction, ceterms:renewal, ceterms:renewalFrequency, ceterms:renewedBy, ceterms:renewedIn, ceterms:requires, ceterms:reviewProcess, ceterms:revocation, ceterms:revocationProcess, ceterms:revokedBy, ceterms:revokedIn, ceterms:sameAs, ceterms:subject, ceterms:subjectWebpage, ceterms:supersededBy, ceterms:supersedes, ceterms:targetPathway, ceterms:versionIdentifier .

ceterms:RecognizeAction a rdfs:Class ;
	rdfs:label "Recognize Action"@en-US ;
	rdfs:comment "Action by an independent, neutral, and authoritative agent acknowledging the validity of a resource."@en-US ;
	dct:description "Since an instance of ceterms:CredentialingAction is a claim that a certain agent has taken the action being described, creation of such a ceterms:CredentialingAction should be reserved to the agent of that action."@en-US ;
	vs:term_status vs:stable ;
	meta:changeHistory <http://credreg.net/ctdl/termhistory/ceterms/RecognizeAction/json> ;
	rdfs:subClassOf ceterms:CredentialingAction ;
	meta:domainFor ceterms:actingAgent, ceterms:actionStatusType, ceterms:description, ceterms:endDate, ceterms:evidenceOfAction, ceterms:instrument, ceterms:object, ceterms:participant, ceterms:startDate .

ceterms:RegulateAction a rdfs:Class ;
	rdfs:label "Regulate Action"@en-US ;
	rdfs:comment "Action by an independent, neutral, and authoritative agent enforcing the legal requirements of a resource."@en-US ;
	dct:description "Since an instance of ceterms:CredentialingAction is a claim that a certain agent has taken the action being described, creation of such a ceterms:CredentialingAction should be reserved to the agent of that action."@en-US ;
	vs:term_status vs:unstable ;
	meta:changeHistory <http://credreg.net/ctdl/termhistory/ceterms/RegulateAction/json> ;
	rdfs:subClassOf ceterms:CredentialingAction ;
	meta:domainFor ceterms:actingAgent, ceterms:actionStatusType, ceterms:description, ceterms:endDate, ceterms:evidenceOfAction, ceterms:instrument, ceterms:object, ceterms:participant, ceterms:startDate .

ceterms:RenewAction a rdfs:Class ;
	rdfs:label "Renew Action"@en-US ;
	rdfs:comment "Action by an agent renewing an existing credential assertion."@en-US ;
	dct:description "Since an instance of ceterms:CredentialingAction is a claim that a certain agent has taken the action being described, creation of such a ceterms:CredentialingAction should be reserved to the agent of that action."@en-US ;
	vs:term_status vs:stable ;
	meta:changeHistory <http://credreg.net/ctdl/termhistory/ceterms/RenewAction/json> ;
	rdfs:subClassOf ceterms:CredentialingAction ;
	meta:domainFor ceterms:actingAgent, ceterms:actionStatusType, ceterms:description, ceterms:endDate, ceterms:evidenceOfAction, ceterms:instrument, ceterms:object, ceterms:participant, ceterms:resultingAward, ceterms:startDate .

ceterms:ResearchDoctorate a rdfs:Class ;
	rdfs:label "Research Doctorate"@en-US ;
	rdfs:comment "Doctoral degree conferred for advanced work beyond the master level, including the preparation and defense of a thesis or dissertation based on original research, or the planning and execution of an original project demonstrating substantial artistic or scholarly achievement."@en-US ;
	dct:description "Equivalent to an award at UNESCO ISCED 2011, Level 8."@en-US ;
	vs:term_status vs:stable ;
	meta:changeHistory <http://credreg.net/ctdl/termhistory/ceterms/ResearchDoctorate/json> ;
	rdfs:subClassOf ceterms:DoctoralDegree ;
	meta:domainFor ceterms:accreditedBy, ceterms:accreditedIn, ceterms:administrationProcess, ceterms:advancedStandingFrom, ceterms:aggregateData, ceterms:alternateName, ceterms:appealProcess, ceterms:approvedBy, ceterms:approvedIn, ceterms:assessmentDeliveryType, ceterms:audienceLevelType, ceterms:audienceType, ceterms:availabilityListing, ceterms:availableAt, ceterms:availableOnlineAt, ceterms:broadAlignment, ceterms:commonConditions, ceterms:commonCosts, ceterms:complaintProcess, ceterms:copyrightHolder, ceterms:corequisite, ceterms:credentialId, ceterms:credentialStatusType, ceterms:ctid, ceterms:dateEffective, ceterms:description, ceterms:developmentProcess, ceterms:earnings, ceterms:employmentOutcome, ceterms:estimatedCost, ceterms:estimatedDuration, ceterms:exactAlignment, ceterms:expirationDate, ceterms:financialAssistance, ceterms:hasPart, ceterms:hasProxy, ceterms:holders, ceterms:identifier, ceterms:image, ceterms:industryType, ceterms:inLanguage, ceterms:instructionalProgramType, ceterms:isAdvancedStandingFor, ceterms:isicV4, ceterms:isPartOf, ceterms:isPreparationFor, ceterms:isRecommendedFor, ceterms:isRequiredFor, ceterms:jurisdiction, ceterms:keyword, ceterms:latestVersion, ceterms:learningDeliveryType, ceterms:maintenanceProcess, ceterms:majorAlignment, ceterms:minorAlignment, ceterms:naics, ceterms:name, ceterms:narrowAlignment, ceterms:nextVersion, ceterms:occupationType, ceterms:offeredBy, ceterms:offeredIn, ceterms:ownedBy, ceterms:preparationFrom, ceterms:previousVersion, ceterms:processStandards, ceterms:processStandardsDescription, ceterms:recognizedBy, ceterms:recognizedIn, ceterms:recommends, ceterms:region, ceterms:regulatedBy, ceterms:regulatedIn, ceterms:relatedAction, ceterms:renewal, ceterms:renewalFrequency, ceterms:renewedBy, ceterms:renewedIn, ceterms:requires, ceterms:reviewProcess, ceterms:revocation, ceterms:revocationProcess, ceterms:revokedBy, ceterms:revokedIn, ceterms:sameAs, ceterms:subject, ceterms:subjectWebpage, ceterms:supersededBy, ceterms:supersedes, ceterms:targetPathway, ceterms:versionIdentifier .

ceterms:RevocationProfile a rdfs:Class ;
	rdfs:label "Revocation Profile"@en-US ;
	rdfs:comment "Entity describing conditions and methods by which a credential can be removed from a holder."@en-US ;
	vs:term_status vs:stable ;
	meta:changeHistory <http://credreg.net/ctdl/termhistory/ceterms/RevocationProfile/json> ;
	rdfs:subClassOf schema:CreativeWork ;
	meta:domainFor ceterms:dateEffective, ceterms:description, ceterms:jurisdiction, ceterms:region, ceterms:revocationCriteria, ceterms:revocationCriteriaDescription .

ceterms:RevokeAction a rdfs:Class ;
	rdfs:label "Revoke Action"@en-US ;
	rdfs:comment "Action by an agent removing an awarded credential (credential assertion) from the credential holder based on violations or failure of the holder to renew."@en-US ;
	dct:description "Since an instance of ceterms:CredentialingAction is a claim that a certain agent has taken the action being described, creation of such a ceterms:CredentialingAction should be reserved to the agent of that action."@en-US ;
	vs:term_status vs:stable ;
	meta:changeHistory <http://credreg.net/ctdl/termhistory/ceterms/RevokeAction/json> ;
	rdfs:subClassOf ceterms:CredentialingAction ;
	meta:domainFor ceterms:actingAgent, ceterms:actionStatusType, ceterms:description, ceterms:endDate, ceterms:evidenceOfAction, ceterms:instrument, ceterms:object, ceterms:participant, ceterms:startDate .

ceterms:RightsAction a rdfs:Class ;
	rdfs:label "Rights Action"@en-US ;
	rdfs:comment "Action asserting legal rights by an agent to possess, defend, transfer, license, and grant conditional access to a credential, learning opportunity, or assessment."@en-US ;
	dct:description "Since an instance of ceterms:CredentialingAction is a claim that a certain agent has taken the action being described, creation of such a ceterms:CredentialingAction should be reserved to the agent of that action."@en-US ;
	vs:term_status vs:stable ;
	meta:changeHistory <http://credreg.net/ctdl/termhistory/ceterms/RightsAction/json> ;
	rdfs:subClassOf ceterms:CredentialingAction ;
	meta:domainFor ceterms:actingAgent, ceterms:actionStatusType, ceterms:description, ceterms:endDate, ceterms:evidenceOfAction, ceterms:instrument, ceterms:object, ceterms:participant, ceterms:startDate .

ceterms:ScheduledOffering a rdfs:Class ;
	rdfs:label "Scheduled Offering"@en-US ;
	rdfs:comment "Offering of a Learning Opportunity or Assessment with a schedule associated with a specified location or modality."@en-US ;
	dct:description "Provides data specific to a given scheduled offering; the Learning Opportunity (including Course and Learning Program) or Assessment being offered provides all data that is shared between different offerings."@en-US ;
	vann:usageNote "Rather than repeating data, only use this class if the data differs from the data provided by the resource for which this is an offer."@en-US ;
	vs:term_status vs:unstable ;
	meta:changeHistory <http://credreg.net/ctdl/termhistory/ceterms/ScheduledOffering/json> ;
	meta:domainFor ceterms:aggregateData, ceterms:availabilityListing, ceterms:availableAt, ceterms:availableOnlineAt, ceterms:commonCosts, ceterms:ctid, ceterms:deliveryType, ceterms:deliveryTypeDescription, ceterms:description, ceterms:estimatedCost, ceterms:estimatedDuration, ceterms:name, ceterms:offeredBy, ceterms:offerFrequencyType, ceterms:scheduleFrequencyType, ceterms:scheduleTimingType, ceterms:subjectWebpage .

ceterms:SecondarySchoolDiploma a rdfs:Class ;
	rdfs:label "Secondary School Diploma"@en-US ;
	rdfs:comment "Diploma awarded by secondary education institutions for successful completion of a secondary school program of study."@en-US ;
	dct:description "Equivalent to an award at UNESCO ISCED 2011 Levels 2 or 3."@en-US ;
	vs:term_status vs:stable ;
	meta:changeHistory <http://credreg.net/ctdl/termhistory/ceterms/SecondarySchoolDiploma/json> ;
	rdfs:subClassOf ceterms:Diploma ;
	meta:domainFor ceterms:accreditedBy, ceterms:accreditedIn, ceterms:administrationProcess, ceterms:advancedStandingFrom, ceterms:aggregateData, ceterms:alternateName, ceterms:appealProcess, ceterms:approvedBy, ceterms:approvedIn, ceterms:assessmentDeliveryType, ceterms:audienceLevelType, ceterms:audienceType, ceterms:availabilityListing, ceterms:availableAt, ceterms:availableOnlineAt, ceterms:broadAlignment, ceterms:commonConditions, ceterms:commonCosts, ceterms:complaintProcess, ceterms:copyrightHolder, ceterms:corequisite, ceterms:credentialId, ceterms:credentialStatusType, ceterms:ctid, ceterms:dateEffective, ceterms:description, ceterms:developmentProcess, ceterms:earnings, ceterms:employmentOutcome, ceterms:estimatedCost, ceterms:estimatedDuration, ceterms:exactAlignment, ceterms:expirationDate, ceterms:financialAssistance, ceterms:hasPart, ceterms:hasProxy, ceterms:holders, ceterms:identifier, ceterms:image, ceterms:industryType, ceterms:inLanguage, ceterms:instructionalProgramType, ceterms:isAdvancedStandingFor, ceterms:isicV4, ceterms:isPartOf, ceterms:isPreparationFor, ceterms:isRecommendedFor, ceterms:isRequiredFor, ceterms:jurisdiction, ceterms:keyword, ceterms:latestVersion, ceterms:learningDeliveryType, ceterms:maintenanceProcess, ceterms:majorAlignment, ceterms:minorAlignment, ceterms:naics, ceterms:name, ceterms:narrowAlignment, ceterms:nextVersion, ceterms:occupationType, ceterms:offeredBy, ceterms:offeredIn, ceterms:ownedBy, ceterms:preparationFrom, ceterms:previousVersion, ceterms:processStandards, ceterms:processStandardsDescription, ceterms:recognizedBy, ceterms:recognizedIn, ceterms:recommends, ceterms:region, ceterms:regulatedBy, ceterms:regulatedIn, ceterms:relatedAction, ceterms:renewal, ceterms:renewalFrequency, ceterms:renewedBy, ceterms:renewedIn, ceterms:requires, ceterms:reviewProcess, ceterms:revocation, ceterms:revocationProcess, ceterms:revokedBy, ceterms:revokedIn, ceterms:sameAs, ceterms:subject, ceterms:subjectWebpage, ceterms:supersededBy, ceterms:supersedes, ceterms:targetPathway, ceterms:versionIdentifier .

ceterms:Task a rdfs:Class ;
	rdfs:label "Task"@en-US ;
	rdfs:comment "Specific activity, typically related to performing a function or achieving a goal."@en-US ;
	vs:term_status vs:stable ;
	meta:changeHistory <http://credreg.net/ctdl/termhistory/ceterms/Task/json> ;
	meta:domainFor ceasn:abilityEmbodied, ceasn:comment, ceasn:hasChild, ceasn:isChildOf, ceasn:knowledgeEmbodied, ceasn:listID, ceasn:skillEmbodied, ceterms:classification, ceterms:codedNotation, ceterms:ctid, ceterms:description, ceterms:environmentalHazardType, ceterms:identifier, ceterms:isMemberOf, ceterms:name, ceterms:performanceLevelType, ceterms:physicalCapabilityType, ceterms:sensoryCapabilityType, ceterms:versionIdentifier .

ceterms:TransferIntermediary a rdfs:Class ;
	rdfs:label "Transfer Intermediary"@en-US ;
	rdfs:comment "Surrogate resource to which other resources are mapped in order to indicate their common transferability."@en-US ;
	vann:usageNote "Used when multiple resources such as courses are grouped together to indicate they have mutually agreed upon transfer value."@en-US ;
	vs:term_status vs:unstable ;
	meta:changeHistory <http://credreg.net/ctdl/termhistory/ceterms/TransferIntermediary/json> ;
	meta:domainFor ceterms:codedNotation, ceterms:creditValue, ceterms:ctid, ceterms:description, ceterms:intermediaryFor, ceterms:name, ceterms:ownedBy, ceterms:requires, ceterms:subject, ceterms:subjectWebpage .

ceterms:TransferValueProfile a rdfs:Class ;
	rdfs:label "Transfer Value Profile"@en-US ;
	rdfs:comment "Description of transfer value of a resource."@en-US ;
	vs:term_status vs:stable ;
	meta:changeHistory <http://credreg.net/ctdl/termhistory/ceterms/TransferValueProfile/json> ;
	meta:domainFor ceterms:ctid, ceterms:description, ceterms:developmentProcess, ceterms:endDate, ceterms:identifier, ceterms:lifeCycleStatusType, ceterms:name, ceterms:ownedBy, ceterms:startDate, ceterms:subjectWebpage, ceterms:supersededBy, ceterms:supersedes, ceterms:transferValue, ceterms:transferValueFor, ceterms:transferValueFrom .

ceterms:ValueProfile a rdfs:Class ;
	rdfs:label "Value Profile"@en-US ;
	rdfs:comment "A description of value awarded for, required by, or otherwise related to the resource."@en-US ;
	vs:term_status vs:stable ;
	meta:changeHistory <http://credreg.net/ctdl/termhistory/ceterms/ValueProfile/json> ;
	rdfs:subClassOf schema:QuantitativeValue ;
	meta:domainFor ceterms:creditLevelType, ceterms:creditUnitType, ceterms:subject, qdata:percentage, schema:description, schema:maxValue, schema:minValue, schema:value .

ceterms:VerificationServiceProfile a rdfs:Class ;
	rdfs:label "Verification Service Profile"@en-US ;
	rdfs:comment "Entity describing the means by which someone can verify whether a credential has been attained."@en-US ;
	dct:description "Includes, but is not limited to, verification of whether quality assurance credentials have been issued for organizations, learning opportunities, and assessments."@en-US ;
	vs:term_status vs:stable ;
	meta:changeHistory <http://credreg.net/ctdl/termhistory/ceterms/VerificationServiceProfile/json> ;
	rdfs:subClassOf schema:Intangible ;
	meta:domainFor ceterms:dateEffective, ceterms:description, ceterms:estimatedCost, ceterms:holderMustAuthorize, ceterms:jurisdiction, ceterms:offeredBy, ceterms:offeredIn, ceterms:region, ceterms:subjectWebpage, ceterms:targetCredential, ceterms:verificationDirectory, ceterms:verificationMethodDescription, ceterms:verificationService, ceterms:verifiedClaimType .

ceterms:WorkExperienceComponent a rdfs:Class ;
	rdfs:label "Work Experience Component"@en-US ;
	rdfs:comment "Resource describing an activity or training through which a person gains job experience."@en-US ;
	dct:description "Instances act as proxies or stand-ins for other resources in the context of a particular pathway so that relationships between them as components of that pathway can be stated without implying that the those relationships are true of the resources in other contexts."@en-US ;
	vs:term_status vs:stable ;
	meta:changeHistory <http://credreg.net/ctdl/termhistory/ceterms/WorkExperienceComponent/json> ;
	rdfs:subClassOf ceterms:PathwayComponent ;
	meta:domainFor ceasn:hasChild, ceasn:isChildOf, ceterms:componentDesignation, ceterms:ctid, ceterms:description, ceterms:hasCondition, ceterms:identifier, ceterms:isDestinationComponentOf, ceterms:isPartOf, ceterms:name, ceterms:pointValue, ceterms:precededBy, ceterms:precedes, ceterms:proxyFor, ceterms:sourceData, ceterms:subjectWebpage .

ceterms:WorkforceDemandAction a rdfs:Class ;
	rdfs:label "Workforce Demand Action"@en-US ;
	rdfs:comment "Action taken by an agent asserting that the resource being described has a workforce demand level worthy of note."@en-US ;
	vs:term_status vs:unstable ;
	meta:changeHistory <http://credreg.net/ctdl/termhistory/ceterms/WorkforceDemandAction/json> ;
	rdfs:subClassOf ceterms:CredentialingAction ;
	meta:domainFor ceterms:actingAgent, ceterms:actionStatusType, ceterms:ctid, ceterms:description, ceterms:endDate, ceterms:evidenceOfAction, ceterms:instrument, ceterms:jurisdiction, ceterms:object, ceterms:participant, ceterms:result, ceterms:startDate .

ceterms:WorkRole a rdfs:Class ;
	rdfs:label "Work Role"@en-US ;
	rdfs:comment "Collection of tasks and competencies that embody a particular function in one or more jobs."@en-US ;
	vs:term_status vs:stable ;
	meta:changeHistory <http://credreg.net/ctdl/termhistory/ceterms/WorkRole/json> ;
	meta:domainFor ceasn:abilityEmbodied, ceasn:comment, ceasn:knowledgeEmbodied, ceasn:skillEmbodied, ceterms:classification, ceterms:codedNotation, ceterms:ctid, ceterms:description, ceterms:environmentalHazardType, ceterms:hasTask, ceterms:identifier, ceterms:isMemberOf, ceterms:name, ceterms:performanceLevelType, ceterms:physicalCapabilityType, ceterms:sensoryCapabilityType, ceterms:versionIdentifier .

schema:QuantitativeValue a rdfs:Class ;
	rdfs:label "Quantitative Value"@en-US ;
	rdfs:comment "A point value or interval for product characteristics and other purposes."@en-US ;
	vann:usageNote "Use in CTDL to describe quantitative values such as minimum and maximum credits or credit hours, etc."@en-US ;
	vs:term_status vs:stable ;
	meta:changeHistory <http://credreg.net/ctdl/termhistory/schema/QuantitativeValue/json> ;
	meta:domainFor qdata:percentage, schema:description, schema:maxValue, schema:minValue, schema:unitText, schema:value .

#====================
# PROPERTIES
#====================
ceasn:abilityEmbodied a rdf:Property ;
	rdfs:label "Ability Embodied"@en-US ;
	rdfs:comment "Enduring attributes of the individual that influence performance are embodied either directly or indirectly in this resource."@en-US ;
	vann:usageNote "The abilityEmbodied property may referenced a defined ability in an ontology such as O*NET or an existing competency defined in a competency framework."@en-US ;
	vs:term_status vs:stable ;
	meta:changeHistory <http://credreg.net/ctdl/termhistory/ceasn/abilityEmbodied/json> ;
	schema:domainIncludes ceasn:Competency, ceterms:Job, ceterms:Occupation, ceterms:Task, ceterms:WorkRole ;
	schema:rangeIncludes xsd:anyURI .

ceasn:comment a rdf:Property ;
	rdfs:label "Comment"@en-US ;
	rdfs:comment "Supplemental text provided by the promulgating body that clarifies the nature, scope or use of this resource."@en-US ;
	dct:description "Use this property when the text provides useful context for this resource."@en-US ;
	vs:term_status vs:stable ;
	meta:changeHistory <http://credreg.net/ctdl/termhistory/ceasn/comment/json> ;
	schema:domainIncludes ceasn:Competency, ceterms:Job, ceterms:Occupation, ceterms:Task, ceterms:WorkRole ;
	schema:rangeIncludes rdf:langString ;
	owl:equivalentProperty asn:comment, <https://purl.imsglobal.org/spec/case/v1p0/notes> .

ceasn:hasChild a rdf:Property ;
	rdfs:label "Has Child"@en-US ;
	rdfs:comment "The referenced resource is lower in some arbitrary hierarchy than this resource."@en-US ;
	dct:description "This property identifies a child node in the downward path in the chain of resources in a taxon path."@en-US ;
	vs:term_status vs:stable ;
	meta:changeHistory <http://credreg.net/ctdl/termhistory/ceasn/hasChild/json> ;
	rdfs:subPropertyOf dc:relation ;
	schema:domainIncludes ceasn:Competency, ceterms:AssessmentComponent, ceterms:BasicComponent, ceterms:CocurricularComponent, ceterms:CompetencyComponent, ceterms:CourseComponent, ceterms:CredentialComponent, ceterms:ExtracurricularComponent, ceterms:JobComponent, ceterms:Task, ceterms:WorkExperienceComponent ;
	schema:rangeIncludes ceasn:Competency, ceterms:AssessmentComponent, ceterms:BasicComponent, ceterms:CocurricularComponent, ceterms:CompetencyComponent, ceterms:CourseComponent, ceterms:CredentialComponent, ceterms:ExtracurricularComponent, ceterms:JobComponent, ceterms:Task, ceterms:WorkExperienceComponent ;
	owl:equivalentProperty gemq:hasChild .

ceasn:isChildOf a rdf:Property ;
	rdfs:label "Is Child Of"@en-US ;
	rdfs:comment "The referenced resource is higher in some arbitrary hierarchy than this resource."@en-US ;
	vs:term_status vs:stable ;
	meta:changeHistory <http://credreg.net/ctdl/termhistory/ceasn/isChildOf/json> ;
	rdfs:subPropertyOf dc:relation ;
	schema:domainIncludes ceasn:Competency, ceterms:AssessmentComponent, ceterms:BasicComponent, ceterms:CocurricularComponent, ceterms:CompetencyComponent, ceterms:CourseComponent, ceterms:CredentialComponent, ceterms:ExtracurricularComponent, ceterms:JobComponent, ceterms:Task, ceterms:WorkExperienceComponent ;
	schema:rangeIncludes ceasn:Competency, ceterms:AssessmentComponent, ceterms:BasicComponent, ceterms:CocurricularComponent, ceterms:CompetencyComponent, ceterms:CourseComponent, ceterms:CredentialComponent, ceterms:ExtracurricularComponent, ceterms:JobComponent, ceterms:Pathway, ceterms:Task, ceterms:WorkExperienceComponent ;
	owl:equivalentProperty gemq:isChildOf .

ceasn:knowledgeEmbodied a rdf:Property ;
	rdfs:label "Knowledge Embodied"@en-US ;
	rdfs:comment "Body of information embodied either directly or indirectly in this resource."@en-US ;
	vs:term_status vs:stable ;
	meta:changeHistory <http://credreg.net/ctdl/termhistory/ceasn/knowledgeEmbodied/json> ;
	schema:domainIncludes ceasn:Competency, ceterms:Job, ceterms:Occupation, ceterms:Task, ceterms:WorkRole ;
	schema:rangeIncludes xsd:anyURI .

ceasn:listID a rdf:Property ;
	rdfs:label "List ID"@en-US ;
	rdfs:comment "An alphanumeric string indicating the relative position of a resource in an ordered list of resources such as \"A\", \"B\", or \"a\", \"b\", or \"I\", \"II\", or \"1\", \"2\"."@en-US ;
	vann:usageNote "Punctuation accompanying alphanumeric strings should not be included."@en-US ;
	vs:term_status vs:stable ;
	meta:changeHistory <http://credreg.net/ctdl/termhistory/ceasn/listID/json> ;
	rdfs:subPropertyOf asn:listID ;
	schema:domainIncludes ceasn:Competency, ceterms:Task ;
	schema:rangeIncludes xsd:string ;
	owl:equivalentProperty <https://purl.imsglobal.org/spec/case/v1p0/listEnumeration> .

ceasn:skillEmbodied a rdf:Property ;
	rdfs:label "Skill Embodied"@en-US ;
	rdfs:comment "Ability to apply knowledge and use know-how to complete tasks and solve problems including types or categories of developed proficiency or dexterity in mental operations and physical processes is embodied either directly or indirectly in this resource."@en-US ;
	vann:usageNote "The skillEmbodied property may reference a defined skill in an ontology such as O*NET or an existing competency defined in a competency framework."@en-US ;
	vs:term_status vs:stable ;
	meta:changeHistory <http://credreg.net/ctdl/termhistory/ceasn/skillEmbodied/json> ;
	schema:domainIncludes ceasn:Competency, ceterms:Job, ceterms:Occupation, ceterms:Task, ceterms:WorkRole ;
	schema:rangeIncludes xsd:anyURI ;
	owl:equivalentProperty asn:skillEmbodied .

ceterms:accreditedBy a rdf:Property ;
	rdfs:label "Accredited By"@en-US ;
	rdfs:comment "Quality assurance organization that provides official authorization to, or approval of, a credential, organization, assessment, or learning opportunity."@en-US ;
	vs:term_status vs:stable ;
	meta:changeHistory <http://credreg.net/ctdl/termhistory/ceterms/accreditedBy/json> ;
	schema:domainIncludes ceterms:ApprenticeshipCertificate, ceterms:AssessmentProfile, ceterms:AssociateDegree, ceterms:BachelorDegree, ceterms:Badge, ceterms:Certificate, ceterms:CertificateOfCompletion, ceterms:Certification, ceterms:Course, ceterms:Credential, ceterms:CredentialOrganization, ceterms:Degree, ceterms:DigitalBadge, ceterms:Diploma, ceterms:DoctoralDegree, ceterms:GeneralEducationDevelopment, ceterms:JourneymanCertificate, ceterms:LearningOpportunityProfile, ceterms:LearningProgram, ceterms:License, ceterms:MasterCertificate, ceterms:MasterDegree, ceterms:MicroCredential, ceterms:OpenBadge, ceterms:Organization, ceterms:ProfessionalDoctorate, ceterms:QACredentialOrganization, ceterms:QualityAssuranceCredential, ceterms:ResearchDoctorate, ceterms:SecondarySchoolDiploma ;
	schema:rangeIncludes ceterms:Organization, ceterms:QACredentialOrganization .

ceterms:accreditedIn a rdf:Property ;
	rdfs:label "Accredited In"@en-US ;
	rdfs:comment "Region or political jurisdiction such as a state, province or locale in which the credential, learning opportunity or assessment is accredited."@en-US ;
	vs:term_status vs:stable ;
	meta:changeHistory <http://credreg.net/ctdl/termhistory/ceterms/accreditedIn/json> ;
	schema:domainIncludes ceterms:ApprenticeshipCertificate, ceterms:AssessmentProfile, ceterms:AssociateDegree, ceterms:BachelorDegree, ceterms:Badge, ceterms:Certificate, ceterms:CertificateOfCompletion, ceterms:Certification, ceterms:Course, ceterms:Credential, ceterms:CredentialOrganization, ceterms:Degree, ceterms:DigitalBadge, ceterms:Diploma, ceterms:DoctoralDegree, ceterms:GeneralEducationDevelopment, ceterms:JourneymanCertificate, ceterms:LearningOpportunityProfile, ceterms:LearningProgram, ceterms:License, ceterms:MasterCertificate, ceterms:MasterDegree, ceterms:MicroCredential, ceterms:OpenBadge, ceterms:Organization, ceterms:ProfessionalDoctorate, ceterms:QACredentialOrganization, ceterms:QualityAssuranceCredential, ceterms:ResearchDoctorate, ceterms:SecondarySchoolDiploma ;
	schema:rangeIncludes ceterms:JurisdictionProfile .

ceterms:accredits a rdf:Property ;
	rdfs:label "Accredits"@en-US ;
	rdfs:comment "Credential, assessment, organization, or learning opportunity for which this organization provides official authorization or approval based on prescribed standards or criteria."@en-US ;
	vann:usageNote "Accredits includes the ongoing monitoring to confirm continued conformance to standards to maintain accreditation."@en-US ;
	vs:term_status vs:stable ;
	meta:changeHistory <http://credreg.net/ctdl/termhistory/ceterms/accredits/json> ;
	schema:domainIncludes ceterms:Organization, ceterms:QACredentialOrganization ;
	schema:rangeIncludes ceasn:CompetencyFramework, ceterms:ApprenticeshipCertificate, ceterms:AssessmentProfile, ceterms:AssociateDegree, ceterms:BachelorDegree, ceterms:Badge, ceterms:Certificate, ceterms:CertificateOfCompletion, ceterms:Certification, ceterms:Course, ceterms:Credential, ceterms:CredentialOrganization, ceterms:Degree, ceterms:DigitalBadge, ceterms:Diploma, ceterms:DoctoralDegree, ceterms:GeneralEducationDevelopment, ceterms:JourneymanCertificate, ceterms:LearningOpportunityProfile, ceterms:LearningProgram, ceterms:License, ceterms:MasterCertificate, ceterms:MasterDegree, ceterms:MicroCredential, ceterms:OpenBadge, ceterms:Organization, ceterms:ProfessionalDoctorate, ceterms:QACredentialOrganization, ceterms:QualityAssuranceCredential, ceterms:ResearchDoctorate, ceterms:SecondarySchoolDiploma .

ceterms:actingAgent a rdf:Property ;
	rdfs:label "Acting Agent"@en-US ;
	rdfs:comment "Organization or person performing an action."@en-US ;
	vs:term_status vs:stable ;
	meta:changeHistory <http://credreg.net/ctdl/termhistory/ceterms/actingAgent/json> ;
	schema:domainIncludes ceterms:AccreditAction, ceterms:AdvancedStandingAction, ceterms:ApproveAction, ceterms:CredentialingAction, ceterms:OfferAction, ceterms:RecognizeAction, ceterms:RegulateAction, ceterms:RenewAction, ceterms:RevokeAction, ceterms:RightsAction, ceterms:WorkforceDemandAction ;
	schema:rangeIncludes ceterms:CredentialOrganization, ceterms:Organization, ceterms:QACredentialOrganization ;
	owl:equivalentProperty schema:agent .

ceterms:actionStatusType a rdf:Property ;
	rdfs:label "Action Status Type"@en-US ;
	rdfs:comment "Entity describing the current disposition or standing of an action; select from an existing enumeration of such types."@en-US ;
	vs:term_status vs:stable ;
	meta:changeHistory <http://credreg.net/ctdl/termhistory/ceterms/actionStatusType/json> ;
	rdfs:subPropertyOf ceterms:credentialAlignment ;
	schema:domainIncludes ceterms:AccreditAction, ceterms:AdvancedStandingAction, ceterms:ApproveAction, ceterms:CredentialingAction, ceterms:OfferAction, ceterms:RecognizeAction, ceterms:RegulateAction, ceterms:RenewAction, ceterms:RevokeAction, ceterms:RightsAction, ceterms:WorkforceDemandAction ;
	schema:rangeIncludes ceterms:CredentialAlignmentObject ;
	meta:targetScheme ceterms:ActionStatus ;
	owl:equivalentProperty schema:actionStatusType .

ceterms:address a rdf:Property ;
	rdfs:label "Address"@en-US ;
	rdfs:comment "Particulars describing the location of the place."@en-US ;
	vs:term_status vs:stable ;
	meta:changeHistory <http://credreg.net/ctdl/termhistory/ceterms/address/json> ;
	schema:domainIncludes ceterms:CredentialOrganization, ceterms:Organization, ceterms:QACredentialOrganization ;
	schema:rangeIncludes ceterms:Place ;
	owl:equivalentProperty schema:address .

ceterms:addressCountry a rdf:Property ;
	rdfs:label "Address Country"@en-US ;
	rdfs:comment "Nation with its own government and occupying a particular territory identified by the two-letter ISO 3166-1 alpha-2 country code."@en-US ;
	vs:term_status vs:stable ;
	meta:changeHistory <http://credreg.net/ctdl/termhistory/ceterms/addressCountry/json> ;
	schema:domainIncludes ceterms:Place, ceterms:PostalAddress ;
	schema:rangeIncludes rdf:langString ;
	owl:equivalentProperty schema:addressCountry .

ceterms:addressLocality a rdf:Property ;
	rdfs:label "Address Locality"@en-US ;
	rdfs:comment "Town, city, or village in which a particular location is situtated."@en-US ;
	vs:term_status vs:stable ;
	meta:changeHistory <http://credreg.net/ctdl/termhistory/ceterms/addressLocality/json> ;
	schema:domainIncludes ceterms:Place, ceterms:PostalAddress ;
	schema:rangeIncludes rdf:langString ;
	owl:equivalentProperty schema:addressLocality .

ceterms:addressRegion a rdf:Property ;
	rdfs:label "Address Region"@en-US ;
	rdfs:comment "State or province in which a particular location is situated."@en-US ;
	vs:term_status vs:stable ;
	meta:changeHistory <http://credreg.net/ctdl/termhistory/ceterms/addressRegion/json> ;
	schema:domainIncludes ceterms:Place, ceterms:PostalAddress ;
	schema:rangeIncludes rdf:langString ;
	owl:equivalentProperty schema:addressRegion .

ceterms:administrationProcess a rdf:Property ;
	rdfs:label "Administration Process"@en-US ;
	rdfs:comment "Entity describing the process by which a credential, assessment, organization, or aspects of it, are administered."@en-US ;
	dct:description "Processes described include the execution of events and the development of resources in the lifecycle of a credential or organization, such as the process for the proctoring of assessments."@en-US ;
	vs:term_status vs:stable ;
	meta:changeHistory <http://credreg.net/ctdl/termhistory/ceterms/administrationProcess/json> ;
	schema:domainIncludes ceterms:ApprenticeshipCertificate, ceterms:AssessmentProfile, ceterms:AssociateDegree, ceterms:BachelorDegree, ceterms:Badge, ceterms:Certificate, ceterms:CertificateOfCompletion, ceterms:Certification, ceterms:Credential, ceterms:CredentialOrganization, ceterms:Degree, ceterms:DigitalBadge, ceterms:Diploma, ceterms:DoctoralDegree, ceterms:GeneralEducationDevelopment, ceterms:JourneymanCertificate, ceterms:License, ceterms:MasterCertificate, ceterms:MasterDegree, ceterms:MicroCredential, ceterms:OpenBadge, ceterms:Organization, ceterms:ProfessionalDoctorate, ceterms:QACredentialOrganization, ceterms:QualityAssuranceCredential, ceterms:ResearchDoctorate, ceterms:SecondarySchoolDiploma ;
	schema:rangeIncludes ceterms:ProcessProfile .

ceterms:advancedStandingFrom a rdf:Property ;
	rdfs:label "Advanced Standing From"@en-US ;
	rdfs:comment "Credential that has its time or cost reduced by another credential, assessment or learning opportunity."@en-US ;
	vs:term_status vs:stable ;
	meta:changeHistory <http://credreg.net/ctdl/termhistory/ceterms/advancedStandingFrom/json> ;
	schema:domainIncludes ceterms:ApprenticeshipCertificate, ceterms:AssessmentProfile, ceterms:AssociateDegree, ceterms:BachelorDegree, ceterms:Badge, ceterms:Certificate, ceterms:CertificateOfCompletion, ceterms:Certification, ceterms:Course, ceterms:Credential, ceterms:Degree, ceterms:DigitalBadge, ceterms:Diploma, ceterms:DoctoralDegree, ceterms:GeneralEducationDevelopment, ceterms:JourneymanCertificate, ceterms:LearningOpportunityProfile, ceterms:LearningProgram, ceterms:License, ceterms:MasterCertificate, ceterms:MasterDegree, ceterms:MicroCredential, ceterms:OpenBadge, ceterms:ProfessionalDoctorate, ceterms:QualityAssuranceCredential, ceterms:ResearchDoctorate, ceterms:SecondarySchoolDiploma ;
	schema:rangeIncludes ceterms:ApprenticeshipCertificate, ceterms:AssessmentProfile, ceterms:AssociateDegree, ceterms:BachelorDegree, ceterms:Badge, ceterms:Certificate, ceterms:CertificateOfCompletion, ceterms:Certification, ceterms:ConditionProfile, ceterms:Course, ceterms:Credential, ceterms:Degree, ceterms:DigitalBadge, ceterms:Diploma, ceterms:DoctoralDegree, ceterms:GeneralEducationDevelopment, ceterms:JourneymanCertificate, ceterms:LearningOpportunityProfile, ceterms:LearningProgram, ceterms:License, ceterms:MasterCertificate, ceterms:MasterDegree, ceterms:MicroCredential, ceterms:OpenBadge, ceterms:ProfessionalDoctorate, ceterms:QualityAssuranceCredential, ceterms:ResearchDoctorate, ceterms:SecondarySchoolDiploma .

ceterms:affiliatedAgent a rdf:Property ;
	rdfs:label "Affiliated Agent"@en-US ;
	rdfs:comment "Organization or person that plays some role in assigning, performing, assisting with, facilitating, approving of, or otherwise being involved with the task being described."@en-US ;
	vs:term_status vs:stable ;
	meta:changeHistory <http://credreg.net/ctdl/termhistory/ceterms/affiliatedAgent/json> ;
	schema:rangeIncludes ceterms:CredentialOrganization, ceterms:Organization, ceterms:QACredentialOrganization .

ceterms:affiliation a rdf:Property ;
	rdfs:label "Affiliation"@en-US ;
	rdfs:comment "Organization to which a person is formally related through work, sudy, or social engagement."@en-US ;
	vs:term_status vs:stable ;
	meta:changeHistory <http://credreg.net/ctdl/termhistory/ceterms/affiliation/json> ;
	schema:domainIncludes ceterms:CredentialPerson ;
	schema:rangeIncludes ceterms:CredentialOrganization, ceterms:Organization, ceterms:QACredentialOrganization ;
	owl:equivalentProperty schema:affiliation .

ceterms:agentPurpose a rdf:Property ;
	rdfs:label "Agent Purpose"@en-US ;
	rdfs:comment "Organization's primary purpose as found on an \"about\" page of a website."@en-US ;
	vs:term_status vs:stable ;
	meta:changeHistory <http://credreg.net/ctdl/termhistory/ceterms/agentPurpose/json> ;
	schema:domainIncludes ceterms:CredentialOrganization, ceterms:Organization, ceterms:QACredentialOrganization ;
	schema:rangeIncludes xsd:anyURI .

ceterms:agentPurposeDescription a rdf:Property ;
	rdfs:label "Agent Purpose Description"@en-US ;
	rdfs:comment "Short, key phrases describing the primary purpose of an organization as might be derived from the \"about\" page of it's website."@en-US ;
	vs:term_status vs:stable ;
	meta:changeHistory <http://credreg.net/ctdl/termhistory/ceterms/agentPurposeDescription/json> ;
	schema:domainIncludes ceterms:CredentialOrganization, ceterms:Organization, ceterms:QACredentialOrganization ;
	schema:rangeIncludes rdf:langString .

ceterms:agentSectorType a rdf:Property ;
	rdfs:label "Agent Sector Type"@en-US ;
	rdfs:comment "Type of sociological, economic, or political subdivision served by an organization; select from an existing enumeration of such types."@en-US ;
	vann:usageNote "Recommended best practice for credentials in the Credential Engine Registry is to use concepts from the ceterms:AgentSector vocabulary."@en-US ;
	vs:term_status vs:stable ;
	meta:changeHistory <http://credreg.net/ctdl/termhistory/ceterms/agentSectorType/json> ;
	rdfs:subPropertyOf ceterms:credentialAlignment ;
	schema:domainIncludes ceterms:CredentialOrganization, ceterms:Organization, ceterms:QACredentialOrganization ;
	schema:rangeIncludes ceterms:CredentialAlignmentObject ;
	meta:targetScheme ceterms:AgentSector .

ceterms:agentType a rdf:Property ;
	rdfs:label "Agent Type"@en-US ;
	rdfs:comment "Type of organization such as educational institution, credentialing organization or quality assurance body; select from an existing enumeration of such types."@en-US ;
	vann:usageNote "Best practice for developing credential descriptions for the Credential Engine Registry is to use the ceterms:OrganizationType vocabulary."@en-US ;
	vs:term_status vs:stable ;
	meta:changeHistory <http://credreg.net/ctdl/termhistory/ceterms/agentType/json> ;
	schema:domainIncludes ceterms:CredentialOrganization, ceterms:Organization, ceterms:QACredentialOrganization ;
	schema:rangeIncludes ceterms:CredentialAlignmentObject ;
	meta:targetScheme ceterms:OrganizationType .

ceterms:aggregateData a rdf:Property ;
	rdfs:label "Aggregate Data"@en-US ;
	rdfs:comment "Statistical information about the resource."@en-US ;
	vs:term_status vs:stable ;
	meta:changeHistory <http://credreg.net/ctdl/termhistory/ceterms/aggregateData/json> ;
	schema:domainIncludes ceterms:ApprenticeshipCertificate, ceterms:AssociateDegree, ceterms:BachelorDegree, ceterms:Badge, ceterms:Certificate, ceterms:CertificateOfCompletion, ceterms:Certification, ceterms:Credential, ceterms:Degree, ceterms:DigitalBadge, ceterms:Diploma, ceterms:DoctoralDegree, ceterms:GeneralEducationDevelopment, ceterms:JourneymanCertificate, ceterms:License, ceterms:MasterCertificate, ceterms:MasterDegree, ceterms:MicroCredential, ceterms:OpenBadge, ceterms:ProfessionalDoctorate, ceterms:QualityAssuranceCredential, ceterms:ResearchDoctorate, ceterms:ScheduledOffering, ceterms:SecondarySchoolDiploma ;
	schema:rangeIncludes ceterms:AggregateDataProfile .

ceterms:alignmentDate a rdf:Property ;
	rdfs:label "Alignment Date"@en-US ;
	rdfs:comment "The date  the alignment was made."@en-US ;
	vs:term_status vs:stable ;
	meta:changeHistory <http://credreg.net/ctdl/termhistory/ceterms/alignmentDate/json> ;
	rdfs:subPropertyOf ceterms:temporalCoverage ;
	schema:domainIncludes ceterms:CredentialAlignmentObject, ceterms:FinancialAlignmentObject ;
	schema:rangeIncludes xsd:date .

ceterms:alignmentType a rdf:Property ;
	rdfs:label "Alignment Type"@en-US ;
	rdfs:comment "Type of relationship between two entities."@en-US ;
	dct:description "In CTDL, the alignment type value is definitively identified by the property for which the AlignmentObject is the rdfs:range; therefore, use of this property is generally redundant."@en-US ;
	vs:term_status vs:stable ;
	meta:changeHistory <http://credreg.net/ctdl/termhistory/ceterms/alignmentType/json> ;
	schema:domainIncludes ceterms:CredentialAlignmentObject, ceterms:FinancialAlignmentObject ;
	schema:rangeIncludes xsd:string ;
	owl:equivalentProperty lrmi:alignmentType, schema:alignmentType .

ceterms:alternateName a rdf:Property ;
	rdfs:label "Alternate Name"@en-US ;
	rdfs:comment "Alias for the entity including acronyms, alpha-numeric notations, and other forms of name abbreviations in common use such as PhD, MA, and BA."@en-US ;
	vs:term_status vs:stable ;
	meta:changeHistory <http://credreg.net/ctdl/termhistory/ceterms/alternateName/json> ;
	schema:domainIncludes ceterms:ApprenticeshipCertificate, ceterms:AssociateDegree, ceterms:BachelorDegree, ceterms:Badge, ceterms:Certificate, ceterms:CertificateOfCompletion, ceterms:Certification, ceterms:Credential, ceterms:CredentialOrganization, ceterms:Degree, ceterms:DigitalBadge, ceterms:Diploma, ceterms:DoctoralDegree, ceterms:GeneralEducationDevelopment, ceterms:JourneymanCertificate, ceterms:License, ceterms:MasterCertificate, ceterms:MasterDegree, ceterms:MicroCredential, ceterms:OpenBadge, ceterms:Organization, ceterms:ProfessionalDoctorate, ceterms:QACredentialOrganization, ceterms:QualityAssuranceCredential, ceterms:ResearchDoctorate, ceterms:SecondarySchoolDiploma ;
	schema:rangeIncludes rdf:langString .

ceterms:alternativeCondition a rdf:Property ;
	rdfs:label "Alternative Condition"@en-US ;
	rdfs:comment "Constraints, prerequisites, entry conditions, or requirements in a context where more than one alternative condition or path has been defined and from which any one path fulfills the parent condition."@en-US ;
	dct:description "A set of alternative conditions are not necessarily mutually exclusive paths; for example, a set of alternative concentrations for a degree may allow a person to optionally complete more than one concentration even though only one is required to earn the degree."@en-US ;
	vs:term_status vs:stable ;
	meta:changeHistory <http://credreg.net/ctdl/termhistory/ceterms/alternativeCondition/json> ;
	schema:domainIncludes ceterms:ConditionProfile ;
	schema:rangeIncludes ceterms:ConditionProfile .

ceterms:appealProcess a rdf:Property ;
	rdfs:label "Appeal Process"@en-US ;
	rdfs:comment "Formal process for objecting to decisions of the organization regarding credentials, assessments or processes."@en-US ;
	vs:term_status vs:stable ;
	meta:changeHistory <http://credreg.net/ctdl/termhistory/ceterms/appealProcess/json> ;
	schema:domainIncludes ceterms:ApprenticeshipCertificate, ceterms:AssociateDegree, ceterms:BachelorDegree, ceterms:Badge, ceterms:Certificate, ceterms:CertificateOfCompletion, ceterms:Certification, ceterms:Credential, ceterms:CredentialOrganization, ceterms:Degree, ceterms:DigitalBadge, ceterms:Diploma, ceterms:DoctoralDegree, ceterms:GeneralEducationDevelopment, ceterms:JourneymanCertificate, ceterms:License, ceterms:MasterCertificate, ceterms:MasterDegree, ceterms:MicroCredential, ceterms:OpenBadge, ceterms:Organization, ceterms:ProfessionalDoctorate, ceterms:QACredentialOrganization, ceterms:QualityAssuranceCredential, ceterms:ResearchDoctorate, ceterms:SecondarySchoolDiploma ;
	schema:rangeIncludes ceterms:ProcessProfile .

ceterms:approvedBy a rdf:Property ;
	rdfs:label "Approved By"@en-US ;
	rdfs:comment "Organization that pronounces favorable judgment for this credential, assessment, learning opportunity, or organization."@en-US ;
	vs:term_status vs:stable ;
	meta:changeHistory <http://credreg.net/ctdl/termhistory/ceterms/approvedBy/json> ;
	schema:domainIncludes ceterms:ApprenticeshipCertificate, ceterms:AssessmentProfile, ceterms:AssociateDegree, ceterms:BachelorDegree, ceterms:Badge, ceterms:Certificate, ceterms:CertificateOfCompletion, ceterms:Certification, ceterms:Course, ceterms:Credential, ceterms:CredentialOrganization, ceterms:Degree, ceterms:DigitalBadge, ceterms:Diploma, ceterms:DoctoralDegree, ceterms:GeneralEducationDevelopment, ceterms:JourneymanCertificate, ceterms:LearningOpportunityProfile, ceterms:LearningProgram, ceterms:License, ceterms:MasterCertificate, ceterms:MasterDegree, ceterms:MicroCredential, ceterms:OpenBadge, ceterms:Organization, ceterms:ProfessionalDoctorate, ceterms:QACredentialOrganization, ceterms:QualityAssuranceCredential, ceterms:ResearchDoctorate, ceterms:SecondarySchoolDiploma ;
	schema:rangeIncludes ceterms:CredentialOrganization, ceterms:Organization, ceterms:QACredentialOrganization .

ceterms:approvedIn a rdf:Property ;
	rdfs:label "Approved In"@en-US ;
	rdfs:comment "Region or political jurisdiction such as a state, province or locale in which an organization pronounces favorable judgment for this credential, assessment, learning opportunity, or organization."@en-US ;
	vs:term_status vs:stable ;
	meta:changeHistory <http://credreg.net/ctdl/termhistory/ceterms/approvedIn/json> ;
	schema:domainIncludes ceterms:ApprenticeshipCertificate, ceterms:AssessmentProfile, ceterms:AssociateDegree, ceterms:BachelorDegree, ceterms:Badge, ceterms:Certificate, ceterms:CertificateOfCompletion, ceterms:Certification, ceterms:Course, ceterms:Credential, ceterms:CredentialOrganization, ceterms:Degree, ceterms:DigitalBadge, ceterms:Diploma, ceterms:DoctoralDegree, ceterms:GeneralEducationDevelopment, ceterms:JourneymanCertificate, ceterms:LearningOpportunityProfile, ceterms:LearningProgram, ceterms:License, ceterms:MasterCertificate, ceterms:MasterDegree, ceterms:MicroCredential, ceterms:OpenBadge, ceterms:Organization, ceterms:ProfessionalDoctorate, ceterms:QACredentialOrganization, ceterms:QualityAssuranceCredential, ceterms:ResearchDoctorate, ceterms:SecondarySchoolDiploma ;
	schema:rangeIncludes ceterms:JurisdictionProfile .

ceterms:approves a rdf:Property ;
	rdfs:label "Approves"@en-US ;
	rdfs:comment "Credential, assessment, learning opportunity, or organization for which this organization pronounces favorable judgment."@en-US ;
	vs:term_status vs:stable ;
	meta:changeHistory <http://credreg.net/ctdl/termhistory/ceterms/approves/json> ;
	schema:domainIncludes ceterms:CredentialOrganization, ceterms:Organization, ceterms:QACredentialOrganization ;
	schema:rangeIncludes ceasn:CompetencyFramework, ceterms:ApprenticeshipCertificate, ceterms:AssessmentProfile, ceterms:AssociateDegree, ceterms:BachelorDegree, ceterms:Badge, ceterms:Certificate, ceterms:CertificateOfCompletion, ceterms:Certification, ceterms:Course, ceterms:Credential, ceterms:CredentialOrganization, ceterms:CredentialPerson, ceterms:Degree, ceterms:DigitalBadge, ceterms:Diploma, ceterms:DoctoralDegree, ceterms:GeneralEducationDevelopment, ceterms:JourneymanCertificate, ceterms:LearningOpportunityProfile, ceterms:LearningProgram, ceterms:License, ceterms:MasterCertificate, ceterms:MasterDegree, ceterms:MicroCredential, ceterms:OpenBadge, ceterms:Organization, ceterms:ProfessionalDoctorate, ceterms:QACredentialOrganization, ceterms:QualityAssuranceCredential, ceterms:ResearchDoctorate, ceterms:SecondarySchoolDiploma .

ceterms:assertedBy a rdf:Property ;
	rdfs:label "Asserted By"@en-US ;
	rdfs:comment "Agent making a statement based on fact or belief."@en-US ;
	vs:term_status vs:stable ;
	meta:changeHistory <http://credreg.net/ctdl/termhistory/ceterms/assertedBy/json> ;
	schema:domainIncludes ceterms:ConditionProfile, ceterms:JurisdictionProfile ;
	schema:rangeIncludes ceterms:CredentialOrganization, ceterms:Organization, ceterms:QACredentialOrganization .

ceterms:assesses a rdf:Property ;
	rdfs:label "Assesses"@en-US ;
	rdfs:comment "Competency evaluated through the assessment."@en-US ;
	vs:term_status vs:stable ;
	meta:changeHistory <http://credreg.net/ctdl/termhistory/ceterms/assesses/json> ;
	rdfs:subPropertyOf ceterms:targetCompetency ;
	schema:domainIncludes ceterms:AssessmentProfile ;
	schema:rangeIncludes ceasn:Competency, ceterms:CredentialAlignmentObject .

ceterms:assessmentDeliveryType a rdf:Property ;
	rdfs:label "Assessment Delivery Type"@en-US ;
	rdfs:comment "Delivery type for the assessment for the credential."@en-US ;
	dct:description "Indicates the delivery type for the assessment for the credential."@en-US ;
	vs:term_status vs:stable ;
	meta:changeHistory <http://credreg.net/ctdl/termhistory/ceterms/assessmentDeliveryType/json> ;
	rdfs:subPropertyOf ceterms:deliveryType ;
	schema:domainIncludes ceterms:ApprenticeshipCertificate, ceterms:AssociateDegree, ceterms:BachelorDegree, ceterms:Badge, ceterms:Certificate, ceterms:CertificateOfCompletion, ceterms:Certification, ceterms:Credential, ceterms:Degree, ceterms:DigitalBadge, ceterms:Diploma, ceterms:DoctoralDegree, ceterms:GeneralEducationDevelopment, ceterms:JourneymanCertificate, ceterms:License, ceterms:MasterCertificate, ceterms:MasterDegree, ceterms:MicroCredential, ceterms:OpenBadge, ceterms:ProfessionalDoctorate, ceterms:QualityAssuranceCredential, ceterms:ResearchDoctorate, ceterms:SecondarySchoolDiploma ;
	schema:rangeIncludes ceterms:CredentialAlignmentObject ;
	meta:targetScheme ceterms:Delivery .

ceterms:assessmentExample a rdf:Property ;
	rdfs:label "Assessment Example"@en-US ;
	rdfs:comment "Example assessment or assessment item."@en-US ;
	vs:term_status vs:stable ;
	meta:changeHistory <http://credreg.net/ctdl/termhistory/ceterms/assessmentExample/json> ;
	schema:domainIncludes ceterms:AssessmentProfile ;
	schema:rangeIncludes xsd:anyURI .

ceterms:assessmentExampleDescription a rdf:Property ;
	rdfs:label "Assessment Example Description"@en-US ;
	rdfs:comment "Text of an example assessment or assessment item."@en-US ;
	vs:term_status vs:stable ;
	meta:changeHistory <http://credreg.net/ctdl/termhistory/ceterms/assessmentExampleDescription/json> ;
	schema:domainIncludes ceterms:AssessmentProfile ;
	schema:rangeIncludes rdf:langString .

ceterms:assessmentMethodDescription a rdf:Property ;
	rdfs:label "Assessment Method Description"@en-US ;
	rdfs:comment "Description of the methods used to conduct assessment."@en-US ;
	vs:term_status vs:stable ;
	meta:changeHistory <http://credreg.net/ctdl/termhistory/ceterms/assessmentMethodDescription/json> ;
	schema:domainIncludes ceterms:AssessmentProfile, ceterms:Course, ceterms:LearningOpportunityProfile, ceterms:LearningProgram ;
	schema:rangeIncludes rdf:langString .

ceterms:assessmentMethodType a rdf:Property ;
	rdfs:label "Assessment Method Type"@en-US ;
	rdfs:comment "Type of method used to conduct an assessment; select from an existing enumeration of such types."@en-US ;
	vann:usageNote "Best practice for developing credential descriptions for the Credential Engine Registry is to use the ceterms:AssessmentMethod vocabulary."@en-US ;
	vs:term_status vs:stable ;
	meta:changeHistory <http://credreg.net/ctdl/termhistory/ceterms/assessmentMethodType/json> ;
	schema:domainIncludes ceterms:AssessmentProfile, ceterms:Course, ceterms:LearningOpportunityProfile, ceterms:LearningProgram ;
	schema:rangeIncludes ceterms:CredentialAlignmentObject ;
	meta:targetScheme ceterms:AssessmentMethod .

ceterms:assessmentOutput a rdf:Property ;
	rdfs:label "Assessment Output"@en-US ;
	rdfs:comment "Description of the assessment artifact, performance or examination."@en-US ;
	vs:term_status vs:stable ;
	meta:changeHistory <http://credreg.net/ctdl/termhistory/ceterms/assessmentOutput/json> ;
	schema:domainIncludes ceterms:AssessmentProfile ;
	schema:rangeIncludes rdf:langString .

ceterms:assessmentUseType a rdf:Property ;
	rdfs:label "Assessment Use Type"@en-US ;
	rdfs:comment "Type of intended use of the assessment; select from an existing enumeration of such types."@en-US ;
	vann:usageNote "Best practice for developing credential descriptions for the Credential Engine Registry is to use the ceterms:AssessmentUse vocabulary."@en-US ;
	vs:term_status vs:stable ;
	meta:changeHistory <http://credreg.net/ctdl/termhistory/ceterms/assessmentUseType/json> ;
	schema:domainIncludes ceterms:AssessmentProfile ;
	schema:rangeIncludes ceterms:CredentialAlignmentObject ;
	meta:targetScheme ceterms:AssessmentUse .

ceterms:audienceLevelType a rdf:Property ;
	rdfs:label "Audience Level Type"@en-US ;
	rdfs:comment "Type of level indicating a point in a progression through an educational or training context, for which the credential is intended; select from an existing enumeration of such types."@en-US ;
	vann:usageNote "Best practice is to use terms from the CTDL Audience Level vocabulary."@en-US ;
	vs:term_status vs:stable ;
	meta:changeHistory <http://credreg.net/ctdl/termhistory/ceterms/audienceLevelType/json> ;
	rdfs:subPropertyOf ceterms:credentialAlignment ;
	schema:domainIncludes ceterms:ApprenticeshipCertificate, ceterms:AssessmentProfile, ceterms:AssociateDegree, ceterms:BachelorDegree, ceterms:Badge, ceterms:Certificate, ceterms:CertificateOfCompletion, ceterms:Certification, ceterms:ConditionProfile, ceterms:Course, ceterms:Credential, ceterms:Degree, ceterms:DigitalBadge, ceterms:Diploma, ceterms:DoctoralDegree, ceterms:GeneralEducationDevelopment, ceterms:JourneymanCertificate, ceterms:LearningOpportunityProfile, ceterms:LearningProgram, ceterms:License, ceterms:MasterCertificate, ceterms:MasterDegree, ceterms:MicroCredential, ceterms:OpenBadge, ceterms:ProfessionalDoctorate, ceterms:QualityAssuranceCredential, ceterms:ResearchDoctorate, ceterms:SecondarySchoolDiploma ;
	schema:rangeIncludes ceterms:CredentialAlignmentObject ;
	meta:targetScheme ceterms:AudienceLevel ;
	owl:equivalentProperty dct:educationLevel .

ceterms:audienceType a rdf:Property ;
	rdfs:label "Audience Type"@en-US ;
	rdfs:comment "The type of audience for which the resource is applicable, intended, or useful; select from an existing enumeration of such types."@en-US ;
	vann:usageNote "Best practice for developing credential descriptions for the Credential Engine Registry is to use the ceterms:Audience vocabulary."@en-US ;
	vs:term_status vs:stable ;
	meta:changeHistory <http://credreg.net/ctdl/termhistory/ceterms/audienceType/json> ;
	rdfs:subPropertyOf ceterms:credentialAlignment ;
	schema:domainIncludes ceterms:ApprenticeshipCertificate, ceterms:AssessmentProfile, ceterms:AssociateDegree, ceterms:BachelorDegree, ceterms:Badge, ceterms:Certificate, ceterms:CertificateOfCompletion, ceterms:Certification, ceterms:ConditionProfile, ceterms:CostProfile, ceterms:Course, ceterms:Credential, ceterms:Degree, ceterms:DigitalBadge, ceterms:Diploma, ceterms:DoctoralDegree, ceterms:GeneralEducationDevelopment, ceterms:JourneymanCertificate, ceterms:LearningOpportunityProfile, ceterms:LearningProgram, ceterms:License, ceterms:MasterCertificate, ceterms:MasterDegree, ceterms:MicroCredential, ceterms:OpenBadge, ceterms:ProfessionalDoctorate, ceterms:QualityAssuranceCredential, ceterms:ResearchDoctorate, ceterms:SecondarySchoolDiploma ;
	schema:rangeIncludes ceterms:CredentialAlignmentObject ;
	meta:targetScheme ceterms:Audience .

ceterms:availabilityListing a rdf:Property ;
	rdfs:label "Availability Listing"@en-US ;
	rdfs:comment "Listing of online and/or physical locations where a credential can be pursued."@en-US ;
	vs:term_status vs:stable ;
	meta:changeHistory <http://credreg.net/ctdl/termhistory/ceterms/availabilityListing/json> ;
	schema:domainIncludes ceterms:ApprenticeshipCertificate, ceterms:AssessmentProfile, ceterms:AssociateDegree, ceterms:BachelorDegree, ceterms:Badge, ceterms:Certificate, ceterms:CertificateOfCompletion, ceterms:Certification, ceterms:Course, ceterms:Credential, ceterms:CredentialOrganization, ceterms:Degree, ceterms:DigitalBadge, ceterms:Diploma, ceterms:DoctoralDegree, ceterms:GeneralEducationDevelopment, ceterms:JourneymanCertificate, ceterms:LearningOpportunityProfile, ceterms:LearningProgram, ceterms:License, ceterms:MasterCertificate, ceterms:MasterDegree, ceterms:MicroCredential, ceterms:OpenBadge, ceterms:Organization, ceterms:ProfessionalDoctorate, ceterms:QACredentialOrganization, ceterms:QualityAssuranceCredential, ceterms:ResearchDoctorate, ceterms:ScheduledOffering, ceterms:SecondarySchoolDiploma ;
	schema:rangeIncludes xsd:anyURI .

ceterms:availableAt a rdf:Property ;
	rdfs:label "Available At"@en-US ;
	rdfs:comment "Physical location where the credential, assessment, or learning opportunity can be pursued."@en-US ;
	vs:term_status vs:stable ;
	meta:changeHistory <http://credreg.net/ctdl/termhistory/ceterms/availableAt/json> ;
	rdfs:subPropertyOf ceterms:spatialCoverage ;
	schema:domainIncludes ceterms:ApprenticeshipCertificate, ceterms:AssessmentProfile, ceterms:AssociateDegree, ceterms:BachelorDegree, ceterms:Badge, ceterms:Certificate, ceterms:CertificateOfCompletion, ceterms:Certification, ceterms:Course, ceterms:Credential, ceterms:Degree, ceterms:DigitalBadge, ceterms:Diploma, ceterms:DoctoralDegree, ceterms:GeneralEducationDevelopment, ceterms:JourneymanCertificate, ceterms:LearningOpportunityProfile, ceterms:LearningProgram, ceterms:License, ceterms:MasterCertificate, ceterms:MasterDegree, ceterms:MicroCredential, ceterms:OpenBadge, ceterms:ProfessionalDoctorate, ceterms:QualityAssuranceCredential, ceterms:ResearchDoctorate, ceterms:ScheduledOffering, ceterms:SecondarySchoolDiploma ;
	schema:rangeIncludes ceterms:Place .

ceterms:availableOnlineAt a rdf:Property ;
	rdfs:label "Available Online At"@en-US ;
	rdfs:comment "Online location where the credential, assessment, or learning opportunity can be pursued."@en-US ;
	vs:term_status vs:stable ;
	meta:changeHistory <http://credreg.net/ctdl/termhistory/ceterms/availableOnlineAt/json> ;
	schema:domainIncludes ceterms:ApprenticeshipCertificate, ceterms:AssessmentProfile, ceterms:AssociateDegree, ceterms:BachelorDegree, ceterms:Badge, ceterms:Certificate, ceterms:CertificateOfCompletion, ceterms:Certification, ceterms:Course, ceterms:Credential, ceterms:Degree, ceterms:DigitalBadge, ceterms:Diploma, ceterms:DoctoralDegree, ceterms:GeneralEducationDevelopment, ceterms:JourneymanCertificate, ceterms:LearningOpportunityProfile, ceterms:LearningProgram, ceterms:License, ceterms:MasterCertificate, ceterms:MasterDegree, ceterms:MicroCredential, ceterms:OpenBadge, ceterms:ProfessionalDoctorate, ceterms:QualityAssuranceCredential, ceterms:ResearchDoctorate, ceterms:ScheduledOffering, ceterms:SecondarySchoolDiploma ;
	schema:rangeIncludes xsd:anyURI .

ceterms:broadAlignment a rdf:Property ;
	rdfs:label "Broad Alignment"@en-US ;
	rdfs:comment "Item that covers all of the relevant concepts in the item being described as well as additional relevant concepts."@en-US ;
	vs:term_status vs:stable ;
	meta:changeHistory <http://credreg.net/ctdl/termhistory/ceterms/broadAlignment/json> ;
	rdfs:subPropertyOf ceterms:isSimilarTo ;
	schema:domainIncludes ceterms:ApprenticeshipCertificate, ceterms:AssociateDegree, ceterms:BachelorDegree, ceterms:Badge, ceterms:Certificate, ceterms:CertificateOfCompletion, ceterms:Certification, ceterms:Credential, ceterms:Degree, ceterms:DigitalBadge, ceterms:Diploma, ceterms:DoctoralDegree, ceterms:GeneralEducationDevelopment, ceterms:JourneymanCertificate, ceterms:License, ceterms:MasterCertificate, ceterms:MasterDegree, ceterms:MicroCredential, ceterms:OpenBadge, ceterms:ProfessionalDoctorate, ceterms:QualityAssuranceCredential, ceterms:ResearchDoctorate, ceterms:SecondarySchoolDiploma ;
	schema:rangeIncludes ceterms:ApprenticeshipCertificate, ceterms:AssociateDegree, ceterms:BachelorDegree, ceterms:Badge, ceterms:Certificate, ceterms:CertificateOfCompletion, ceterms:Certification, ceterms:Credential, ceterms:Degree, ceterms:DigitalBadge, ceterms:Diploma, ceterms:DoctoralDegree, ceterms:GeneralEducationDevelopment, ceterms:JourneymanCertificate, ceterms:License, ceterms:MasterCertificate, ceterms:MasterDegree, ceterms:MicroCredential, ceterms:OpenBadge, ceterms:ProfessionalDoctorate, ceterms:QualityAssuranceCredential, ceterms:ResearchDoctorate, ceterms:SecondarySchoolDiploma ;
	owl:equivalentProperty asn:broadAlignment, skos:broader .

ceterms:classification a rdf:Property ;
	rdfs:label "Classification"@en-US ;
	rdfs:comment "Category or classification of this resource."@en-US ;
	vann:usageNote "Where a more specific property exists, such as ceterms:naics, ceterms:isicV4, ceterms:credentialType, etc., use that property instead of this one."@en-US ;
	vs:term_status vs:stable ;
	meta:changeHistory <http://credreg.net/ctdl/termhistory/ceterms/classification/json> ;
	schema:domainIncludes ceasn:Collection, ceterms:Collection, ceterms:Job, ceterms:Occupation, ceterms:Task, ceterms:WorkRole ;
	schema:rangeIncludes skos:Concept .

ceterms:codedNotation a rdf:Property ;
	rdfs:label "Coded Notation"@en-US ;
	rdfs:comment "Set of alpha-numeric symbols as defined by the body responsible for this resource that uniquely identifies this resource and supports its discovery and use."@en-US ;
	dct:description "Examples include the alpha-numeric code \"CCSS.MATH.CONTENT.HSA.CED.A.2\" identifying a node in the U.S. Common Core State Standards on creating equations in algebra, or, the code \"8021\" in the U.S. Standard Industrial Classification (SIC) for identifying the occupational context for \"Offices and Clinics of Dentists\"."@en-US ;
	vann:usageNote "For identifiers that come from a recognized identification scheme use the specific property for that identifier type, such as ceterms:opeID, ceterms:ncesID, ceterms:leiCode, etc., or use ceterms:identifier so that the identification schema can be named."@en-US ;
	vs:term_status vs:stable ;
	meta:changeHistory <http://credreg.net/ctdl/termhistory/ceterms/codedNotation/json> ;
	schema:domainIncludes ceterms:Collection, ceterms:Course, ceterms:CredentialAlignmentObject, ceterms:Job, ceterms:LearningOpportunityProfile, ceterms:LearningProgram, ceterms:Occupation, ceterms:Task, ceterms:TransferIntermediary, ceterms:WorkRole ;
	schema:rangeIncludes xsd:string .

ceterms:collectionType a rdf:Property ;
	rdfs:label "Collection Type"@en-US ;
	rdfs:comment "Type of collection, list, array, or other grouping of resources; select from an existing enumeration of such types."@en-US ;
	vs:term_status vs:unstable ;
	meta:changeHistory <http://credreg.net/ctdl/termhistory/ceterms/collectionType/json> ;
	schema:domainIncludes ceterms:Collection ;
	schema:rangeIncludes ceterms:CredentialAlignmentObject ;
	meta:targetScheme ceterms:CollectionCategory .

ceterms:commonConditions a rdf:Property ;
	rdfs:label "Common Conditions"@en-US ;
	rdfs:comment "Set constraints, prerequisites, entry conditions, or requirements that are shared across an organization, organizational subdivision, set of credentials, or category of entities and activities."@en-US ;
	vs:term_status vs:stable ;
	meta:changeHistory <http://credreg.net/ctdl/termhistory/ceterms/commonConditions/json> ;
	schema:domainIncludes ceterms:ApprenticeshipCertificate, ceterms:AssessmentProfile, ceterms:AssociateDegree, ceterms:BachelorDegree, ceterms:Badge, ceterms:Certificate, ceterms:CertificateOfCompletion, ceterms:Certification, ceterms:Course, ceterms:Credential, ceterms:Degree, ceterms:DigitalBadge, ceterms:Diploma, ceterms:DoctoralDegree, ceterms:GeneralEducationDevelopment, ceterms:JourneymanCertificate, ceterms:LearningOpportunityProfile, ceterms:LearningProgram, ceterms:License, ceterms:MasterCertificate, ceterms:MasterDegree, ceterms:MicroCredential, ceterms:OpenBadge, ceterms:ProfessionalDoctorate, ceterms:QualityAssuranceCredential, ceterms:ResearchDoctorate, ceterms:SecondarySchoolDiploma ;
	schema:rangeIncludes ceterms:ConditionManifest .

ceterms:commonCosts a rdf:Property ;
	rdfs:label "Common Costs"@en-US ;
	rdfs:comment "Set of costs maintained at an organizational or sub-organizational level, which apply to this credential, assessment, or learning opportunity."@en-US ;
	vs:term_status vs:stable ;
	meta:changeHistory <http://credreg.net/ctdl/termhistory/ceterms/commonCosts/json> ;
	schema:domainIncludes ceterms:ApprenticeshipCertificate, ceterms:AssessmentProfile, ceterms:AssociateDegree, ceterms:BachelorDegree, ceterms:Badge, ceterms:Certificate, ceterms:CertificateOfCompletion, ceterms:Certification, ceterms:ConditionProfile, ceterms:Course, ceterms:Credential, ceterms:Degree, ceterms:DigitalBadge, ceterms:Diploma, ceterms:DoctoralDegree, ceterms:GeneralEducationDevelopment, ceterms:JourneymanCertificate, ceterms:LearningOpportunityProfile, ceterms:LearningProgram, ceterms:License, ceterms:MasterCertificate, ceterms:MasterDegree, ceterms:MicroCredential, ceterms:OpenBadge, ceterms:ProfessionalDoctorate, ceterms:QualityAssuranceCredential, ceterms:ResearchDoctorate, ceterms:ScheduledOffering, ceterms:SecondarySchoolDiploma ;
	schema:rangeIncludes ceterms:CostManifest .

ceterms:comparator a rdf:Property ;
	rdfs:label "Comparator"@en-US ;
	rdfs:comment "Type of symbol that denotes an operator in a constraint expression such as \"GTEQ\" (greater than or equal to), \"EQ\" (equal to), \"LT\" (less than); select from an existing enumeration of such types."@en-US ;
	vs:term_status vs:unstable ;
	meta:changeHistory <http://credreg.net/ctdl/termhistory/ceterms/comparator/json> ;
	schema:domainIncludes ceterms:Constraint ;
	schema:rangeIncludes skos:Concept ;
	meta:targetScheme ceterms:ComparatorCategory .

ceterms:complaintProcess a rdf:Property ;
	rdfs:label "Complaint Process"@en-US ;
	rdfs:comment "Process for handling complaints about a credential, or aspects of it including related learning opportunities and assessments."@en-US ;
	vs:term_status vs:stable ;
	meta:changeHistory <http://credreg.net/ctdl/termhistory/ceterms/complaintProcess/json> ;
	schema:domainIncludes ceterms:ApprenticeshipCertificate, ceterms:AssociateDegree, ceterms:BachelorDegree, ceterms:Badge, ceterms:Certificate, ceterms:CertificateOfCompletion, ceterms:Certification, ceterms:Credential, ceterms:CredentialOrganization, ceterms:Degree, ceterms:DigitalBadge, ceterms:Diploma, ceterms:DoctoralDegree, ceterms:GeneralEducationDevelopment, ceterms:JourneymanCertificate, ceterms:License, ceterms:MasterCertificate, ceterms:MasterDegree, ceterms:MicroCredential, ceterms:OpenBadge, ceterms:Organization, ceterms:ProfessionalDoctorate, ceterms:QACredentialOrganization, ceterms:QualityAssuranceCredential, ceterms:ResearchDoctorate, ceterms:SecondarySchoolDiploma ;
	schema:rangeIncludes ceterms:ProcessProfile .

ceterms:componentCategory a rdf:Property ;
	rdfs:label "Component Category"@en-US ;
	rdfs:comment "Identifies the type of PathwayComponent subclass not explicitly covered in the current array of PathwayComponent subclasses."@en-US ;
	vs:term_status vs:stable ;
	meta:changeHistory <http://credreg.net/ctdl/termhistory/ceterms/componentCategory/json> ;
	schema:domainIncludes ceterms:BasicComponent, ceterms:CocurricularComponent, ceterms:ExtracurricularComponent ;
	schema:rangeIncludes rdf:langString .

ceterms:componentDesignation a rdf:Property ;
	rdfs:label "Component Designation"@en-US ;
	rdfs:comment "Label identifying the category to further distinguish one component from another as designated by the promulgating body."@en-US ;
	dct:description "Examples may include \"Required\", \"Core\", \"General Education\", \"Elective\", etc."@en-US ;
	vs:term_status vs:stable ;
	meta:changeHistory <http://credreg.net/ctdl/termhistory/ceterms/componentDesignation/json> ;
	schema:domainIncludes ceterms:AssessmentComponent, ceterms:BasicComponent, ceterms:CocurricularComponent, ceterms:CompetencyComponent, ceterms:CourseComponent, ceterms:CredentialComponent, ceterms:ExtracurricularComponent, ceterms:JobComponent, ceterms:WorkExperienceComponent ;
	schema:rangeIncludes ceterms:CredentialAlignmentObject .

ceterms:condition a rdf:Property ;
	rdfs:label "Condition"@en-US ;
	rdfs:comment "Single constraint, prerequisite, entry condition, requirement, or cost."@en-US ;
	vs:term_status vs:stable ;
	meta:changeHistory <http://credreg.net/ctdl/termhistory/ceterms/condition/json> ;
	rdfs:subPropertyOf ceterms:description ;
	schema:domainIncludes ceterms:ConditionProfile, ceterms:CostProfile ;
	schema:rangeIncludes rdf:langString .

ceterms:conditionManifestOf a rdf:Property ;
	rdfs:label "Condition Manifest Of"@en-US ;
	rdfs:comment "Organization maintaining the condition manifest."@en-US ;
	vs:term_status vs:stable ;
	meta:changeHistory <http://credreg.net/ctdl/termhistory/ceterms/conditionManifestOf/json> ;
	schema:domainIncludes ceterms:ConditionManifest ;
	schema:rangeIncludes ceterms:CredentialOrganization, ceterms:Organization, ceterms:QACredentialOrganization .

ceterms:contactType a rdf:Property ;
	rdfs:label "Contact Type"@en-US ;
	rdfs:comment "Text identifying the type of service provided by an organizational contact."@en-US ;
	dct:description "A person or organization may have different contact points for different services. The contact type property provides for adding text to identity the service; e.g., \"toll-free number\" or \"support for hearing-impaired callers\"."@en-US ;
	vs:term_status vs:stable ;
	meta:changeHistory <http://credreg.net/ctdl/termhistory/ceterms/contactType/json> ;
	schema:domainIncludes ceterms:ContactPoint ;
	schema:rangeIncludes rdf:langString .

ceterms:copyrightHolder a rdf:Property ;
	rdfs:label "Copyright Holder"@en-US ;
	rdfs:comment "Person or organization holding the rights in copyright to entities such as credentials, learning opportunities, assessments, competencies or concept schemes."@en-US ;
	vs:term_status vs:stable ;
	meta:changeHistory <http://credreg.net/ctdl/termhistory/ceterms/copyrightHolder/json> ;
	schema:domainIncludes ceterms:ApprenticeshipCertificate, ceterms:AssociateDegree, ceterms:BachelorDegree, ceterms:Badge, ceterms:Certificate, ceterms:CertificateOfCompletion, ceterms:Certification, ceterms:Credential, ceterms:Degree, ceterms:DigitalBadge, ceterms:Diploma, ceterms:DoctoralDegree, ceterms:GeneralEducationDevelopment, ceterms:JourneymanCertificate, ceterms:License, ceterms:MasterCertificate, ceterms:MasterDegree, ceterms:MicroCredential, ceterms:OpenBadge, ceterms:ProfessionalDoctorate, ceterms:QualityAssuranceCredential, ceterms:ResearchDoctorate, ceterms:SecondarySchoolDiploma ;
	schema:rangeIncludes ceterms:CredentialOrganization, ceterms:CredentialPerson, ceterms:Organization, ceterms:QACredentialOrganization ;
	owl:equivalentProperty schema:copyrightHolder .

ceterms:corequisite a rdf:Property ;
	rdfs:label "Corequisite"@en-US ;
	rdfs:comment "Credentials that must be pursued concurrently."@en-US ;
	dct:description "Includes dual (double) degrees that cannot be earned independently of each other."@en-US ;
	vs:term_status vs:stable ;
	meta:changeHistory <http://credreg.net/ctdl/termhistory/ceterms/corequisite/json> ;
	schema:domainIncludes ceterms:ApprenticeshipCertificate, ceterms:AssessmentProfile, ceterms:AssociateDegree, ceterms:BachelorDegree, ceterms:Badge, ceterms:Certificate, ceterms:CertificateOfCompletion, ceterms:Certification, ceterms:ConditionManifest, ceterms:Course, ceterms:Credential, ceterms:Degree, ceterms:DigitalBadge, ceterms:Diploma, ceterms:DoctoralDegree, ceterms:GeneralEducationDevelopment, ceterms:JourneymanCertificate, ceterms:LearningOpportunityProfile, ceterms:LearningProgram, ceterms:License, ceterms:MasterCertificate, ceterms:MasterDegree, ceterms:MicroCredential, ceterms:OpenBadge, ceterms:ProfessionalDoctorate, ceterms:QualityAssuranceCredential, ceterms:ResearchDoctorate, ceterms:SecondarySchoolDiploma ;
	schema:rangeIncludes ceterms:ConditionProfile .

ceterms:costDetails a rdf:Property ;
	rdfs:label "Cost Details"@en-US ;
	rdfs:comment "Webpage or online document containing human-readable, in-depth information about costs."@en-US ;
	vs:term_status vs:stable ;
	meta:changeHistory <http://credreg.net/ctdl/termhistory/ceterms/costDetails/json> ;
	schema:domainIncludes ceterms:CostManifest, ceterms:CostProfile ;
	schema:rangeIncludes xsd:anyURI .

ceterms:costManifestOf a rdf:Property ;
	rdfs:label "Cost Manifest Of"@en-US ;
	rdfs:comment "Organization maintaining the cost manifest."@en-US ;
	vs:term_status vs:stable ;
	meta:changeHistory <http://credreg.net/ctdl/termhistory/ceterms/costManifestOf/json> ;
	schema:domainIncludes ceterms:CostManifest ;
	schema:rangeIncludes ceterms:CredentialOrganization, ceterms:Organization, ceterms:QACredentialOrganization .

ceterms:credentialId a rdf:Property ;
	rdfs:label "Credential Identifier"@en-US ;
	rdfs:comment "Globally unique identifier by which the creator, owner or provider of a credential recognizes that credential in transactions with the external environment (e.g., in verifiable claims involving the credential)."@en-US ;
	dct:description "The  identifier may take the form of a URN, UUID, ARK, DOI, INFO or any other publicly recognized, globally unique identifier scheme."@en-US ;
	vann:usageNote "Best practice for descriptions intended for the Credential Engine Registry is to use the ceterms:ctid property for this purpose; ceterms:ctid is declared as a subproperty of ceterms:credentialId."@en-US ;
	vs:term_status vs:stable ;
	meta:changeHistory <http://credreg.net/ctdl/termhistory/ceterms/credentialId/json> ;
	schema:domainIncludes ceterms:ApprenticeshipCertificate, ceterms:AssociateDegree, ceterms:BachelorDegree, ceterms:Badge, ceterms:Certificate, ceterms:CertificateOfCompletion, ceterms:Certification, ceterms:Credential, ceterms:Degree, ceterms:DigitalBadge, ceterms:Diploma, ceterms:DoctoralDegree, ceterms:GeneralEducationDevelopment, ceterms:JourneymanCertificate, ceterms:License, ceterms:MasterCertificate, ceterms:MasterDegree, ceterms:MicroCredential, ceterms:OpenBadge, ceterms:ProfessionalDoctorate, ceterms:QualityAssuranceCredential, ceterms:ResearchDoctorate, ceterms:SecondarySchoolDiploma ;
	schema:rangeIncludes xsd:string .

ceterms:credentialingAction a rdf:Property ;
	rdfs:label "Credentialing Action"@en-US ;
	rdfs:comment "Indicates a past or potential credentialing action in which the resource being described plays an 'object' role."@en-US ;
	vs:term_status vs:stable ;
	meta:changeHistory <http://credreg.net/ctdl/termhistory/ceterms/credentialingAction/json> ;
	schema:domainIncludes ceterms:CredentialOrganization, ceterms:Organization, ceterms:QACredentialOrganization ;
	schema:rangeIncludes ceterms:AccreditAction, ceterms:AdvancedStandingAction, ceterms:ApproveAction, ceterms:CredentialingAction, ceterms:OfferAction, ceterms:RecognizeAction, ceterms:RegulateAction, ceterms:RenewAction, ceterms:RevokeAction, ceterms:RightsAction .

ceterms:credentialStatusType a rdf:Property ;
	rdfs:label "Credential Status Type"@en-US ;
	rdfs:comment "Type of official status of the credential; select from an enumeration of such types."@en-US ;
	vann:usageNote "Best practice for developing credential descriptions for the Credential Engine Registry is to use the ceterms:CredentialStatus vocabulary."@en-US ;
	vs:term_status vs:stable ;
	meta:changeHistory <http://credreg.net/ctdl/termhistory/ceterms/credentialStatusType/json> ;
	rdfs:subPropertyOf ceterms:lifeCycleStatusType ;
	schema:domainIncludes ceterms:ApprenticeshipCertificate, ceterms:AssociateDegree, ceterms:BachelorDegree, ceterms:Badge, ceterms:Certificate, ceterms:CertificateOfCompletion, ceterms:Certification, ceterms:Credential, ceterms:Degree, ceterms:DigitalBadge, ceterms:Diploma, ceterms:DoctoralDegree, ceterms:GeneralEducationDevelopment, ceterms:JourneymanCertificate, ceterms:License, ceterms:MasterCertificate, ceterms:MasterDegree, ceterms:MicroCredential, ceterms:OpenBadge, ceterms:ProfessionalDoctorate, ceterms:QualityAssuranceCredential, ceterms:ResearchDoctorate, ceterms:SecondarySchoolDiploma ;
	schema:rangeIncludes ceterms:CredentialAlignmentObject ;
	meta:targetScheme ceterms:CredentialStatus .

ceterms:credentialType a rdf:Property ;
	rdfs:label "Credential Type"@en-US ;
	rdfs:comment "Type of credential such as badge, certification, bachelor degree."@en-US ;
	dct:description "A general property for use where a resource needs to identify a specific sub-class of the ceterms:Credential type."@en-US ;
	vs:term_status vs:stable ;
	meta:changeHistory <http://credreg.net/ctdl/termhistory/ceterms/credentialType/json> ;
	schema:domainIncludes ceterms:CredentialComponent ;
	schema:rangeIncludes ceterms:ApprenticeshipCertificate, ceterms:AssociateDegree, ceterms:BachelorDegree, ceterms:Badge, ceterms:Certificate, ceterms:CertificateOfCompletion, ceterms:Certification, ceterms:Degree, ceterms:DigitalBadge, ceterms:Diploma, ceterms:DoctoralDegree, ceterms:GeneralEducationDevelopment, ceterms:JourneymanCertificate, ceterms:License, ceterms:MasterCertificate, ceterms:MasterDegree, ceterms:MicroCredential, ceterms:OpenBadge, ceterms:ProfessionalDoctorate, ceterms:QualityAssuranceCredential, ceterms:ResearchDoctorate, ceterms:SecondarySchoolDiploma .

ceterms:creditLevelType a rdf:Property ;
	rdfs:label "Credit Level Type"@en-US ;
	rdfs:comment "The level of credit associated with the credit awarded or required."@en-US ;
	vs:term_status vs:stable ;
	meta:changeHistory <http://credreg.net/ctdl/termhistory/ceterms/creditLevelType/json> ;
	schema:domainIncludes ceterms:ValueProfile ;
	schema:rangeIncludes skos:Concept ;
	meta:targetScheme ceterms:AudienceLevel .

ceterms:creditUnitType a rdf:Property ;
	rdfs:label "Credit Unit Type"@en-US ;
	rdfs:comment "The type of credit associated with the credit awarded or required."@en-US ;
	vs:term_status vs:stable ;
	meta:changeHistory <http://credreg.net/ctdl/termhistory/ceterms/creditUnitType/json> ;
	schema:domainIncludes ceterms:ValueProfile ;
	schema:rangeIncludes skos:Concept ;
	meta:targetScheme ceterms:CreditUnit .

ceterms:creditUnitTypeDescription a rdf:Property ;
	rdfs:label "Credit Unit Type Description"@en-US ;
	rdfs:comment "Detailed description of credit unit type."@en-US ;
	vs:term_status vs:stable ;
	meta:changeHistory <http://credreg.net/ctdl/termhistory/ceterms/creditUnitTypeDescription/json> ;
	schema:domainIncludes ceterms:AssessmentProfile, ceterms:ConditionProfile, ceterms:Course, ceterms:LearningOpportunityProfile, ceterms:LearningProgram ;
	schema:rangeIncludes rdf:langString .

ceterms:creditValue a rdf:Property ;
	rdfs:label "Credit Value"@en-US ;
	rdfs:comment "A credit-related value."@en-US ;
	vs:term_status vs:stable ;
	meta:changeHistory <http://credreg.net/ctdl/termhistory/ceterms/creditValue/json> ;
	schema:domainIncludes ceterms:AssessmentProfile, ceterms:ConditionProfile, ceterms:Course, ceterms:CourseComponent, ceterms:LearningOpportunityProfile, ceterms:LearningProgram, ceterms:TransferIntermediary ;
	schema:rangeIncludes ceterms:ValueProfile .

ceterms:ctid a rdf:Property ;
	rdfs:label "CTID"@en-US ;
	rdfs:comment "Globally unique Credential Transparency Identifier (CTID) by which the creator, owner or provider of a resource recognizes it in transactions with the external environment (e.g., in verifiable claims involving the resource)."@en-US ;
	dct:description "The CTID is the equivalent of a version identifier for the resource. Different versions of a resource are considered distinct expressions and each must be assigned its own CTID. Each version of a resource can have only one CTID assigned. However, a single version of a resource may have distinct identifier values for both the ctid property and the credentialId property. In such a case both identifiers will be recognized by the resource creator/owner/provider in transactions with the external environment."@en-US ;
	vs:term_status vs:stable ;
	meta:changeHistory <http://credreg.net/ctdl/termhistory/ceterms/ctid/json> ;
	rdfs:subPropertyOf ceterms:credentialId ;
	schema:domainIncludes asn:ProgressionLevel, asn:ProgressionModel, ceasn:Collection, ceasn:Competency, ceasn:CompetencyFramework, ceterms:ApprenticeshipCertificate, ceterms:AssessmentComponent, ceterms:AssessmentProfile, ceterms:AssociateDegree, ceterms:BachelorDegree, ceterms:Badge, ceterms:BasicComponent, ceterms:Certificate, ceterms:CertificateOfCompletion, ceterms:Certification, ceterms:CocurricularComponent, ceterms:Collection, ceterms:CompetencyComponent, ceterms:ConditionManifest, ceterms:CostManifest, ceterms:Course, ceterms:CourseComponent, ceterms:Credential, ceterms:CredentialComponent, ceterms:CredentialOrganization, ceterms:Degree, ceterms:DigitalBadge, ceterms:Diploma, ceterms:DoctoralDegree, ceterms:ExtracurricularComponent, ceterms:GeneralEducationDevelopment, ceterms:Job, ceterms:JobComponent, ceterms:JourneymanCertificate, ceterms:LearningOpportunityProfile, ceterms:LearningProgram, ceterms:License, ceterms:MasterCertificate, ceterms:MasterDegree, ceterms:MicroCredential, ceterms:Occupation, ceterms:OpenBadge, ceterms:Organization, ceterms:Pathway, ceterms:PathwaySet, ceterms:ProfessionalDoctorate, ceterms:QACredentialOrganization, ceterms:QualityAssuranceCredential, ceterms:ResearchDoctorate, ceterms:ScheduledOffering, ceterms:SecondarySchoolDiploma, ceterms:Task, ceterms:TransferIntermediary, ceterms:TransferValueProfile, ceterms:WorkExperienceComponent, ceterms:WorkforceDemandAction, ceterms:WorkRole, skos:Concept, skos:ConceptScheme ;
	schema:rangeIncludes xsd:string .

ceterms:currency a rdf:Property ;
	rdfs:label "Currency"@en-US ;
	rdfs:comment "Currency in which the monetary amount is expressed in 3-letter ISO 4217 format such as \"USD\"."@en-US ;
	vs:term_status vs:stable ;
	meta:changeHistory <http://credreg.net/ctdl/termhistory/ceterms/currency/json> ;
	schema:domainIncludes ceterms:AggregateDataProfile, ceterms:CostProfile ;
	schema:rangeIncludes xsd:string ;
	owl:equivalentProperty schema:currency .

ceterms:dateEffective a rdf:Property ;
	rdfs:label "Date Effective"@en-US ;
	rdfs:comment "Effective date of the content of a credential, assessment or learning opportunity."@en-US ;
	vs:term_status vs:stable ;
	meta:changeHistory <http://credreg.net/ctdl/termhistory/ceterms/dateEffective/json> ;
	rdfs:subPropertyOf ceterms:temporalCoverage ;
	schema:domainIncludes ceterms:AggregateDataProfile, ceterms:ApprenticeshipCertificate, ceterms:AssessmentProfile, ceterms:AssociateDegree, ceterms:BachelorDegree, ceterms:Badge, ceterms:Certificate, ceterms:CertificateOfCompletion, ceterms:Certification, ceterms:Collection, ceterms:ConditionProfile, ceterms:Course, ceterms:Credential, ceterms:Degree, ceterms:DigitalBadge, ceterms:Diploma, ceterms:DoctoralDegree, ceterms:EarningsProfile, ceterms:EmploymentOutcomeProfile, ceterms:GeneralEducationDevelopment, ceterms:HoldersProfile, ceterms:JourneymanCertificate, ceterms:LearningOpportunityProfile, ceterms:LearningProgram, ceterms:License, ceterms:MasterCertificate, ceterms:MasterDegree, ceterms:MicroCredential, ceterms:OpenBadge, ceterms:ProcessProfile, ceterms:ProfessionalDoctorate, ceterms:QualityAssuranceCredential, ceterms:ResearchDoctorate, ceterms:RevocationProfile, ceterms:SecondarySchoolDiploma, ceterms:VerificationServiceProfile ;
	schema:rangeIncludes xsd:date .

ceterms:degreeConcentration a rdf:Property ;
	rdfs:label "Degree Concentration"@en-US ;
	rdfs:comment "Focused plan of study within a college or university degree such as a concentration in Aerospace Engineering within an Engineering degree."@en-US ;
	vann:usageNote "Where possible, values should be taken from published frameworks defining degree majors, minors, and concentrations such as the U.S. National Center for Education Statistics' (NCES) Classification of Instructional Programs (CIP)."@en-US ;
	vs:term_status vs:stable ;
	meta:changeHistory <http://credreg.net/ctdl/termhistory/ceterms/degreeConcentration/json> ;
	schema:domainIncludes ceterms:AssociateDegree, ceterms:BachelorDegree, ceterms:Degree, ceterms:DoctoralDegree, ceterms:MasterDegree ;
	schema:rangeIncludes ceterms:CredentialAlignmentObject .

ceterms:degreeMajor a rdf:Property ;
	rdfs:label "Degree Major"@en-US ;
	rdfs:comment "Primary field of study of a degree-seeking student."@en-US ;
	vann:usageNote "Where possible, values should be taken from published frameworks defining degree majors, minors, and concentrations such as the U.S. National Center for Education Statistics' (NCES) Classification of Instructional Programs (CIP)."@en-US ;
	vs:term_status vs:stable ;
	meta:changeHistory <http://credreg.net/ctdl/termhistory/ceterms/degreeMajor/json> ;
	schema:domainIncludes ceterms:AssociateDegree, ceterms:BachelorDegree, ceterms:Degree, ceterms:DoctoralDegree, ceterms:MasterDegree ;
	schema:rangeIncludes ceterms:CredentialAlignmentObject .

ceterms:degreeMinor a rdf:Property ;
	rdfs:label "Degree Minor"@en-US ;
	rdfs:comment "Optional, secondary field of study of a degree-seeking student."@en-US ;
	vann:usageNote "Where possible, values should be taken from published frameworks defining degree majors, minors, and concentrations such as the U.S. National Center for Education Statistics' (NCES) Classification of Instructional Programs (CIP)."@en-US ;
	vs:term_status vs:stable ;
	meta:changeHistory <http://credreg.net/ctdl/termhistory/ceterms/degreeMinor/json> ;
	schema:domainIncludes ceterms:AssociateDegree, ceterms:BachelorDegree, ceterms:Degree, ceterms:DoctoralDegree, ceterms:MasterDegree ;
	schema:rangeIncludes ceterms:CredentialAlignmentObject .

ceterms:deliveryType a rdf:Property ;
	rdfs:label "Delivery Type"@en-US ;
	rdfs:comment "Type of means by which a learning opportunity or assessment is delivered to credential seekers and by which they interact; select from an existing enumeration of such types."@en-US ;
	vann:usageNote "Best practice is to use concepts from a controlled vocabulary such as the ceterms:DeliveryType vocabulary."@en-US ;
	vs:term_status vs:stable ;
	meta:changeHistory <http://credreg.net/ctdl/termhistory/ceterms/deliveryType/json> ;
	schema:domainIncludes ceterms:AssessmentProfile, ceterms:Course, ceterms:LearningOpportunityProfile, ceterms:LearningProgram, ceterms:ScheduledOffering ;
	schema:rangeIncludes ceterms:CredentialAlignmentObject ;
	meta:targetScheme ceterms:Delivery .

ceterms:deliveryTypeDescription a rdf:Property ;
	rdfs:label "Delivery Type Description"@en-US ;
	rdfs:comment "Detailed description of the delivery type of an assessment or learning opportunity."@en-US ;
	vs:term_status vs:stable ;
	meta:changeHistory <http://credreg.net/ctdl/termhistory/ceterms/deliveryTypeDescription/json> ;
	schema:domainIncludes ceterms:AssessmentProfile, ceterms:Course, ceterms:LearningOpportunityProfile, ceterms:LearningProgram, ceterms:ScheduledOffering ;
	schema:rangeIncludes rdf:langString .

ceterms:demographicInformation a rdf:Property ;
	rdfs:label "Demographic Information"@en-US ;
	rdfs:comment "Aggregate data or summaries of statistical data relating to the population of credential holders including data about gender, geopolitical regions, age, education levels, and other categories of interest."@en-US ;
	vs:term_status vs:stable ;
	meta:changeHistory <http://credreg.net/ctdl/termhistory/ceterms/demographicInformation/json> ;
	schema:domainIncludes ceterms:AggregateDataProfile, ceterms:HoldersProfile ;
	schema:rangeIncludes rdf:langString .

ceterms:department a rdf:Property ;
	rdfs:label "Department"@en-US ;
	rdfs:comment "Department of the organization."@en-US ;
	vs:term_status vs:stable ;
	meta:changeHistory <http://credreg.net/ctdl/termhistory/ceterms/department/json> ;
	rdfs:subPropertyOf ceterms:subOrganization ;
	schema:domainIncludes ceterms:CredentialOrganization, ceterms:Organization, ceterms:QACredentialOrganization ;
	schema:rangeIncludes ceterms:CredentialOrganization, ceterms:Organization, ceterms:QACredentialOrganization ;
	owl:equivalentProperty schema:department .

ceterms:description a rdf:Property ;
	rdfs:label "Description"@en-US ;
	rdfs:comment "Statement, characterization or account of the entity."@en-US ;
	vs:term_status vs:stable ;
	meta:changeHistory <http://credreg.net/ctdl/termhistory/ceterms/description/json> ;
	schema:domainIncludes ceterms:AccreditAction, ceterms:AdvancedStandingAction, ceterms:AggregateDataProfile, ceterms:ApprenticeshipCertificate, ceterms:ApproveAction, ceterms:AssessmentComponent, ceterms:AssessmentProfile, ceterms:AssociateDegree, ceterms:BachelorDegree, ceterms:Badge, ceterms:BasicComponent, ceterms:Certificate, ceterms:CertificateOfCompletion, ceterms:Certification, ceterms:CocurricularComponent, ceterms:Collection, ceterms:CollectionMember, ceterms:CompetencyComponent, ceterms:ComponentCondition, ceterms:ConditionManifest, ceterms:ConditionProfile, ceterms:Constraint, ceterms:CostManifest, ceterms:CostProfile, ceterms:Course, ceterms:CourseComponent, ceterms:Credential, ceterms:CredentialComponent, ceterms:CredentialingAction, ceterms:CredentialOrganization, ceterms:Degree, ceterms:DigitalBadge, ceterms:Diploma, ceterms:DoctoralDegree, ceterms:DurationProfile, ceterms:EmploymentOutcomeProfile, ceterms:ExtracurricularComponent, ceterms:FinancialAssistanceProfile, ceterms:GeneralEducationDevelopment, ceterms:HoldersProfile, ceterms:Job, ceterms:JobComponent, ceterms:JourneymanCertificate, ceterms:JurisdictionProfile, ceterms:LearningOpportunityProfile, ceterms:LearningProgram, ceterms:License, ceterms:MasterCertificate, ceterms:MasterDegree, ceterms:MicroCredential, ceterms:Occupation, ceterms:OfferAction, ceterms:OpenBadge, ceterms:Organization, ceterms:Pathway, ceterms:PathwaySet, ceterms:Place, ceterms:ProcessProfile, ceterms:ProfessionalDoctorate, ceterms:QACredentialOrganization, ceterms:QualityAssuranceCredential, ceterms:RecognizeAction, ceterms:RegulateAction, ceterms:RenewAction, ceterms:ResearchDoctorate, ceterms:RevocationProfile, ceterms:RevokeAction, ceterms:RightsAction, ceterms:RuleSetProfile, ceterms:ScheduledOffering, ceterms:SecondarySchoolDiploma, ceterms:Task, ceterms:TransferIntermediary, ceterms:TransferValueProfile, ceterms:VerificationServiceProfile, ceterms:WorkExperienceComponent, ceterms:WorkforceDemandAction, ceterms:WorkRole ;
	schema:rangeIncludes rdf:langString ;
	owl:equivalentProperty dct:description, schema:description .

ceterms:developmentProcess a rdf:Property ;
	rdfs:label "Development Process"@en-US ;
	rdfs:comment "Entity describing the process by which a credential, or aspects of it, were created."@en-US ;
	vs:term_status vs:stable ;
	meta:changeHistory <http://credreg.net/ctdl/termhistory/ceterms/developmentProcess/json> ;
	schema:domainIncludes ceterms:ApprenticeshipCertificate, ceterms:AssessmentProfile, ceterms:AssociateDegree, ceterms:BachelorDegree, ceterms:Badge, ceterms:Certificate, ceterms:CertificateOfCompletion, ceterms:Certification, ceterms:Credential, ceterms:CredentialOrganization, ceterms:Degree, ceterms:DigitalBadge, ceterms:Diploma, ceterms:DoctoralDegree, ceterms:GeneralEducationDevelopment, ceterms:JourneymanCertificate, ceterms:License, ceterms:MasterCertificate, ceterms:MasterDegree, ceterms:MicroCredential, ceterms:OpenBadge, ceterms:Organization, ceterms:ProfessionalDoctorate, ceterms:QACredentialOrganization, ceterms:QualityAssuranceCredential, ceterms:ResearchDoctorate, ceterms:SecondarySchoolDiploma, ceterms:TransferValueProfile ;
	schema:rangeIncludes ceterms:ProcessProfile .

ceterms:directCostType a rdf:Property ;
	rdfs:label "Direct Cost Type"@en-US ;
	rdfs:comment "Types of direct costs associated with earning or completing a credential, assessment or learning opportunity; select from an existing enumeration of such types."@en-US ;
	vann:usageNote "Best practice for developing credential descriptions for the Credential Engine Registry is to use the ceterms:CostType vocabulary."@en-US ;
	vs:term_status vs:stable ;
	meta:changeHistory <http://credreg.net/ctdl/termhistory/ceterms/directCostType/json> ;
	rdfs:subPropertyOf ceterms:credentialAlignment ;
	schema:domainIncludes ceterms:CostProfile ;
	schema:rangeIncludes ceterms:CredentialAlignmentObject ;
	meta:targetScheme ceterms:CostType .

ceterms:duns a rdf:Property ;
	rdfs:label "DUNS"@en-US ;
	rdfs:comment "Dun & Bradstreet DUNS number for identifying an organization or business person."@en-US ;
	vs:term_status vs:stable ;
	meta:changeHistory <http://credreg.net/ctdl/termhistory/ceterms/duns/json> ;
	schema:domainIncludes ceterms:CredentialOrganization, ceterms:Organization, ceterms:QACredentialOrganization ;
	schema:rangeIncludes xsd:string ;
	owl:equivalentProperty schema:duns .

ceterms:earnings a rdf:Property ;
	rdfs:label "Earnings"@en-US ;
	rdfs:comment "Entity describing aggregate credential holder earnings data."@en-US ;
	vann:usageNote "The use of ceterms:aggregateData instead of this property is strongly recommended."@en-US ;
	vs:term_status vs:stable ;
	meta:changeHistory <http://credreg.net/ctdl/termhistory/ceterms/earnings/json> ;
	rdfs:subPropertyOf ceterms:aggregateData ;
	schema:domainIncludes ceterms:ApprenticeshipCertificate, ceterms:AssociateDegree, ceterms:BachelorDegree, ceterms:Badge, ceterms:Certificate, ceterms:CertificateOfCompletion, ceterms:Certification, ceterms:Credential, ceterms:Degree, ceterms:DigitalBadge, ceterms:Diploma, ceterms:DoctoralDegree, ceterms:GeneralEducationDevelopment, ceterms:JourneymanCertificate, ceterms:License, ceterms:MasterCertificate, ceterms:MasterDegree, ceterms:MicroCredential, ceterms:OpenBadge, ceterms:ProfessionalDoctorate, ceterms:QualityAssuranceCredential, ceterms:ResearchDoctorate, ceterms:SecondarySchoolDiploma ;
	schema:rangeIncludes ceterms:EarningsProfile .

ceterms:email a rdf:Property ;
	rdfs:label "Email"@en-US ;
	rdfs:comment "Email address of the organization or person."@en-US ;
	vs:term_status vs:stable ;
	meta:changeHistory <http://credreg.net/ctdl/termhistory/ceterms/email/json> ;
	schema:domainIncludes ceterms:ContactPoint, ceterms:CredentialOrganization, ceterms:Organization, ceterms:QACredentialOrganization ;
	schema:rangeIncludes xsd:string ;
	owl:equivalentProperty schema:email .

ceterms:employee a rdf:Property ;
	rdfs:label "Employee"@en-US ;
	rdfs:comment "Person employed for wages or salary by the organization."@en-US ;
	vs:term_status vs:stable ;
	meta:changeHistory <http://credreg.net/ctdl/termhistory/ceterms/employee/json> ;
	schema:domainIncludes ceterms:CredentialOrganization, ceterms:Organization, ceterms:QACredentialOrganization ;
	schema:rangeIncludes ceterms:CredentialPerson ;
	owl:equivalentProperty schema:employee .

ceterms:employmentOutcome a rdf:Property ;
	rdfs:label "Employment Outcome"@en-US ;
	rdfs:comment "Entity describing aggregate data on jobs obtained with the credential by occupation and industry for a given period of time in a specific region."@en-US ;
	vann:usageNote "The use of ceterms:aggregateData instead of this property is strongly recommended."@en-US ;
	vs:term_status vs:stable ;
	meta:changeHistory <http://credreg.net/ctdl/termhistory/ceterms/employmentOutcome/json> ;
	rdfs:subPropertyOf ceterms:aggregateData ;
	schema:domainIncludes ceterms:ApprenticeshipCertificate, ceterms:AssociateDegree, ceterms:BachelorDegree, ceterms:Badge, ceterms:Certificate, ceterms:CertificateOfCompletion, ceterms:Certification, ceterms:Credential, ceterms:Degree, ceterms:DigitalBadge, ceterms:Diploma, ceterms:DoctoralDegree, ceterms:GeneralEducationDevelopment, ceterms:JourneymanCertificate, ceterms:License, ceterms:MasterCertificate, ceterms:MasterDegree, ceterms:MicroCredential, ceterms:OpenBadge, ceterms:ProfessionalDoctorate, ceterms:QualityAssuranceCredential, ceterms:ResearchDoctorate, ceterms:SecondarySchoolDiploma ;
	schema:rangeIncludes ceterms:EmploymentOutcomeProfile .

ceterms:endDate a rdf:Property ;
	rdfs:label "End Date"@en-US ;
	rdfs:comment "Date some event or activity ends."@en-US ;
	vs:term_status vs:stable ;
	meta:changeHistory <http://credreg.net/ctdl/termhistory/ceterms/endDate/json> ;
	rdfs:subPropertyOf ceterms:temporalCoverage ;
	schema:domainIncludes ceterms:AccreditAction, ceterms:AdvancedStandingAction, ceterms:ApproveAction, ceterms:CollectionMember, ceterms:CostManifest, ceterms:CostProfile, ceterms:CredentialingAction, ceterms:OfferAction, ceterms:RecognizeAction, ceterms:RegulateAction, ceterms:RenewAction, ceterms:RevokeAction, ceterms:RightsAction, ceterms:TransferValueProfile, ceterms:WorkforceDemandAction ;
	schema:rangeIncludes xsd:date ;
	owl:equivalentProperty schema:endDate .

ceterms:endTime a rdf:Property ;
	rdfs:label "End Time"@en-US ;
	rdfs:comment "Time some event or activity ends."@en-US ;
	vs:term_status vs:stable ;
	meta:changeHistory <http://credreg.net/ctdl/termhistory/ceterms/endTime/json> ;
	rdfs:subPropertyOf ceterms:temporalCoverage ;
	schema:rangeIncludes xsd:dateTime ;
	owl:equivalentProperty schema:endTime .

ceterms:entryCondition a rdf:Property ;
	rdfs:label "Entry Condition"@en-US ;
	rdfs:comment "Prerequisites for entry into a credentialing program, a learning opportunity or an assessment including transcripts, records of previous experience, and lower-level learning opportunities."@en-US ;
	vs:term_status vs:stable ;
	meta:changeHistory <http://credreg.net/ctdl/termhistory/ceterms/entryCondition/json> ;
	rdfs:subPropertyOf ceterms:requires ;
	schema:domainIncludes ceterms:AssessmentProfile, ceterms:ConditionManifest, ceterms:Course, ceterms:LearningOpportunityProfile, ceterms:LearningProgram ;
	schema:rangeIncludes ceterms:ConditionProfile .

ceterms:environmentalHazardType a rdf:Property ;
	rdfs:label "Environmental Hazard Type"@en-US ;
	rdfs:comment "Type of condition in the physical work performance environment that entails risk exposures requiring mitigating processes; select from an existing enumeration of such types."@en-US ;
	dct:description "Such types may include exposure to bloodborne pathogens, airborne communicable diseases and dangerous chemicals, battlefield conditions, fire fighting, law enforcement, and so on."@en-US ;
	vs:term_status vs:unstable ;
	meta:changeHistory <http://credreg.net/ctdl/termhistory/ceterms/environmentalHazardType/json> ;
	schema:domainIncludes ceasn:Competency, ceterms:Job, ceterms:Task, ceterms:WorkRole ;
	schema:rangeIncludes skos:Concept .

ceterms:estimatedCost a rdf:Property ;
	rdfs:label "Estimated Cost"@en-US ;
	rdfs:comment "Estimated cost of a credential, learning opportunity or assessment."@en-US ;
	vs:term_status vs:stable ;
	meta:changeHistory <http://credreg.net/ctdl/termhistory/ceterms/estimatedCost/json> ;
	schema:domainIncludes ceterms:ApprenticeshipCertificate, ceterms:AssessmentProfile, ceterms:AssociateDegree, ceterms:BachelorDegree, ceterms:Badge, ceterms:Certificate, ceterms:CertificateOfCompletion, ceterms:Certification, ceterms:ConditionProfile, ceterms:CostManifest, ceterms:Course, ceterms:Credential, ceterms:Degree, ceterms:DigitalBadge, ceterms:Diploma, ceterms:DoctoralDegree, ceterms:GeneralEducationDevelopment, ceterms:JourneymanCertificate, ceterms:LearningOpportunityProfile, ceterms:LearningProgram, ceterms:License, ceterms:MasterCertificate, ceterms:MasterDegree, ceterms:MicroCredential, ceterms:OpenBadge, ceterms:ProfessionalDoctorate, ceterms:QualityAssuranceCredential, ceterms:ResearchDoctorate, ceterms:ScheduledOffering, ceterms:SecondarySchoolDiploma, ceterms:VerificationServiceProfile ;
	schema:rangeIncludes ceterms:CostProfile .

ceterms:estimatedDuration a rdf:Property ;
	rdfs:label "Estimated Duration"@en-US ;
	rdfs:comment "Estimated time it will take to complete a credential, learning opportunity or assessment."@en-US ;
	vs:term_status vs:stable ;
	meta:changeHistory <http://credreg.net/ctdl/termhistory/ceterms/estimatedDuration/json> ;
	schema:domainIncludes ceterms:ApprenticeshipCertificate, ceterms:AssessmentProfile, ceterms:AssociateDegree, ceterms:BachelorDegree, ceterms:Badge, ceterms:Certificate, ceterms:CertificateOfCompletion, ceterms:Certification, ceterms:Course, ceterms:Credential, ceterms:Degree, ceterms:DigitalBadge, ceterms:Diploma, ceterms:DoctoralDegree, ceterms:GeneralEducationDevelopment, ceterms:JourneymanCertificate, ceterms:LearningOpportunityProfile, ceterms:LearningProgram, ceterms:License, ceterms:MasterCertificate, ceterms:MasterDegree, ceterms:MicroCredential, ceterms:OpenBadge, ceterms:ProfessionalDoctorate, ceterms:QualityAssuranceCredential, ceterms:ResearchDoctorate, ceterms:ScheduledOffering, ceterms:SecondarySchoolDiploma ;
	schema:rangeIncludes ceterms:DurationProfile .

ceterms:evidenceOfAction a rdf:Property ;
	rdfs:label "Evidence of Action"@en-US ;
	rdfs:comment "Entity that proves that the action occured or that the action continues to be valid."@en-US ;
	dct:description "The evidence verifies the information in the action and is particular to it. It is not a directory of such evidentiary entities or a description of how such verifications might generically be characterized."@en-US ;
	vs:term_status vs:stable ;
	meta:changeHistory <http://credreg.net/ctdl/termhistory/ceterms/evidenceOfAction/json> ;
	schema:domainIncludes ceterms:AccreditAction, ceterms:AdvancedStandingAction, ceterms:ApproveAction, ceterms:CredentialingAction, ceterms:OfferAction, ceterms:RecognizeAction, ceterms:RegulateAction, ceterms:RenewAction, ceterms:RevokeAction, ceterms:RightsAction, ceterms:WorkforceDemandAction ;
	schema:rangeIncludes xsd:anyURI .

ceterms:exactAlignment a rdf:Property ;
	rdfs:label "Exact Alignment"@en-US ;
	rdfs:comment "Relevant concepts in two entities being compared are coextensive."@en-US ;
	vs:term_status vs:stable ;
	meta:changeHistory <http://credreg.net/ctdl/termhistory/ceterms/exactAlignment/json> ;
	rdfs:subPropertyOf ceterms:isSimilarTo ;
	schema:domainIncludes ceterms:ApprenticeshipCertificate, ceterms:AssociateDegree, ceterms:BachelorDegree, ceterms:Badge, ceterms:Certificate, ceterms:CertificateOfCompletion, ceterms:Certification, ceterms:Credential, ceterms:Degree, ceterms:DigitalBadge, ceterms:Diploma, ceterms:DoctoralDegree, ceterms:GeneralEducationDevelopment, ceterms:JourneymanCertificate, ceterms:License, ceterms:MasterCertificate, ceterms:MasterDegree, ceterms:MicroCredential, ceterms:OpenBadge, ceterms:ProfessionalDoctorate, ceterms:QualityAssuranceCredential, ceterms:ResearchDoctorate, ceterms:SecondarySchoolDiploma ;
	schema:rangeIncludes ceterms:ApprenticeshipCertificate, ceterms:AssociateDegree, ceterms:BachelorDegree, ceterms:Badge, ceterms:Certificate, ceterms:CertificateOfCompletion, ceterms:Certification, ceterms:Credential, ceterms:Degree, ceterms:DigitalBadge, ceterms:Diploma, ceterms:DoctoralDegree, ceterms:GeneralEducationDevelopment, ceterms:JourneymanCertificate, ceterms:License, ceterms:MasterCertificate, ceterms:MasterDegree, ceterms:MicroCredential, ceterms:OpenBadge, ceterms:ProfessionalDoctorate, ceterms:QualityAssuranceCredential, ceterms:ResearchDoctorate, ceterms:SecondarySchoolDiploma ;
	owl:equivalentProperty asn:exactAlignment, skos:exactMatch .

ceterms:exactDuration a rdf:Property ;
	rdfs:label "Exact Duration"@en-US ;
	rdfs:comment "Exact period of time of an activity or event."@en-US ;
	vs:term_status vs:stable ;
	meta:changeHistory <http://credreg.net/ctdl/termhistory/ceterms/exactDuration/json> ;
	schema:domainIncludes ceterms:DurationProfile ;
	schema:rangeIncludes schema:Duration .

ceterms:experience a rdf:Property ;
	rdfs:label "Experience"@en-US ;
	rdfs:comment "Amount and nature of required work, experiential learning or other relevant experience."@en-US ;
	vs:term_status vs:stable ;
	meta:changeHistory <http://credreg.net/ctdl/termhistory/ceterms/experience/json> ;
	schema:domainIncludes ceterms:ConditionProfile ;
	schema:rangeIncludes rdf:langString .

ceterms:expirationDate a rdf:Property ;
	rdfs:label "Expiration Date"@en-US ;
	rdfs:comment "Date beyond which the resource is no longer offered or available."@en-US ;
	dct:description "Previously earned, completed, or attained resources may still be valid even if they are no longer offered."@en-US ;
	vs:term_status vs:stable ;
	meta:changeHistory <http://credreg.net/ctdl/termhistory/ceterms/expirationDate/json> ;
	schema:domainIncludes ceterms:AggregateDataProfile, ceterms:ApprenticeshipCertificate, ceterms:AssessmentProfile, ceterms:AssociateDegree, ceterms:BachelorDegree, ceterms:Badge, ceterms:Certificate, ceterms:CertificateOfCompletion, ceterms:Certification, ceterms:Collection, ceterms:Course, ceterms:Credential, ceterms:Degree, ceterms:DigitalBadge, ceterms:Diploma, ceterms:DoctoralDegree, ceterms:GeneralEducationDevelopment, ceterms:JourneymanCertificate, ceterms:LearningOpportunityProfile, ceterms:LearningProgram, ceterms:License, ceterms:MasterCertificate, ceterms:MasterDegree, ceterms:MicroCredential, ceterms:OpenBadge, ceterms:ProfessionalDoctorate, ceterms:QualityAssuranceCredential, ceterms:ResearchDoctorate, ceterms:SecondarySchoolDiploma ;
	schema:rangeIncludes xsd:date .

ceterms:externalInputType a rdf:Property ;
	rdfs:label "External Input Type"@en-US ;
	rdfs:comment "Types of external stakeholders that provide input to an entity's processes or resources; select from an existing enumeration of such types."@en-US ;
	vann:usageNote "Best practice for developing credential descriptions for the Credential Engine Registry is to use the ceterms:ExternalInput vocabulary."@en-US ;
	vs:term_status vs:stable ;
	meta:changeHistory <http://credreg.net/ctdl/termhistory/ceterms/externalInputType/json> ;
	rdfs:subPropertyOf ceterms:credentialAlignment ;
	schema:domainIncludes ceterms:ProcessProfile ;
	schema:rangeIncludes ceterms:CredentialAlignmentObject ;
	meta:targetScheme ceterms:ExternalInput .

ceterms:externalResearch a rdf:Property ;
	rdfs:label "External Research"@en-US ;
	rdfs:comment "Research that supports or validates one or more aspects of the entity."@en-US ;
	vs:term_status vs:stable ;
	meta:changeHistory <http://credreg.net/ctdl/termhistory/ceterms/externalResearch/json> ;
	schema:domainIncludes ceterms:AssessmentProfile ;
	schema:rangeIncludes xsd:anyURI .

ceterms:familyName a rdf:Property ;
	rdfs:label "Family Name"@en-US ;
	rdfs:comment "Family name such as the last name of a person in the U.S.."@en-US ;
	dct:description "The ceterms:familyName property can be used along with givenName instead of the ceterms:name property."@en-US ;
	vs:term_status vs:stable ;
	meta:changeHistory <http://credreg.net/ctdl/termhistory/ceterms/familyName/json> ;
	schema:domainIncludes ceterms:CredentialPerson ;
	schema:rangeIncludes rdf:langString ;
	owl:equivalentProperty schema:familyName .

ceterms:faxNumber a rdf:Property ;
	rdfs:label "Fax Number"@en-US ;
	rdfs:comment "Fax number."@en-US ;
	vs:term_status vs:stable ;
	meta:changeHistory <http://credreg.net/ctdl/termhistory/ceterms/faxNumber/json> ;
	schema:domainIncludes ceterms:ContactPoint ;
	schema:rangeIncludes xsd:string ;
	owl:equivalentProperty schema:faxNumber .

ceterms:fein a rdf:Property ;
	rdfs:label "FEIN"@en-US ;
	rdfs:comment "Federal Employer Identification Number (FEIN) identifying organizations, persons, states, government agencies, corporations, and companies."@en-US ;
	vs:term_status vs:stable ;
	meta:changeHistory <http://credreg.net/ctdl/termhistory/ceterms/fein/json> ;
	schema:domainIncludes ceterms:CredentialOrganization, ceterms:Organization, ceterms:QACredentialOrganization ;
	schema:rangeIncludes xsd:string .

ceterms:financialAssistance a rdf:Property ;
	rdfs:label "Financial Assistance"@en-US ;
	rdfs:comment "Entity that describes financial assistance for which this credential, assessment, or learning opportunity qualifies."@en-US ;
	dct:description "Whether the financial aid in question is associated with a credential, an assessment, or a learning opportunity is dependent on context."@en-US ;
	vs:term_status vs:stable ;
	meta:changeHistory <http://credreg.net/ctdl/termhistory/ceterms/financialAssistance/json> ;
	schema:domainIncludes ceterms:ApprenticeshipCertificate, ceterms:AssessmentProfile, ceterms:AssociateDegree, ceterms:BachelorDegree, ceterms:Badge, ceterms:Certificate, ceterms:CertificateOfCompletion, ceterms:Certification, ceterms:Course, ceterms:Credential, ceterms:Degree, ceterms:DigitalBadge, ceterms:Diploma, ceterms:DoctoralDegree, ceterms:GeneralEducationDevelopment, ceterms:JourneymanCertificate, ceterms:LearningOpportunityProfile, ceterms:LearningProgram, ceterms:License, ceterms:MasterCertificate, ceterms:MasterDegree, ceterms:MicroCredential, ceterms:OpenBadge, ceterms:ProfessionalDoctorate, ceterms:QualityAssuranceCredential, ceterms:ResearchDoctorate, ceterms:SecondarySchoolDiploma ;
	schema:rangeIncludes ceterms:FinancialAssistanceProfile .

ceterms:financialAssistanceType a rdf:Property ;
	rdfs:label "Financial Assistance Type"@en-US ;
	rdfs:comment "Type of financial assistance; select from an existing enumeration of such types."@en-US ;
	vs:term_status vs:stable ;
	meta:changeHistory <http://credreg.net/ctdl/termhistory/ceterms/financialAssistanceType/json> ;
	schema:domainIncludes ceterms:FinancialAssistanceProfile ;
	schema:rangeIncludes ceterms:CredentialAlignmentObject ;
	meta:targetScheme ceterms:FinancialAssistance .

ceterms:financialAssistanceValue a rdf:Property ;
	rdfs:label "Financial Assistance Value"@en-US ;
	rdfs:comment "Description of the amount of financial assistance available."@en-US ;
	vs:term_status vs:stable ;
	meta:changeHistory <http://credreg.net/ctdl/termhistory/ceterms/financialAssistanceValue/json> ;
	schema:domainIncludes ceterms:FinancialAssistanceProfile ;
	schema:rangeIncludes schema:QuantitativeValue .

ceterms:foundingDate a rdf:Property ;
	rdfs:label "Founding Date"@en-US ;
	rdfs:comment "Date the organization was founded."@en-US ;
	vs:term_status vs:stable ;
	meta:changeHistory <http://credreg.net/ctdl/termhistory/ceterms/foundingDate/json> ;
	rdfs:subPropertyOf ceterms:temporalCoverage ;
	schema:domainIncludes ceterms:CredentialOrganization, ceterms:Organization, ceterms:QACredentialOrganization ;
	schema:rangeIncludes xsd:string ;
	owl:equivalentProperty schema:foundingDate .

ceterms:framework a rdf:Property ;
	rdfs:label "Framework URL"@en-US ;
	rdfs:comment "Credential framework to which the entity is aligned."@en-US ;
	dct:description "Frameworks may include, but are not limited to, competency frameworks and concept schemes such as industry, occupation, and instructional program codes."@en-US ;
	vs:term_status vs:stable ;
	meta:changeHistory <http://credreg.net/ctdl/termhistory/ceterms/framework/json> ;
	schema:domainIncludes ceterms:CredentialAlignmentObject, ceterms:FinancialAlignmentObject ;
	schema:rangeIncludes xsd:anyURI .

ceterms:frameworkName a rdf:Property ;
	rdfs:label "Framework Name"@en-US ;
	rdfs:comment "Name of the framework."@en-US ;
	vs:term_status vs:stable ;
	meta:changeHistory <http://credreg.net/ctdl/termhistory/ceterms/frameworkName/json> ;
	schema:domainIncludes ceterms:CredentialAlignmentObject, ceterms:FinancialAlignmentObject ;
	schema:rangeIncludes rdf:langString ;
	owl:equivalentProperty schema:educationalFramework .

ceterms:geoURI a rdf:Property ;
	rdfs:label "Geographic URI"@en-US ;
	rdfs:comment "Entity that describes the longitude, latitude and other location details of a place."@en-US ;
	dct:description "This may define a place at any scale. Examples include a city, state, province, country, or continent."@en-US ;
	vann:usageNote "It is recommended to use services such as http://www.geonames.org to provide values for this property."@en-US ;
	vs:term_status vs:stable ;
	meta:changeHistory <http://credreg.net/ctdl/termhistory/ceterms/geoURI/json> ;
	schema:domainIncludes ceterms:GeoCoordinates, ceterms:Place ;
	schema:rangeIncludes xsd:anyURI .

ceterms:givenName a rdf:Property ;
	rdfs:label "Given Name"@en-US ;
	rdfs:comment "First name of a person."@en-US ;
	vann:usageNote "Family name can be used along with familyName instead of the name property."@en-US ;
	vs:term_status vs:stable ;
	meta:changeHistory <http://credreg.net/ctdl/termhistory/ceterms/givenName/json> ;
	schema:domainIncludes ceterms:CredentialPerson ;
	schema:rangeIncludes rdf:langString ;
	owl:equivalentProperty schema:givenName .

ceterms:globalJurisdiction a rdf:Property ;
	rdfs:label "Global Jurisdiction"@en-US ;
	rdfs:comment "Whether or not the credential is useful, applicable or recognized everywhere."@en-US ;
	dct:description "Exceptions indicated by the ceterms:jurisdictionException property apply."@en-US ;
	vs:term_status vs:stable ;
	meta:changeHistory <http://credreg.net/ctdl/termhistory/ceterms/globalJurisdiction/json> ;
	schema:domainIncludes ceterms:JurisdictionProfile ;
	schema:rangeIncludes xsd:boolean .

ceterms:hasAlignmentMap a rdf:Property ;
	rdfs:label "Alignment Map"@en-US ;
	rdfs:comment "Alignment map owned by the agent."@en-US ;
	vs:term_status vs:stable ;
	meta:changeHistory <http://credreg.net/ctdl/termhistory/ceterms/hasAlignmentMap/json> ;
	schema:domainIncludes ceterms:CredentialOrganization, ceterms:Organization, ceterms:QACredentialOrganization ;
	schema:rangeIncludes ceterms:AlignmentMap .

ceterms:hasCondition a rdf:Property ;
	rdfs:label "Has Condition"@en-US ;
	rdfs:comment "Resource referenced defines a condition by which this resource is satisfied in full or in part."@en-US ;
	vs:term_status vs:stable ;
	meta:changeHistory <http://credreg.net/ctdl/termhistory/ceterms/hasCondition/json> ;
	schema:domainIncludes ceterms:AssessmentComponent, ceterms:BasicComponent, ceterms:CocurricularComponent, ceterms:CompetencyComponent, ceterms:ComponentCondition, ceterms:CourseComponent, ceterms:CredentialComponent, ceterms:ExtracurricularComponent, ceterms:JobComponent, ceterms:WorkExperienceComponent ;
	schema:rangeIncludes ceterms:ComponentCondition .

ceterms:hasConditionManifest a rdf:Property ;
	rdfs:label "Has Condition Manifest"@en-US ;
	rdfs:comment "Entity that describes a set of constraints, prerequisites, entry conditions, or requirements applicable across the organization, sub-organization or sets of credentials or acitivites."@en-US ;
	vs:term_status vs:stable ;
	meta:changeHistory <http://credreg.net/ctdl/termhistory/ceterms/hasConditionManifest/json> ;
	schema:domainIncludes ceterms:CredentialOrganization, ceterms:Organization, ceterms:QACredentialOrganization ;
	schema:rangeIncludes ceterms:ConditionManifest .

ceterms:hasConstraint a rdf:Property ;
	rdfs:label "Has Constraint"@en-US ;
	rdfs:comment "Referenced resource defines a single constraint."@en-US ;
	vs:term_status vs:unstable ;
	meta:changeHistory <http://credreg.net/ctdl/termhistory/ceterms/hasConstraint/json> ;
	schema:domainIncludes ceterms:ComponentCondition ;
	schema:rangeIncludes ceterms:Constraint .

ceterms:hasCostManifest a rdf:Property ;
	rdfs:label "Has Cost Manifest"@en-US ;
	rdfs:comment "Entity that describes a set of cost data applicable across the organization, sub-organization or sets of credentials or acitivites."@en-US ;
	vs:term_status vs:stable ;
	meta:changeHistory <http://credreg.net/ctdl/termhistory/ceterms/hasCostManifest/json> ;
	schema:domainIncludes ceterms:CredentialOrganization, ceterms:Organization, ceterms:QACredentialOrganization ;
	schema:rangeIncludes ceterms:CostManifest .

ceterms:hasDestinationComponent a rdf:Property ;
	rdfs:label "Has Destination Component"@en-US ;
	rdfs:comment "Goal or destination node of the pathway."@en-US ;
	vs:term_status vs:stable ;
	meta:changeHistory <http://credreg.net/ctdl/termhistory/ceterms/hasDestinationComponent/json> ;
	schema:domainIncludes ceterms:Pathway ;
	schema:rangeIncludes ceterms:AssessmentComponent, ceterms:BasicComponent, ceterms:CocurricularComponent, ceterms:CompetencyComponent, ceterms:CourseComponent, ceterms:CredentialComponent, ceterms:ExtracurricularComponent, ceterms:JobComponent, ceterms:WorkExperienceComponent .

ceterms:hasGroupEvaluation a rdf:Property ;
	rdfs:label "Has Group Evaluation"@en-US ;
	rdfs:comment "Whether or not the assessment activity is scored as a group."@en-US ;
	vs:term_status vs:stable ;
	meta:changeHistory <http://credreg.net/ctdl/termhistory/ceterms/hasGroupEvaluation/json> ;
	schema:domainIncludes ceterms:AssessmentProfile ;
	schema:rangeIncludes xsd:boolean .

ceterms:hasGroupParticipation a rdf:Property ;
	rdfs:label "Has Group Participation"@en-US ;
	rdfs:comment "Whether or not two or more participants are required to complete the assessment activity."@en-US ;
	vs:term_status vs:stable ;
	meta:changeHistory <http://credreg.net/ctdl/termhistory/ceterms/hasGroupParticipation/json> ;
	schema:domainIncludes ceterms:AssessmentProfile ;
	schema:rangeIncludes xsd:boolean .

ceterms:hasJob a rdf:Property ;
	rdfs:label "Has Job"@en-US ;
	rdfs:comment "Job related to this resource."@en-US ;
	vs:term_status vs:stable ;
	meta:changeHistory <http://credreg.net/ctdl/termhistory/ceterms/hasJob/json> ;
	schema:domainIncludes ceterms:Occupation ;
	schema:rangeIncludes ceterms:Job .

ceterms:hasMember a rdf:Property ;
	rdfs:label "Has Member"@en-US ;
	rdfs:comment "Resource in a Collection."@en-US ;
	vs:term_status vs:unstable ;
	meta:changeHistory <http://credreg.net/ctdl/termhistory/ceterms/hasMember/json> ;
	schema:domainIncludes ceterms:Collection ;
	schema:rangeIncludes ceasn:Competency, ceterms:CollectionMember, ceterms:Course, ceterms:Job, ceterms:LearningOpportunityProfile, ceterms:LearningProgram, ceterms:Task, ceterms:WorkRole .

ceterms:hasOccupation a rdf:Property ;
	rdfs:label "Has Occupation"@en-US ;
	rdfs:comment "Occupation related to this resource."@en-US ;
	vs:term_status vs:stable ;
	meta:changeHistory <http://credreg.net/ctdl/termhistory/ceterms/hasOccupation/json> ;
	schema:domainIncludes ceterms:Job ;
	schema:rangeIncludes ceterms:Occupation .

ceterms:hasOffering a rdf:Property ;
	rdfs:label "Has Offering"@en-US ;
	rdfs:comment "Indicates an offering and typical schedule."@en-US ;
	vann:usageNote "Only use this property when it is necessary and useful to provide data about specific offerings of a learning opportunity or assessment, such as particular combinations of schedule, location, and delivery."@en-US ;
	vs:term_status vs:unstable ;
	meta:changeHistory <http://credreg.net/ctdl/termhistory/ceterms/hasOffering/json> ;
	schema:domainIncludes ceterms:AssessmentProfile, ceterms:Course, ceterms:LearningOpportunityProfile, ceterms:LearningProgram ;
	schema:rangeIncludes ceterms:ScheduledOffering .

ceterms:hasPart a rdf:Property ;
	rdfs:label "Has Part"@en-US ;
	rdfs:comment "Indicates a separately identifiable and independently useful component of the entity."@en-US ;
	dct:description "Such partitive components can frequently be used in more than one context."@en-US ;
	vs:term_status vs:stable ;
	meta:changeHistory <http://credreg.net/ctdl/termhistory/ceterms/hasPart/json> ;
	schema:domainIncludes ceterms:ApprenticeshipCertificate, ceterms:AssociateDegree, ceterms:BachelorDegree, ceterms:Badge, ceterms:Certificate, ceterms:CertificateOfCompletion, ceterms:Certification, ceterms:Course, ceterms:Credential, ceterms:Degree, ceterms:DigitalBadge, ceterms:Diploma, ceterms:DoctoralDegree, ceterms:GeneralEducationDevelopment, ceterms:JourneymanCertificate, ceterms:LearningOpportunityProfile, ceterms:LearningProgram, ceterms:License, ceterms:MasterCertificate, ceterms:MasterDegree, ceterms:MicroCredential, ceterms:OpenBadge, ceterms:Pathway, ceterms:ProfessionalDoctorate, ceterms:QualityAssuranceCredential, ceterms:ResearchDoctorate, ceterms:SecondarySchoolDiploma ;
	schema:rangeIncludes ceterms:ApprenticeshipCertificate, ceterms:AssessmentComponent, ceterms:AssociateDegree, ceterms:BachelorDegree, ceterms:Badge, ceterms:BasicComponent, ceterms:Certificate, ceterms:CertificateOfCompletion, ceterms:Certification, ceterms:CocurricularComponent, ceterms:CompetencyComponent, ceterms:Course, ceterms:CourseComponent, ceterms:Credential, ceterms:CredentialComponent, ceterms:Degree, ceterms:DigitalBadge, ceterms:Diploma, ceterms:DoctoralDegree, ceterms:ExtracurricularComponent, ceterms:GeneralEducationDevelopment, ceterms:JobComponent, ceterms:JourneymanCertificate, ceterms:LearningOpportunityProfile, ceterms:LearningProgram, ceterms:License, ceterms:MasterCertificate, ceterms:MasterDegree, ceterms:MicroCredential, ceterms:OpenBadge, ceterms:ProfessionalDoctorate, ceterms:QualityAssuranceCredential, ceterms:ResearchDoctorate, ceterms:SecondarySchoolDiploma, ceterms:WorkExperienceComponent ;
	owl:equivalentProperty dct:hasPart, schema:hasPart .

ceterms:hasPathway a rdf:Property ;
	rdfs:label "Has Pathway"@en-US ;
	rdfs:comment "A pathway related to this resource."@en-US ;
	vs:term_status vs:stable ;
	meta:changeHistory <http://credreg.net/ctdl/termhistory/ceterms/hasPathway/json> ;
	schema:domainIncludes ceterms:PathwaySet ;
	schema:rangeIncludes ceterms:Pathway .

ceterms:hasProxy a rdf:Property ;
	rdfs:label "Has Proxy"@en-US ;
	rdfs:comment "Indicates a resource that acts as a stand-in for the resource."@en-US ;
	vs:term_status vs:unstable ;
	meta:changeHistory <http://credreg.net/ctdl/termhistory/ceterms/hasProxy/json> ;
	schema:domainIncludes ceterms:ApprenticeshipCertificate, ceterms:AssessmentProfile, ceterms:AssociateDegree, ceterms:BachelorDegree, ceterms:Badge, ceterms:Certificate, ceterms:CertificateOfCompletion, ceterms:Certification, ceterms:Course, ceterms:Credential, ceterms:Degree, ceterms:DigitalBadge, ceterms:Diploma, ceterms:DoctoralDegree, ceterms:GeneralEducationDevelopment, ceterms:JourneymanCertificate, ceterms:LearningOpportunityProfile, ceterms:LearningProgram, ceterms:License, ceterms:MasterCertificate, ceterms:MasterDegree, ceterms:MicroCredential, ceterms:OpenBadge, ceterms:ProfessionalDoctorate, ceterms:QualityAssuranceCredential, ceterms:ResearchDoctorate, ceterms:SecondarySchoolDiploma ;
	schema:rangeIncludes ceterms:AssessmentComponent, ceterms:BasicComponent, ceterms:CocurricularComponent, ceterms:CollectionMember, ceterms:CompetencyComponent, ceterms:CourseComponent, ceterms:CredentialComponent, ceterms:ExtracurricularComponent, ceterms:JobComponent, ceterms:WorkExperienceComponent .

ceterms:hasSpecialization a rdf:Property ;
	rdfs:label "Has Specialization"@en-US ;
	rdfs:comment "More specialized profession, trade, or career field that is encompassed by the one being described."@en-US ;
	vs:term_status vs:stable ;
	meta:changeHistory <http://credreg.net/ctdl/termhistory/ceterms/hasSpecialization/json> ;
	schema:domainIncludes ceterms:Occupation ;
	schema:rangeIncludes ceterms:Occupation .

ceterms:hasStatement a rdf:Property ;
	rdfs:label "Has Statement"@en-US ;
	rdfs:comment "Alignment assertion belonging to the alignment map."@en-US ;
	vs:term_status vs:stable ;
	meta:changeHistory <http://credreg.net/ctdl/termhistory/ceterms/hasStatement/json> ;
	schema:domainIncludes ceterms:AlignmentMap ;
	schema:rangeIncludes rdf:Statement .

ceterms:hasTask a rdf:Property ;
	rdfs:label "Has Task"@en-US ;
	rdfs:comment "Task related to this resource."@en-US ;
	vs:term_status vs:stable ;
	meta:changeHistory <http://credreg.net/ctdl/termhistory/ceterms/hasTask/json> ;
	schema:domainIncludes ceasn:Competency, ceterms:Job, ceterms:WorkRole ;
	schema:rangeIncludes ceterms:Task .

ceterms:hasVerificationService a rdf:Property ;
	rdfs:label "Has Verification Service"@en-US ;
	rdfs:comment "Entity describing available systems provided by the agent to verify credential holders."@en-US ;
	dct:description "Systems in place to verify credential holders and communicate the current credentialing status of all credential holders to employers and other labor market participants, as well as to education and workforce development funders and regulators."@en-US ;
	vs:term_status vs:stable ;
	meta:changeHistory <http://credreg.net/ctdl/termhistory/ceterms/hasVerificationService/json> ;
	schema:domainIncludes ceterms:CredentialOrganization, ceterms:Organization, ceterms:QACredentialOrganization ;
	schema:rangeIncludes ceterms:VerificationServiceProfile .

ceterms:hasWorkforceDemand a rdf:Property ;
	rdfs:label "Has Workforce Demand"@en-US ;
	rdfs:comment "Indicates the level of demand for a resource via a demand level action."@en-US ;
	vs:term_status vs:unstable ;
	meta:changeHistory <http://credreg.net/ctdl/termhistory/ceterms/hasWorkforceDemand/json> ;
	rdfs:subPropertyOf ceterms:relatedAction ;
	schema:domainIncludes ceasn:Competency, ceterms:Occupation ;
	schema:rangeIncludes ceterms:WorkforceDemandAction .

ceterms:hasWorkRole a rdf:Property ;
	rdfs:label "Has Work Role"@en-US ;
	rdfs:comment "Work Role related to this resource."@en-US ;
	vs:term_status vs:stable ;
	meta:changeHistory <http://credreg.net/ctdl/termhistory/ceterms/hasWorkRole/json> ;
	schema:domainIncludes ceterms:Job, ceterms:Occupation ;
	schema:rangeIncludes ceterms:WorkRole .

ceterms:highEarnings a rdf:Property ;
	rdfs:label "High Earnings"@en-US ;
	rdfs:comment "Upper interquartile earnings."@en-US ;
	vs:term_status vs:stable ;
	meta:changeHistory <http://credreg.net/ctdl/termhistory/ceterms/highEarnings/json> ;
	schema:domainIncludes ceterms:AggregateDataProfile, ceterms:EarningsProfile ;
	schema:rangeIncludes xsd:integer .

ceterms:holderMustAuthorize a rdf:Property ;
	rdfs:label "Holder Must Authorize"@en-US ;
	rdfs:comment "Whether or not the credential holder must authorize the organization to provide the verification service."@en-US ;
	vs:term_status vs:stable ;
	meta:changeHistory <http://credreg.net/ctdl/termhistory/ceterms/holderMustAuthorize/json> ;
	schema:domainIncludes ceterms:VerificationServiceProfile ;
	schema:rangeIncludes xsd:boolean .

ceterms:holders a rdf:Property ;
	rdfs:label "Holders"@en-US ;
	rdfs:comment "Entity describing the number and characteristics of credentialed individuals and their geographic location."@en-US ;
	vann:usageNote "The use of ceterms:aggregateData instead of this property is strongly recommended."@en-US ;
	vs:term_status vs:stable ;
	meta:changeHistory <http://credreg.net/ctdl/termhistory/ceterms/holders/json> ;
	rdfs:subPropertyOf ceterms:aggregateData ;
	schema:domainIncludes ceterms:ApprenticeshipCertificate, ceterms:AssociateDegree, ceterms:BachelorDegree, ceterms:Badge, ceterms:Certificate, ceterms:CertificateOfCompletion, ceterms:Certification, ceterms:Credential, ceterms:Degree, ceterms:DigitalBadge, ceterms:Diploma, ceterms:DoctoralDegree, ceterms:GeneralEducationDevelopment, ceterms:JourneymanCertificate, ceterms:License, ceterms:MasterCertificate, ceterms:MasterDegree, ceterms:MicroCredential, ceterms:OpenBadge, ceterms:ProfessionalDoctorate, ceterms:QualityAssuranceCredential, ceterms:ResearchDoctorate, ceterms:SecondarySchoolDiploma ;
	schema:rangeIncludes ceterms:HoldersProfile .

ceterms:honorificSuffix a rdf:Property ;
	rdfs:label "Honorific Suffix"@en-US ;
	rdfs:comment "Honorific suffix preceding a person's name such as M.D. , PhD, or MSCSW."@en-US ;
	vs:term_status vs:stable ;
	meta:changeHistory <http://credreg.net/ctdl/termhistory/ceterms/honorificSuffix/json> ;
	schema:domainIncludes ceterms:CredentialPerson ;
	schema:rangeIncludes rdf:langString ;
	owl:equivalentProperty ceterms:ContactPoint .

ceterms:identifier a rdf:Property ;
	rdfs:label "Identifier"@en-US ;
	rdfs:comment "Alphanumeric token that identifies this resource and information about the token's originating context or scheme."@en-US ;
	vann:usageNote "Where a specific property for the originating context or scheme exists, such as ceterms:opeID, ceterms:ncesID, ceterms:leiCode, etc., use that property instead of this one. Where the identifier has no nameable originating context or scheme other than that of the resource being identified, ceterms:codedNotation may be used."@en-US ;
	vs:term_status vs:stable ;
	meta:changeHistory <http://credreg.net/ctdl/termhistory/ceterms/identifier/json> ;
	schema:domainIncludes ceterms:ApprenticeshipCertificate, ceterms:AssessmentComponent, ceterms:AssessmentProfile, ceterms:AssociateDegree, ceterms:BachelorDegree, ceterms:Badge, ceterms:BasicComponent, ceterms:Certificate, ceterms:CertificateOfCompletion, ceterms:Certification, ceterms:CocurricularComponent, ceterms:CompetencyComponent, ceterms:Course, ceterms:CourseComponent, ceterms:Credential, ceterms:CredentialComponent, ceterms:CredentialOrganization, ceterms:Degree, ceterms:DigitalBadge, ceterms:Diploma, ceterms:DoctoralDegree, ceterms:ExtracurricularComponent, ceterms:GeneralEducationDevelopment, ceterms:Job, ceterms:JobComponent, ceterms:JourneymanCertificate, ceterms:LearningOpportunityProfile, ceterms:LearningProgram, ceterms:License, ceterms:MasterCertificate, ceterms:MasterDegree, ceterms:MicroCredential, ceterms:Occupation, ceterms:OpenBadge, ceterms:Organization, ceterms:Place, ceterms:ProfessionalDoctorate, ceterms:QACredentialOrganization, ceterms:QualityAssuranceCredential, ceterms:ResearchDoctorate, ceterms:SecondarySchoolDiploma, ceterms:Task, ceterms:TransferValueProfile, ceterms:WorkExperienceComponent, ceterms:WorkRole ;
	schema:rangeIncludes ceterms:IdentifierValue .

ceterms:identifierType a rdf:Property ;
	rdfs:label "Identifier Type"@en-US ;
	rdfs:comment "Framework, scheme, type, or other organizing principle of this identifier."@en-US ;
	vs:term_status vs:stable ;
	meta:changeHistory <http://credreg.net/ctdl/termhistory/ceterms/identifierType/json> ;
	schema:domainIncludes ceterms:IdentifierValue ;
	schema:rangeIncludes xsd:anyURI .

ceterms:identifierTypeName a rdf:Property ;
	rdfs:label "Identifier Type Name"@en-US ;
	rdfs:comment "Formal name or acronym of the framework, scheme, type, or other organizing principle of this identifier, such as ISBN or ISSN."@en-US ;
	vs:term_status vs:stable ;
	meta:changeHistory <http://credreg.net/ctdl/termhistory/ceterms/identifierTypeName/json> ;
	schema:domainIncludes ceterms:IdentifierValue ;
	schema:rangeIncludes rdf:langString .

ceterms:identifierValueCode a rdf:Property ;
	rdfs:label "Identifier Value Code"@en-US ;
	rdfs:comment "Alphanumeric string identifier of the entity."@en-US ;
	dct:description "Where a formal identification system exists for the identifier, recommended best practice is to use a string conforming to that system."@en-US ;
	vs:term_status vs:stable ;
	meta:changeHistory <http://credreg.net/ctdl/termhistory/ceterms/identifierValueCode/json> ;
	schema:domainIncludes ceterms:IdentifierValue ;
	schema:rangeIncludes xsd:string .

ceterms:image a rdf:Property ;
	rdfs:label "Image"@en-US ;
	rdfs:comment "Image, icon or logo that represents the entity including registered trade or service marks."@en-US ;
	vs:term_status vs:stable ;
	meta:changeHistory <http://credreg.net/ctdl/termhistory/ceterms/image/json> ;
	schema:domainIncludes ceterms:ApprenticeshipCertificate, ceterms:AssociateDegree, ceterms:BachelorDegree, ceterms:Badge, ceterms:Certificate, ceterms:CertificateOfCompletion, ceterms:Certification, ceterms:Credential, ceterms:CredentialOrganization, ceterms:Degree, ceterms:DigitalBadge, ceterms:Diploma, ceterms:DoctoralDegree, ceterms:GeneralEducationDevelopment, ceterms:JourneymanCertificate, ceterms:License, ceterms:MasterCertificate, ceterms:MasterDegree, ceterms:MicroCredential, ceterms:OpenBadge, ceterms:Organization, ceterms:ProfessionalDoctorate, ceterms:QACredentialOrganization, ceterms:QualityAssuranceCredential, ceterms:ResearchDoctorate, ceterms:SecondarySchoolDiploma ;
	schema:rangeIncludes xsd:anyURI ;
	owl:equivalentProperty schema:image .

ceterms:inAlignmentMap a rdf:Property ;
	rdfs:label "In Alignment Map"@en-US ;
	rdfs:comment "Alignment map to which the statement belongs."@en-US ;
	vs:term_status vs:stable ;
	meta:changeHistory <http://credreg.net/ctdl/termhistory/ceterms/inAlignmentMap/json> ;
	schema:domainIncludes rdf:Statement ;
	schema:rangeIncludes ceterms:AlignmentMap .

ceterms:inDemandAction a rdf:Property ;
	rdfs:label "In Demand Action"@en-US ;
	rdfs:comment "Assertion by an agent that this resource has a specific workforce demand level."@en-US ;
	vs:term_status vs:unstable ;
	meta:changeHistory <http://credreg.net/ctdl/termhistory/ceterms/inDemandAction/json> ;
	rdfs:subPropertyOf ceterms:relatedAction ;
	schema:domainIncludes ceterms:CredentialOrganization, ceterms:Organization, ceterms:QACredentialOrganization ;
	schema:rangeIncludes ceterms:WorkforceDemandAction .

ceterms:industryType a rdf:Property ;
	rdfs:label "Industry Type"@en-US ;
	rdfs:comment "Type of industry; select from an existing enumeration of such types such as the SIC, NAICS, and ISIC classifications."@en-US ;
	vann:usageNote "Best practice in identifying industries for U.S. resources is to provide the NAICS code using the ceterms:naics property. Other resources may use the ceterms:industrytype property and any framework of the class ceterms:IndustryClassification."@en-US ;
	vs:term_status vs:stable ;
	meta:changeHistory <http://credreg.net/ctdl/termhistory/ceterms/industryType/json> ;
	rdfs:subPropertyOf ceterms:credentialAlignment ;
	schema:domainIncludes ceasn:Collection, ceasn:CompetencyFramework, ceterms:ApprenticeshipCertificate, ceterms:AssessmentProfile, ceterms:AssociateDegree, ceterms:BachelorDegree, ceterms:Badge, ceterms:Certificate, ceterms:CertificateOfCompletion, ceterms:Certification, ceterms:Collection, ceterms:Course, ceterms:Credential, ceterms:CredentialOrganization, ceterms:Degree, ceterms:DigitalBadge, ceterms:Diploma, ceterms:DoctoralDegree, ceterms:GeneralEducationDevelopment, ceterms:Job, ceterms:JobComponent, ceterms:JourneymanCertificate, ceterms:LearningOpportunityProfile, ceterms:LearningProgram, ceterms:License, ceterms:MasterCertificate, ceterms:MasterDegree, ceterms:MicroCredential, ceterms:Occupation, ceterms:OpenBadge, ceterms:Organization, ceterms:Pathway, ceterms:ProfessionalDoctorate, ceterms:QACredentialOrganization, ceterms:QualityAssuranceCredential, ceterms:ResearchDoctorate, ceterms:SecondarySchoolDiploma ;
	schema:rangeIncludes ceterms:CredentialAlignmentObject ;
	meta:targetScheme ceterms:IndustryClassification .

ceterms:inLanguage a rdf:Property ;
	rdfs:label "In Language"@en-US ;
	rdfs:comment "The primary language or languages of the entity, even if it makes use of other languages; e.g., a course offered in English to teach Spanish would have an inLanguage of English, while a credential in Quebec could have an inLanguage of both French and English."@en-US ;
	vs:term_status vs:stable ;
	meta:changeHistory <http://credreg.net/ctdl/termhistory/ceterms/inLanguage/json> ;
	schema:domainIncludes ceterms:ApprenticeshipCertificate, ceterms:AssessmentProfile, ceterms:AssociateDegree, ceterms:BachelorDegree, ceterms:Badge, ceterms:Certificate, ceterms:CertificateOfCompletion, ceterms:Certification, ceterms:Collection, ceterms:Course, ceterms:Credential, ceterms:Degree, ceterms:DigitalBadge, ceterms:Diploma, ceterms:DoctoralDegree, ceterms:GeneralEducationDevelopment, ceterms:JourneymanCertificate, ceterms:LearningOpportunityProfile, ceterms:LearningProgram, ceterms:License, ceterms:MasterCertificate, ceterms:MasterDegree, ceterms:MicroCredential, ceterms:OpenBadge, ceterms:ProfessionalDoctorate, ceterms:QualityAssuranceCredential, ceterms:ResearchDoctorate, ceterms:SecondarySchoolDiploma ;
	schema:rangeIncludes xsd:language ;
	owl:equivalentProperty schema:inLanguage .

ceterms:instructionalProgramType a rdf:Property ;
	rdfs:label "Instructional Program Type"@en-US ;
	rdfs:comment "Type of instructional program; select from an existing enumeration of such types."@en-US ;
	vann:usageNote "For U.S. credentials, best practice is to use a framework such as the CIP (Classification of Instructional Programs). Other credentials may use any framework of the class CTDL InstructionalProgramClassification."@en-US ;
	vs:term_status vs:stable ;
	meta:changeHistory <http://credreg.net/ctdl/termhistory/ceterms/instructionalProgramType/json> ;
	rdfs:subPropertyOf ceterms:credentialAlignment ;
	schema:domainIncludes ceasn:Collection, ceterms:ApprenticeshipCertificate, ceterms:AssessmentProfile, ceterms:AssociateDegree, ceterms:BachelorDegree, ceterms:Badge, ceterms:Certificate, ceterms:CertificateOfCompletion, ceterms:Certification, ceterms:Collection, ceterms:Course, ceterms:Credential, ceterms:Degree, ceterms:DigitalBadge, ceterms:Diploma, ceterms:DoctoralDegree, ceterms:GeneralEducationDevelopment, ceterms:JourneymanCertificate, ceterms:LearningOpportunityProfile, ceterms:LearningProgram, ceterms:License, ceterms:MasterCertificate, ceterms:MasterDegree, ceterms:MicroCredential, ceterms:OpenBadge, ceterms:Pathway, ceterms:ProfessionalDoctorate, ceterms:QualityAssuranceCredential, ceterms:ResearchDoctorate, ceterms:SecondarySchoolDiploma ;
	schema:rangeIncludes ceterms:CredentialAlignmentObject ;
	meta:targetScheme ceterms:InstructionalProgramClassification .

ceterms:instrument a rdf:Property ;
	rdfs:label "Instrument"@en-US ;
	rdfs:comment "Object that helped the agent perform the action. e.g. John wrote a book with a pen."@en-US ;
	dct:description "A credential or other instrument whose criteria was applied in executing the action."@en-US ;
	vs:term_status vs:stable ;
	meta:changeHistory <http://credreg.net/ctdl/termhistory/ceterms/instrument/json> ;
	schema:domainIncludes ceterms:AccreditAction, ceterms:AdvancedStandingAction, ceterms:ApproveAction, ceterms:CredentialingAction, ceterms:OfferAction, ceterms:RecognizeAction, ceterms:RegulateAction, ceterms:RenewAction, ceterms:RevokeAction, ceterms:RightsAction, ceterms:WorkforceDemandAction ;
	schema:rangeIncludes ceterms:ApprenticeshipCertificate, ceterms:AssociateDegree, ceterms:BachelorDegree, ceterms:Badge, ceterms:Certificate, ceterms:CertificateOfCompletion, ceterms:Certification, ceterms:Credential, ceterms:Degree, ceterms:DigitalBadge, ceterms:Diploma, ceterms:DoctoralDegree, ceterms:GeneralEducationDevelopment, ceterms:JourneymanCertificate, ceterms:License, ceterms:MasterCertificate, ceterms:MasterDegree, ceterms:MicroCredential, ceterms:OpenBadge, ceterms:ProfessionalDoctorate, ceterms:QualityAssuranceCredential, ceterms:ResearchDoctorate, ceterms:SecondarySchoolDiploma ;
	owl:equivalentProperty schema:instrument .

ceterms:intermediaryFor a rdf:Property ;
	rdfs:label "Intermediary For"@en-US ;
	rdfs:comment "Resource for which this resource is an intermediary."@en-US ;
	vs:term_status vs:unstable ;
	meta:changeHistory <http://credreg.net/ctdl/termhistory/ceterms/intermediaryFor/json> ;
	schema:domainIncludes ceterms:TransferIntermediary ;
	schema:rangeIncludes ceterms:TransferValueProfile .

ceterms:ipedsID a rdf:Property ;
	rdfs:label "IPEDS ID"@en-US ;
	rdfs:comment "Unique six digit identifier assigned to all U.S. institutions that have submitted data to the Integrated Postsecondary Education Data System (IPEDS)."@en-US ;
	vs:term_status vs:stable ;
	meta:changeHistory <http://credreg.net/ctdl/termhistory/ceterms/ipedsID/json> ;
	schema:domainIncludes ceterms:CredentialOrganization, ceterms:Organization, ceterms:QACredentialOrganization ;
	schema:rangeIncludes xsd:string .

ceterms:isAdvancedStandingFor a rdf:Property ;
	rdfs:label "Is Advanced Standing For"@en-US ;
	rdfs:comment "This credential, assessment, or learning opportunity reduces the time or cost required to earn or complete the referenced credential, assessment, or learning opportunity."@en-US ;
	vann:usageNote "A third-party credential agent claiming that its credential provides advanced standing for the credential of another credential agent should consider using ceterms:recommendedFor instead of ceterms:advancedStandingFor in the absence of an explicit and verifiable agreement on advanced standing between the agents of the two credentials."@en-US ;
	vs:term_status vs:stable ;
	meta:changeHistory <http://credreg.net/ctdl/termhistory/ceterms/isAdvancedStandingFor/json> ;
	schema:domainIncludes ceterms:ApprenticeshipCertificate, ceterms:AssessmentProfile, ceterms:AssociateDegree, ceterms:BachelorDegree, ceterms:Badge, ceterms:Certificate, ceterms:CertificateOfCompletion, ceterms:Certification, ceterms:Course, ceterms:Credential, ceterms:Degree, ceterms:DigitalBadge, ceterms:Diploma, ceterms:DoctoralDegree, ceterms:GeneralEducationDevelopment, ceterms:JourneymanCertificate, ceterms:LearningOpportunityProfile, ceterms:LearningProgram, ceterms:License, ceterms:MasterCertificate, ceterms:MasterDegree, ceterms:MicroCredential, ceterms:OpenBadge, ceterms:ProfessionalDoctorate, ceterms:QualityAssuranceCredential, ceterms:ResearchDoctorate, ceterms:SecondarySchoolDiploma ;
	schema:rangeIncludes ceterms:ApprenticeshipCertificate, ceterms:AssessmentProfile, ceterms:AssociateDegree, ceterms:BachelorDegree, ceterms:Badge, ceterms:Certificate, ceterms:CertificateOfCompletion, ceterms:Certification, ceterms:ConditionProfile, ceterms:Course, ceterms:Credential, ceterms:Degree, ceterms:DigitalBadge, ceterms:Diploma, ceterms:DoctoralDegree, ceterms:GeneralEducationDevelopment, ceterms:JourneymanCertificate, ceterms:LearningOpportunityProfile, ceterms:LearningProgram, ceterms:License, ceterms:MasterCertificate, ceterms:MasterDegree, ceterms:MicroCredential, ceterms:OpenBadge, ceterms:ProfessionalDoctorate, ceterms:QualityAssuranceCredential, ceterms:ResearchDoctorate, ceterms:SecondarySchoolDiploma .

ceterms:isDestinationComponentOf a rdf:Property ;
	rdfs:label "Is Destination Component Of"@en-US ;
	rdfs:comment "Pathway for which this resource is the goal or destination."@en-US ;
	vs:term_status vs:stable ;
	meta:changeHistory <http://credreg.net/ctdl/termhistory/ceterms/isDestinationComponentOf/json> ;
	schema:domainIncludes ceterms:AssessmentComponent, ceterms:BasicComponent, ceterms:CocurricularComponent, ceterms:CompetencyComponent, ceterms:CourseComponent, ceterms:CredentialComponent, ceterms:ExtracurricularComponent, ceterms:JobComponent, ceterms:WorkExperienceComponent ;
	schema:rangeIncludes ceterms:Pathway .

ceterms:isicV4 a rdf:Property ;
	rdfs:label "ISIC Revision 4 Code"@en-US ;
	rdfs:comment "The International Standard of Industrial Classification of All Economic Activities (ISIC), Revision 4 code for a particular organization, business person, or place."@en-US ;
	vs:term_status vs:stable ;
	meta:changeHistory <http://credreg.net/ctdl/termhistory/ceterms/isicV4/json> ;
	schema:domainIncludes ceterms:ApprenticeshipCertificate, ceterms:AssociateDegree, ceterms:BachelorDegree, ceterms:Badge, ceterms:Certificate, ceterms:CertificateOfCompletion, ceterms:Certification, ceterms:Credential, ceterms:CredentialOrganization, ceterms:Degree, ceterms:DigitalBadge, ceterms:Diploma, ceterms:DoctoralDegree, ceterms:GeneralEducationDevelopment, ceterms:JourneymanCertificate, ceterms:License, ceterms:MasterCertificate, ceterms:MasterDegree, ceterms:MicroCredential, ceterms:OpenBadge, ceterms:Organization, ceterms:ProfessionalDoctorate, ceterms:QACredentialOrganization, ceterms:QualityAssuranceCredential, ceterms:ResearchDoctorate, ceterms:SecondarySchoolDiploma ;
	schema:rangeIncludes xsd:string ;
	owl:equivalentProperty schema:isicV4 .

ceterms:isMemberOf a rdf:Property ;
	rdfs:label "Is Member Of"@en-US ;
	rdfs:comment "Collection to which this resource belongs."@en-US ;
	vs:term_status vs:unstable ;
	meta:changeHistory <http://credreg.net/ctdl/termhistory/ceterms/isMemberOf/json> ;
	schema:domainIncludes ceasn:Competency, ceterms:Course, ceterms:Job, ceterms:LearningOpportunityProfile, ceterms:LearningProgram, ceterms:Task, ceterms:WorkRole ;
	schema:rangeIncludes ceterms:Collection .

ceterms:isNonCredit a rdf:Property ;
	rdfs:label "Is Non-Credit"@en-US ;
	rdfs:comment "Resource carries or confers no official academic credit towards a program or a credential."@en-US ;
	vs:term_status vs:unstable ;
	meta:changeHistory <http://credreg.net/ctdl/termhistory/ceterms/isNonCredit/json> ;
	schema:domainIncludes ceterms:AssessmentProfile, ceterms:Course, ceterms:LearningOpportunityProfile, ceterms:LearningProgram ;
	schema:rangeIncludes xsd:boolean .

ceterms:isPartOf a rdf:Property ;
	rdfs:label "Is Part Of"@en-US ;
	rdfs:comment "Indicates another entity of which this entity is a component."@en-US ;
	dct:description "Covers partitive notions such as \"embedded\"."@en-US ;
	vs:term_status vs:stable ;
	meta:changeHistory <http://credreg.net/ctdl/termhistory/ceterms/isPartOf/json> ;
	schema:domainIncludes ceterms:ApprenticeshipCertificate, ceterms:AssessmentComponent, ceterms:AssociateDegree, ceterms:BachelorDegree, ceterms:Badge, ceterms:BasicComponent, ceterms:Certificate, ceterms:CertificateOfCompletion, ceterms:Certification, ceterms:CocurricularComponent, ceterms:CompetencyComponent, ceterms:Course, ceterms:CourseComponent, ceterms:Credential, ceterms:CredentialComponent, ceterms:Degree, ceterms:DigitalBadge, ceterms:Diploma, ceterms:DoctoralDegree, ceterms:ExtracurricularComponent, ceterms:GeneralEducationDevelopment, ceterms:JobComponent, ceterms:JourneymanCertificate, ceterms:LearningOpportunityProfile, ceterms:LearningProgram, ceterms:License, ceterms:MasterCertificate, ceterms:MasterDegree, ceterms:MicroCredential, ceterms:OpenBadge, ceterms:ProfessionalDoctorate, ceterms:QualityAssuranceCredential, ceterms:ResearchDoctorate, ceterms:SecondarySchoolDiploma, ceterms:WorkExperienceComponent ;
	schema:rangeIncludes ceterms:ApprenticeshipCertificate, ceterms:AssociateDegree, ceterms:BachelorDegree, ceterms:Badge, ceterms:Certificate, ceterms:CertificateOfCompletion, ceterms:Certification, ceterms:Course, ceterms:Credential, ceterms:Degree, ceterms:DigitalBadge, ceterms:Diploma, ceterms:DoctoralDegree, ceterms:GeneralEducationDevelopment, ceterms:JourneymanCertificate, ceterms:LearningOpportunityProfile, ceterms:LearningProgram, ceterms:License, ceterms:MasterCertificate, ceterms:MasterDegree, ceterms:MicroCredential, ceterms:OpenBadge, ceterms:Pathway, ceterms:ProfessionalDoctorate, ceterms:QualityAssuranceCredential, ceterms:ResearchDoctorate, ceterms:SecondarySchoolDiploma ;
	owl:equivalentProperty dct:isPartOf, schema:isPartOf .

ceterms:isPreparationFor a rdf:Property ;
	rdfs:label "Is Preparation For"@en-US ;
	rdfs:comment "This credential, assessment, or learning opportunity provides preparation for the credential, assessment, or learning opportunity being referenced."@en-US ;
	vs:term_status vs:stable ;
	meta:changeHistory <http://credreg.net/ctdl/termhistory/ceterms/isPreparationFor/json> ;
	schema:domainIncludes ceterms:ApprenticeshipCertificate, ceterms:AssessmentProfile, ceterms:AssociateDegree, ceterms:BachelorDegree, ceterms:Badge, ceterms:Certificate, ceterms:CertificateOfCompletion, ceterms:Certification, ceterms:Course, ceterms:Credential, ceterms:Degree, ceterms:DigitalBadge, ceterms:Diploma, ceterms:DoctoralDegree, ceterms:GeneralEducationDevelopment, ceterms:JourneymanCertificate, ceterms:LearningOpportunityProfile, ceterms:LearningProgram, ceterms:License, ceterms:MasterCertificate, ceterms:MasterDegree, ceterms:MicroCredential, ceterms:OpenBadge, ceterms:ProfessionalDoctorate, ceterms:QualityAssuranceCredential, ceterms:ResearchDoctorate, ceterms:SecondarySchoolDiploma ;
	schema:rangeIncludes ceterms:ApprenticeshipCertificate, ceterms:AssessmentProfile, ceterms:AssociateDegree, ceterms:BachelorDegree, ceterms:Badge, ceterms:Certificate, ceterms:CertificateOfCompletion, ceterms:Certification, ceterms:ConditionProfile, ceterms:Course, ceterms:Credential, ceterms:Degree, ceterms:DigitalBadge, ceterms:Diploma, ceterms:DoctoralDegree, ceterms:GeneralEducationDevelopment, ceterms:JourneymanCertificate, ceterms:LearningOpportunityProfile, ceterms:LearningProgram, ceterms:License, ceterms:MasterCertificate, ceterms:MasterDegree, ceterms:MicroCredential, ceterms:OpenBadge, ceterms:ProfessionalDoctorate, ceterms:QualityAssuranceCredential, ceterms:ResearchDoctorate, ceterms:SecondarySchoolDiploma .

ceterms:isProctored a rdf:Property ;
	rdfs:label "Is Proctored"@en-US ;
	rdfs:comment "Whether or not the assessment is supervised or monitored by an agent."@en-US ;
	dct:description "Such supervision or proctoring includes: (1)  guaranteeing of the identities of the examinees; (2) the conditions of the examination including instructions, time, materials, equipment and completion, and (3) completed without unauthorized assistance."@en-US ;
	vs:term_status vs:stable ;
	meta:changeHistory <http://credreg.net/ctdl/termhistory/ceterms/isProctored/json> ;
	schema:domainIncludes ceterms:AssessmentProfile ;
	schema:rangeIncludes xsd:boolean .

ceterms:isRecommendedFor a rdf:Property ;
	rdfs:label "Is Recommended For"@en-US ;
	rdfs:comment "It is recommended to earn or complete this credential, assessment, or learning opportunity before attempting to earn or complete the referenced credential, assessment, or learning opportunity."@en-US ;
	vs:term_status vs:stable ;
	meta:changeHistory <http://credreg.net/ctdl/termhistory/ceterms/isRecommendedFor/json> ;
	schema:domainIncludes ceterms:ApprenticeshipCertificate, ceterms:AssessmentProfile, ceterms:AssociateDegree, ceterms:BachelorDegree, ceterms:Badge, ceterms:Certificate, ceterms:CertificateOfCompletion, ceterms:Certification, ceterms:Course, ceterms:Credential, ceterms:Degree, ceterms:DigitalBadge, ceterms:Diploma, ceterms:DoctoralDegree, ceterms:GeneralEducationDevelopment, ceterms:JourneymanCertificate, ceterms:LearningOpportunityProfile, ceterms:LearningProgram, ceterms:License, ceterms:MasterCertificate, ceterms:MasterDegree, ceterms:MicroCredential, ceterms:OpenBadge, ceterms:ProfessionalDoctorate, ceterms:QualityAssuranceCredential, ceterms:ResearchDoctorate, ceterms:SecondarySchoolDiploma ;
	schema:rangeIncludes ceterms:ApprenticeshipCertificate, ceterms:AssessmentProfile, ceterms:AssociateDegree, ceterms:BachelorDegree, ceterms:Badge, ceterms:Certificate, ceterms:CertificateOfCompletion, ceterms:Certification, ceterms:ConditionProfile, ceterms:Course, ceterms:Credential, ceterms:Degree, ceterms:DigitalBadge, ceterms:Diploma, ceterms:DoctoralDegree, ceterms:GeneralEducationDevelopment, ceterms:JourneymanCertificate, ceterms:LearningOpportunityProfile, ceterms:LearningProgram, ceterms:License, ceterms:MasterCertificate, ceterms:MasterDegree, ceterms:MicroCredential, ceterms:OpenBadge, ceterms:ProfessionalDoctorate, ceterms:QualityAssuranceCredential, ceterms:ResearchDoctorate, ceterms:SecondarySchoolDiploma .

ceterms:isRequiredFor a rdf:Property ;
	rdfs:label "Is Required For"@en-US ;
	rdfs:comment "This credential, assessment, or learning opportunity must be earned or completed prior to attempting to earn or complete the referenced credential, assessment, or learning opportunity."@en-US ;
	vs:term_status vs:stable ;
	meta:changeHistory <http://credreg.net/ctdl/termhistory/ceterms/isRequiredFor/json> ;
	schema:domainIncludes ceterms:ApprenticeshipCertificate, ceterms:AssessmentProfile, ceterms:AssociateDegree, ceterms:BachelorDegree, ceterms:Badge, ceterms:Certificate, ceterms:CertificateOfCompletion, ceterms:Certification, ceterms:Course, ceterms:Credential, ceterms:Degree, ceterms:DigitalBadge, ceterms:Diploma, ceterms:DoctoralDegree, ceterms:GeneralEducationDevelopment, ceterms:JourneymanCertificate, ceterms:LearningOpportunityProfile, ceterms:LearningProgram, ceterms:License, ceterms:MasterCertificate, ceterms:MasterDegree, ceterms:MicroCredential, ceterms:OpenBadge, ceterms:ProfessionalDoctorate, ceterms:QualityAssuranceCredential, ceterms:ResearchDoctorate, ceterms:SecondarySchoolDiploma ;
	schema:rangeIncludes ceterms:ApprenticeshipCertificate, ceterms:AssessmentProfile, ceterms:AssociateDegree, ceterms:BachelorDegree, ceterms:Badge, ceterms:Certificate, ceterms:CertificateOfCompletion, ceterms:Certification, ceterms:ConditionProfile, ceterms:Course, ceterms:Credential, ceterms:Degree, ceterms:DigitalBadge, ceterms:Diploma, ceterms:DoctoralDegree, ceterms:GeneralEducationDevelopment, ceterms:JourneymanCertificate, ceterms:LearningOpportunityProfile, ceterms:LearningProgram, ceterms:License, ceterms:MasterCertificate, ceterms:MasterDegree, ceterms:MicroCredential, ceterms:OpenBadge, ceterms:ProfessionalDoctorate, ceterms:QualityAssuranceCredential, ceterms:ResearchDoctorate, ceterms:SecondarySchoolDiploma .

ceterms:isSimilarTo a rdf:Property ;
	rdfs:label "Is Similar To"@en-US ;
	rdfs:comment "Another functionally similar entity."@en-US ;
	dct:description "The property is generally applicable in describing the similarity between any two entities."@en-US ;
	vs:term_status vs:stable ;
	meta:changeHistory <http://credreg.net/ctdl/termhistory/ceterms/isSimilarTo/json> ;
	schema:rangeIncludes xsd:anyURI ;
	owl:equivalentProperty schema:isSimilarTo, skos:related .

ceterms:isSpecializationOf a rdf:Property ;
	rdfs:label "Is Specialization Of"@en-US ;
	rdfs:comment "Less specialized profession, trade, or career field that encompasses the one being described."@en-US ;
	vs:term_status vs:stable ;
	meta:changeHistory <http://credreg.net/ctdl/termhistory/ceterms/isSpecializationOf/json> ;
	schema:domainIncludes ceterms:Occupation ;
	schema:rangeIncludes ceterms:Occupation .

ceterms:jobsObtained a rdf:Property ;
	rdfs:label "Jobs Obtained"@en-US ;
	rdfs:comment "Number of jobs obtained in the region during a given timeframe."@en-US ;
	vs:term_status vs:stable ;
	meta:changeHistory <http://credreg.net/ctdl/termhistory/ceterms/jobsObtained/json> ;
	schema:domainIncludes ceterms:AggregateDataProfile, ceterms:EmploymentOutcomeProfile ;
	schema:rangeIncludes schema:QuantitativeValue .

ceterms:jurisdiction a rdf:Property ;
	rdfs:label "Jurisdiction"@en-US ;
	rdfs:comment "Geographic or political region in which the credential is formally applicable or an organization has authority to act."@en-US ;
	vs:term_status vs:stable ;
	meta:changeHistory <http://credreg.net/ctdl/termhistory/ceterms/jurisdiction/json> ;
	schema:domainIncludes ceterms:AggregateDataProfile, ceterms:ApprenticeshipCertificate, ceterms:AssessmentProfile, ceterms:AssociateDegree, ceterms:BachelorDegree, ceterms:Badge, ceterms:Certificate, ceterms:CertificateOfCompletion, ceterms:Certification, ceterms:ConditionProfile, ceterms:CostProfile, ceterms:Course, ceterms:Credential, ceterms:CredentialOrganization, ceterms:Degree, ceterms:DigitalBadge, ceterms:Diploma, ceterms:DoctoralDegree, ceterms:EarningsProfile, ceterms:EmploymentOutcomeProfile, ceterms:GeneralEducationDevelopment, ceterms:HoldersProfile, ceterms:JourneymanCertificate, ceterms:LearningOpportunityProfile, ceterms:LearningProgram, ceterms:License, ceterms:MasterCertificate, ceterms:MasterDegree, ceterms:MicroCredential, ceterms:OpenBadge, ceterms:Organization, ceterms:ProcessProfile, ceterms:ProfessionalDoctorate, ceterms:QACredentialOrganization, ceterms:QualityAssuranceCredential, ceterms:ResearchDoctorate, ceterms:RevocationProfile, ceterms:SecondarySchoolDiploma, ceterms:VerificationServiceProfile, ceterms:WorkforceDemandAction ;
	schema:rangeIncludes ceterms:JurisdictionProfile .

ceterms:jurisdictionException a rdf:Property ;
	rdfs:label "Jurisdiction Exception"@en-US ;
	rdfs:comment "Geographic or political region in which the credential is not formally recognized or an organization has no authority to act ."@en-US ;
	dct:description "The ceterms:jurisdictionalException property is used in conjunction with the ceterms:jurisdiction property and expresses any exceptions to a more general statement; e.g., the United states except for Colorado."@en-US ;
	vs:term_status vs:stable ;
	meta:changeHistory <http://credreg.net/ctdl/termhistory/ceterms/jurisdictionException/json> ;
	rdfs:subPropertyOf ceterms:spatialCoverage ;
	schema:domainIncludes ceterms:JurisdictionProfile ;
	schema:rangeIncludes ceterms:Place .

ceterms:keyword a rdf:Property ;
	rdfs:label "Keyword"@en-US ;
	rdfs:comment "Keyword or key phrase describing relevant aspects of an entity."@en-US ;
	vann:usageNote "Use the keyword property to enter free text keywords. A subject concept in a controlled vocabulary should use the subject property."@en-US ;
	vs:term_status vs:stable ;
	meta:changeHistory <http://credreg.net/ctdl/termhistory/ceterms/keyword/json> ;
	rdfs:subPropertyOf schema:about ;
	schema:domainIncludes ceterms:ApprenticeshipCertificate, ceterms:AssessmentProfile, ceterms:AssociateDegree, ceterms:BachelorDegree, ceterms:Badge, ceterms:Certificate, ceterms:CertificateOfCompletion, ceterms:Certification, ceterms:Collection, ceterms:Course, ceterms:Credential, ceterms:CredentialOrganization, ceterms:Degree, ceterms:DigitalBadge, ceterms:Diploma, ceterms:DoctoralDegree, ceterms:GeneralEducationDevelopment, ceterms:Job, ceterms:JourneymanCertificate, ceterms:LearningOpportunityProfile, ceterms:LearningProgram, ceterms:License, ceterms:MasterCertificate, ceterms:MasterDegree, ceterms:MicroCredential, ceterms:Occupation, ceterms:OpenBadge, ceterms:Organization, ceterms:Pathway, ceterms:ProfessionalDoctorate, ceterms:QACredentialOrganization, ceterms:QualityAssuranceCredential, ceterms:ResearchDoctorate, ceterms:SecondarySchoolDiploma ;
	schema:rangeIncludes rdf:langString ;
	owl:equivalentProperty ceasn:conceptKeyword .

ceterms:latestVersion a rdf:Property ;
	rdfs:label "Latest Version"@en-US ;
	rdfs:comment "Latest version of the credential."@en-US ;
	vs:term_status vs:stable ;
	meta:changeHistory <http://credreg.net/ctdl/termhistory/ceterms/latestVersion/json> ;
	schema:domainIncludes ceterms:ApprenticeshipCertificate, ceterms:AssociateDegree, ceterms:BachelorDegree, ceterms:Badge, ceterms:Certificate, ceterms:CertificateOfCompletion, ceterms:Certification, ceterms:Credential, ceterms:Degree, ceterms:DigitalBadge, ceterms:Diploma, ceterms:DoctoralDegree, ceterms:GeneralEducationDevelopment, ceterms:JourneymanCertificate, ceterms:License, ceterms:MasterCertificate, ceterms:MasterDegree, ceterms:MicroCredential, ceterms:OpenBadge, ceterms:ProfessionalDoctorate, ceterms:QualityAssuranceCredential, ceterms:ResearchDoctorate, ceterms:SecondarySchoolDiploma ;
	schema:rangeIncludes ceterms:ApprenticeshipCertificate, ceterms:AssociateDegree, ceterms:BachelorDegree, ceterms:Badge, ceterms:Certificate, ceterms:CertificateOfCompletion, ceterms:Certification, ceterms:Credential, ceterms:Degree, ceterms:DigitalBadge, ceterms:Diploma, ceterms:DoctoralDegree, ceterms:GeneralEducationDevelopment, ceterms:JourneymanCertificate, ceterms:License, ceterms:MasterCertificate, ceterms:MasterDegree, ceterms:MicroCredential, ceterms:OpenBadge, ceterms:ProfessionalDoctorate, ceterms:QualityAssuranceCredential, ceterms:ResearchDoctorate, ceterms:SecondarySchoolDiploma .

ceterms:latitude a rdf:Property ;
	rdfs:label "Latitude"@en-US ;
	rdfs:comment "Latitude of a location."@en-US ;
	dct:description "For example 37.42242 (WGS 84)"@en-US ;
	vs:term_status vs:stable ;
	meta:changeHistory <http://credreg.net/ctdl/termhistory/ceterms/latitude/json> ;
	schema:domainIncludes ceterms:GeoCoordinates, ceterms:Place ;
	schema:rangeIncludes xsd:float ;
	owl:equivalentProperty schema:latitude .

ceterms:learningDeliveryType a rdf:Property ;
	rdfs:label "Learning Delivery Type"@en-US ;
	rdfs:comment "Delivery type for the learning opportunity for the credential."@en-US ;
	dct:description "Indicates the delivery type for the learning opportunity for the credential."@en-US ;
	vs:term_status vs:stable ;
	meta:changeHistory <http://credreg.net/ctdl/termhistory/ceterms/learningDeliveryType/json> ;
	rdfs:subPropertyOf ceterms:deliveryType ;
	schema:domainIncludes ceterms:ApprenticeshipCertificate, ceterms:AssociateDegree, ceterms:BachelorDegree, ceterms:Badge, ceterms:Certificate, ceterms:CertificateOfCompletion, ceterms:Certification, ceterms:Credential, ceterms:Degree, ceterms:DigitalBadge, ceterms:Diploma, ceterms:DoctoralDegree, ceterms:GeneralEducationDevelopment, ceterms:JourneymanCertificate, ceterms:License, ceterms:MasterCertificate, ceterms:MasterDegree, ceterms:MicroCredential, ceterms:OpenBadge, ceterms:ProfessionalDoctorate, ceterms:QualityAssuranceCredential, ceterms:ResearchDoctorate, ceterms:SecondarySchoolDiploma ;
	schema:rangeIncludes ceterms:CredentialAlignmentObject ;
	meta:targetScheme ceterms:Delivery .

ceterms:learningMethodDescription a rdf:Property ;
	rdfs:label "Learning Method Description"@en-US ;
	rdfs:comment "Description of the methods used to conduct learning."@en-US ;
	vs:term_status vs:stable ;
	meta:changeHistory <http://credreg.net/ctdl/termhistory/ceterms/learningMethodDescription/json> ;
	schema:domainIncludes ceterms:AssessmentProfile, ceterms:Course, ceterms:LearningOpportunityProfile, ceterms:LearningProgram ;
	schema:rangeIncludes rdf:langString .

ceterms:learningMethodType a rdf:Property ;
	rdfs:label "Learning Method Type"@en-US ;
	rdfs:comment "Types of methods used to conduct the learning opportunity; select from an existing enumeration of such types."@en-US ;
	vann:usageNote "Best practice is to use concepts from a controlled vocabulary such as the ceterms:LearningMethod."@en-US ;
	vs:term_status vs:stable ;
	meta:changeHistory <http://credreg.net/ctdl/termhistory/ceterms/learningMethodType/json> ;
	schema:domainIncludes ceterms:Course, ceterms:LearningOpportunityProfile, ceterms:LearningProgram ;
	schema:rangeIncludes ceterms:CredentialAlignmentObject ;
	meta:targetScheme ceterms:LearningMethod .

ceterms:leftAction a rdf:Property ;
	rdfs:label "Left Action"@en-US ;
	rdfs:comment "Action performed on the left source; select from an existing enumeration of such types."@en-US ;
	vs:term_status vs:unstable ;
	meta:changeHistory <http://credreg.net/ctdl/termhistory/ceterms/leftAction/json> ;
	schema:domainIncludes ceterms:Constraint ;
	schema:rangeIncludes skos:Concept ;
	meta:targetScheme ceterms:ArrayOperationCategory .

ceterms:leftSource a rdf:Property ;
	rdfs:label "Left Source"@en-US ;
	rdfs:comment "Left hand parameter of a constraint."@en-US ;
	vs:term_status vs:unstable ;
	meta:changeHistory <http://credreg.net/ctdl/termhistory/ceterms/leftSource/json> ;
	schema:domainIncludes ceterms:Constraint ;
	schema:rangeIncludes rdf:Property, rdfs:Class, rdfs:Literal, skos:Concept .

ceterms:leiCode a rdf:Property ;
	rdfs:label "Legal Entity Identifier Code"@en-US ;
	rdfs:comment "A 20-digit, alpha-numeric code, based on the ISO 17442 standard, for identifying legal entities participating in financial transactions."@en-US ;
	vs:term_status vs:stable ;
	meta:changeHistory <http://credreg.net/ctdl/termhistory/ceterms/leiCode/json> ;
	schema:domainIncludes ceterms:CredentialOrganization, ceterms:Organization, ceterms:QACredentialOrganization ;
	schema:rangeIncludes xsd:string ;
	owl:equivalentProperty schema:leiCode .

ceterms:lifeCycleStatusType a rdf:Property ;
	rdfs:label "Life Cycle Status Type"@en-US ;
	rdfs:comment "Type of state of the resource in terms of its stage in a life cycle; select from an enumeration of such types."@en-US ;
	vs:term_status vs:unstable ;
	meta:changeHistory <http://credreg.net/ctdl/termhistory/ceterms/lifeCycleStatusType/json> ;
	schema:domainIncludes ceterms:AssessmentProfile, ceterms:Collection, ceterms:Course, ceterms:CredentialOrganization, ceterms:LearningOpportunityProfile, ceterms:LearningProgram, ceterms:Organization, ceterms:QACredentialOrganization, ceterms:TransferValueProfile ;
	schema:rangeIncludes ceterms:CredentialAlignmentObject ;
	meta:targetScheme ceterms:LifeCycleStatus .

ceterms:logicalOperator a rdf:Property ;
	rdfs:label "Logical Operator"@en-US ;
	rdfs:comment "Type that denotes a logical operation such as \"And\", \"Or\", \"OnlyOne\"; select from an existing enumeration of such types."@en-US ;
	dct:description "Only a single instance of logicalOperator is allowed defining operations on two or more nested ComponentCondition entities, Constraint entities, or a mix of ComponentCondition and Constraint entities."@en-US ;
	vs:term_status vs:unstable ;
	meta:changeHistory <http://credreg.net/ctdl/termhistory/ceterms/logicalOperator/json> ;
	schema:domainIncludes ceterms:ComponentCondition ;
	schema:rangeIncludes skos:Concept ;
	meta:targetScheme ceterms:LogicalOperatorCategory .

ceterms:longitude a rdf:Property ;
	rdfs:label "Longitude"@en-US ;
	rdfs:comment "The longitude of a location."@en-US ;
	dct:description "For example -122.08585 (WGS 84)."@en-US ;
	vs:term_status vs:stable ;
	meta:changeHistory <http://credreg.net/ctdl/termhistory/ceterms/longitude/json> ;
	schema:domainIncludes ceterms:GeoCoordinates, ceterms:Place ;
	schema:rangeIncludes xsd:float ;
	owl:equivalentProperty schema:longitude .

ceterms:lowEarnings a rdf:Property ;
	rdfs:label "Low Earnings"@en-US ;
	rdfs:comment "Lower interquartile earnings."@en-US ;
	vs:term_status vs:stable ;
	meta:changeHistory <http://credreg.net/ctdl/termhistory/ceterms/lowEarnings/json> ;
	schema:domainIncludes ceterms:AggregateDataProfile, ceterms:EarningsProfile ;
	schema:rangeIncludes xsd:integer .

ceterms:mainJurisdiction a rdf:Property ;
	rdfs:label "Main Jurisdiction"@en-US ;
	rdfs:comment "Primary geographic or political region in which the credential is recognized as applicable or in which an organization has recognized authority to act."@en-US ;
	vs:term_status vs:stable ;
	meta:changeHistory <http://credreg.net/ctdl/termhistory/ceterms/mainJurisdiction/json> ;
	rdfs:subPropertyOf ceterms:spatialCoverage ;
	schema:domainIncludes ceterms:JurisdictionProfile ;
	schema:rangeIncludes ceterms:Place .

ceterms:maintenanceProcess a rdf:Property ;
	rdfs:label "Maintenance Process"@en-US ;
	rdfs:comment "Entity describing the process by which the credential is maintained including review and updating."@en-US ;
	dct:description "Such maintenance does not include renewal of a credential by an individual holder."@en-US ;
	vs:term_status vs:stable ;
	meta:changeHistory <http://credreg.net/ctdl/termhistory/ceterms/maintenanceProcess/json> ;
	schema:domainIncludes ceterms:ApprenticeshipCertificate, ceterms:AssessmentProfile, ceterms:AssociateDegree, ceterms:BachelorDegree, ceterms:Badge, ceterms:Certificate, ceterms:CertificateOfCompletion, ceterms:Certification, ceterms:Credential, ceterms:CredentialOrganization, ceterms:Degree, ceterms:DigitalBadge, ceterms:Diploma, ceterms:DoctoralDegree, ceterms:GeneralEducationDevelopment, ceterms:JourneymanCertificate, ceterms:License, ceterms:MasterCertificate, ceterms:MasterDegree, ceterms:MicroCredential, ceterms:OpenBadge, ceterms:Organization, ceterms:ProfessionalDoctorate, ceterms:QACredentialOrganization, ceterms:QualityAssuranceCredential, ceterms:ResearchDoctorate, ceterms:SecondarySchoolDiploma ;
	schema:rangeIncludes ceterms:ProcessProfile .

ceterms:majorAlignment a rdf:Property ;
	rdfs:label "Major Alignment"@en-US ;
	rdfs:comment "Major overlap of relevant concepts between the two resources being compared."@en-US ;
	vs:term_status vs:stable ;
	meta:changeHistory <http://credreg.net/ctdl/termhistory/ceterms/majorAlignment/json> ;
	rdfs:subPropertyOf ceterms:isSimilarTo ;
	schema:domainIncludes ceterms:ApprenticeshipCertificate, ceterms:AssociateDegree, ceterms:BachelorDegree, ceterms:Badge, ceterms:Certificate, ceterms:CertificateOfCompletion, ceterms:Certification, ceterms:Credential, ceterms:Degree, ceterms:DigitalBadge, ceterms:Diploma, ceterms:DoctoralDegree, ceterms:GeneralEducationDevelopment, ceterms:JourneymanCertificate, ceterms:License, ceterms:MasterCertificate, ceterms:MasterDegree, ceterms:MicroCredential, ceterms:OpenBadge, ceterms:ProfessionalDoctorate, ceterms:QualityAssuranceCredential, ceterms:ResearchDoctorate, ceterms:SecondarySchoolDiploma ;
	schema:rangeIncludes ceterms:ApprenticeshipCertificate, ceterms:AssociateDegree, ceterms:BachelorDegree, ceterms:Badge, ceterms:Certificate, ceterms:CertificateOfCompletion, ceterms:Certification, ceterms:Credential, ceterms:Degree, ceterms:DigitalBadge, ceterms:Diploma, ceterms:DoctoralDegree, ceterms:GeneralEducationDevelopment, ceterms:JourneymanCertificate, ceterms:License, ceterms:MasterCertificate, ceterms:MasterDegree, ceterms:MicroCredential, ceterms:OpenBadge, ceterms:ProfessionalDoctorate, ceterms:QualityAssuranceCredential, ceterms:ResearchDoctorate, ceterms:SecondarySchoolDiploma ;
	owl:equivalentProperty asn:majorAlignment .

ceterms:maximumDuration a rdf:Property ;
	rdfs:label "Maximum Duration"@en-US ;
	rdfs:comment "Maximum amount of time it will take to complete the activity."@en-US ;
	dct:description "The value of ceterms:maximumDuration denotes an approximation of duration."@en-US ;
	vann:usageNote "Do not use ceterms:maximumDuration to identify the renewal frequency of a credential; use ceterms:renewalFrequency instead."@en-US ;
	vs:term_status vs:stable ;
	meta:changeHistory <http://credreg.net/ctdl/termhistory/ceterms/maximumDuration/json> ;
	schema:domainIncludes ceterms:DurationProfile ;
	schema:rangeIncludes schema:Duration .

ceterms:medianEarnings a rdf:Property ;
	rdfs:label "Median earnings"@en-US ;
	rdfs:comment "Median earnings."@en-US ;
	vs:term_status vs:stable ;
	meta:changeHistory <http://credreg.net/ctdl/termhistory/ceterms/medianEarnings/json> ;
	schema:domainIncludes ceterms:AggregateDataProfile, ceterms:EarningsProfile ;
	schema:rangeIncludes xsd:integer .

ceterms:membershipCondition a rdf:Property ;
	rdfs:label "Membership Condition"@en-US ;
	rdfs:comment "Conditions and requirements to be included as a member."@en-US ;
	vs:term_status vs:unstable ;
	meta:changeHistory <http://credreg.net/ctdl/termhistory/ceterms/membershipCondition/json> ;
	schema:domainIncludes ceterms:Collection ;
	schema:rangeIncludes ceterms:ConditionProfile .

ceterms:minimumAge a rdf:Property ;
	rdfs:label "Minimum Age"@en-US ;
	rdfs:comment "Minimum allowed age at which a person is eligible for the credential."@en-US ;
	vs:term_status vs:stable ;
	meta:changeHistory <http://credreg.net/ctdl/termhistory/ceterms/minimumAge/json> ;
	schema:domainIncludes ceterms:ConditionProfile ;
	schema:rangeIncludes xsd:integer .

ceterms:minimumDuration a rdf:Property ;
	rdfs:label "Minimum Duration"@en-US ;
	rdfs:comment "Minimum amount of time it will take to complete the activity."@en-US ;
	dct:description "The value of ceterms:minimumDuration denotes an approximation of duration."@en-US ;
	vs:term_status vs:stable ;
	meta:changeHistory <http://credreg.net/ctdl/termhistory/ceterms/minimumDuration/json> ;
	schema:domainIncludes ceterms:DurationProfile ;
	schema:rangeIncludes schema:Duration .

ceterms:minorAlignment a rdf:Property ;
	rdfs:label "Minor Alignment"@en-US ;
	rdfs:comment "Minor overlap of relevant concepts between the two credentials being compared."@en-US ;
	vs:term_status vs:stable ;
	meta:changeHistory <http://credreg.net/ctdl/termhistory/ceterms/minorAlignment/json> ;
	rdfs:subPropertyOf ceterms:isSimilarTo ;
	schema:domainIncludes ceterms:ApprenticeshipCertificate, ceterms:AssociateDegree, ceterms:BachelorDegree, ceterms:Badge, ceterms:Certificate, ceterms:CertificateOfCompletion, ceterms:Certification, ceterms:Credential, ceterms:Degree, ceterms:DigitalBadge, ceterms:Diploma, ceterms:DoctoralDegree, ceterms:GeneralEducationDevelopment, ceterms:JourneymanCertificate, ceterms:License, ceterms:MasterCertificate, ceterms:MasterDegree, ceterms:MicroCredential, ceterms:OpenBadge, ceterms:ProfessionalDoctorate, ceterms:QualityAssuranceCredential, ceterms:ResearchDoctorate, ceterms:SecondarySchoolDiploma ;
	schema:rangeIncludes ceterms:ApprenticeshipCertificate, ceterms:AssociateDegree, ceterms:BachelorDegree, ceterms:Badge, ceterms:Certificate, ceterms:CertificateOfCompletion, ceterms:Certification, ceterms:Credential, ceterms:Degree, ceterms:DigitalBadge, ceterms:Diploma, ceterms:DoctoralDegree, ceterms:GeneralEducationDevelopment, ceterms:JourneymanCertificate, ceterms:License, ceterms:MasterCertificate, ceterms:MasterDegree, ceterms:MicroCredential, ceterms:OpenBadge, ceterms:ProfessionalDoctorate, ceterms:QualityAssuranceCredential, ceterms:ResearchDoctorate, ceterms:SecondarySchoolDiploma ;
	owl:equivalentProperty asn:minorAlignment .

ceterms:missionAndGoalsStatement a rdf:Property ;
	rdfs:label "Mission and Goals Statement"@en-US ;
	rdfs:comment "Webpage or online document that defines or explains the mission and goals of the organization."@en-US ;
	vs:term_status vs:stable ;
	meta:changeHistory <http://credreg.net/ctdl/termhistory/ceterms/missionAndGoalsStatement/json> ;
	schema:domainIncludes ceterms:CredentialOrganization, ceterms:Organization, ceterms:QACredentialOrganization ;
	schema:rangeIncludes xsd:anyURI .

ceterms:missionAndGoalsStatementDescription a rdf:Property ;
	rdfs:label "Mission and Goals Statement Description"@en-US ;
	rdfs:comment "Textual statement of the mission and goals of the organization."@en-US ;
	vs:term_status vs:stable ;
	meta:changeHistory <http://credreg.net/ctdl/termhistory/ceterms/missionAndGoalsStatementDescription/json> ;
	schema:domainIncludes ceterms:CredentialOrganization, ceterms:Organization, ceterms:QACredentialOrganization ;
	schema:rangeIncludes rdf:langString .

ceterms:naics a rdf:Property ;
	rdfs:label "NAICS"@en-US ;
	rdfs:comment "North American Industry Classification System (NAICS) code of an organization or business person."@en-US ;
	vs:term_status vs:stable ;
	meta:changeHistory <http://credreg.net/ctdl/termhistory/ceterms/naics/json> ;
	schema:domainIncludes ceterms:ApprenticeshipCertificate, ceterms:AssociateDegree, ceterms:BachelorDegree, ceterms:Badge, ceterms:Certificate, ceterms:CertificateOfCompletion, ceterms:Certification, ceterms:Credential, ceterms:CredentialOrganization, ceterms:Degree, ceterms:DigitalBadge, ceterms:Diploma, ceterms:DoctoralDegree, ceterms:GeneralEducationDevelopment, ceterms:JourneymanCertificate, ceterms:License, ceterms:MasterCertificate, ceterms:MasterDegree, ceterms:MicroCredential, ceterms:OpenBadge, ceterms:Organization, ceterms:ProfessionalDoctorate, ceterms:QACredentialOrganization, ceterms:QualityAssuranceCredential, ceterms:ResearchDoctorate, ceterms:SecondarySchoolDiploma ;
	schema:rangeIncludes xsd:string ;
	owl:equivalentProperty schema:naics .

ceterms:name a rdf:Property ;
	rdfs:label "Name"@en-US ;
	rdfs:comment "Name or title of the resource."@en-US ;
	vs:term_status vs:stable ;
	meta:changeHistory <http://credreg.net/ctdl/termhistory/ceterms/name/json> ;
	schema:domainIncludes ceterms:AggregateDataProfile, ceterms:ApprenticeshipCertificate, ceterms:AssessmentComponent, ceterms:AssessmentProfile, ceterms:AssociateDegree, ceterms:BachelorDegree, ceterms:Badge, ceterms:BasicComponent, ceterms:Certificate, ceterms:CertificateOfCompletion, ceterms:Certification, ceterms:CocurricularComponent, ceterms:Collection, ceterms:CollectionMember, ceterms:CompetencyComponent, ceterms:ComponentCondition, ceterms:ConditionManifest, ceterms:ConditionProfile, ceterms:Constraint, ceterms:ContactPoint, ceterms:CostManifest, ceterms:CostProfile, ceterms:Course, ceterms:CourseComponent, ceterms:Credential, ceterms:CredentialComponent, ceterms:CredentialOrganization, ceterms:Degree, ceterms:DigitalBadge, ceterms:Diploma, ceterms:DoctoralDegree, ceterms:ExtracurricularComponent, ceterms:FinancialAssistanceProfile, ceterms:GeneralEducationDevelopment, ceterms:GeoCoordinates, ceterms:HoldersProfile, ceterms:Job, ceterms:JobComponent, ceterms:JourneymanCertificate, ceterms:LearningOpportunityProfile, ceterms:LearningProgram, ceterms:License, ceterms:MasterCertificate, ceterms:MasterDegree, ceterms:MicroCredential, ceterms:Occupation, ceterms:OpenBadge, ceterms:Organization, ceterms:Pathway, ceterms:PathwaySet, ceterms:Place, ceterms:PostalAddress, ceterms:ProfessionalDoctorate, ceterms:QACredentialOrganization, ceterms:QualityAssuranceCredential, ceterms:ResearchDoctorate, ceterms:RuleSetProfile, ceterms:ScheduledOffering, ceterms:SecondarySchoolDiploma, ceterms:Task, ceterms:TransferIntermediary, ceterms:TransferValueProfile, ceterms:WorkExperienceComponent, ceterms:WorkRole ;
	schema:rangeIncludes rdf:langString ;
	owl:equivalentProperty schema:name .

ceterms:narrowAlignment a rdf:Property ;
	rdfs:label "Narrow Alignment"@en-US ;
	rdfs:comment "Credential covers all of the relevant concepts in another credential as well as relevant concepts not found in the other credential."@en-US ;
	vs:term_status vs:stable ;
	meta:changeHistory <http://credreg.net/ctdl/termhistory/ceterms/narrowAlignment/json> ;
	rdfs:subPropertyOf ceterms:isSimilarTo ;
	schema:domainIncludes ceterms:ApprenticeshipCertificate, ceterms:AssociateDegree, ceterms:BachelorDegree, ceterms:Badge, ceterms:Certificate, ceterms:CertificateOfCompletion, ceterms:Certification, ceterms:Credential, ceterms:Degree, ceterms:DigitalBadge, ceterms:Diploma, ceterms:DoctoralDegree, ceterms:GeneralEducationDevelopment, ceterms:JourneymanCertificate, ceterms:License, ceterms:MasterCertificate, ceterms:MasterDegree, ceterms:MicroCredential, ceterms:OpenBadge, ceterms:ProfessionalDoctorate, ceterms:QualityAssuranceCredential, ceterms:ResearchDoctorate, ceterms:SecondarySchoolDiploma ;
	schema:rangeIncludes ceterms:ApprenticeshipCertificate, ceterms:AssociateDegree, ceterms:BachelorDegree, ceterms:Badge, ceterms:Certificate, ceterms:CertificateOfCompletion, ceterms:Certification, ceterms:Credential, ceterms:Degree, ceterms:DigitalBadge, ceterms:Diploma, ceterms:DoctoralDegree, ceterms:GeneralEducationDevelopment, ceterms:JourneymanCertificate, ceterms:License, ceterms:MasterCertificate, ceterms:MasterDegree, ceterms:MicroCredential, ceterms:OpenBadge, ceterms:ProfessionalDoctorate, ceterms:QualityAssuranceCredential, ceterms:ResearchDoctorate, ceterms:SecondarySchoolDiploma ;
	owl:equivalentProperty asn:narrowAlignment, skos:narrower .

ceterms:ncesID a rdf:Property ;
	rdfs:label "NCES ID"@en-US ;
	rdfs:comment "Identifier comprised of a 12 digit code issued by the National Center for Education Statistics (NCES) for educational institutions where the first 7 digits are the NCES District ID."@en-US ;
	vs:term_status vs:stable ;
	meta:changeHistory <http://credreg.net/ctdl/termhistory/ceterms/ncesID/json> ;
	schema:domainIncludes ceterms:CredentialOrganization ;
	schema:rangeIncludes xsd:string .

ceterms:nextVersion a rdf:Property ;
	rdfs:label "Next Version"@en-US ;
	rdfs:comment "Version of the resource that immediately follows this version."@en-US ;
	vs:term_status vs:stable ;
	meta:changeHistory <http://credreg.net/ctdl/termhistory/ceterms/nextVersion/json> ;
	schema:domainIncludes ceterms:ApprenticeshipCertificate, ceterms:AssociateDegree, ceterms:BachelorDegree, ceterms:Badge, ceterms:Certificate, ceterms:CertificateOfCompletion, ceterms:Certification, ceterms:Credential, ceterms:Degree, ceterms:DigitalBadge, ceterms:Diploma, ceterms:DoctoralDegree, ceterms:GeneralEducationDevelopment, ceterms:JourneymanCertificate, ceterms:License, ceterms:MasterCertificate, ceterms:MasterDegree, ceterms:MicroCredential, ceterms:OpenBadge, ceterms:ProfessionalDoctorate, ceterms:QualityAssuranceCredential, ceterms:ResearchDoctorate, ceterms:SecondarySchoolDiploma ;
	schema:rangeIncludes ceterms:ApprenticeshipCertificate, ceterms:AssociateDegree, ceterms:BachelorDegree, ceterms:Badge, ceterms:Certificate, ceterms:CertificateOfCompletion, ceterms:Certification, ceterms:Credential, ceterms:Degree, ceterms:DigitalBadge, ceterms:Diploma, ceterms:DoctoralDegree, ceterms:GeneralEducationDevelopment, ceterms:JourneymanCertificate, ceterms:License, ceterms:MasterCertificate, ceterms:MasterDegree, ceterms:MicroCredential, ceterms:OpenBadge, ceterms:ProfessionalDoctorate, ceterms:QualityAssuranceCredential, ceterms:ResearchDoctorate, ceterms:SecondarySchoolDiploma .

ceterms:numberAwarded a rdf:Property ;
	rdfs:label "Number Awarded"@en-US ;
	rdfs:comment "Number of credentials awarded."@en-US ;
	vs:term_status vs:stable ;
	meta:changeHistory <http://credreg.net/ctdl/termhistory/ceterms/numberAwarded/json> ;
	schema:domainIncludes ceterms:AggregateDataProfile, ceterms:HoldersProfile ;
	schema:rangeIncludes xsd:integer .

ceterms:object a rdf:Property ;
	rdfs:label "Object"@en-US ;
	rdfs:comment "Object upon which the action is carried out, whose state is kept intact or changed."@en-US ;
	vs:term_status vs:stable ;
	meta:changeHistory <http://credreg.net/ctdl/termhistory/ceterms/object/json> ;
	schema:domainIncludes ceterms:AccreditAction, ceterms:AdvancedStandingAction, ceterms:ApproveAction, ceterms:CredentialingAction, ceterms:OfferAction, ceterms:RecognizeAction, ceterms:RegulateAction, ceterms:RenewAction, ceterms:RevokeAction, ceterms:RightsAction, ceterms:WorkforceDemandAction ;
	schema:rangeIncludes ceasn:Competency, ceasn:CompetencyFramework, ceterms:ApprenticeshipCertificate, ceterms:AssessmentProfile, ceterms:AssociateDegree, ceterms:BachelorDegree, ceterms:Badge, ceterms:Certificate, ceterms:CertificateOfCompletion, ceterms:Certification, ceterms:Course, ceterms:Credential, ceterms:CredentialOrganization, ceterms:CredentialPerson, ceterms:Degree, ceterms:DigitalBadge, ceterms:Diploma, ceterms:DoctoralDegree, ceterms:GeneralEducationDevelopment, ceterms:JourneymanCertificate, ceterms:LearningOpportunityProfile, ceterms:LearningProgram, ceterms:License, ceterms:MasterCertificate, ceterms:MasterDegree, ceterms:MicroCredential, ceterms:OpenBadge, ceterms:Organization, ceterms:ProfessionalDoctorate, ceterms:QACredentialOrganization, ceterms:QualityAssuranceCredential, ceterms:ResearchDoctorate, ceterms:SecondarySchoolDiploma ;
	owl:equivalentProperty schema:object .

ceterms:occupationType a rdf:Property ;
	rdfs:label "Occupation Type"@en-US ;
	rdfs:comment "Type of occupation; select from an existing enumeration of such types."@en-US ;
	vann:usageNote "For U.S. resources, best practice is to identify an occupation using a framework such as the ONet. Other resources may use any framework of the class ceterms:OccupationClassification, such as the EU's ESCO, ISCO-08, and SOC 2010."@en-US ;
	vs:term_status vs:stable ;
	meta:changeHistory <http://credreg.net/ctdl/termhistory/ceterms/occupationType/json> ;
	rdfs:subPropertyOf ceterms:credentialAlignment ;
	schema:domainIncludes ceasn:Collection, ceasn:CompetencyFramework, ceterms:ApprenticeshipCertificate, ceterms:AssessmentProfile, ceterms:AssociateDegree, ceterms:BachelorDegree, ceterms:Badge, ceterms:Certificate, ceterms:CertificateOfCompletion, ceterms:Certification, ceterms:Collection, ceterms:Course, ceterms:Credential, ceterms:Degree, ceterms:DigitalBadge, ceterms:Diploma, ceterms:DoctoralDegree, ceterms:GeneralEducationDevelopment, ceterms:Job, ceterms:JobComponent, ceterms:JourneymanCertificate, ceterms:LearningOpportunityProfile, ceterms:LearningProgram, ceterms:License, ceterms:MasterCertificate, ceterms:MasterDegree, ceterms:MicroCredential, ceterms:Occupation, ceterms:OpenBadge, ceterms:Pathway, ceterms:ProfessionalDoctorate, ceterms:QualityAssuranceCredential, ceterms:ResearchDoctorate, ceterms:SecondarySchoolDiploma ;
	schema:rangeIncludes ceterms:CredentialAlignmentObject ;
	meta:targetScheme ceterms:OccupationClassification ;
	owl:equivalentProperty schema:occupationalCategory .

ceterms:offeredBy a rdf:Property ;
	rdfs:label "Offered By"@en-US ;
	rdfs:comment "Agent that offers the resource."@en-US ;
	vs:term_status vs:stable ;
	meta:changeHistory <http://credreg.net/ctdl/termhistory/ceterms/offeredBy/json> ;
	schema:domainIncludes ceterms:ApprenticeshipCertificate, ceterms:AssessmentProfile, ceterms:AssociateDegree, ceterms:BachelorDegree, ceterms:Badge, ceterms:Certificate, ceterms:CertificateOfCompletion, ceterms:Certification, ceterms:Course, ceterms:Credential, ceterms:Degree, ceterms:DigitalBadge, ceterms:Diploma, ceterms:DoctoralDegree, ceterms:GeneralEducationDevelopment, ceterms:Job, ceterms:JourneymanCertificate, ceterms:LearningOpportunityProfile, ceterms:LearningProgram, ceterms:License, ceterms:MasterCertificate, ceterms:MasterDegree, ceterms:MicroCredential, ceterms:OpenBadge, ceterms:Pathway, ceterms:PathwaySet, ceterms:ProfessionalDoctorate, ceterms:QualityAssuranceCredential, ceterms:ResearchDoctorate, ceterms:ScheduledOffering, ceterms:SecondarySchoolDiploma, ceterms:VerificationServiceProfile ;
	schema:rangeIncludes ceterms:CredentialOrganization, ceterms:Organization, ceterms:QACredentialOrganization ;
	owl:equivalentProperty schema:provider .

ceterms:offeredIn a rdf:Property ;
	rdfs:label "Offered In"@en-US ;
	rdfs:comment "Region or political jurisdiction such as a state, province or locale where the credential, learning resource or assessment is offered."@en-US ;
	vs:term_status vs:stable ;
	meta:changeHistory <http://credreg.net/ctdl/termhistory/ceterms/offeredIn/json> ;
	schema:domainIncludes ceterms:ApprenticeshipCertificate, ceterms:AssessmentProfile, ceterms:AssociateDegree, ceterms:BachelorDegree, ceterms:Badge, ceterms:Certificate, ceterms:CertificateOfCompletion, ceterms:Certification, ceterms:Course, ceterms:Credential, ceterms:Degree, ceterms:DigitalBadge, ceterms:Diploma, ceterms:DoctoralDegree, ceterms:GeneralEducationDevelopment, ceterms:JourneymanCertificate, ceterms:LearningOpportunityProfile, ceterms:LearningProgram, ceterms:License, ceterms:MasterCertificate, ceterms:MasterDegree, ceterms:MicroCredential, ceterms:OpenBadge, ceterms:ProfessionalDoctorate, ceterms:QualityAssuranceCredential, ceterms:ResearchDoctorate, ceterms:SecondarySchoolDiploma, ceterms:VerificationServiceProfile ;
	schema:rangeIncludes ceterms:JurisdictionProfile .

ceterms:offerFrequencyType a rdf:Property ;
	rdfs:label "Offer Frequency Type"@en-US ;
	rdfs:comment "Type of frequency at which a resource is offered; select from an existing enumeration of such types."@en-US ;
	dct:description "This relates to how often something starts."@en-US ;
	vann:usageNote "For information relating to the frequency of events associated with a resource when it is running, use ceterms:scheduleFrequencyType."@en-US ;
	vs:term_status vs:unstable ;
	meta:changeHistory <http://credreg.net/ctdl/termhistory/ceterms/offerFrequencyType/json> ;
	schema:domainIncludes ceterms:AssessmentProfile, ceterms:Course, ceterms:LearningOpportunityProfile, ceterms:LearningProgram, ceterms:ScheduledOffering ;
	schema:rangeIncludes ceterms:CredentialAlignmentObject ;
	meta:targetScheme ceterms:ScheduleFrequency .

ceterms:offers a rdf:Property ;
	rdfs:label "Offers"@en-US ;
	rdfs:comment "Resource offered or conferred by the organization or person."@en-US ;
	vs:term_status vs:stable ;
	meta:changeHistory <http://credreg.net/ctdl/termhistory/ceterms/offers/json> ;
	schema:domainIncludes ceterms:CredentialOrganization, ceterms:Organization, ceterms:QACredentialOrganization ;
	schema:rangeIncludes ceterms:ApprenticeshipCertificate, ceterms:AssessmentProfile, ceterms:AssociateDegree, ceterms:BachelorDegree, ceterms:Badge, ceterms:Certificate, ceterms:CertificateOfCompletion, ceterms:Certification, ceterms:Course, ceterms:Credential, ceterms:Degree, ceterms:DigitalBadge, ceterms:Diploma, ceterms:DoctoralDegree, ceterms:GeneralEducationDevelopment, ceterms:Job, ceterms:JourneymanCertificate, ceterms:LearningOpportunityProfile, ceterms:LearningProgram, ceterms:License, ceterms:MasterCertificate, ceterms:MasterDegree, ceterms:MicroCredential, ceterms:OpenBadge, ceterms:Pathway, ceterms:ProfessionalDoctorate, ceterms:QualityAssuranceCredential, ceterms:ResearchDoctorate, ceterms:SecondarySchoolDiploma .

ceterms:opeID a rdf:Property ;
	rdfs:label "OPE ID"@en-US ;
	rdfs:comment "OPE ID number (U.S. Office of Postsecondary Education Identification), sometimes referred to as the Federal School Code."@en-US ;
	dct:description "Identification number used by the U.S. Department of Education's Office of Postsecondary Education (OPE) to identify schools that have Program Participation Agreements (PPA) so that its students are eligible to participate in Federal Student Financial Assistance (FAFSA) programs under Title IV regulations. This is a 6-digit number followed by a 2-digit suffix used to identify branches, additional locations, and other entities that are part of the eligible institution."@en-US ;
	vs:term_status vs:stable ;
	meta:changeHistory <http://credreg.net/ctdl/termhistory/ceterms/opeID/json> ;
	schema:domainIncludes ceterms:CredentialOrganization, ceterms:Organization, ceterms:QACredentialOrganization ;
	schema:rangeIncludes xsd:string .

ceterms:ownedBy a rdf:Property ;
	rdfs:label "Owned By"@en-US ;
	rdfs:comment "Organization or person with an enforceable claim or legal title to the resource."@en-US ;
	dct:description "Agent includes credentialing organizations, quality assurance organizations and persons. It does not not include credential holders."@en-US ;
	vs:term_status vs:stable ;
	meta:changeHistory <http://credreg.net/ctdl/termhistory/ceterms/ownedBy/json> ;
	schema:domainIncludes ceterms:ApprenticeshipCertificate, ceterms:AssessmentProfile, ceterms:AssociateDegree, ceterms:BachelorDegree, ceterms:Badge, ceterms:Certificate, ceterms:CertificateOfCompletion, ceterms:Certification, ceterms:Collection, ceterms:Course, ceterms:Credential, ceterms:Degree, ceterms:DigitalBadge, ceterms:Diploma, ceterms:DoctoralDegree, ceterms:GeneralEducationDevelopment, ceterms:JourneymanCertificate, ceterms:LearningOpportunityProfile, ceterms:LearningProgram, ceterms:License, ceterms:MasterCertificate, ceterms:MasterDegree, ceterms:MicroCredential, ceterms:OpenBadge, ceterms:Pathway, ceterms:PathwaySet, ceterms:ProfessionalDoctorate, ceterms:QualityAssuranceCredential, ceterms:ResearchDoctorate, ceterms:SecondarySchoolDiploma, ceterms:TransferIntermediary, ceterms:TransferValueProfile ;
	schema:rangeIncludes ceterms:CredentialOrganization, ceterms:Organization, ceterms:QACredentialOrganization .

ceterms:owns a rdf:Property ;
	rdfs:label "Owns"@en-US ;
	rdfs:comment "Resource over which the organization or person claims legal title."@en-US ;
	dct:description "Generally, the value of the property should be one of the subclasses of ceterms:Credential or ceterms:Pathway."@en-US ;
	vs:term_status vs:stable ;
	meta:changeHistory <http://credreg.net/ctdl/termhistory/ceterms/owns/json> ;
	schema:domainIncludes ceterms:CredentialOrganization, ceterms:Organization, ceterms:QACredentialOrganization ;
	schema:rangeIncludes ceterms:ApprenticeshipCertificate, ceterms:AssessmentProfile, ceterms:AssociateDegree, ceterms:BachelorDegree, ceterms:Badge, ceterms:Certificate, ceterms:CertificateOfCompletion, ceterms:Certification, ceterms:Course, ceterms:Credential, ceterms:Degree, ceterms:DigitalBadge, ceterms:Diploma, ceterms:DoctoralDegree, ceterms:GeneralEducationDevelopment, ceterms:JourneymanCertificate, ceterms:LearningOpportunityProfile, ceterms:LearningProgram, ceterms:License, ceterms:MasterCertificate, ceterms:MasterDegree, ceterms:MicroCredential, ceterms:OpenBadge, ceterms:Pathway, ceterms:ProfessionalDoctorate, ceterms:QualityAssuranceCredential, ceterms:ResearchDoctorate, ceterms:SecondarySchoolDiploma, ceterms:TransferValueProfile .

ceterms:parentOrganization a rdf:Property ;
	rdfs:label "Parent Organization"@en-US ;
	rdfs:comment "Larger organization exercising authority over the organization being described."@en-US ;
	vs:term_status vs:stable ;
	meta:changeHistory <http://credreg.net/ctdl/termhistory/ceterms/parentOrganization/json> ;
	schema:domainIncludes ceterms:CredentialOrganization, ceterms:Organization, ceterms:QACredentialOrganization ;
	schema:rangeIncludes ceterms:CredentialOrganization, ceterms:Organization, ceterms:QACredentialOrganization ;
	owl:equivalentProperty schema:parentOrganization .

ceterms:participant a rdf:Property ;
	rdfs:label "Participant"@en-US ;
	rdfs:comment "Co-agents that participated in the action indirectly."@en-US ;
	vs:term_status vs:stable ;
	meta:changeHistory <http://credreg.net/ctdl/termhistory/ceterms/participant/json> ;
	schema:domainIncludes ceterms:AccreditAction, ceterms:AdvancedStandingAction, ceterms:ApproveAction, ceterms:CredentialingAction, ceterms:OfferAction, ceterms:RecognizeAction, ceterms:RegulateAction, ceterms:RenewAction, ceterms:RevokeAction, ceterms:RightsAction, ceterms:WorkforceDemandAction ;
	schema:rangeIncludes ceterms:CredentialOrganization, ceterms:Organization, ceterms:QACredentialOrganization ;
	owl:equivalentProperty schema:participant .

ceterms:paymentPattern a rdf:Property ;
	rdfs:label "Payment Pattern"@en-US ;
	rdfs:comment "Applicable pattern for payments such as \"per semester\" and \"every three months\"."@en-US ;
	vs:term_status vs:stable ;
	meta:changeHistory <http://credreg.net/ctdl/termhistory/ceterms/paymentPattern/json> ;
	schema:domainIncludes ceterms:CostProfile ;
	schema:rangeIncludes rdf:langString .

ceterms:performanceLevelType a rdf:Property ;
	rdfs:label "Performance Level Type"@en-US ;
	rdfs:comment "Type of required or expected human performance level; select from an existing enumeration of such types."@en-US ;
	vs:term_status vs:unstable ;
	meta:changeHistory <http://credreg.net/ctdl/termhistory/ceterms/performanceLevelType/json> ;
	schema:domainIncludes ceasn:Competency, ceterms:Job, ceterms:Task, ceterms:WorkRole ;
	schema:rangeIncludes skos:Concept .

ceterms:physicalCapabilityType a rdf:Property ;
	rdfs:label "Physical Capability Type"@en-US ;
	rdfs:comment "Type of physical activity required or expected in performance; select from an existing enumeration of such types."@en-US ;
	dct:description "Such types may include fine motor activity, repetitive actions, climbing, kneeling, crawling, lifting heavy objects, and so on."@en-US ;
	vs:term_status vs:unstable ;
	meta:changeHistory <http://credreg.net/ctdl/termhistory/ceterms/physicalCapabilityType/json> ;
	schema:domainIncludes ceasn:Competency, ceterms:Job, ceterms:Task, ceterms:WorkRole ;
	schema:rangeIncludes skos:Concept .

ceterms:pointValue a rdf:Property ;
	rdfs:label "Point Value"@en-US ;
	rdfs:comment "Points associated with this resource, or points possible."@en-US ;
	vs:term_status vs:stable ;
	meta:changeHistory <http://credreg.net/ctdl/termhistory/ceterms/pointValue/json> ;
	schema:domainIncludes ceterms:AssessmentComponent, ceterms:BasicComponent, ceterms:CocurricularComponent, ceterms:CompetencyComponent, ceterms:CourseComponent, ceterms:CredentialComponent, ceterms:ExtracurricularComponent, ceterms:JobComponent, ceterms:WorkExperienceComponent ;
	schema:rangeIncludes schema:QuantitativeValue .

ceterms:postalCode a rdf:Property ;
	rdfs:label "Postal Code"@en-US ;
	rdfs:comment "The postal code. For example, 94043."@en-US ;
	vs:term_status vs:stable ;
	meta:changeHistory <http://credreg.net/ctdl/termhistory/ceterms/postalCode/json> ;
	schema:domainIncludes ceterms:Place, ceterms:PostalAddress ;
	schema:rangeIncludes xsd:string ;
	owl:equivalentProperty schema:postalCode .

ceterms:postOfficeBoxNumber a rdf:Property ;
	rdfs:label "Post Office Box Number"@en-US ;
	rdfs:comment "Post office box number for post office addresses."@en-US ;
	vs:term_status vs:stable ;
	meta:changeHistory <http://credreg.net/ctdl/termhistory/ceterms/postOfficeBoxNumber/json> ;
	schema:domainIncludes ceterms:Place, ceterms:PostalAddress ;
	schema:rangeIncludes xsd:string ;
	owl:equivalentProperty schema:postOfficeBoxNumber .

ceterms:postReceiptMonths a rdf:Property ;
	rdfs:label "Post Receipt Months"@en-US ;
	rdfs:comment "Number of months after earning a credential when employment and earnings data is collected."@en-US ;
	dct:description "Number of months usually range between 3 months (one quarter) to ten years."@en-US ;
	vs:term_status vs:stable ;
	meta:changeHistory <http://credreg.net/ctdl/termhistory/ceterms/postReceiptMonths/json> ;
	schema:domainIncludes ceterms:AggregateDataProfile, ceterms:EarningsProfile ;
	schema:rangeIncludes xsd:integer .

ceterms:precededBy a rdf:Property ;
	rdfs:label "Preceded By"@en-US ;
	rdfs:comment "Resource that logically comes before this resource."@en-US ;
	vs:term_status vs:unstable ;
	meta:changeHistory <http://credreg.net/ctdl/termhistory/ceterms/precededBy/json> ;
	schema:domainIncludes asn:ProgressionLevel, ceterms:AssessmentComponent, ceterms:BasicComponent, ceterms:CocurricularComponent, ceterms:CompetencyComponent, ceterms:CourseComponent, ceterms:CredentialComponent, ceterms:ExtracurricularComponent, ceterms:JobComponent, ceterms:WorkExperienceComponent, skos:Concept ;
	schema:rangeIncludes ceterms:AssessmentComponent, ceterms:BasicComponent, ceterms:CocurricularComponent, ceterms:CompetencyComponent, ceterms:CourseComponent, ceterms:CredentialComponent, ceterms:ExtracurricularComponent, ceterms:JobComponent, ceterms:WorkExperienceComponent, skos:Concept .

ceterms:precedes a rdf:Property ;
	rdfs:label "Precedes"@en-US ;
	rdfs:comment "Resource that logically comes after this resource."@en-US ;
	dct:description "The ceterms:precedes property indicates a simple or suggested ordering of resources."@en-US ;
	vs:term_status vs:stable ;
	meta:changeHistory <http://credreg.net/ctdl/termhistory/ceterms/precedes/json> ;
	schema:domainIncludes asn:ProgressionLevel, ceterms:AssessmentComponent, ceterms:BasicComponent, ceterms:CocurricularComponent, ceterms:CompetencyComponent, ceterms:CourseComponent, ceterms:CredentialComponent, ceterms:ExtracurricularComponent, ceterms:JobComponent, ceterms:WorkExperienceComponent, skos:Concept ;
	schema:rangeIncludes ceterms:AssessmentComponent, ceterms:BasicComponent, ceterms:CocurricularComponent, ceterms:CompetencyComponent, ceterms:CourseComponent, ceterms:CredentialComponent, ceterms:ExtracurricularComponent, ceterms:JobComponent, ceterms:WorkExperienceComponent, skos:Concept .

ceterms:preparationFrom a rdf:Property ;
	rdfs:label "Preparation From"@en-US ;
	rdfs:comment "Another credential, learning opportunity or assessment that provides preparation for this credential, learning opportunity or assessment."@en-US ;
	vs:term_status vs:stable ;
	meta:changeHistory <http://credreg.net/ctdl/termhistory/ceterms/preparationFrom/json> ;
	schema:domainIncludes ceterms:ApprenticeshipCertificate, ceterms:AssessmentProfile, ceterms:AssociateDegree, ceterms:BachelorDegree, ceterms:Badge, ceterms:Certificate, ceterms:CertificateOfCompletion, ceterms:Certification, ceterms:Course, ceterms:Credential, ceterms:Degree, ceterms:DigitalBadge, ceterms:Diploma, ceterms:DoctoralDegree, ceterms:GeneralEducationDevelopment, ceterms:JourneymanCertificate, ceterms:LearningOpportunityProfile, ceterms:LearningProgram, ceterms:License, ceterms:MasterCertificate, ceterms:MasterDegree, ceterms:MicroCredential, ceterms:OpenBadge, ceterms:ProfessionalDoctorate, ceterms:QualityAssuranceCredential, ceterms:ResearchDoctorate, ceterms:SecondarySchoolDiploma ;
	schema:rangeIncludes ceterms:ApprenticeshipCertificate, ceterms:AssessmentProfile, ceterms:AssociateDegree, ceterms:BachelorDegree, ceterms:Badge, ceterms:Certificate, ceterms:CertificateOfCompletion, ceterms:Certification, ceterms:ConditionProfile, ceterms:Course, ceterms:Credential, ceterms:Degree, ceterms:DigitalBadge, ceterms:Diploma, ceterms:DoctoralDegree, ceterms:GeneralEducationDevelopment, ceterms:JourneymanCertificate, ceterms:LearningOpportunityProfile, ceterms:LearningProgram, ceterms:License, ceterms:MasterCertificate, ceterms:MasterDegree, ceterms:MicroCredential, ceterms:OpenBadge, ceterms:ProfessionalDoctorate, ceterms:QualityAssuranceCredential, ceterms:ResearchDoctorate, ceterms:SecondarySchoolDiploma .

ceterms:prerequisite a rdf:Property ;
	rdfs:label "Prerequisite"@en-US ;
	rdfs:comment "Resource that is required as a prior condition to this resource."@en-US ;
	vs:term_status vs:stable ;
	meta:changeHistory <http://credreg.net/ctdl/termhistory/ceterms/prerequisite/json> .

ceterms:previousVersion a rdf:Property ;
	rdfs:label "Previous Version"@en-US ;
	rdfs:comment "Version of the resource that immediately precedes this version."@en-US ;
	vs:term_status vs:stable ;
	meta:changeHistory <http://credreg.net/ctdl/termhistory/ceterms/previousVersion/json> ;
	schema:domainIncludes ceterms:ApprenticeshipCertificate, ceterms:AssociateDegree, ceterms:BachelorDegree, ceterms:Badge, ceterms:Certificate, ceterms:CertificateOfCompletion, ceterms:Certification, ceterms:Credential, ceterms:Degree, ceterms:DigitalBadge, ceterms:Diploma, ceterms:DoctoralDegree, ceterms:GeneralEducationDevelopment, ceterms:JourneymanCertificate, ceterms:License, ceterms:MasterCertificate, ceterms:MasterDegree, ceterms:MicroCredential, ceterms:OpenBadge, ceterms:ProfessionalDoctorate, ceterms:QualityAssuranceCredential, ceterms:ResearchDoctorate, ceterms:SecondarySchoolDiploma ;
	schema:rangeIncludes ceterms:ApprenticeshipCertificate, ceterms:AssociateDegree, ceterms:BachelorDegree, ceterms:Badge, ceterms:Certificate, ceterms:CertificateOfCompletion, ceterms:Certification, ceterms:Credential, ceterms:Degree, ceterms:DigitalBadge, ceterms:Diploma, ceterms:DoctoralDegree, ceterms:GeneralEducationDevelopment, ceterms:JourneymanCertificate, ceterms:License, ceterms:MasterCertificate, ceterms:MasterDegree, ceterms:MicroCredential, ceterms:OpenBadge, ceterms:ProfessionalDoctorate, ceterms:QualityAssuranceCredential, ceterms:ResearchDoctorate, ceterms:SecondarySchoolDiploma .

ceterms:price a rdf:Property ;
	rdfs:label "Price"@en-US ;
	rdfs:comment "Offer price of a credential, learning resource, assessment, related activity or resource."@en-US ;
	vs:term_status vs:stable ;
	meta:changeHistory <http://credreg.net/ctdl/termhistory/ceterms/price/json> ;
	schema:domainIncludes ceterms:CostProfile ;
	schema:rangeIncludes xsd:decimal ;
	owl:equivalentProperty schema:price .

ceterms:processFrequency a rdf:Property ;
	rdfs:label "Process Frequency"@en-US ;
	rdfs:comment "Interval of process occurence."@en-US ;
	vs:term_status vs:stable ;
	meta:changeHistory <http://credreg.net/ctdl/termhistory/ceterms/processFrequency/json> ;
	schema:domainIncludes ceterms:ProcessProfile ;
	schema:rangeIncludes rdf:langString .

ceterms:processingAgent a rdf:Property ;
	rdfs:label "Processing Agent"@en-US ;
	rdfs:comment "Organization or person performing the process."@en-US ;
	vs:term_status vs:stable ;
	meta:changeHistory <http://credreg.net/ctdl/termhistory/ceterms/processingAgent/json> ;
	schema:domainIncludes ceterms:ProcessProfile ;
	schema:rangeIncludes ceterms:CredentialOrganization, ceterms:Organization, ceterms:QACredentialOrganization .

ceterms:processMethod a rdf:Property ;
	rdfs:label "Process Method"@en-US ;
	rdfs:comment "Webpage or online document that describes the process methods."@en-US ;
	vs:term_status vs:stable ;
	meta:changeHistory <http://credreg.net/ctdl/termhistory/ceterms/processMethod/json> ;
	schema:domainIncludes ceterms:ProcessProfile ;
	schema:rangeIncludes xsd:anyURI .

ceterms:processMethodDescription a rdf:Property ;
	rdfs:label "Process Method Description"@en-US ;
	rdfs:comment "Textual description of the process methods."@en-US ;
	vs:term_status vs:stable ;
	meta:changeHistory <http://credreg.net/ctdl/termhistory/ceterms/processMethodDescription/json> ;
	schema:domainIncludes ceterms:ProcessProfile ;
	schema:rangeIncludes rdf:langString .

ceterms:processStandards a rdf:Property ;
	rdfs:label "Process Standards"@en-US ;
	rdfs:comment "Webpage or online document that describes the criteria, standards, and/or requirements used with a process."@en-US ;
	vs:term_status vs:stable ;
	meta:changeHistory <http://credreg.net/ctdl/termhistory/ceterms/processStandards/json> ;
	schema:domainIncludes ceterms:ApprenticeshipCertificate, ceterms:AssessmentProfile, ceterms:AssociateDegree, ceterms:BachelorDegree, ceterms:Badge, ceterms:Certificate, ceterms:CertificateOfCompletion, ceterms:Certification, ceterms:Credential, ceterms:Degree, ceterms:DigitalBadge, ceterms:Diploma, ceterms:DoctoralDegree, ceterms:GeneralEducationDevelopment, ceterms:JourneymanCertificate, ceterms:License, ceterms:MasterCertificate, ceterms:MasterDegree, ceterms:MicroCredential, ceterms:OpenBadge, ceterms:ProcessProfile, ceterms:ProfessionalDoctorate, ceterms:QualityAssuranceCredential, ceterms:ResearchDoctorate, ceterms:SecondarySchoolDiploma ;
	schema:rangeIncludes xsd:anyURI .

ceterms:processStandardsDescription a rdf:Property ;
	rdfs:label "Process Standards Description"@en-US ;
	rdfs:comment "Textual description of the criteria, standards, and/or requirements used with a process."@en-US ;
	vs:term_status vs:stable ;
	meta:changeHistory <http://credreg.net/ctdl/termhistory/ceterms/processStandardsDescription/json> ;
	schema:domainIncludes ceterms:ApprenticeshipCertificate, ceterms:AssessmentProfile, ceterms:AssociateDegree, ceterms:BachelorDegree, ceterms:Badge, ceterms:Certificate, ceterms:CertificateOfCompletion, ceterms:Certification, ceterms:Credential, ceterms:Degree, ceterms:DigitalBadge, ceterms:Diploma, ceterms:DoctoralDegree, ceterms:GeneralEducationDevelopment, ceterms:JourneymanCertificate, ceterms:License, ceterms:MasterCertificate, ceterms:MasterDegree, ceterms:MicroCredential, ceterms:OpenBadge, ceterms:ProcessProfile, ceterms:ProfessionalDoctorate, ceterms:QualityAssuranceCredential, ceterms:ResearchDoctorate, ceterms:SecondarySchoolDiploma ;
	schema:rangeIncludes rdf:langString .

ceterms:programTerm a rdf:Property ;
	rdfs:label "Program Term"@en-US ;
	rdfs:comment "Categorization of a term sequence based on the normative time between entry into a program of study and its completion such as \"1st quarter\", \"2nd quarter\"...\"5th quarter\"."@en-US ;
	vs:term_status vs:stable ;
	meta:changeHistory <http://credreg.net/ctdl/termhistory/ceterms/programTerm/json> ;
	schema:domainIncludes ceterms:CourseComponent ;
	schema:rangeIncludes ceterms:CredentialAlignmentObject .

ceterms:proxyFor a rdf:Property ;
	rdfs:label "Proxy For"@en-US ;
	rdfs:comment "Indicates the resource for which a pathway component or similar proxy resource is a stand-in."@en-US ;
	dct:description "The subject for this property will be acting as proxy in a context such as a pathway for the resource that is its object, so that assertions can be made about relationships between things in that context that are not universally true of the resources for which they are proxies."@en-US ;
	vs:term_status vs:unstable ;
	meta:changeHistory <http://credreg.net/ctdl/termhistory/ceterms/proxyFor/json> ;
	schema:domainIncludes ceterms:AssessmentComponent, ceterms:BasicComponent, ceterms:CocurricularComponent, ceterms:CollectionMember, ceterms:CompetencyComponent, ceterms:CourseComponent, ceterms:CredentialComponent, ceterms:ExtracurricularComponent, ceterms:JobComponent, ceterms:WorkExperienceComponent ;
	schema:rangeIncludes xsd:anyURI .

ceterms:qualityAssuranceTargetType a rdf:Property ;
	rdfs:label "Quality Assurance Target Type"@en-US ;
	rdfs:comment "Types of entities that the agent accredits, endorses, approves, or recognizes; select from an existing enumeration of such types."@en-US ;
	vs:term_status vs:stable ;
	meta:changeHistory <http://credreg.net/ctdl/termhistory/ceterms/qualityAssuranceTargetType/json> ;
	schema:domainIncludes ceterms:Organization, ceterms:QACredentialOrganization ;
	schema:rangeIncludes ceasn:CompetencyFramework, ceterms:ApprenticeshipCertificate, ceterms:AssessmentProfile, ceterms:AssociateDegree, ceterms:BachelorDegree, ceterms:Badge, ceterms:Certificate, ceterms:CertificateOfCompletion, ceterms:Certification, ceterms:Course, ceterms:Credential, ceterms:CredentialOrganization, ceterms:CredentialPerson, ceterms:Degree, ceterms:DigitalBadge, ceterms:Diploma, ceterms:DoctoralDegree, ceterms:GeneralEducationDevelopment, ceterms:JourneymanCertificate, ceterms:LearningOpportunityProfile, ceterms:LearningProgram, ceterms:License, ceterms:MasterCertificate, ceterms:MasterDegree, ceterms:MicroCredential, ceterms:OpenBadge, ceterms:Organization, ceterms:ProfessionalDoctorate, ceterms:QACredentialOrganization, ceterms:QualityAssuranceCredential, ceterms:ResearchDoctorate, ceterms:SecondarySchoolDiploma .

ceterms:recognizedBy a rdf:Property ;
	rdfs:label "Recognized By"@en-US ;
	rdfs:comment "Agent that acknowledges the validity of the credential, learning opportunity of assessment."@en-US ;
	vs:term_status vs:stable ;
	meta:changeHistory <http://credreg.net/ctdl/termhistory/ceterms/recognizedBy/json> ;
	schema:domainIncludes ceterms:ApprenticeshipCertificate, ceterms:AssessmentProfile, ceterms:AssociateDegree, ceterms:BachelorDegree, ceterms:Badge, ceterms:Certificate, ceterms:CertificateOfCompletion, ceterms:Certification, ceterms:Course, ceterms:Credential, ceterms:CredentialOrganization, ceterms:Degree, ceterms:DigitalBadge, ceterms:Diploma, ceterms:DoctoralDegree, ceterms:GeneralEducationDevelopment, ceterms:JourneymanCertificate, ceterms:LearningOpportunityProfile, ceterms:LearningProgram, ceterms:License, ceterms:MasterCertificate, ceterms:MasterDegree, ceterms:MicroCredential, ceterms:OpenBadge, ceterms:Organization, ceterms:ProfessionalDoctorate, ceterms:QACredentialOrganization, ceterms:QualityAssuranceCredential, ceterms:ResearchDoctorate, ceterms:SecondarySchoolDiploma ;
	schema:rangeIncludes ceterms:CredentialOrganization, ceterms:Organization, ceterms:QACredentialOrganization .

ceterms:recognizedIn a rdf:Property ;
	rdfs:label "Recognized In"@en-US ;
	rdfs:comment "Region or political jurisdiction such as a state, province or locale in which the credential, learning resource, or assessment has been publicly recommended, acknowledged or endorsed."@en-US ;
	vs:term_status vs:stable ;
	meta:changeHistory <http://credreg.net/ctdl/termhistory/ceterms/recognizedIn/json> ;
	schema:domainIncludes ceterms:ApprenticeshipCertificate, ceterms:AssessmentProfile, ceterms:AssociateDegree, ceterms:BachelorDegree, ceterms:Badge, ceterms:Certificate, ceterms:CertificateOfCompletion, ceterms:Certification, ceterms:Course, ceterms:Credential, ceterms:CredentialOrganization, ceterms:Degree, ceterms:DigitalBadge, ceterms:Diploma, ceterms:DoctoralDegree, ceterms:GeneralEducationDevelopment, ceterms:JourneymanCertificate, ceterms:LearningOpportunityProfile, ceterms:LearningProgram, ceterms:License, ceterms:MasterCertificate, ceterms:MasterDegree, ceterms:MicroCredential, ceterms:OpenBadge, ceterms:Organization, ceterms:ProfessionalDoctorate, ceterms:QACredentialOrganization, ceterms:QualityAssuranceCredential, ceterms:ResearchDoctorate, ceterms:SecondarySchoolDiploma ;
	schema:rangeIncludes ceterms:JurisdictionProfile .

ceterms:recognizes a rdf:Property ;
	rdfs:label "Recognizes"@en-US ;
	rdfs:comment "Resource that the agent recommends, endorses, indicates preference for, or otherwise provides a positive judgment."@en-US ;
	vann:usageNote "The agent being described may or may not use a set of formal recognition criteria."@en-US ;
	vs:term_status vs:stable ;
	meta:changeHistory <http://credreg.net/ctdl/termhistory/ceterms/recognizes/json> ;
	schema:domainIncludes ceterms:CredentialOrganization, ceterms:Organization, ceterms:QACredentialOrganization ;
	schema:rangeIncludes ceasn:CompetencyFramework, ceterms:ApprenticeshipCertificate, ceterms:AssessmentProfile, ceterms:AssociateDegree, ceterms:BachelorDegree, ceterms:Badge, ceterms:Certificate, ceterms:CertificateOfCompletion, ceterms:Certification, ceterms:Course, ceterms:Credential, ceterms:CredentialOrganization, ceterms:CredentialPerson, ceterms:Degree, ceterms:DigitalBadge, ceterms:Diploma, ceterms:DoctoralDegree, ceterms:GeneralEducationDevelopment, ceterms:JourneymanCertificate, ceterms:LearningOpportunityProfile, ceterms:LearningProgram, ceterms:License, ceterms:MasterCertificate, ceterms:MasterDegree, ceterms:MicroCredential, ceterms:OpenBadge, ceterms:Organization, ceterms:ProfessionalDoctorate, ceterms:QACredentialOrganization, ceterms:QualityAssuranceCredential, ceterms:ResearchDoctorate, ceterms:SecondarySchoolDiploma, ceterms:TransferValueProfile .

ceterms:recommends a rdf:Property ;
	rdfs:label "Recommends"@en-US ;
	rdfs:comment "Recommended credential, learning opportunity or assessment."@en-US ;
	vs:term_status vs:stable ;
	meta:changeHistory <http://credreg.net/ctdl/termhistory/ceterms/recommends/json> ;
	schema:domainIncludes ceterms:ApprenticeshipCertificate, ceterms:AssessmentProfile, ceterms:AssociateDegree, ceterms:BachelorDegree, ceterms:Badge, ceterms:Certificate, ceterms:CertificateOfCompletion, ceterms:Certification, ceterms:ConditionManifest, ceterms:Course, ceterms:Credential, ceterms:Degree, ceterms:DigitalBadge, ceterms:Diploma, ceterms:DoctoralDegree, ceterms:GeneralEducationDevelopment, ceterms:JourneymanCertificate, ceterms:LearningOpportunityProfile, ceterms:LearningProgram, ceterms:License, ceterms:MasterCertificate, ceterms:MasterDegree, ceterms:MicroCredential, ceterms:OpenBadge, ceterms:ProfessionalDoctorate, ceterms:QualityAssuranceCredential, ceterms:ResearchDoctorate, ceterms:SecondarySchoolDiploma ;
	schema:rangeIncludes ceasn:Competency, ceterms:ApprenticeshipCertificate, ceterms:AssessmentProfile, ceterms:AssociateDegree, ceterms:BachelorDegree, ceterms:Badge, ceterms:Certificate, ceterms:CertificateOfCompletion, ceterms:Certification, ceterms:ConditionProfile, ceterms:Course, ceterms:Credential, ceterms:CredentialAlignmentObject, ceterms:Degree, ceterms:DigitalBadge, ceterms:Diploma, ceterms:DoctoralDegree, ceterms:GeneralEducationDevelopment, ceterms:JourneymanCertificate, ceterms:LearningOpportunityProfile, ceterms:LearningProgram, ceterms:License, ceterms:MasterCertificate, ceterms:MasterDegree, ceterms:MicroCredential, ceterms:OpenBadge, ceterms:ProfessionalDoctorate, ceterms:QualityAssuranceCredential, ceterms:ResearchDoctorate, ceterms:SecondarySchoolDiploma .

ceterms:region a rdf:Property ;
	rdfs:label "Region"@en-US ;
	rdfs:comment "Entity that describes the longitude, latitude and other location details of an area."@en-US ;
	vs:term_status vs:stable ;
	meta:changeHistory <http://credreg.net/ctdl/termhistory/ceterms/region/json> ;
	rdfs:subPropertyOf ceterms:spatialCoverage ;
	schema:domainIncludes ceterms:ApprenticeshipCertificate, ceterms:AssessmentProfile, ceterms:AssociateDegree, ceterms:BachelorDegree, ceterms:Badge, ceterms:Certificate, ceterms:CertificateOfCompletion, ceterms:Certification, ceterms:CostProfile, ceterms:Course, ceterms:Credential, ceterms:Degree, ceterms:DigitalBadge, ceterms:Diploma, ceterms:DoctoralDegree, ceterms:EarningsProfile, ceterms:GeneralEducationDevelopment, ceterms:HoldersProfile, ceterms:JourneymanCertificate, ceterms:LearningOpportunityProfile, ceterms:LearningProgram, ceterms:License, ceterms:MasterCertificate, ceterms:MasterDegree, ceterms:MicroCredential, ceterms:OpenBadge, ceterms:ProcessProfile, ceterms:ProfessionalDoctorate, ceterms:QualityAssuranceCredential, ceterms:ResearchDoctorate, ceterms:RevocationProfile, ceterms:SecondarySchoolDiploma, ceterms:VerificationServiceProfile ;
	schema:rangeIncludes ceterms:Place .

ceterms:regulatedBy a rdf:Property ;
	rdfs:label "Regulated By"@en-US ;
	rdfs:comment "Quality assurance organization that enforces the legal requirements of the credential, learning resource or assessment."@en-US ;
	vs:term_status vs:stable ;
	meta:changeHistory <http://credreg.net/ctdl/termhistory/ceterms/regulatedBy/json> ;
	schema:domainIncludes ceterms:ApprenticeshipCertificate, ceterms:AssessmentProfile, ceterms:AssociateDegree, ceterms:BachelorDegree, ceterms:Badge, ceterms:Certificate, ceterms:CertificateOfCompletion, ceterms:Certification, ceterms:Course, ceterms:Credential, ceterms:CredentialOrganization, ceterms:Degree, ceterms:DigitalBadge, ceterms:Diploma, ceterms:DoctoralDegree, ceterms:GeneralEducationDevelopment, ceterms:JourneymanCertificate, ceterms:LearningOpportunityProfile, ceterms:LearningProgram, ceterms:License, ceterms:MasterCertificate, ceterms:MasterDegree, ceterms:MicroCredential, ceterms:OpenBadge, ceterms:Organization, ceterms:ProfessionalDoctorate, ceterms:QACredentialOrganization, ceterms:QualityAssuranceCredential, ceterms:ResearchDoctorate, ceterms:SecondarySchoolDiploma ;
	schema:rangeIncludes ceterms:Organization, ceterms:QACredentialOrganization .

ceterms:regulatedIn a rdf:Property ;
	rdfs:label "Regulated In"@en-US ;
	rdfs:comment "Region or political jurisdiction such as a state, province or locale in which the credential, learning opportunity or resource is regulated."@en-US ;
	vs:term_status vs:stable ;
	meta:changeHistory <http://credreg.net/ctdl/termhistory/ceterms/regulatedIn/json> ;
	schema:domainIncludes ceterms:ApprenticeshipCertificate, ceterms:AssessmentProfile, ceterms:AssociateDegree, ceterms:BachelorDegree, ceterms:Badge, ceterms:Certificate, ceterms:CertificateOfCompletion, ceterms:Certification, ceterms:Course, ceterms:Credential, ceterms:CredentialOrganization, ceterms:Degree, ceterms:DigitalBadge, ceterms:Diploma, ceterms:DoctoralDegree, ceterms:GeneralEducationDevelopment, ceterms:JourneymanCertificate, ceterms:LearningOpportunityProfile, ceterms:LearningProgram, ceterms:License, ceterms:MasterCertificate, ceterms:MasterDegree, ceterms:MicroCredential, ceterms:OpenBadge, ceterms:Organization, ceterms:ProfessionalDoctorate, ceterms:QACredentialOrganization, ceterms:QualityAssuranceCredential, ceterms:ResearchDoctorate, ceterms:SecondarySchoolDiploma ;
	schema:rangeIncludes ceterms:JurisdictionProfile .

ceterms:regulates a rdf:Property ;
	rdfs:label "Regulates"@en-US ;
	rdfs:comment "Credential, learning opportunity, assessment or organization that this quality assurance organization monitors, including enforcement of applicable legal requirements or standards."@en-US ;
	dct:description "Regulation of organizations includes authorization to act or operate."@en-US ;
	vs:term_status vs:stable ;
	meta:changeHistory <http://credreg.net/ctdl/termhistory/ceterms/regulates/json> ;
	schema:domainIncludes ceterms:Organization, ceterms:QACredentialOrganization ;
	schema:rangeIncludes ceasn:CompetencyFramework, ceterms:ApprenticeshipCertificate, ceterms:AssessmentProfile, ceterms:AssociateDegree, ceterms:BachelorDegree, ceterms:Badge, ceterms:Certificate, ceterms:CertificateOfCompletion, ceterms:Certification, ceterms:Course, ceterms:Credential, ceterms:CredentialOrganization, ceterms:Degree, ceterms:DigitalBadge, ceterms:Diploma, ceterms:DoctoralDegree, ceterms:GeneralEducationDevelopment, ceterms:JourneymanCertificate, ceterms:LearningOpportunityProfile, ceterms:LearningProgram, ceterms:License, ceterms:MasterCertificate, ceterms:MasterDegree, ceterms:MicroCredential, ceterms:OpenBadge, ceterms:Organization, ceterms:ProfessionalDoctorate, ceterms:QACredentialOrganization, ceterms:QualityAssuranceCredential, ceterms:ResearchDoctorate, ceterms:SecondarySchoolDiploma .

ceterms:relatedAction a rdf:Property ;
	rdfs:label "Related Action"@en-US ;
	rdfs:comment "Action related to the resource."@en-US ;
	vs:term_status vs:stable ;
	meta:changeHistory <http://credreg.net/ctdl/termhistory/ceterms/relatedAction/json> ;
	schema:domainIncludes ceterms:ApprenticeshipCertificate, ceterms:AssociateDegree, ceterms:BachelorDegree, ceterms:Badge, ceterms:Certificate, ceterms:CertificateOfCompletion, ceterms:Certification, ceterms:Credential, ceterms:Degree, ceterms:DigitalBadge, ceterms:Diploma, ceterms:DoctoralDegree, ceterms:GeneralEducationDevelopment, ceterms:JourneymanCertificate, ceterms:License, ceterms:MasterCertificate, ceterms:MasterDegree, ceterms:MicroCredential, ceterms:OpenBadge, ceterms:ProfessionalDoctorate, ceterms:QualityAssuranceCredential, ceterms:ResearchDoctorate, ceterms:SecondarySchoolDiploma ;
	schema:rangeIncludes ceterms:AccreditAction, ceterms:AdvancedStandingAction, ceterms:ApproveAction, ceterms:CredentialingAction, ceterms:OfferAction, ceterms:RecognizeAction, ceterms:RegulateAction, ceterms:RenewAction, ceterms:RevokeAction, ceterms:RightsAction .

ceterms:renewal a rdf:Property ;
	rdfs:label "Renewal"@en-US ;
	rdfs:comment "Entity describing the constraints, prerequisites, entry conditions, or requirements necessary to maintenance and renewal of an awarded credential."@en-US ;
	dct:description "Generally, renewal applies to certifications and licenses; however, it may occasionally apply to other types of credentials."@en-US ;
	vs:term_status vs:stable ;
	meta:changeHistory <http://credreg.net/ctdl/termhistory/ceterms/renewal/json> ;
	schema:domainIncludes ceterms:ApprenticeshipCertificate, ceterms:AssociateDegree, ceterms:BachelorDegree, ceterms:Badge, ceterms:Certificate, ceterms:CertificateOfCompletion, ceterms:Certification, ceterms:ConditionManifest, ceterms:Credential, ceterms:Degree, ceterms:DigitalBadge, ceterms:Diploma, ceterms:DoctoralDegree, ceterms:GeneralEducationDevelopment, ceterms:JourneymanCertificate, ceterms:License, ceterms:MasterCertificate, ceterms:MasterDegree, ceterms:MicroCredential, ceterms:OpenBadge, ceterms:ProfessionalDoctorate, ceterms:QualityAssuranceCredential, ceterms:ResearchDoctorate, ceterms:SecondarySchoolDiploma ;
	schema:rangeIncludes ceterms:ConditionProfile .

ceterms:renewalFrequency a rdf:Property ;
	rdfs:label "Renewal Frequency"@en-US ;
	rdfs:comment "Frequency with which the credential needs to be renewed."@en-US ;
	vs:term_status vs:stable ;
	meta:changeHistory <http://credreg.net/ctdl/termhistory/ceterms/renewalFrequency/json> ;
	rdfs:subPropertyOf ceterms:maximumDuration ;
	schema:domainIncludes ceterms:ApprenticeshipCertificate, ceterms:AssociateDegree, ceterms:BachelorDegree, ceterms:Badge, ceterms:Certificate, ceterms:CertificateOfCompletion, ceterms:Certification, ceterms:Credential, ceterms:Degree, ceterms:DigitalBadge, ceterms:Diploma, ceterms:DoctoralDegree, ceterms:GeneralEducationDevelopment, ceterms:JourneymanCertificate, ceterms:License, ceterms:MasterCertificate, ceterms:MasterDegree, ceterms:MicroCredential, ceterms:OpenBadge, ceterms:ProfessionalDoctorate, ceterms:QualityAssuranceCredential, ceterms:ResearchDoctorate, ceterms:SecondarySchoolDiploma ;
	schema:rangeIncludes schema:Duration .

ceterms:renewedBy a rdf:Property ;
	rdfs:label "Renewed By"@en-US ;
	rdfs:comment "Organization or person that handles the renewal of the credential."@en-US ;
	vs:term_status vs:stable ;
	meta:changeHistory <http://credreg.net/ctdl/termhistory/ceterms/renewedBy/json> ;
	schema:domainIncludes ceterms:ApprenticeshipCertificate, ceterms:AssociateDegree, ceterms:BachelorDegree, ceterms:Badge, ceterms:Certificate, ceterms:CertificateOfCompletion, ceterms:Certification, ceterms:Credential, ceterms:Degree, ceterms:DigitalBadge, ceterms:Diploma, ceterms:DoctoralDegree, ceterms:GeneralEducationDevelopment, ceterms:JourneymanCertificate, ceterms:License, ceterms:MasterCertificate, ceterms:MasterDegree, ceterms:MicroCredential, ceterms:OpenBadge, ceterms:ProfessionalDoctorate, ceterms:QualityAssuranceCredential, ceterms:ResearchDoctorate, ceterms:SecondarySchoolDiploma ;
	schema:rangeIncludes ceterms:CredentialOrganization, ceterms:Organization, ceterms:QACredentialOrganization .

ceterms:renewedIn a rdf:Property ;
	rdfs:label "Renewed In"@en-US ;
	rdfs:comment "Region or political jurisdiction such as a state, province or locale in which the credential is renewable."@en-US ;
	vs:term_status vs:stable ;
	meta:changeHistory <http://credreg.net/ctdl/termhistory/ceterms/renewedIn/json> ;
	schema:domainIncludes ceterms:ApprenticeshipCertificate, ceterms:AssociateDegree, ceterms:BachelorDegree, ceterms:Badge, ceterms:Certificate, ceterms:CertificateOfCompletion, ceterms:Certification, ceterms:Credential, ceterms:Degree, ceterms:DigitalBadge, ceterms:Diploma, ceterms:DoctoralDegree, ceterms:GeneralEducationDevelopment, ceterms:JourneymanCertificate, ceterms:License, ceterms:MasterCertificate, ceterms:MasterDegree, ceterms:MicroCredential, ceterms:OpenBadge, ceterms:ProfessionalDoctorate, ceterms:QualityAssuranceCredential, ceterms:ResearchDoctorate, ceterms:SecondarySchoolDiploma ;
	schema:rangeIncludes ceterms:JurisdictionProfile .

ceterms:renews a rdf:Property ;
	rdfs:label "Renews"@en-US ;
	rdfs:comment "Credential type that has its validity extended by the organization or person."@en-US ;
	dct:description "The value of ceterms:renews should be one of the specific subclasses of ceterms:Credential."@en-US ;
	vs:term_status vs:stable ;
	meta:changeHistory <http://credreg.net/ctdl/termhistory/ceterms/renews/json> ;
	schema:domainIncludes ceterms:CredentialOrganization, ceterms:Organization, ceterms:QACredentialOrganization ;
	schema:rangeIncludes ceterms:ApprenticeshipCertificate, ceterms:AssociateDegree, ceterms:BachelorDegree, ceterms:Badge, ceterms:Certificate, ceterms:CertificateOfCompletion, ceterms:Certification, ceterms:Credential, ceterms:Degree, ceterms:DigitalBadge, ceterms:Diploma, ceterms:DoctoralDegree, ceterms:GeneralEducationDevelopment, ceterms:JourneymanCertificate, ceterms:License, ceterms:MasterCertificate, ceterms:MasterDegree, ceterms:MicroCredential, ceterms:OpenBadge, ceterms:ProfessionalDoctorate, ceterms:QualityAssuranceCredential, ceterms:ResearchDoctorate, ceterms:SecondarySchoolDiploma .

ceterms:requiredNumber a rdf:Property ;
	rdfs:label "Required Number"@en-US ;
	rdfs:comment "Number of targetComponent resources that must be fulfilled in order to satisfy the ComponentCondition."@en-US ;
	vs:term_status vs:stable ;
	meta:changeHistory <http://credreg.net/ctdl/termhistory/ceterms/requiredNumber/json> ;
	schema:domainIncludes ceterms:ComponentCondition ;
	schema:rangeIncludes xsd:integer .

ceterms:requires a rdf:Property ;
	rdfs:label "Requires"@en-US ;
	rdfs:comment "Requirement or set of requirements for this resource."@en-US ;
	vs:term_status vs:stable ;
	meta:changeHistory <http://credreg.net/ctdl/termhistory/ceterms/requires/json> ;
	schema:domainIncludes ceterms:ApprenticeshipCertificate, ceterms:AssessmentProfile, ceterms:AssociateDegree, ceterms:BachelorDegree, ceterms:Badge, ceterms:Certificate, ceterms:CertificateOfCompletion, ceterms:Certification, ceterms:ConditionManifest, ceterms:Course, ceterms:Credential, ceterms:Degree, ceterms:DigitalBadge, ceterms:Diploma, ceterms:DoctoralDegree, ceterms:GeneralEducationDevelopment, ceterms:Job, ceterms:JourneymanCertificate, ceterms:LearningOpportunityProfile, ceterms:LearningProgram, ceterms:License, ceterms:MasterCertificate, ceterms:MasterDegree, ceterms:MicroCredential, ceterms:Occupation, ceterms:OpenBadge, ceterms:ProfessionalDoctorate, ceterms:QualityAssuranceCredential, ceterms:ResearchDoctorate, ceterms:SecondarySchoolDiploma, ceterms:TransferIntermediary ;
	schema:rangeIncludes ceasn:Competency, ceterms:ApprenticeshipCertificate, ceterms:AssessmentProfile, ceterms:AssociateDegree, ceterms:BachelorDegree, ceterms:Badge, ceterms:Certificate, ceterms:CertificateOfCompletion, ceterms:Certification, ceterms:ConditionProfile, ceterms:Course, ceterms:Credential, ceterms:CredentialAlignmentObject, ceterms:Degree, ceterms:DigitalBadge, ceterms:Diploma, ceterms:DoctoralDegree, ceterms:GeneralEducationDevelopment, ceterms:JourneymanCertificate, ceterms:LearningOpportunityProfile, ceterms:LearningProgram, ceterms:License, ceterms:MasterCertificate, ceterms:MasterDegree, ceterms:MicroCredential, ceterms:OpenBadge, ceterms:ProfessionalDoctorate, ceterms:QualityAssuranceCredential, ceterms:ResearchDoctorate, ceterms:SecondarySchoolDiploma .

ceterms:residencyType a rdf:Property ;
	rdfs:label "Residency Type"@en-US ;
	rdfs:comment "Type of legal residency status of a person; select from an existing enumeration of such types."@en-US ;
	dct:description "Residency defines the duration of stay required by national, state, provincial or local laws that entitles a person to the legal protection and benefits provided to the applicable type."@en-US ;
	vann:usageNote "Best practice for U.S. credentials and for submission to the Credential Engine Registry, is to use concepts from the ceterms:Residency vocabulary."@en-US ;
	vs:term_status vs:stable ;
	meta:changeHistory <http://credreg.net/ctdl/termhistory/ceterms/residencyType/json> ;
	rdfs:subPropertyOf ceterms:credentialAlignment ;
	schema:domainIncludes ceterms:CostProfile ;
	schema:rangeIncludes ceterms:CredentialAlignmentObject ;
	meta:targetScheme ceterms:Residency .

ceterms:residentOf a rdf:Property ;
	rdfs:label "Resident Of"@en-US ;
	rdfs:comment "Geographic or political region of which a person must be a legal resident or citizen in order to be eligible for the credential."@en-US ;
	dct:description "Residency defines the duration of stay required by national, state, provincial or local laws that entitles a person to the legal protection and benefits provided to the applicable type."@en-US ;
	vs:term_status vs:stable ;
	meta:changeHistory <http://credreg.net/ctdl/termhistory/ceterms/residentOf/json> ;
	schema:domainIncludes ceterms:ConditionProfile ;
	schema:rangeIncludes ceterms:JurisdictionProfile .

ceterms:result a rdf:Property ;
	rdfs:label "Result"@en-US ;
	rdfs:comment "Outcome produced in the action."@en-US ;
	vs:term_status vs:unstable ;
	meta:changeHistory <http://credreg.net/ctdl/termhistory/ceterms/result/json> ;
	schema:domainIncludes ceterms:WorkforceDemandAction ;
	schema:rangeIncludes ceterms:CredentialAlignmentObject .

ceterms:resultingAward a rdf:Property ;
	rdfs:label "Resulting Award"@en-US ;
	rdfs:comment "Awarded credential resulting from an action."@en-US ;
	dct:description "An awarded credential is of the type ceterms:CredentialAssertion."@en-US ;
	vs:term_status vs:stable ;
	meta:changeHistory <http://credreg.net/ctdl/termhistory/ceterms/resultingAward/json> ;
	rdfs:subPropertyOf ceterms:result ;
	schema:domainIncludes ceterms:AccreditAction, ceterms:RenewAction ;
	schema:rangeIncludes ceterms:CredentialAssertion .

ceterms:reviewProcess a rdf:Property ;
	rdfs:label "Review Process"@en-US ;
	rdfs:comment "Entity that describes the process by which the credential, or aspects of it, are reviewed."@en-US ;
	vs:term_status vs:stable ;
	meta:changeHistory <http://credreg.net/ctdl/termhistory/ceterms/reviewProcess/json> ;
	schema:domainIncludes ceterms:ApprenticeshipCertificate, ceterms:AssociateDegree, ceterms:BachelorDegree, ceterms:Badge, ceterms:Certificate, ceterms:CertificateOfCompletion, ceterms:Certification, ceterms:Credential, ceterms:CredentialOrganization, ceterms:Degree, ceterms:DigitalBadge, ceterms:Diploma, ceterms:DoctoralDegree, ceterms:GeneralEducationDevelopment, ceterms:JourneymanCertificate, ceterms:License, ceterms:MasterCertificate, ceterms:MasterDegree, ceterms:MicroCredential, ceterms:OpenBadge, ceterms:Organization, ceterms:ProfessionalDoctorate, ceterms:QACredentialOrganization, ceterms:QualityAssuranceCredential, ceterms:ResearchDoctorate, ceterms:SecondarySchoolDiploma ;
	schema:rangeIncludes ceterms:ProcessProfile .

ceterms:revocation a rdf:Property ;
	rdfs:label "Revocation"@en-US ;
	rdfs:comment "Entity that describes the processes and criteria for ending (revoking) the validity or operation of an awarded credential."@en-US ;
	dct:description "Generally, revocation applies to certifications and licenses; however, it may also apply to other types of credential under extraordinary circumstances."@en-US ;
	vs:term_status vs:stable ;
	meta:changeHistory <http://credreg.net/ctdl/termhistory/ceterms/revocation/json> ;
	schema:domainIncludes ceterms:ApprenticeshipCertificate, ceterms:AssociateDegree, ceterms:BachelorDegree, ceterms:Badge, ceterms:Certificate, ceterms:CertificateOfCompletion, ceterms:Certification, ceterms:Credential, ceterms:Degree, ceterms:DigitalBadge, ceterms:Diploma, ceterms:DoctoralDegree, ceterms:GeneralEducationDevelopment, ceterms:JourneymanCertificate, ceterms:License, ceterms:MasterCertificate, ceterms:MasterDegree, ceterms:MicroCredential, ceterms:OpenBadge, ceterms:ProfessionalDoctorate, ceterms:QualityAssuranceCredential, ceterms:ResearchDoctorate, ceterms:SecondarySchoolDiploma ;
	schema:rangeIncludes ceterms:RevocationProfile .

ceterms:revocationCriteria a rdf:Property ;
	rdfs:label "Revocation Criteria"@en-US ;
	rdfs:comment "Webpage or online document that provides information about the removal criteria for an awarded credential."@en-US ;
	vs:term_status vs:stable ;
	meta:changeHistory <http://credreg.net/ctdl/termhistory/ceterms/revocationCriteria/json> ;
	schema:domainIncludes ceterms:RevocationProfile ;
	schema:rangeIncludes xsd:anyURI .

ceterms:revocationCriteriaDescription a rdf:Property ;
	rdfs:label "Revocation Criteria"@en-US ;
	rdfs:comment "Textual description providing information about the removal criteria for an awarded credential."@en-US ;
	vs:term_status vs:stable ;
	meta:changeHistory <http://credreg.net/ctdl/termhistory/ceterms/revocationCriteriaDescription/json> ;
	schema:domainIncludes ceterms:RevocationProfile ;
	schema:rangeIncludes rdf:langString .

ceterms:revocationProcess a rdf:Property ;
	rdfs:label "Revocation Process"@en-US ;
	rdfs:comment "Entity describing the process by which the credential is revoked."@en-US ;
	vs:term_status vs:stable ;
	meta:changeHistory <http://credreg.net/ctdl/termhistory/ceterms/revocationProcess/json> ;
	schema:domainIncludes ceterms:ApprenticeshipCertificate, ceterms:AssociateDegree, ceterms:BachelorDegree, ceterms:Badge, ceterms:Certificate, ceterms:CertificateOfCompletion, ceterms:Certification, ceterms:Credential, ceterms:CredentialOrganization, ceterms:Degree, ceterms:DigitalBadge, ceterms:Diploma, ceterms:DoctoralDegree, ceterms:GeneralEducationDevelopment, ceterms:JourneymanCertificate, ceterms:License, ceterms:MasterCertificate, ceterms:MasterDegree, ceterms:MicroCredential, ceterms:OpenBadge, ceterms:Organization, ceterms:ProfessionalDoctorate, ceterms:QACredentialOrganization, ceterms:QualityAssuranceCredential, ceterms:ResearchDoctorate, ceterms:SecondarySchoolDiploma ;
	schema:rangeIncludes ceterms:ProcessProfile .

ceterms:revokedBy a rdf:Property ;
	rdfs:label "Revoked By"@en-US ;
	rdfs:comment "Organization or person that handles revocation of an awarded credential due to violations or failure to renew."@en-US ;
	vs:term_status vs:stable ;
	meta:changeHistory <http://credreg.net/ctdl/termhistory/ceterms/revokedBy/json> ;
	schema:domainIncludes ceterms:ApprenticeshipCertificate, ceterms:AssociateDegree, ceterms:BachelorDegree, ceterms:Badge, ceterms:Certificate, ceterms:CertificateOfCompletion, ceterms:Certification, ceterms:Credential, ceterms:Degree, ceterms:DigitalBadge, ceterms:Diploma, ceterms:DoctoralDegree, ceterms:GeneralEducationDevelopment, ceterms:JourneymanCertificate, ceterms:License, ceterms:MasterCertificate, ceterms:MasterDegree, ceterms:MicroCredential, ceterms:OpenBadge, ceterms:ProfessionalDoctorate, ceterms:QualityAssuranceCredential, ceterms:ResearchDoctorate, ceterms:SecondarySchoolDiploma ;
	schema:rangeIncludes ceterms:CredentialOrganization, ceterms:Organization, ceterms:QACredentialOrganization .

ceterms:revokedIn a rdf:Property ;
	rdfs:label "Revoked In"@en-US ;
	rdfs:comment "Region or political jurisdiction such as a state, province or locale in which the credential can be revoked."@en-US ;
	vs:term_status vs:stable ;
	meta:changeHistory <http://credreg.net/ctdl/termhistory/ceterms/revokedIn/json> ;
	schema:domainIncludes ceterms:ApprenticeshipCertificate, ceterms:AssociateDegree, ceterms:BachelorDegree, ceterms:Badge, ceterms:Certificate, ceterms:CertificateOfCompletion, ceterms:Certification, ceterms:Credential, ceterms:Degree, ceterms:DigitalBadge, ceterms:Diploma, ceterms:DoctoralDegree, ceterms:GeneralEducationDevelopment, ceterms:JourneymanCertificate, ceterms:License, ceterms:MasterCertificate, ceterms:MasterDegree, ceterms:MicroCredential, ceterms:OpenBadge, ceterms:ProfessionalDoctorate, ceterms:QualityAssuranceCredential, ceterms:ResearchDoctorate, ceterms:SecondarySchoolDiploma ;
	schema:rangeIncludes ceterms:JurisdictionProfile .

ceterms:revokes a rdf:Property ;
	rdfs:label "Revokes"@en-US ;
	rdfs:comment "Credential type that can be invalidated or retracted by the awarding agent."@en-US ;
	dct:description "The value of ceterms:revokes should be one of the specific subclasses of ceterms:Credential."@en-US ;
	vs:term_status vs:stable ;
	meta:changeHistory <http://credreg.net/ctdl/termhistory/ceterms/revokes/json> ;
	schema:domainIncludes ceterms:CredentialOrganization, ceterms:Organization, ceterms:QACredentialOrganization ;
	schema:rangeIncludes ceterms:ApprenticeshipCertificate, ceterms:AssociateDegree, ceterms:BachelorDegree, ceterms:Badge, ceterms:Certificate, ceterms:CertificateOfCompletion, ceterms:Certification, ceterms:Credential, ceterms:Degree, ceterms:DigitalBadge, ceterms:Diploma, ceterms:DoctoralDegree, ceterms:GeneralEducationDevelopment, ceterms:JourneymanCertificate, ceterms:License, ceterms:MasterCertificate, ceterms:MasterDegree, ceterms:MicroCredential, ceterms:OpenBadge, ceterms:ProfessionalDoctorate, ceterms:QualityAssuranceCredential, ceterms:ResearchDoctorate, ceterms:SecondarySchoolDiploma .

ceterms:rightAction a rdf:Property ;
	rdfs:label "Right Action"@en-US ;
	rdfs:comment "Action performed on the right source; select from an existing enumeration of such types."@en-US ;
	vs:term_status vs:unstable ;
	meta:changeHistory <http://credreg.net/ctdl/termhistory/ceterms/rightAction/json> ;
	schema:domainIncludes ceterms:Constraint ;
	schema:rangeIncludes skos:Concept ;
	meta:targetScheme ceterms:ArrayOperationCategory .

ceterms:rightSource a rdf:Property ;
	rdfs:label "Right Source"@en-US ;
	rdfs:comment "Right hand parameter of a constraint."@en-US ;
	vs:term_status vs:unstable ;
	meta:changeHistory <http://credreg.net/ctdl/termhistory/ceterms/rightSource/json> ;
	schema:domainIncludes ceterms:Constraint ;
	schema:rangeIncludes rdf:Property, rdfs:Class, rdfs:Literal, skos:Concept .

ceterms:sameAs a rdf:Property ;
	rdfs:label "Same As"@en-US ;
	rdfs:comment "Another source of information about the entity being described."@en-US ;
	dct:description "Other sources may include descriptions of entities in open databases such as DBpedia, Wikidata, the Credential Engine Registry, or other platforms."@en-US ;
	vs:term_status vs:stable ;
	meta:changeHistory <http://credreg.net/ctdl/termhistory/ceterms/sameAs/json> ;
	schema:domainIncludes ceterms:ApprenticeshipCertificate, ceterms:AssessmentProfile, ceterms:AssociateDegree, ceterms:BachelorDegree, ceterms:Badge, ceterms:Certificate, ceterms:CertificateOfCompletion, ceterms:Certification, ceterms:Course, ceterms:Credential, ceterms:CredentialOrganization, ceterms:Degree, ceterms:DigitalBadge, ceterms:Diploma, ceterms:DoctoralDegree, ceterms:GeneralEducationDevelopment, ceterms:Job, ceterms:JourneymanCertificate, ceterms:LearningOpportunityProfile, ceterms:LearningProgram, ceterms:License, ceterms:MasterCertificate, ceterms:MasterDegree, ceterms:MicroCredential, ceterms:Occupation, ceterms:OpenBadge, ceterms:Organization, ceterms:ProfessionalDoctorate, ceterms:QACredentialOrganization, ceterms:QualityAssuranceCredential, ceterms:ResearchDoctorate, ceterms:SecondarySchoolDiploma ;
	schema:rangeIncludes xsd:anyURI .

ceterms:sced a rdf:Property ;
	rdfs:label "SCED"@en-US ;
	rdfs:comment "School Courses for the Exchange of Data code for a course."@en-US ;
	vann:usageNote "It is preferable to record the whole 12 character alphanumeric code, however it is also valid to record just the five digit subject code + course number."@en-US ;
	vs:term_status vs:unstable ;
	meta:changeHistory <http://credreg.net/ctdl/termhistory/ceterms/sced/json> ;
	schema:domainIncludes ceterms:Course ;
	schema:rangeIncludes xsd:string .

ceterms:scheduleFrequencyType a rdf:Property ;
	rdfs:label "Schedule Frequency Type"@en-US ;
	rdfs:comment "Type of frequency indicating the cadence at which events associated with a resource typically occur; select from an existing enumeration of such types."@en-US ;
	dct:description "This relates to the frequency of events associated with a resource once it is running."@en-US ;
	vann:usageNote "For information relating to how often something starts, use ceterms:offerFrequencyType."@en-US ;
	vs:term_status vs:unstable ;
	meta:changeHistory <http://credreg.net/ctdl/termhistory/ceterms/scheduleFrequencyType/json> ;
	schema:domainIncludes ceterms:AssessmentProfile, ceterms:Course, ceterms:LearningOpportunityProfile, ceterms:LearningProgram, ceterms:ScheduledOffering ;
	schema:rangeIncludes ceterms:CredentialAlignmentObject ;
	meta:targetScheme ceterms:ScheduleFrequency .

ceterms:scheduleTimingType a rdf:Property ;
	rdfs:label "Schedule Timing Type"@en-US ;
	rdfs:comment "Type of time at which events typically occur; select from an existing enumeration of such types."@en-US ;
	vs:term_status vs:unstable ;
	meta:changeHistory <http://credreg.net/ctdl/termhistory/ceterms/scheduleTimingType/json> ;
	schema:domainIncludes ceterms:AssessmentProfile, ceterms:Course, ceterms:LearningOpportunityProfile, ceterms:LearningProgram, ceterms:ScheduledOffering ;
	schema:rangeIncludes ceterms:CredentialAlignmentObject ;
	meta:targetScheme ceterms:ScheduleTiming .

ceterms:scoringMethodDescription a rdf:Property ;
	rdfs:label "Scoring Method Description"@en-US ;
	rdfs:comment "Textual description of the method used to score the assessment."@en-US ;
	vs:term_status vs:stable ;
	meta:changeHistory <http://credreg.net/ctdl/termhistory/ceterms/scoringMethodDescription/json> ;
	schema:domainIncludes ceterms:AssessmentProfile, ceterms:ProcessProfile ;
	schema:rangeIncludes rdf:langString .

ceterms:scoringMethodExample a rdf:Property ;
	rdfs:label "Scoring Method Example"@en-US ;
	rdfs:comment "Webpage or online document providing an example of the method or tool used to score the assessment."@en-US ;
	vs:term_status vs:stable ;
	meta:changeHistory <http://credreg.net/ctdl/termhistory/ceterms/scoringMethodExample/json> ;
	schema:domainIncludes ceterms:AssessmentProfile, ceterms:ProcessProfile ;
	schema:rangeIncludes xsd:anyURI .

ceterms:scoringMethodExampleDescription a rdf:Property ;
	rdfs:label "Scoring Method Example Description"@en-US ;
	rdfs:comment "Textual example of the method or tool used to score the assessment."@en-US ;
	vs:term_status vs:stable ;
	meta:changeHistory <http://credreg.net/ctdl/termhistory/ceterms/scoringMethodExampleDescription/json> ;
	schema:domainIncludes ceterms:AssessmentProfile, ceterms:ProcessProfile ;
	schema:rangeIncludes rdf:langString .

ceterms:scoringMethodType a rdf:Property ;
	rdfs:label "Scoring Method Type"@en-US ;
	rdfs:comment "Type of method used to score the assessment; select from an existing enumeration of such types."@en-US ;
	vann:usageNote "Best practice for U.S. credentials and for submission to the Credential Engine Registry, is to use concepts from the ceterms:ScoringMethod vocabulary."@en-US ;
	vs:term_status vs:stable ;
	meta:changeHistory <http://credreg.net/ctdl/termhistory/ceterms/scoringMethodType/json> ;
	schema:domainIncludes ceterms:AssessmentProfile ;
	schema:rangeIncludes ceterms:CredentialAlignmentObject ;
	meta:targetScheme ceterms:ScoringMethod .

ceterms:sensoryCapabilityType a rdf:Property ;
	rdfs:label "Sensory Capability Type"@en-US ;
	rdfs:comment "Type of required or expected sensory capability; select from an existing enumeration of such types."@en-US ;
	dct:description "Such types may include smell, color discrimination, depth perception, and so on."@en-US ;
	vs:term_status vs:unstable ;
	meta:changeHistory <http://credreg.net/ctdl/termhistory/ceterms/sensoryCapabilityType/json> ;
	schema:domainIncludes ceasn:Competency, ceterms:Job, ceterms:Task, ceterms:WorkRole ;
	schema:rangeIncludes skos:Concept .

ceterms:serviceType a rdf:Property ;
	rdfs:label "Service Type"@en-US ;
	rdfs:comment "Type of service offered by the agent being described; select from an existing enumeration of such terms."@en-US ;
	vann:usageNote "Recommended best practice for credentials in the Credential Engine Registry is to use concepts from the ceterms:AgentServiceType vocabulary."@en-US ;
	vs:term_status vs:stable ;
	meta:changeHistory <http://credreg.net/ctdl/termhistory/ceterms/serviceType/json> ;
	schema:domainIncludes ceterms:CredentialOrganization, ceterms:Organization, ceterms:QACredentialOrganization ;
	schema:rangeIncludes ceterms:CredentialAlignmentObject ;
	meta:targetScheme ceterms:AgentServiceType .

ceterms:socialMedia a rdf:Property ;
	rdfs:label "Social Media"@en-US ;
	rdfs:comment "Social media access point for an agent or an agent's contact point."@en-US ;
	vs:term_status vs:stable ;
	meta:changeHistory <http://credreg.net/ctdl/termhistory/ceterms/socialMedia/json> ;
	schema:domainIncludes ceterms:ContactPoint, ceterms:CredentialOrganization, ceterms:Organization, ceterms:QACredentialOrganization ;
	schema:rangeIncludes xsd:anyURI .

ceterms:source a rdf:Property ;
	rdfs:label "Source URL"@en-US ;
	rdfs:comment "Authoritative source of an entity's information."@en-US ;
	dct:description "Citation or description of an authoritative souce from which information or description has been derived."@en-US ;
	vs:term_status vs:stable ;
	meta:changeHistory <http://credreg.net/ctdl/termhistory/ceterms/source/json> ;
	schema:domainIncludes ceterms:AggregateDataProfile, ceterms:EarningsProfile, ceterms:EmploymentOutcomeProfile, ceterms:HoldersProfile ;
	schema:rangeIncludes xsd:anyURI .

ceterms:sourceData a rdf:Property ;
	rdfs:label "Source Data"@en-US ;
	rdfs:comment "Structured data representing the resource."@en-US ;
	dct:description "The preferred data serialization is JSON-LD or some other serialization of RDF."@en-US ;
	vs:term_status vs:stable ;
	meta:changeHistory <http://credreg.net/ctdl/termhistory/ceterms/sourceData/json> ;
	schema:domainIncludes ceterms:AssessmentComponent, ceterms:BasicComponent, ceterms:CocurricularComponent, ceterms:CompetencyComponent, ceterms:CourseComponent, ceterms:CredentialComponent, ceterms:ExtracurricularComponent, ceterms:JobComponent, ceterms:WorkExperienceComponent ;
	schema:rangeIncludes xsd:anyURI .

ceterms:spatialCoverage a rdf:Property ;
	rdfs:label "Spatial Coverage"@en-US ;
	rdfs:comment "Spatial coverage of an entity indicates the place(s) to which its content applies or in which it occurres."@en-US ;
	dct:description "In the CTDL, the ceterms:spatialCoverage property serves as a super-property for an array of sub-properties defining location-dependent or area-dependent aspects of a resource."@en-US ;
	vs:term_status vs:stable ;
	meta:changeHistory <http://credreg.net/ctdl/termhistory/ceterms/spatialCoverage/json> ;
	schema:rangeIncludes ceterms:GeoCoordinates, ceterms:JurisdictionProfile, ceterms:Place, ceterms:PostalAddress ;
	owl:equivalentProperty schema:spatialCoverage .

ceterms:startDate a rdf:Property ;
	rdfs:label "Start Date"@en-US ;
	rdfs:comment "Date the validity or usefulness of the information in this resource begins."@en-US ;
	vs:term_status vs:stable ;
	meta:changeHistory <http://credreg.net/ctdl/termhistory/ceterms/startDate/json> ;
	rdfs:subPropertyOf ceterms:temporalCoverage ;
	schema:domainIncludes ceterms:AccreditAction, ceterms:AdvancedStandingAction, ceterms:ApproveAction, ceterms:CollectionMember, ceterms:CostManifest, ceterms:CostProfile, ceterms:CredentialingAction, ceterms:OfferAction, ceterms:RecognizeAction, ceterms:RegulateAction, ceterms:RenewAction, ceterms:RevokeAction, ceterms:RightsAction, ceterms:TransferValueProfile, ceterms:WorkforceDemandAction ;
	schema:rangeIncludes xsd:date ;
	owl:equivalentProperty schema:startDate .

ceterms:startTime a rdf:Property ;
	rdfs:label "Start Time"@en-US ;
	rdfs:comment "Start time of an event or activity."@en-US ;
	vs:term_status vs:stable ;
	meta:changeHistory <http://credreg.net/ctdl/termhistory/ceterms/startTime/json> ;
	rdfs:subPropertyOf ceterms:temporalCoverage ;
	schema:rangeIncludes xsd:dateTime ;
	owl:equivalentProperty schema:startTime .

ceterms:streetAddress a rdf:Property ;
	rdfs:label "Street Address"@en-US ;
	rdfs:comment "Street address. e.g. \"1600 Amphitheatre Pkwy\"."@en-US ;
	vs:term_status vs:stable ;
	meta:changeHistory <http://credreg.net/ctdl/termhistory/ceterms/streetAddress/json> ;
	schema:domainIncludes ceterms:Place, ceterms:PostalAddress ;
	schema:rangeIncludes rdf:langString ;
	owl:equivalentProperty schema:streetAddress .

ceterms:subject a rdf:Property ;
	rdfs:label "Subject"@en-US ;
	rdfs:comment "Words or brief phrases describing the topicality of the entity; select subject terms from an existing enumeration of such terms."@en-US ;
	vann:usageNote "Use the subject property to reference a concept in a controlled vocabulary. Free text subjects should use the keyword property."@en-US ;
	vs:term_status vs:stable ;
	meta:changeHistory <http://credreg.net/ctdl/termhistory/ceterms/subject/json> ;
	rdfs:subPropertyOf schema:about ;
	schema:domainIncludes ceterms:ApprenticeshipCertificate, ceterms:AssessmentProfile, ceterms:AssociateDegree, ceterms:BachelorDegree, ceterms:Badge, ceterms:Certificate, ceterms:CertificateOfCompletion, ceterms:Certification, ceterms:Collection, ceterms:Course, ceterms:Credential, ceterms:Degree, ceterms:DigitalBadge, ceterms:Diploma, ceterms:DoctoralDegree, ceterms:GeneralEducationDevelopment, ceterms:JourneymanCertificate, ceterms:LearningOpportunityProfile, ceterms:LearningProgram, ceterms:License, ceterms:MasterCertificate, ceterms:MasterDegree, ceterms:MicroCredential, ceterms:OpenBadge, ceterms:Pathway, ceterms:ProfessionalDoctorate, ceterms:QualityAssuranceCredential, ceterms:ResearchDoctorate, ceterms:SecondarySchoolDiploma, ceterms:TransferIntermediary, ceterms:ValueProfile ;
	schema:rangeIncludes ceterms:CredentialAlignmentObject .

ceterms:subjectWebpage a rdf:Property ;
	rdfs:label "Subject Webpage"@en-US ;
	rdfs:comment "Webpage that describes this entity."@en-US ;
	dct:description "The web page being referenced describes the entity. The value of subjectWebpage is an authoritative location for information about the subject but should not assumed to be a persistent identifier of the subject."@en-US ;
	vs:term_status vs:stable ;
	meta:changeHistory <http://credreg.net/ctdl/termhistory/ceterms/subjectWebpage/json> ;
	schema:domainIncludes ceterms:ApprenticeshipCertificate, ceterms:AssessmentComponent, ceterms:AssessmentProfile, ceterms:AssociateDegree, ceterms:BachelorDegree, ceterms:Badge, ceterms:BasicComponent, ceterms:Certificate, ceterms:CertificateOfCompletion, ceterms:Certification, ceterms:CocurricularComponent, ceterms:Collection, ceterms:CompetencyComponent, ceterms:ConditionManifest, ceterms:ConditionProfile, ceterms:Course, ceterms:CourseComponent, ceterms:Credential, ceterms:CredentialComponent, ceterms:CredentialOrganization, ceterms:Degree, ceterms:DigitalBadge, ceterms:Diploma, ceterms:DoctoralDegree, ceterms:ExtracurricularComponent, ceterms:FinancialAssistanceProfile, ceterms:GeneralEducationDevelopment, ceterms:Job, ceterms:JobComponent, ceterms:JourneymanCertificate, ceterms:LearningOpportunityProfile, ceterms:LearningProgram, ceterms:License, ceterms:MasterCertificate, ceterms:MasterDegree, ceterms:MicroCredential, ceterms:Occupation, ceterms:OpenBadge, ceterms:Organization, ceterms:Pathway, ceterms:PathwaySet, ceterms:ProcessProfile, ceterms:ProfessionalDoctorate, ceterms:QACredentialOrganization, ceterms:QualityAssuranceCredential, ceterms:ResearchDoctorate, ceterms:ScheduledOffering, ceterms:SecondarySchoolDiploma, ceterms:TransferIntermediary, ceterms:TransferValueProfile, ceterms:VerificationServiceProfile, ceterms:WorkExperienceComponent ;
	schema:rangeIncludes xsd:anyURI ;
	owl:equivalentProperty schema:mainEntityOfPage .

ceterms:submissionOf a rdf:Property ;
	rdfs:label "Submission Of"@en-US ;
	rdfs:comment "Artifact to be submitted such as a transcript, portfolio, or an affidavit."@en-US ;
	vs:term_status vs:stable ;
	meta:changeHistory <http://credreg.net/ctdl/termhistory/ceterms/submissionOf/json> ;
	schema:domainIncludes ceterms:ConditionProfile ;
	schema:rangeIncludes xsd:anyURI .

ceterms:submissionOfDescription a rdf:Property ;
	rdfs:label "Submission Of Description"@en-US ;
	rdfs:comment "Name, label, or description of an artifact to be submitted such as a transcript, portfolio, or an affidavit."@en-US ;
	vs:term_status vs:stable ;
	meta:changeHistory <http://credreg.net/ctdl/termhistory/ceterms/submissionOfDescription/json> ;
	schema:domainIncludes ceterms:ConditionProfile ;
	schema:rangeIncludes rdf:langString .

ceterms:subOrganization a rdf:Property ;
	rdfs:label "Sub-Organization"@en-US ;
	rdfs:comment "Organization in a subordinate or lower position than a parent organization."@en-US ;
	vs:term_status vs:stable ;
	meta:changeHistory <http://credreg.net/ctdl/termhistory/ceterms/subOrganization/json> ;
	schema:domainIncludes ceterms:CredentialOrganization, ceterms:Organization, ceterms:QACredentialOrganization ;
	schema:rangeIncludes ceterms:CredentialOrganization, ceterms:Organization, ceterms:QACredentialOrganization ;
	owl:equivalentProperty schema:subOrganization .

ceterms:supersededBy a rdf:Property ;
	rdfs:label "Superseded By"@en-US ;
	rdfs:comment "Resource that replaces this resource."@en-US ;
	dct:description "For example, a credential that outright replaces the credential being described, and is not simply a newer version of the same credential (the two credentials have different CTIDs)."@en-US ;
	vs:term_status vs:stable ;
	meta:changeHistory <http://credreg.net/ctdl/termhistory/ceterms/supersededBy/json> ;
	schema:domainIncludes ceterms:ApprenticeshipCertificate, ceterms:AssessmentProfile, ceterms:AssociateDegree, ceterms:BachelorDegree, ceterms:Badge, ceterms:Certificate, ceterms:CertificateOfCompletion, ceterms:Certification, ceterms:Course, ceterms:Credential, ceterms:CredentialOrganization, ceterms:Degree, ceterms:DigitalBadge, ceterms:Diploma, ceterms:DoctoralDegree, ceterms:GeneralEducationDevelopment, ceterms:JourneymanCertificate, ceterms:LearningOpportunityProfile, ceterms:LearningProgram, ceterms:License, ceterms:MasterCertificate, ceterms:MasterDegree, ceterms:MicroCredential, ceterms:OpenBadge, ceterms:Organization, ceterms:ProfessionalDoctorate, ceterms:QACredentialOrganization, ceterms:QualityAssuranceCredential, ceterms:ResearchDoctorate, ceterms:SecondarySchoolDiploma, ceterms:TransferValueProfile ;
	schema:rangeIncludes ceterms:ApprenticeshipCertificate, ceterms:AssessmentProfile, ceterms:AssociateDegree, ceterms:BachelorDegree, ceterms:Badge, ceterms:Certificate, ceterms:CertificateOfCompletion, ceterms:Certification, ceterms:Course, ceterms:Credential, ceterms:CredentialOrganization, ceterms:Degree, ceterms:DigitalBadge, ceterms:Diploma, ceterms:DoctoralDegree, ceterms:GeneralEducationDevelopment, ceterms:JourneymanCertificate, ceterms:LearningOpportunityProfile, ceterms:LearningProgram, ceterms:License, ceterms:MasterCertificate, ceterms:MasterDegree, ceterms:MicroCredential, ceterms:OpenBadge, ceterms:Organization, ceterms:ProfessionalDoctorate, ceterms:QACredentialOrganization, ceterms:QualityAssuranceCredential, ceterms:ResearchDoctorate, ceterms:SecondarySchoolDiploma, ceterms:TransferValueProfile .

ceterms:supersedes a rdf:Property ;
	rdfs:label "Supersedes"@en-US ;
	rdfs:comment "Resource that this resource replaces."@en-US ;
	dct:description "For example, the credential that is outright replaced by the credential being described, and is not simply an older version of the same credential (the two credentials have different CTIDs)."@en-US ;
	vs:term_status vs:stable ;
	meta:changeHistory <http://credreg.net/ctdl/termhistory/ceterms/supersedes/json> ;
	schema:domainIncludes ceterms:ApprenticeshipCertificate, ceterms:AssessmentProfile, ceterms:AssociateDegree, ceterms:BachelorDegree, ceterms:Badge, ceterms:Certificate, ceterms:CertificateOfCompletion, ceterms:Certification, ceterms:Course, ceterms:Credential, ceterms:CredentialOrganization, ceterms:Degree, ceterms:DigitalBadge, ceterms:Diploma, ceterms:DoctoralDegree, ceterms:GeneralEducationDevelopment, ceterms:JourneymanCertificate, ceterms:LearningOpportunityProfile, ceterms:LearningProgram, ceterms:License, ceterms:MasterCertificate, ceterms:MasterDegree, ceterms:MicroCredential, ceterms:OpenBadge, ceterms:Organization, ceterms:ProfessionalDoctorate, ceterms:QACredentialOrganization, ceterms:QualityAssuranceCredential, ceterms:ResearchDoctorate, ceterms:SecondarySchoolDiploma, ceterms:TransferValueProfile ;
	schema:rangeIncludes ceterms:ApprenticeshipCertificate, ceterms:AssessmentProfile, ceterms:AssociateDegree, ceterms:BachelorDegree, ceterms:Badge, ceterms:Certificate, ceterms:CertificateOfCompletion, ceterms:Certification, ceterms:Course, ceterms:Credential, ceterms:CredentialOrganization, ceterms:Degree, ceterms:DigitalBadge, ceterms:Diploma, ceterms:DoctoralDegree, ceterms:GeneralEducationDevelopment, ceterms:JourneymanCertificate, ceterms:LearningOpportunityProfile, ceterms:LearningProgram, ceterms:License, ceterms:MasterCertificate, ceterms:MasterDegree, ceterms:MicroCredential, ceterms:OpenBadge, ceterms:Organization, ceterms:ProfessionalDoctorate, ceterms:QACredentialOrganization, ceterms:QualityAssuranceCredential, ceterms:ResearchDoctorate, ceterms:SecondarySchoolDiploma, ceterms:TransferValueProfile .

ceterms:targetAssessment a rdf:Property ;
	rdfs:label "Target Assessment"@en-US ;
	rdfs:comment "Assessment that provides direct, indirect, formative or summative evaluation or estimation of the nature, ability, or quality for an entity."@en-US ;
	vs:term_status vs:stable ;
	meta:changeHistory <http://credreg.net/ctdl/termhistory/ceterms/targetAssessment/json> ;
	schema:domainIncludes ceterms:AssessmentProfile, ceterms:ConditionProfile, ceterms:Course, ceterms:LearningOpportunityProfile, ceterms:LearningProgram, ceterms:ProcessProfile ;
	schema:rangeIncludes ceterms:Assessment, ceterms:AssessmentProfile .

ceterms:targetCompetency a rdf:Property ;
	rdfs:label "Target Competency"@en-US ;
	rdfs:comment "A competency relevant to the condition being described."@en-US ;
	vs:term_status vs:stable ;
	meta:changeHistory <http://credreg.net/ctdl/termhistory/ceterms/targetCompetency/json> ;
	rdfs:subPropertyOf ceterms:credentialAlignment ;
	schema:domainIncludes ceterms:ConditionProfile ;
	schema:rangeIncludes ceasn:Competency, ceterms:CredentialAlignmentObject .

ceterms:targetCompetencyFramework a rdf:Property ;
	rdfs:label "Target Competency Framework"@en-US ;
	rdfs:comment "Competency framework relevant to the process being described."@en-US ;
	vs:term_status vs:stable ;
	meta:changeHistory <http://credreg.net/ctdl/termhistory/ceterms/targetCompetencyFramework/json> ;
	rdfs:subPropertyOf ceterms:credentialAlignment ;
	schema:domainIncludes ceterms:ProcessProfile ;
	schema:rangeIncludes ceasn:CompetencyFramework, ceterms:CredentialAlignmentObject .

ceterms:targetComponent a rdf:Property ;
	rdfs:label "Target Component"@en-US ;
	rdfs:comment "Candidate PathwayComponent for the ComponentCondition."@en-US ;
	vs:term_status vs:stable ;
	meta:changeHistory <http://credreg.net/ctdl/termhistory/ceterms/targetComponent/json> ;
	schema:domainIncludes ceterms:ComponentCondition ;
	schema:rangeIncludes ceterms:AssessmentComponent, ceterms:BasicComponent, ceterms:CocurricularComponent, ceterms:CompetencyComponent, ceterms:CourseComponent, ceterms:CredentialComponent, ceterms:ExtracurricularComponent, ceterms:JobComponent, ceterms:WorkExperienceComponent .

ceterms:targetContactPoint a rdf:Property ;
	rdfs:label "Target Contact Point"@en-US ;
	rdfs:comment "Options for contacting the organization or person."@en-US ;
	vs:term_status vs:stable ;
	meta:changeHistory <http://credreg.net/ctdl/termhistory/ceterms/targetContactPoint/json> ;
	schema:domainIncludes ceterms:CredentialPerson, ceterms:Place ;
	schema:rangeIncludes ceterms:ContactPoint ;
	owl:equivalentProperty schema:contactPoint .

ceterms:targetCredential a rdf:Property ;
	rdfs:label "Target Credential"@en-US ;
	rdfs:comment "Credential that is a focus or target of the condition, process or verification service."@en-US ;
	vs:term_status vs:stable ;
	meta:changeHistory <http://credreg.net/ctdl/termhistory/ceterms/targetCredential/json> ;
	schema:domainIncludes ceterms:ConditionProfile, ceterms:ProcessProfile, ceterms:VerificationServiceProfile ;
	schema:rangeIncludes ceterms:ApprenticeshipCertificate, ceterms:AssociateDegree, ceterms:BachelorDegree, ceterms:Badge, ceterms:Certificate, ceterms:CertificateOfCompletion, ceterms:Certification, ceterms:Credential, ceterms:Degree, ceterms:DigitalBadge, ceterms:Diploma, ceterms:DoctoralDegree, ceterms:GeneralEducationDevelopment, ceterms:JourneymanCertificate, ceterms:License, ceterms:MasterCertificate, ceterms:MasterDegree, ceterms:MicroCredential, ceterms:OpenBadge, ceterms:ProfessionalDoctorate, ceterms:QualityAssuranceCredential, ceterms:ResearchDoctorate, ceterms:SecondarySchoolDiploma .

ceterms:targetLearningOpportunity a rdf:Property ;
	rdfs:label "Target Learning Opportunity"@en-US ;
	rdfs:comment "Learning opportunity that is the focus of a condition, process or another learning opportunity."@en-US ;
	vs:term_status vs:stable ;
	meta:changeHistory <http://credreg.net/ctdl/termhistory/ceterms/targetLearningOpportunity/json> ;
	schema:domainIncludes ceterms:ConditionProfile, ceterms:Course, ceterms:LearningOpportunityProfile, ceterms:LearningProgram, ceterms:ProcessProfile ;
	schema:rangeIncludes ceterms:Course, ceterms:LearningOpportunity, ceterms:LearningOpportunityProfile, ceterms:LearningProgram .

ceterms:targetLearningResource a rdf:Property ;
	rdfs:label "Target Learning Resource"@en-US ;
	rdfs:comment "Learning object or resource that is used as part of an learning activity."@en-US ;
	dct:description "Examples include a textbook or lesson plan that describes or records the educational activity (e.g. an audio- or video-recording of a lesson)."@en-US ;
	vs:term_status vs:stable ;
	meta:changeHistory <http://credreg.net/ctdl/termhistory/ceterms/targetLearningResource/json> ;
	schema:domainIncludes ceterms:AssessmentProfile, ceterms:Course, ceterms:LearningOpportunityProfile, ceterms:LearningProgram ;
	schema:rangeIncludes ceterms:LearningResource .

ceterms:targetNode a rdf:Property ;
	rdfs:label "Target Node"@en-US ;
	rdfs:comment "Individual entry in a formally defined framework such as a competency or an industry, instructional program, or occupation code."@en-US ;
	dct:description "The target node returned must be the exact competency or concept being described and no other competency or concept. References to data or a document that returns all of the competencies or concepts in the framework to which the target node belongs should use the ceterms:framework property."@en-US ;
	vs:term_status vs:stable ;
	meta:changeHistory <http://credreg.net/ctdl/termhistory/ceterms/targetNode/json> ;
	schema:domainIncludes ceterms:CredentialAlignmentObject, ceterms:FinancialAlignmentObject ;
	schema:rangeIncludes xsd:anyURI ;
	owl:equivalentProperty lrmi:targetUrl, schema:targetUrl .

ceterms:targetNodeDescription a rdf:Property ;
	rdfs:label "Target Description"@en-US ;
	rdfs:comment "Textual description of an individual concept or competency in a formally defined framework."@en-US ;
	vs:term_status vs:stable ;
	meta:changeHistory <http://credreg.net/ctdl/termhistory/ceterms/targetNodeDescription/json> ;
	schema:domainIncludes ceterms:CredentialAlignmentObject, ceterms:FinancialAlignmentObject ;
	schema:rangeIncludes rdf:langString ;
	owl:equivalentProperty lrmi:targetDescription, schema:targetDescription .

ceterms:targetNodeName a rdf:Property ;
	rdfs:label "Target Node Name"@en-US ;
	rdfs:comment "Name of an individual concept or competency in a formally defined framework."@en-US ;
	vs:term_status vs:stable ;
	meta:changeHistory <http://credreg.net/ctdl/termhistory/ceterms/targetNodeName/json> ;
	schema:domainIncludes ceterms:CredentialAlignmentObject, ceterms:FinancialAlignmentObject ;
	schema:rangeIncludes rdf:langString ;
	owl:equivalentProperty lrmi:targetName, schema:targetName .

ceterms:targetPathway a rdf:Property ;
	rdfs:label "Target Pathway"@en-US ;
	rdfs:comment "Pathway in which this resource is a potential component."@en-US ;
	vs:term_status vs:stable ;
	meta:changeHistory <http://credreg.net/ctdl/termhistory/ceterms/targetPathway/json> ;
	schema:domainIncludes ceterms:ApprenticeshipCertificate, ceterms:AssessmentProfile, ceterms:AssociateDegree, ceterms:BachelorDegree, ceterms:Badge, ceterms:Certificate, ceterms:CertificateOfCompletion, ceterms:Certification, ceterms:Course, ceterms:Credential, ceterms:Degree, ceterms:DigitalBadge, ceterms:Diploma, ceterms:DoctoralDegree, ceterms:GeneralEducationDevelopment, ceterms:JourneymanCertificate, ceterms:LearningOpportunityProfile, ceterms:LearningProgram, ceterms:License, ceterms:MasterCertificate, ceterms:MasterDegree, ceterms:MicroCredential, ceterms:OpenBadge, ceterms:ProfessionalDoctorate, ceterms:QualityAssuranceCredential, ceterms:ResearchDoctorate, ceterms:SecondarySchoolDiploma ;
	schema:rangeIncludes ceterms:Pathway .

ceterms:teaches a rdf:Property ;
	rdfs:label "Teaches"@en-US ;
	rdfs:comment "Competency that the learning opportunity is intended to teach."@en-US ;
	vs:term_status vs:stable ;
	meta:changeHistory <http://credreg.net/ctdl/termhistory/ceterms/teaches/json> ;
	rdfs:subPropertyOf ceterms:targetCompetency ;
	schema:domainIncludes ceterms:Course, ceterms:LearningOpportunityProfile, ceterms:LearningProgram ;
	schema:rangeIncludes ceasn:Competency, ceterms:CredentialAlignmentObject .

ceterms:telephone a rdf:Property ;
	rdfs:label "Telephone"@en-US ;
	rdfs:comment "Telephone number."@en-US ;
	vs:term_status vs:stable ;
	meta:changeHistory <http://credreg.net/ctdl/termhistory/ceterms/telephone/json> ;
	schema:domainIncludes ceterms:ContactPoint ;
	schema:rangeIncludes xsd:string ;
	owl:equivalentProperty schema:telephone .

ceterms:temporalCoverage a rdf:Property ;
	rdfs:label "Temporal Coverage"@en-US ;
	rdfs:comment "Indicates the time period to which the entity's content applies or during which it occurres."@en-US ;
	dct:description "In the CTDL, the ceterms:temporalCoverage property serves as a super-property for an array of sub-properties defining time-dependent aspects of a resource."@en-US ;
	vs:term_status vs:stable ;
	meta:changeHistory <http://credreg.net/ctdl/termhistory/ceterms/temporalCoverage/json> ;
	schema:rangeIncludes xsd:date ;
	owl:equivalentProperty schema:temporalCoverage .

ceterms:transferValue a rdf:Property ;
	rdfs:label "Transfer Value"@en-US ;
	rdfs:comment "An explicit amount of transfer value."@en-US ;
	vs:term_status vs:stable ;
	meta:changeHistory <http://credreg.net/ctdl/termhistory/ceterms/transferValue/json> ;
	schema:domainIncludes ceterms:TransferValueProfile ;
	schema:rangeIncludes ceterms:ValueProfile .

ceterms:transferValueFor a rdf:Property ;
	rdfs:label "Transfer Value For"@en-US ;
	rdfs:comment "Resource for which the described transfer value is applicable."@en-US ;
	dct:description "When this property references multiple resources, those resources should be treated as a set for which, collectively, the transfer value is applicable."@en-US ;
	vs:term_status vs:stable ;
	meta:changeHistory <http://credreg.net/ctdl/termhistory/ceterms/transferValueFor/json> ;
	schema:domainIncludes ceterms:TransferValueProfile ;
	schema:rangeIncludes ceasn:Competency, ceterms:ApprenticeshipCertificate, ceterms:AssessmentProfile, ceterms:AssociateDegree, ceterms:BachelorDegree, ceterms:Badge, ceterms:Certificate, ceterms:CertificateOfCompletion, ceterms:Certification, ceterms:Course, ceterms:Credential, ceterms:Degree, ceterms:DigitalBadge, ceterms:Diploma, ceterms:DoctoralDegree, ceterms:GeneralEducationDevelopment, ceterms:Job, ceterms:JourneymanCertificate, ceterms:LearningOpportunityProfile, ceterms:LearningProgram, ceterms:License, ceterms:MasterCertificate, ceterms:MasterDegree, ceterms:MicroCredential, ceterms:Occupation, ceterms:OpenBadge, ceterms:ProfessionalDoctorate, ceterms:QualityAssuranceCredential, ceterms:ResearchDoctorate, ceterms:SecondarySchoolDiploma .

ceterms:transferValueFrom a rdf:Property ;
	rdfs:label "Transfer Value From"@en-US ;
	rdfs:comment "Resource from which the described transfer value originates."@en-US ;
	dct:description "When this property references multiple resources, those resources should be treated as a set from which, collectively, the transfer value originates."@en-US ;
	vs:term_status vs:stable ;
	meta:changeHistory <http://credreg.net/ctdl/termhistory/ceterms/transferValueFrom/json> ;
	schema:domainIncludes ceterms:TransferValueProfile ;
	schema:rangeIncludes ceasn:Competency, ceterms:ApprenticeshipCertificate, ceterms:AssessmentProfile, ceterms:AssociateDegree, ceterms:BachelorDegree, ceterms:Badge, ceterms:Certificate, ceterms:CertificateOfCompletion, ceterms:Certification, ceterms:Course, ceterms:Credential, ceterms:Degree, ceterms:DigitalBadge, ceterms:Diploma, ceterms:DoctoralDegree, ceterms:GeneralEducationDevelopment, ceterms:Job, ceterms:JourneymanCertificate, ceterms:LearningOpportunityProfile, ceterms:LearningProgram, ceterms:License, ceterms:MasterCertificate, ceterms:MasterDegree, ceterms:MicroCredential, ceterms:Occupation, ceterms:OpenBadge, ceterms:ProfessionalDoctorate, ceterms:QualityAssuranceCredential, ceterms:ResearchDoctorate, ceterms:SecondarySchoolDiploma .

ceterms:transferValueStatement a rdf:Property ;
	rdfs:label "Transfer Value Statement"@en-US ;
	rdfs:comment "Webpage or online document that defines or explains the nature of transfer value handled by the organization."@en-US ;
	vs:term_status vs:stable ;
	meta:changeHistory <http://credreg.net/ctdl/termhistory/ceterms/transferValueStatement/json> ;
	schema:domainIncludes ceterms:CredentialOrganization, ceterms:Organization, ceterms:QACredentialOrganization ;
	schema:rangeIncludes xsd:anyURI .

ceterms:transferValueStatementDescription a rdf:Property ;
	rdfs:label "Transfer Value Statement Description"@en-US ;
	rdfs:comment "Description of the nature of transfer value handled by the organization."@en-US ;
	vs:term_status vs:stable ;
	meta:changeHistory <http://credreg.net/ctdl/termhistory/ceterms/transferValueStatementDescription/json> ;
	schema:domainIncludes ceterms:CredentialOrganization, ceterms:Organization, ceterms:QACredentialOrganization ;
	schema:rangeIncludes rdf:langString .

ceterms:verificationDirectory a rdf:Property ;
	rdfs:label "Verification Directory"@en-US ;
	rdfs:comment "Directory of credential holders and their current statuses."@en-US ;
	vs:term_status vs:stable ;
	meta:changeHistory <http://credreg.net/ctdl/termhistory/ceterms/verificationDirectory/json> ;
	schema:domainIncludes ceterms:VerificationServiceProfile ;
	schema:rangeIncludes xsd:anyURI .

ceterms:verificationMethodDescription a rdf:Property ;
	rdfs:label "Verification Method Description"@en-US ;
	rdfs:comment "Textual description of the methods used to evaluate an assessment, learning opportunity, process or verificaiton service for validity or reliability."@en-US ;
	vs:term_status vs:stable ;
	meta:changeHistory <http://credreg.net/ctdl/termhistory/ceterms/verificationMethodDescription/json> ;
	schema:domainIncludes ceterms:ProcessProfile, ceterms:VerificationServiceProfile ;
	schema:rangeIncludes rdf:langString .

ceterms:verificationService a rdf:Property ;
	rdfs:label "Verification Service URL"@en-US ;
	rdfs:comment "Direct access to the verification service."@en-US ;
	dct:description "This property identifies machine-accessible services, such as API endpoints, that provide direct access to the verification service being described."@en-US ;
	vann:usageNote "For general webpages describing the service, use the subjectWebpage property."@en-US ;
	vs:term_status vs:stable ;
	meta:changeHistory <http://credreg.net/ctdl/termhistory/ceterms/verificationService/json> ;
	schema:domainIncludes ceterms:VerificationServiceProfile ;
	schema:rangeIncludes xsd:anyURI .

ceterms:verifiedClaimType a rdf:Property ;
	rdfs:label "Verified Claim Type"@en-US ;
	rdfs:comment "Type of claim provided through a verification service; select from an existing enumeration of such types."@en-US ;
	vann:usageNote "Best practice for developing credential descriptions for the Credential Engine Registry is to use the ceterms:ClaimType vocabulary."@en-US ;
	vs:term_status vs:stable ;
	meta:changeHistory <http://credreg.net/ctdl/termhistory/ceterms/verifiedClaimType/json> ;
	schema:domainIncludes ceterms:VerificationServiceProfile ;
	schema:rangeIncludes ceterms:CredentialAlignmentObject ;
	meta:targetScheme ceterms:ClaimType .

ceterms:versionIdentifier a rdf:Property ;
	rdfs:label "Version Identifier"@en-US ;
	rdfs:comment "Alphanumeric identifier of the version of the credential that is unique within the organizational context of its owner."@en-US ;
	dct:description "The credential version captured here is any local identifier used by the credential owner to identify the version of the credential in the its local system."@en-US ;
	vann:usageNote "Locally unique identifiers are acceptable; however, globally unique URI or GUID/UUID are preferred."@en-US ;
	vs:term_status vs:stable ;
	meta:changeHistory <http://credreg.net/ctdl/termhistory/ceterms/versionIdentifier/json> ;
	schema:domainIncludes ceterms:ApprenticeshipCertificate, ceterms:AssessmentProfile, ceterms:AssociateDegree, ceterms:BachelorDegree, ceterms:Badge, ceterms:Certificate, ceterms:CertificateOfCompletion, ceterms:Certification, ceterms:Course, ceterms:Credential, ceterms:Degree, ceterms:DigitalBadge, ceterms:Diploma, ceterms:DoctoralDegree, ceterms:GeneralEducationDevelopment, ceterms:Job, ceterms:JourneymanCertificate, ceterms:LearningOpportunityProfile, ceterms:LearningProgram, ceterms:License, ceterms:MasterCertificate, ceterms:MasterDegree, ceterms:MicroCredential, ceterms:Occupation, ceterms:OpenBadge, ceterms:ProfessionalDoctorate, ceterms:QualityAssuranceCredential, ceterms:ResearchDoctorate, ceterms:SecondarySchoolDiploma, ceterms:Task, ceterms:WorkRole ;
	schema:rangeIncludes ceterms:IdentifierValue .

ceterms:weight a rdf:Property ;
	rdfs:label "Weight"@en-US ;
	rdfs:comment "Measurement of the weight, degree, percent, or strength of a recommendation, requirement, or comparison."@en-US ;
	vann:usageNote "Best practice is to assign a decimal value weight between 0 and 1 that indicates the strength of the assertion, with 0 being weakest and 1 being strongest."@en-US ;
	vs:term_status vs:stable ;
	meta:changeHistory <http://credreg.net/ctdl/termhistory/ceterms/weight/json> ;
	schema:domainIncludes ceterms:ConditionProfile, ceterms:CredentialAlignmentObject, ceterms:FinancialAlignmentObject ;
	schema:rangeIncludes xsd:float .

ceterms:worksFor a rdf:Property ;
	rdfs:label "Works For"@en-US ;
	rdfs:comment "Person's place of employment."@en-US ;
	vs:term_status vs:stable ;
	meta:changeHistory <http://credreg.net/ctdl/termhistory/ceterms/worksFor/json> ;
	schema:domainIncludes ceterms:CredentialPerson ;
	schema:rangeIncludes ceterms:CredentialOrganization, ceterms:Organization, ceterms:QACredentialOrganization ;
	owl:equivalentProperty schema:worksFor .

ceterms:yearsOfExperience a rdf:Property ;
	rdfs:label "Years of Experience"@en-US ;
	rdfs:comment "Years of relevant experience."@en-US ;
	vann:usageNote "Non-integer year values may be expressed as point value, for example, 0.25, 1.5, etc."@en-US ;
	vs:term_status vs:stable ;
	meta:changeHistory <http://credreg.net/ctdl/termhistory/ceterms/yearsOfExperience/json> ;
	schema:domainIncludes ceterms:ConditionProfile ;
	schema:rangeIncludes xsd:float .

owl:sameAs a rdf:Property ;
	rdfs:label "Same As"@en-US ;
	rdfs:comment "Links an individual to an individual; such an owl:sameAs statement indicates that two URI references actually refer to the same thing: the individuals have the same \"identity\"."@en-US ;
	vs:term_status vs:unstable ;
	meta:changeHistory <http://credreg.net/ctdl/termhistory/owl/sameAs/json> ;
	schema:domainIncludes rdfs:Resource ;
	schema:rangeIncludes rdfs:Resource .

qdata:dataCollectionMethodType a rdf:Property ;
	rdfs:label "Data Collection Method Type"@en-US ;
	rdfs:comment "Type of method by which the data was collected."@en-US ;
	vs:term_status vs:stable ;
	meta:changeHistory <http://credreg.net/ctdl/termhistory/qdata/dataCollectionMethodType/json> ;
	schema:domainIncludes ceterms:ProcessProfile ;
	schema:rangeIncludes skos:Concept ;
	meta:targetScheme qdata:CollectionMethod .

qdata:dataProvider a rdf:Property ;
	rdfs:label "Data Provider"@en-US ;
	rdfs:comment "Credentialing organization or a third party providing the data."@en-US ;
	vs:term_status vs:stable ;
	meta:changeHistory <http://credreg.net/ctdl/termhistory/qdata/dataProvider/json> ;
	schema:domainIncludes qdata:DataSetProfile ;
	schema:rangeIncludes ceterms:Agent .

qdata:percentage a rdf:Property ;
	rdfs:label "Percentage"@en-US ;
	rdfs:comment "Quotient of two values of the data set, expressed as a percentage."@en-US ;
	vann:usageNote "Best practice is to treat the value of this property as a verbatim percentage; for example, a value of 1.5 should be interpreted as 1.5%"@en-US ;
	vs:term_status vs:stable ;
	meta:changeHistory <http://credreg.net/ctdl/termhistory/qdata/percentage/json> ;
	schema:domainIncludes ceterms:ValueProfile, schema:QuantitativeValue ;
	schema:rangeIncludes xsd:float .

qdata:relevantDataSet a rdf:Property ;
	rdfs:label "Relevant Data Set"@en-US ;
	rdfs:comment "Data Set on which earnings or employment data is based."@en-US ;
	vs:term_status vs:stable ;
	meta:changeHistory <http://credreg.net/ctdl/termhistory/qdata/relevantDataSet/json> ;
	schema:domainIncludes ceterms:AggregateDataProfile, ceterms:EarningsProfile, ceterms:EmploymentOutcomeProfile, ceterms:HoldersProfile ;
	schema:rangeIncludes qdata:DataSetProfile .

schema:description a rdf:Property ;
	rdfs:label "Description"@en-US ;
	rdfs:comment "A description of the item."@en-US ;
	vs:term_status vs:stable ;
	meta:changeHistory <http://credreg.net/ctdl/termhistory/schema/description/json> ;
	schema:domainIncludes ceterms:ValueProfile, schema:QuantitativeValue ;
	schema:rangeIncludes rdf:langString .

schema:maxValue a rdf:Property ;
	rdfs:label "Maximum Value"@en-US ;
	rdfs:comment "The upper value of some characteristic or property."@en-US ;
	vann:usageNote "For single values, use schema:value. For ranges, use schema:minValue and schema:maxValue."@en-US ;
	vs:term_status vs:stable ;
	meta:changeHistory <http://credreg.net/ctdl/termhistory/schema/maxValue/json> ;
	schema:domainIncludes ceterms:ValueProfile, schema:QuantitativeValue ;
	schema:rangeIncludes xsd:float .

schema:minValue a rdf:Property ;
	rdfs:label "Minimum Value"@en-US ;
	rdfs:comment "The lower value of some characteristic or property."@en-US ;
	vann:usageNote "For single values, use schema:value. For ranges, use schema:minValue and schema:maxValue."@en-US ;
	vs:term_status vs:stable ;
	meta:changeHistory <http://credreg.net/ctdl/termhistory/schema/minValue/json> ;
	schema:domainIncludes ceterms:ValueProfile, schema:QuantitativeValue ;
	schema:rangeIncludes xsd:float .

schema:unitText a rdf:Property ;
	rdfs:label "Unit Text"@en-US ;
	rdfs:comment "A string or text indicating the unit of measurement."@en-US ;
	vs:term_status vs:stable ;
	meta:changeHistory <http://credreg.net/ctdl/termhistory/schema/unitText/json> ;
	schema:domainIncludes schema:QuantitativeValue ;
	schema:rangeIncludes ceterms:CredentialAlignmentObject .

schema:value a rdf:Property ;
	rdfs:label "Value"@en-US ;
	rdfs:comment "The value of the property value node."@en-US ;
	vann:usageNote "For single values, use schema:value. For ranges, use schema:minValue and schema:maxValue."@en-US ;
	vs:term_status vs:stable ;
	meta:changeHistory <http://credreg.net/ctdl/termhistory/schema/value/json> ;
	schema:domainIncludes ceterms:ValueProfile, schema:QuantitativeValue ;
	schema:rangeIncludes xsd:float .

#====================
# CONCEPT SCHEMES
#====================
ceterms:ActionStatus a skos:ConceptScheme ;
	rdfs:label "Action Status"@en-US ;
	rdfs:comment "Types of current status of an action."@en-US ;
	dct:description "Available statuses include ActiveActionStatus, CompletedActionStatus, FailedActionStatus, PotentialActionStatus."@en-US ;
	vs:term_status vs:stable ;
	meta:changeHistory <http://credreg.net/ctdl/termhistory/ceterms/ActionStatus/json> ;
	owl:equivalentClass schema:ActionStatus ;
	meta:hasConcept actionStat:ActiveActionStatus, actionStat:CompletedActionStatus, actionStat:FailedActionStatus, actionStat:PotentialActionStatus .

ceterms:AgentSector a skos:ConceptScheme ;
	rdfs:label "Agent Sector"@en-US ;
	rdfs:comment "Types of sociological, economic, or political subdivision of society."@en-US ;
	dct:description "Sectors include public, private for profit, public for profit, and business industry association."@en-US ;
	vs:term_status vs:stable ;
	meta:changeHistory <http://credreg.net/ctdl/termhistory/ceterms/AgentSector/json> ;
	meta:hasConcept agentSector:PrivateForProfit, agentSector:PrivateNonProfit, agentSector:Public .

ceterms:AgentServiceType a skos:ConceptScheme ;
	rdfs:label "Agent Service Type"@en-US ;
	rdfs:comment "Types of services offered by an agent."@en-US ;
	vs:term_status vs:stable ;
	meta:changeHistory <http://credreg.net/ctdl/termhistory/ceterms/AgentServiceType/json> ;
	meta:hasConcept serviceType:AccreditService, serviceType:ApproveService, serviceType:OfferService, serviceType:RecognizeService, serviceType:RegulateService, serviceType:RenewService, serviceType:RevokeService .

ceterms:ArrayOperationCategory a skos:ConceptScheme ;
	rdfs:label "Array Operation Category"@en-US ;
	rdfs:comment "Concepts describing an action to be taken on an array of values."@en-US ;
	vann:usageNote "Used in CTDL for actions performed on arrays, lists or sets or values in order to obtain some other value."@en-US ;
	vs:term_status vs:unstable ;
	meta:changeHistory <http://credreg.net/ctdl/termhistory/ceterms/ArrayOperationCategory/json> ;
	meta:hasConcept array:AllOf, array:AnyOf, array:CountDistinct, array:Max, array:Mean, array:Min, array:OneOf, array:Sum .

ceterms:AssessmentMethod a skos:ConceptScheme ;
	rdfs:label "Assessment Method"@en-US ;
	rdfs:comment "Types of assessment method."@en-US ;
	vs:term_status vs:stable ;
	meta:changeHistory <http://credreg.net/ctdl/termhistory/ceterms/AssessmentMethod/json> ;
	meta:hasConcept assessMethod:Artifact, assessMethod:Exam, assessMethod:Performance .

ceterms:AssessmentUse a skos:ConceptScheme ;
	rdfs:label "Assessment Use"@en-US ;
	rdfs:comment "Types of Intended uses of an assessment."@en-US ;
	vs:term_status vs:stable ;
	meta:changeHistory <http://credreg.net/ctdl/termhistory/ceterms/AssessmentUse/json> ;
	meta:hasConcept assessUse:Formative, assessUse:Summative .

ceterms:Audience a skos:ConceptScheme ;
	rdfs:label "Audience"@en-US ;
	rdfs:comment "Types of audiences for which the resource being described is applicable or available."@en-US ;
	dct:description "If the resource is applicable or available for any type of audience, do not select anything."@en-US ;
	vs:term_status vs:stable ;
	meta:changeHistory <http://credreg.net/ctdl/termhistory/ceterms/Audience/json> ;
	meta:hasConcept audience:Citizen, audience:CurrentMilitary, audience:CurrentMilitaryDependent, audience:CurrentMilitarySpouse, audience:CurrentStudent, audience:FormerMilitary, audience:FormerMilitaryDependent, audience:FormerMilitarySpouse, audience:FormerStudent, audience:FullTime, audience:Member, audience:NonCitizen, audience:NonMember, audience:NonResident, audience:PartTime, audience:PrivateEmployee, audience:PublicEmployee, audience:Resident .

ceterms:AudienceLevel a skos:ConceptScheme ;
	rdfs:label "Audience Level"@en-US ;
	rdfs:comment "Types of levels in an academic or training progression expected of, or to be developed by, the typical person for the resource being described."@en-US ;
	vs:term_status vs:stable ;
	meta:changeHistory <http://credreg.net/ctdl/termhistory/ceterms/AudienceLevel/json> ;
	meta:hasConcept audLevel:AdvancedLevel, audLevel:AssociatesDegreeLevel, audLevel:BachelorsDegreeLevel, audLevel:BeginnerLevel, audLevel:DoctoralDegreeLevel, audLevel:GraduateLevel, audLevel:IntermediateLevel, audLevel:LowerDivisionLevel, audLevel:MastersDegreeLevel, audLevel:PostSecondaryLevel, audLevel:ProfessionalLevel, audLevel:RemedialLevel, audLevel:SecondaryLevel, audLevel:UndergraduateLevel, audLevel:UpperDivisionLevel .

ceterms:ClaimType a skos:ConceptScheme ;
	rdfs:label "Claim Type"@en-US ;
	rdfs:comment "Types of the claims supported by a verification service."@en-US ;
	vs:term_status vs:stable ;
	meta:changeHistory <http://credreg.net/ctdl/termhistory/ceterms/ClaimType/json> ;
	meta:hasConcept claimType:BadgeClaim, claimType:QualityAssuranceClaim, claimType:TranscriptClaim, claimType:Verifiedclaim, claimType:VerifiedClaim .

ceterms:CollectionCategory a skos:ConceptScheme ;
	rdfs:label "Collection Category"@en-US ;
	rdfs:comment "Types of collection, list, or array that groups together other resources."@en-US ;
	vs:term_status vs:unstable ;
	meta:changeHistory <http://credreg.net/ctdl/termhistory/ceterms/CollectionCategory/json> ;
	meta:hasConcept collectionCategory:ETPL, collectionCategory:GIBill, collectionCategory:IndustryRecognized, collectionCategory:Perkins, collectionCategory:PromiseScholarship, collectionCategory:Quality, collectionCategory:StateApprovedPostsecondary .

ceterms:ComparatorCategory a skos:ConceptScheme ;
	rdfs:label "Comparator Category"@en-US ;
	rdfs:comment "Concepts for comparing two values."@en-US ;
	vann:usageNote "Used in CTDL constraints as values of the ceterms:comparator property to make a comparison that should yield true or false. In all cases the left source of data is compared to the right source, sometimes the comparison is made after an action is applied, e.g. finding the mean of several numbers."@en-US ;
	vs:term_status vs:unstable ;
	meta:changeHistory <http://credreg.net/ctdl/termhistory/ceterms/ComparatorCategory/json> ;
	meta:hasConcept compare:EQ, compare:GT, compare:GTEQ, compare:LT, compare:LTEQ, compare:NEQ .

ceterms:CostType a skos:ConceptScheme ;
	rdfs:label "Cost Type"@en-US ;
	rdfs:comment "Entity that describes the types of costs related to earning or completing a credential, assessment, or learning opportunity."@en-US ;
	dct:description "Attainment costs do not include living (e.g., room and board) or travel expenses."@en-US ;
	vs:term_status vs:stable ;
	meta:changeHistory <http://credreg.net/ctdl/termhistory/ceterms/CostType/json> ;
	meta:hasConcept costType:AggregateCost, costType:Application, costType:BackgroundCheck, costType:EnrollmentFee, costType:GraduationFee, costType:LearningResource, costType:Meals, costType:MixedFees, costType:OptionalCharges, costType:ProcessingFee, costType:ProgramSpecificFee, costType:ReexaminationFee, costType:RenewalFee, costType:ReschedulingFee, costType:RoomOrResidency, costType:ScoringFee, costType:StandaloneAssessment, costType:StudentServicesFee, costType:TechnologyFee, costType:Tuition .

ceterms:CredentialStatus a skos:ConceptScheme ;
	rdfs:label "Credential Status"@en-US ;
	rdfs:comment "Types of applicability statuses of a credential."@en-US ;
	vs:term_status vs:stable ;
	meta:changeHistory <http://credreg.net/ctdl/termhistory/ceterms/CredentialStatus/json> ;
	meta:hasConcept credentialStat:Active, credentialStat:Deprecated, credentialStat:Probationary, credentialStat:Superseded, credentialStat:Suspended, credentialStat:TeachOut .

ceterms:CreditUnit a skos:ConceptScheme ;
	rdfs:label "Credit Unit"@en-US ;
	rdfs:comment "Broad descriptions of units used to measure credit associated with a resource."@en-US ;
	vs:term_status vs:stable ;
	meta:changeHistory <http://credreg.net/ctdl/termhistory/ceterms/CreditUnit/json> ;
	meta:hasConcept creditUnit:AcademicYear, creditUnit:CarnegieUnit, creditUnit:CertificateCredit, creditUnit:ClockHour, creditUnit:CompetencyCredit, creditUnit:ContactHour, creditUnit:ContinuingEducationUnit, creditUnit:DegreeCredit, creditUnit:DualCredit, creditUnit:QuarterHour, creditUnit:RequirementCredit, creditUnit:SecondaryDiplomaCredit, creditUnit:SemesterHour, creditUnit:TimeBasedCredit, creditUnit:TypeBasedCredit .

ceterms:Delivery a skos:ConceptScheme ;
	rdfs:label "Delivery Type"@en-US ;
	rdfs:comment "Types of technical form for providing instances of the entity."@en-US ;
	vs:term_status vs:stable ;
	meta:changeHistory <http://credreg.net/ctdl/termhistory/ceterms/Delivery/json> ;
	meta:hasConcept deliveryType:BlendedDelivery, deliveryType:InPerson, deliveryType:OnlineOnly .

ceterms:ExternalInput a skos:ConceptScheme ;
	rdfs:label "External Input"@en-US ;
	rdfs:comment "Types of external stakeholders that provide input to the process."@en-US ;
	vs:term_status vs:stable ;
	meta:changeHistory <http://credreg.net/ctdl/termhistory/ceterms/ExternalInput/json> ;
	meta:hasConcept inputType:Associations, inputType:Business, inputType:BusinessAssociation, inputType:Consumers, inputType:EducationAdministrators, inputType:Educators, inputType:Experts, inputType:Governments, inputType:Guardians, inputType:InternationalBodies, inputType:Practitioners, inputType:Public, inputType:Students .

ceterms:FinancialAssistance a skos:ConceptScheme ;
	rdfs:label "Financial Assistance"@en-US ;
	rdfs:comment "Types of financial assistance typically available in the United States."@en-US ;
	vs:term_status vs:stable ;
	meta:changeHistory <http://credreg.net/ctdl/termhistory/ceterms/FinancialAssistance/json> ;
	meta:hasConcept financialAid:AcademicAssistantship, financialAid:Apprenticeship, financialAid:CoOperative, financialAid:DoDTuitionAssistance, financialAid:FederalGrant, financialAid:FederalScholarship, financialAid:FederalSubsidizedLoan, financialAid:FederalUnsubsidizedLoan, financialAid:FederalWorkStudy, financialAid:General, financialAid:Grant, financialAid:InstitutionalGrant, financialAid:InstitutionalLoan, financialAid:InstitutionalScholarship, financialAid:Internship, financialAid:Loan, financialAid:LoanForgivenessProgram, financialAid:Military, financialAid:OtherGrant, financialAid:OtherLoan, financialAid:OtherOnCampusWork, financialAid:OtherScholarship, financialAid:ParentPLUSLoan, financialAid:PellGrant, financialAid:Post911GIBill, financialAid:PrivateGrant, financialAid:PrivateLoan, financialAid:PrivateScholarship, financialAid:PromiseProgram, financialAid:Scholarship, financialAid:StateLocalGrant, financialAid:StateLocalLoan, financialAid:StateLocalMilitaryAssistance, financialAid:StateLocalScholarship, financialAid:StateLocalWork, financialAid:VEAP, financialAid:VocationalRehabilitation, financialAid:WIOA, financialAid:WorkBased .

ceterms:LearningMethod a skos:ConceptScheme ;
	rdfs:label "Learning Method"@en-US ;
	rdfs:comment "Types of methods used to conduct the learning opportunity."@en-US ;
	vs:term_status vs:stable ;
	meta:changeHistory <http://credreg.net/ctdl/termhistory/ceterms/LearningMethod/json> ;
	meta:hasConcept learnMethod:Applied, learnMethod:ElectronicMediaBased, learnMethod:Gaming, learnMethod:Laboratory, learnMethod:Lecture, learnMethod:Prerecorded, learnMethod:SelfPaced, learnMethod:Seminar, learnMethod:WorkBased .

ceterms:LifeCycleStatus a skos:ConceptScheme ;
	rdfs:label "Life Cycle Status"@en-US ;
	rdfs:comment "Types of states of a resource in terms of its stage in a life cycle."@en-US ;
	vs:term_status vs:unstable ;
	meta:changeHistory <http://credreg.net/ctdl/termhistory/ceterms/LifeCycleStatus/json> ;
	meta:hasConcept lifeCycle:Active, lifeCycle:Ceased, lifeCycle:Ceasing, lifeCycle:Developing, lifeCycle:Suspended, lifeCycle:TeachOut .

ceterms:LogicalOperatorCategory a skos:ConceptScheme ;
	rdfs:label "Logical Operator Category"@en-US ;
	rdfs:comment "Logical operators applicable to two or more items."@en-US ;
	vann:usageNote "Used in CTDL for types of logical operator for combining two or more nested ComponentCondition entities, Constraint entities, or a mix of ComponentCondition and Constraint entities."@en-US ;
	vs:term_status vs:unstable ;
	meta:changeHistory <http://credreg.net/ctdl/termhistory/ceterms/LogicalOperatorCategory/json> ;
	meta:hasConcept logic:And, logic:OnlyOne, logic:Or .

ceterms:OrganizationType a skos:ConceptScheme ;
	rdfs:label "Organization Type"@en-US ;
	rdfs:comment "Types of organization."@en-US ;
	vs:term_status vs:stable ;
	meta:changeHistory <http://credreg.net/ctdl/termhistory/ceterms/OrganizationType/json> ;
	meta:hasConcept orgType:AssessmentBody, orgType:Business, orgType:BusinessAssociation, orgType:CertificationBody, orgType:Collaborative, orgType:CoordinatingBody, orgType:FourYear, orgType:Government, orgType:HighSchool, orgType:LaborUnion, orgType:Magnet, orgType:Military, orgType:NonTraditional, orgType:Postsecondary, orgType:PrimarilyOnline, orgType:ProfessionalAssociation, orgType:QualityAssurance, orgType:SecondarySchool, orgType:Technical, orgType:TrainingProvider, orgType:TwoYear, orgType:Vendor .

ceterms:Residency a skos:ConceptScheme ;
	rdfs:label "Residency"@en-US ;
	rdfs:comment "Types of residency."@en-US ;
	vs:term_status vs:stable ;
	meta:changeHistory <http://credreg.net/ctdl/termhistory/ceterms/Residency/json> ;
	meta:hasConcept residency:InState, residency:International, residency:Local, residency:OutOfState, residency:Regional .

ceterms:ScheduleFrequency a skos:ConceptScheme ;
	rdfs:label "Schedule Frequency"@en-US ;
	rdfs:comment "Types for how often events occur."@en-US ;
	vs:term_status vs:unstable ;
	meta:changeHistory <http://credreg.net/ctdl/termhistory/ceterms/ScheduleFrequency/json> ;
	meta:hasConcept scheduleFrequency:Annually, scheduleFrequency:BiMonthly, scheduleFrequency:EventBased, scheduleFrequency:Irregular, scheduleFrequency:Monthly, scheduleFrequency:MultiplePerWeek, scheduleFrequency:OnDemand, scheduleFrequency:OpenEntryExit, scheduleFrequency:Quarterly, scheduleFrequency:SelfPaced, scheduleFrequency:SemiAnnually, scheduleFrequency:SingleInstance, scheduleFrequency:Weekly .

ceterms:ScheduleTiming a skos:ConceptScheme ;
	rdfs:label "Schedule Timing"@en-US ;
	rdfs:comment "Types for when (in time) events occur."@en-US ;
	vs:term_status vs:unstable ;
	meta:changeHistory <http://credreg.net/ctdl/termhistory/ceterms/ScheduleTiming/json> ;
	meta:hasConcept scheduleTiming:Daytime, scheduleTiming:Evening, scheduleTiming:Weekdays, scheduleTiming:Weekends .

ceterms:ScoringMethod a skos:ConceptScheme ;
	rdfs:label "Scoring Method"@en-US ;
	rdfs:comment "Types of applicable scoring."@en-US ;
	vs:term_status vs:stable ;
	meta:changeHistory <http://credreg.net/ctdl/termhistory/ceterms/ScoringMethod/json> ;
	meta:hasConcept score:CriterionReferenced, score:NormReferenced .

#====================
# CONCEPTS
#====================
actionStat:ActiveActionStatus a skos:Concept ;
	skos:prefLabel "Active Action Status"@en-US ;
	skos:definition "Action that is ongoing."@en-US ;
	dct:description "Examples include: while watching the movie, or driving to a location"@en-US ;
	vs:term_status vs:stable ;
	meta:changeHistory <http://credreg.net/ctdl/termhistory/actionStat/ActiveActionStatus/json> .

actionStat:CompletedActionStatus a skos:Concept ;
	skos:prefLabel "Completed Action Status"@en-US ;
	skos:definition "Action that has already taken place."@en-US ;
	vs:term_status vs:stable ;
	meta:changeHistory <http://credreg.net/ctdl/termhistory/actionStat/CompletedActionStatus/json> .

actionStat:FailedActionStatus a skos:Concept ;
	skos:prefLabel "Failed Action Status"@en-US ;
	skos:definition "Action that failed to complete."@en-US ;
	dct:description "The action's error property and the HTTP return code contain more information about the failure."@en-US ;
	vs:term_status vs:stable ;
	meta:changeHistory <http://credreg.net/ctdl/termhistory/actionStat/FailedActionStatus/json> .

actionStat:PotentialActionStatus a skos:Concept ;
	skos:prefLabel "Potential Action Status"@en-US ;
	skos:definition "Description of an action that is supported."@en-US ;
	vs:term_status vs:stable ;
	meta:changeHistory <http://credreg.net/ctdl/termhistory/actionStat/PotentialActionStatus/json> .

agentSector:PrivateForProfit a skos:Concept ;
	skos:prefLabel "Private For-Profit"@en-US ;
	skos:definition "Sector that contains privately-owned organizations that operate for profit."@en-US ;
	vs:term_status vs:stable ;
	meta:changeHistory <http://credreg.net/ctdl/termhistory/agentSector/PrivateForProfit/json> .

agentSector:PrivateNonProfit a skos:Concept ;
	skos:prefLabel "Private Not-For-Profit"@en-US ;
	skos:definition "Sector that contains privately-owned organizations that operate on a non-profit basis."@en-US ;
	dct:description "These include both independent not-for-profit schools and those affiliated with a religious organization."@en-US ;
	vs:term_status vs:stable ;
	meta:changeHistory <http://credreg.net/ctdl/termhistory/agentSector/PrivateNonProfit/json> .

agentSector:Public a skos:Concept ;
	skos:prefLabel "Public"@en-US ;
	skos:definition "Sector that contains government and quasi-government organizations."@en-US ;
	vs:term_status vs:stable ;
	meta:changeHistory <http://credreg.net/ctdl/termhistory/agentSector/Public/json> .

array:AllOf a skos:Concept ;
	skos:prefLabel "All Of"@en-US ;
	skos:definition "All of the values."@en-US ;
	vs:term_status vs:unstable ;
	meta:changeHistory <http://credreg.net/ctdl/termhistory/array/AllOf/json> .

array:AnyOf a skos:Concept ;
	skos:prefLabel "Any Of"@en-US ;
	skos:definition "Any (one or more) of the values."@en-US ;
	vs:term_status vs:unstable ;
	meta:changeHistory <http://credreg.net/ctdl/termhistory/array/AnyOf/json> .

array:CountDistinct a skos:Concept ;
	skos:prefLabel "Count Distinct"@en-US ;
	skos:definition "The number of unique values; yields a number."@en-US ;
	vs:term_status vs:unstable ;
	meta:changeHistory <http://credreg.net/ctdl/termhistory/array/CountDistinct/json> .

array:Max a skos:Concept ;
	skos:prefLabel "Maximum"@en-US ;
	skos:definition "The highest of all the values."@en-US ;
	vs:term_status vs:unstable ;
	meta:changeHistory <http://credreg.net/ctdl/termhistory/array/Max/json> .

array:Mean a skos:Concept ;
	skos:prefLabel "Mean"@en-US ;
	skos:definition "The arithmetic mean of all the values."@en-US ;
	vs:term_status vs:unstable ;
	meta:changeHistory <http://credreg.net/ctdl/termhistory/array/Mean/json> .

array:Min a skos:Concept ;
	skos:prefLabel "Minimum"@en-US ;
	skos:definition "The lowest of all the values."@en-US ;
	vs:term_status vs:unstable ;
	meta:changeHistory <http://credreg.net/ctdl/termhistory/array/Min/json> .

array:OneOf a skos:Concept ;
	skos:prefLabel "One Of"@en-US ;
	skos:definition "Any one (but no more) of the values."@en-US ;
	vs:term_status vs:unstable ;
	meta:changeHistory <http://credreg.net/ctdl/termhistory/array/OneOf/json> .

array:Sum a skos:Concept ;
	skos:prefLabel "Sum"@en-US ;
	skos:definition "The numeric total obtained by adding all the values."@en-US ;
	vs:term_status vs:unstable ;
	meta:changeHistory <http://credreg.net/ctdl/termhistory/array/Sum/json> .

assessMethod:Artifact a skos:Concept ;
	skos:prefLabel "Artifact"@en-US ;
	skos:definition "Work or product created or produced by the person being assessed."@en-US ;
	dct:description "Artifact includes, but is not limited to, an academic paper, video documentary, computer software, music composition, choreography, novel, short story, journal article, news article, report, lesson plan, product design, portfolio, manufactured product, etc. Methods of evaluation may include multiple evaluators either individually or as an expert panel using general criteria or more structured rubrics whose scores are combined, etc. Criteria and methods of evaluation are often very similar to those for assessing a performance, without the facets specific to a live performance"@en-US ;
	vs:term_status vs:stable ;
	meta:changeHistory <http://credreg.net/ctdl/termhistory/assessMethod/Artifact/json> .

assessMethod:Exam a skos:Concept ;
	skos:prefLabel "Exam"@en-US ;
	skos:definition "Mix of scored items presented in fixed or open response formats including qualifying and comprehensive exams."@en-US ;
	dct:description "Exam includes, but is not limited to, multiple choice, true-false, written essay, short-answer, fill-in or oral response formats that could include measurements of reasoning, problem-solving, critical thinking."@en-US ;
	vs:term_status vs:stable ;
	meta:changeHistory <http://credreg.net/ctdl/termhistory/assessMethod/Exam/json> .

assessMethod:Performance a skos:Concept ;
	skos:prefLabel "Performance"@en-US ;
	skos:definition "Set of behaviors or actions assessed as demonstration of competencies where the assessment occurs either as the actions take place (i.e., live) or through review of recordings of those actions in a persistent media (e.g., video, audio, keystroke records, etc.)"@en-US ;
	dct:description "Performance includes, but is not limited to, dance, music, teaching, acting, medical procedures, truck driving, manufacturing production, etc. Criteria include the categories and benchmarks on which the performance is assessed. Methods of evaluation can include multiple evaluators either individually or as an expert panel using general criteria or more structured rubrics whose scores are combined (e.g., assessing a dance performance, evaluating the performance of a medical procedure, truck driving procedure, manufacturing process such as machining)."@en-US ;
	vs:term_status vs:stable ;
	meta:changeHistory <http://credreg.net/ctdl/termhistory/assessMethod/Performance/json> .

assessUse:Formative a skos:Concept ;
	skos:prefLabel "Formative Assessment"@en-US ;
	skos:definition "Formal and informal assessment procedures conducted during the learning process to support intentional modification in teaching and learning activities in order to improve learner attainment."@en-US ;
	vs:term_status vs:stable ;
	meta:changeHistory <http://credreg.net/ctdl/termhistory/assessUse/Formative/json> .

assessUse:Summative a skos:Concept ;
	skos:prefLabel "Summative Assessment"@en-US ;
	skos:definition "Assessment of learning at the end of an instructional unit to determine whether some established standard or benchmark has been achieved."@en-US ;
	vs:term_status vs:stable ;
	meta:changeHistory <http://credreg.net/ctdl/termhistory/assessUse/Summative/json> .

audience:Citizen a skos:Concept ;
	skos:prefLabel "Citizen"@en-US ;
	skos:definition "Person who is a legally recognized subject of a particular nation, state, province, or commonwealth."@en-US ;
	vs:term_status vs:stable ;
	meta:changeHistory <http://credreg.net/ctdl/termhistory/audience/Citizen/json> .

audience:CurrentMilitary a skos:Concept ;
	skos:prefLabel "Current Military"@en-US ;
	skos:definition "Current member of a nation's military."@en-US ;
	vs:term_status vs:stable ;
	meta:changeHistory <http://credreg.net/ctdl/termhistory/audience/CurrentMilitary/json> .

audience:CurrentMilitaryDependent a skos:Concept ;
	skos:prefLabel "Current Military Dependent"@en-US ;
	skos:definition "Dependent (usually a child) of a current member of a nation's military."@en-US ;
	vs:term_status vs:stable ;
	meta:changeHistory <http://credreg.net/ctdl/termhistory/audience/CurrentMilitaryDependent/json> .

audience:CurrentMilitarySpouse a skos:Concept ;
	skos:prefLabel "Current Military Spouse"@en-US ;
	skos:definition "Spouse of a current member of a nation's military."@en-US ;
	vs:term_status vs:stable ;
	meta:changeHistory <http://credreg.net/ctdl/termhistory/audience/CurrentMilitarySpouse/json> .

audience:CurrentStudent a skos:Concept ;
	skos:prefLabel "Current Student"@en-US ;
	skos:definition "Student currently participating in a learning opportunity."@en-US ;
	vs:term_status vs:stable ;
	meta:changeHistory <http://credreg.net/ctdl/termhistory/audience/CurrentStudent/json> .

audience:FormerMilitary a skos:Concept ;
	skos:prefLabel "Former Military / Veteran"@en-US ;
	skos:definition "Veteran of military service."@en-US ;
	vs:term_status vs:stable ;
	meta:changeHistory <http://credreg.net/ctdl/termhistory/audience/FormerMilitary/json> .

audience:FormerMilitaryDependent a skos:Concept ;
	skos:prefLabel "Former Military Dependent"@en-US ;
	skos:definition "Former dependent (usually a child) of a veteran of a nation's military."@en-US ;
	vs:term_status vs:stable ;
	meta:changeHistory <http://credreg.net/ctdl/termhistory/audience/FormerMilitaryDependent/json> .

audience:FormerMilitarySpouse a skos:Concept ;
	skos:prefLabel "Former Military Spouse"@en-US ;
	skos:definition "Spouse of a veteran of a nation's military."@en-US ;
	vs:term_status vs:stable ;
	meta:changeHistory <http://credreg.net/ctdl/termhistory/audience/FormerMilitarySpouse/json> .

audience:FormerStudent a skos:Concept ;
	skos:prefLabel "Former Student / Alumni"@en-US ;
	skos:definition "Student who previously participated in a learning opportunity."@en-US ;
	vs:term_status vs:stable ;
	meta:changeHistory <http://credreg.net/ctdl/termhistory/audience/FormerStudent/json> .

audience:FullTime a skos:Concept ;
	skos:prefLabel "Full-Time"@en-US ;
	skos:definition "Participation in a learning opportunity to an extent that meets the opportunity's requirements for full-time status."@en-US ;
	vs:term_status vs:stable ;
	meta:changeHistory <http://credreg.net/ctdl/termhistory/audience/FullTime/json> .

audience:Member a skos:Concept ;
	skos:prefLabel "Member"@en-US ;
	skos:definition "Member of an organization, society, or recognized group."@en-US ;
	vs:term_status vs:stable ;
	meta:changeHistory <http://credreg.net/ctdl/termhistory/audience/Member/json> .

audience:NonCitizen a skos:Concept ;
	skos:prefLabel "Non-Citizen"@en-US ;
	skos:definition "Person who is not a legally recognized subject of a particular nation, state, province, or commonwealth."@en-US ;
	vs:term_status vs:stable ;
	meta:changeHistory <http://credreg.net/ctdl/termhistory/audience/NonCitizen/json> .

audience:NonMember a skos:Concept ;
	skos:prefLabel "Non-Member"@en-US ;
	skos:definition "Individual without membership status or privileges conferred by an organization, society, or recognized group."@en-US ;
	vs:term_status vs:stable ;
	meta:changeHistory <http://credreg.net/ctdl/termhistory/audience/NonMember/json> .

audience:NonResident a skos:Concept ;
	skos:prefLabel "Non-Resident"@en-US ;
	skos:definition "Person whose primary residence is not in nation, state, province, or commonwealth of concern."@en-US ;
	vs:term_status vs:stable ;
	meta:changeHistory <http://credreg.net/ctdl/termhistory/audience/NonResident/json> .

audience:PartTime a skos:Concept ;
	skos:prefLabel "Part-Time"@en-US ;
	skos:definition "Participation in a learning opportunity to an extent that meets the opportunity's requirements for part-time status."@en-US ;
	vs:term_status vs:stable ;
	meta:changeHistory <http://credreg.net/ctdl/termhistory/audience/PartTime/json> .

audience:PrivateEmployee a skos:Concept ;
	skos:prefLabel "Private Employee"@en-US ;
	skos:definition "Person employed in the private sector."@en-US ;
	vs:term_status vs:stable ;
	meta:changeHistory <http://credreg.net/ctdl/termhistory/audience/PrivateEmployee/json> .

audience:PublicEmployee a skos:Concept ;
	skos:prefLabel "Public Employee"@en-US ;
	skos:definition "Person employed in the public sector."@en-US ;
	vs:term_status vs:stable ;
	meta:changeHistory <http://credreg.net/ctdl/termhistory/audience/PublicEmployee/json> .

audience:Resident a skos:Concept ;
	skos:prefLabel "Resident"@en-US ;
	skos:definition "Person whose permanent and principal home is in a particular nation, state, province, or commonwealth."@en-US ;
	vs:term_status vs:stable ;
	meta:changeHistory <http://credreg.net/ctdl/termhistory/audience/Resident/json> .

audLevel:AdvancedLevel a skos:Concept ;
	skos:prefLabel "Advanced Level"@en-US ;
	skos:definition "Intended for those with significant experience or expertise where developmental expectations are staged for assessing knowledge, skills, or competencies beyond the novice and intermediate levels."@en-US ;
	vs:term_status vs:stable ;
	meta:changeHistory <http://credreg.net/ctdl/termhistory/audLevel/AdvancedLevel/json> .

audLevel:AssociatesDegreeLevel a skos:Concept ;
	skos:prefLabel "Associates Degree Level"@en-US ;
	skos:definition "Intended for those completing college/university-level programs within their first one to two years (lower-division) of post-secondary education."@en-US ;
	vs:term_status vs:stable ;
	meta:changeHistory <http://credreg.net/ctdl/termhistory/audLevel/AssociatesDegreeLevel/json> ;
	skos:broader audLevel:PostSecondaryLevel .

audLevel:BachelorsDegreeLevel a skos:Concept ;
	skos:prefLabel "Bachelors Degree Level"@en-US ;
	skos:definition "Intended for those completing college/university-level programs within approximately three to four years where course work and activities advance skills from a lower-division or generalist level to an upper-division level."@en-US ;
	vs:term_status vs:stable ;
	meta:changeHistory <http://credreg.net/ctdl/termhistory/audLevel/BachelorsDegreeLevel/json> ;
	skos:broader audLevel:PostSecondaryLevel .

audLevel:BeginnerLevel a skos:Concept ;
	skos:prefLabel "Beginner Level"@en-US ;
	skos:definition "Intended for novices or those with limited experience."@en-US ;
	vs:term_status vs:stable ;
	meta:changeHistory <http://credreg.net/ctdl/termhistory/audLevel/BeginnerLevel/json> .

audLevel:DoctoralDegreeLevel a skos:Concept ;
	skos:prefLabel "Doctoral Degree Level"@en-US ;
	skos:definition "Intended for those who have completed Bachelors and Masters degrees or their equivalent and who will be required to complete either independent research or a significant project or paper."@en-US ;
	vs:term_status vs:stable ;
	meta:changeHistory <http://credreg.net/ctdl/termhistory/audLevel/DoctoralDegreeLevel/json> ;
	skos:broader audLevel:PostSecondaryLevel .

audLevel:GraduateLevel a skos:Concept ;
	skos:prefLabel "Graduate Level"@en-US ;
	skos:definition "Intended for those who enrolled in a degree program or other formal program above the baccalaureate level, such as a masters or doctoral degree program."@en-US ;
	vs:term_status vs:stable ;
	meta:changeHistory <http://credreg.net/ctdl/termhistory/audLevel/GraduateLevel/json> .

audLevel:IntermediateLevel a skos:Concept ;
	skos:prefLabel "Intermediate Level"@en-US ;
	skos:definition "Intended for those with some experience, where knowledge, skills, and competency expectations are staged for development beyond novice-level and in preparation for a more advanced-level."@en-US ;
	dct:description "An individual at this level has foundational competencies to function independently with occasional supervision."@en-US ;
	vs:term_status vs:stable ;
	meta:changeHistory <http://credreg.net/ctdl/termhistory/audLevel/IntermediateLevel/json> .

audLevel:LowerDivisionLevel a skos:Concept ;
	skos:prefLabel "Lower Division Level"@en-US ;
	skos:definition "Intended for those in the first half of an undergraduate level program."@en-US ;
	vs:term_status vs:stable ;
	meta:changeHistory <http://credreg.net/ctdl/termhistory/audLevel/LowerDivisionLevel/json> .

audLevel:MastersDegreeLevel a skos:Concept ;
	skos:prefLabel "Masters Degree Level"@en-US ;
	skos:definition "Intended for those who have completed a Bachelor's Degree or equivalent."@en-US ;
	vs:term_status vs:stable ;
	meta:changeHistory <http://credreg.net/ctdl/termhistory/audLevel/MastersDegreeLevel/json> ;
	skos:broader audLevel:PostSecondaryLevel .

audLevel:PostSecondaryLevel a skos:Concept ;
	skos:prefLabel "Post-Secondary Level"@en-US ;
	skos:definition "Intended for those who have completed secondary level school programs or equivalent."@en-US ;
	vs:term_status vs:stable ;
	meta:changeHistory <http://credreg.net/ctdl/termhistory/audLevel/PostSecondaryLevel/json> ;
	skos:narrower audLevel:AssociatesDegreeLevel, audLevel:BachelorsDegreeLevel, audLevel:DoctoralDegreeLevel, audLevel:MastersDegreeLevel .

audLevel:ProfessionalLevel a skos:Concept ;
	skos:prefLabel "Professional Level"@en-US ;
	skos:definition "Intended for those attending professional programs or equivalent, such as law or medicine."@en-US ;
	dct:description "Other levels can typically be paired with Professional Level to refine a description of a level."@en-US ;
	vs:term_status vs:stable ;
	meta:changeHistory <http://credreg.net/ctdl/termhistory/audLevel/ProfessionalLevel/json> .

audLevel:RemedialLevel a skos:Concept ;
	skos:prefLabel "Remedial Level"@en-US ;
	skos:definition "Intended for those who are under-prepared for learning at a particular level."@en-US ;
	vs:term_status vs:unstable ;
	meta:changeHistory <http://credreg.net/ctdl/termhistory/audLevel/RemedialLevel/json> .

audLevel:SecondaryLevel a skos:Concept ;
	skos:prefLabel "Secondary School or Equivalent"@en-US ;
	skos:definition "Intended for those attending secondary (high-school) level programs."@en-US ;
	vs:term_status vs:stable ;
	meta:changeHistory <http://credreg.net/ctdl/termhistory/audLevel/SecondaryLevel/json> .

audLevel:UndergraduateLevel a skos:Concept ;
	skos:prefLabel "Undergraduate Level"@en-US ;
	skos:definition "Intended for those who are enrolled in a degree program or other formal program at or below the baccalaureate, such as an associateâs degree, vocational, or technical program."@en-US ;
	vs:term_status vs:stable ;
	meta:changeHistory <http://credreg.net/ctdl/termhistory/audLevel/UndergraduateLevel/json> .

audLevel:UpperDivisionLevel a skos:Concept ;
	skos:prefLabel "Upper Division Level"@en-US ;
	skos:definition "Intended for those in the second half of an undergraduate level program."@en-US ;
	vs:term_status vs:stable ;
	meta:changeHistory <http://credreg.net/ctdl/termhistory/audLevel/UpperDivisionLevel/json> .

claimType:BadgeClaim a skos:Concept ;
	skos:prefLabel "Badge Claim"@en-US ;
	skos:definition "Verifiable visual representation that can be shared, embedded, linked, or otherwise used to publicly indicate that an individual has the represented credential."@en-US ;
	vs:term_status vs:stable ;
	meta:changeHistory <http://credreg.net/ctdl/termhistory/claimType/BadgeClaim/json> .

claimType:QualityAssuranceClaim a skos:Concept ;
	skos:prefLabel "Quality Assurance Claim"@en-US ;
	skos:definition "Verifiable representation of quality assurance."@en-US ;
	vs:term_status vs:stable ;
	meta:changeHistory <http://credreg.net/ctdl/termhistory/claimType/QualityAssuranceClaim/json> .

claimType:TranscriptClaim a skos:Concept ;
	skos:prefLabel "Transcript Claim"@en-US ;
	skos:definition "Verifiable representation of postsecondary courses and degrees completed."@en-US ;
	vs:term_status vs:stable ;
	meta:changeHistory <http://credreg.net/ctdl/termhistory/claimType/TranscriptClaim/json> .

claimType:VerifiedClaim a skos:Concept ;
	skos:prefLabel "Verified Claim"@en-US ;
	skos:definition "Verifiable representation of the credential holder's credential."@en-US ;
	vs:term_status vs:stable ;
	meta:changeHistory <http://credreg.net/ctdl/termhistory/claimType/VerifiedClaim/json> .

collectionCategory:ETPL a skos:Concept ;
	skos:prefLabel "Eligible Training Providers List"@en-US ;
	skos:definition "Training providers meeting the requirements stipulated in the U.S. Workforce Innovation and Opportunity Act per the promulgating body."@en-US ;
	dct:description "This list includes the Learning Opportunities and Credentials offered by training providers that have met requirements."@en-US ;
	vs:term_status vs:unstable ;
	meta:changeHistory <http://credreg.net/ctdl/termhistory/collectionCategory/ETPL/json> .

collectionCategory:GIBill a skos:Concept ;
	skos:prefLabel "GI Bill"@en-US ;
	skos:definition "Education and training programs qualifying for the U.S. GI Bill per the promulgating body."@en-US ;
	vs:term_status vs:unstable ;
	meta:changeHistory <http://credreg.net/ctdl/termhistory/collectionCategory/GIBill/json> .

collectionCategory:IndustryRecognized a skos:Concept ;
	skos:prefLabel "Industry Recognized"@en-US ;
	skos:definition "Learning Opportunities, Learning Programs, Courses, Assessments or Credentials recognized in one or more industries based on factors such as job market demand per the promulgating body."@en-US ;
	vs:term_status vs:unstable ;
	meta:changeHistory <http://credreg.net/ctdl/termhistory/collectionCategory/IndustryRecognized/json> .

collectionCategory:Perkins a skos:Concept ;
	skos:prefLabel "Perkins"@en-US ;
	skos:definition "Credentials approved for funding under the U.S. Strengthening Career and Technical Education for the 21st Century Act (Perkins V) per the promulgating body."@en-US ;
	vs:term_status vs:unstable ;
	meta:changeHistory <http://credreg.net/ctdl/termhistory/collectionCategory/Perkins/json> .

collectionCategory:PromiseScholarship a skos:Concept ;
	skos:prefLabel "Promise Scholarship"@en-US ;
	skos:definition "Specified programs in eligible postsecondary educational institutions for which qualified students may receive a Promise Scholarship."@en-US ;
	vs:term_status vs:unstable ;
	meta:changeHistory <http://credreg.net/ctdl/termhistory/collectionCategory/PromiseScholarship/json> .

collectionCategory:Quality a skos:Concept ;
	skos:prefLabel "Quality"@en-US ;
	skos:definition "Learning Opportunities, Learning Programs, Courses, Assessments or Credentials that meet criteria for quality as determined by the promulgating body."@en-US ;
	vs:term_status vs:unstable ;
	meta:changeHistory <http://credreg.net/ctdl/termhistory/collectionCategory/Quality/json> .

collectionCategory:StateApprovedPostsecondary a skos:Concept ;
	skos:prefLabel "State Approved Postsecondary Programs"@en-US ;
	skos:definition "Learning Opportunities, Learning Programs, Courses, Assessments or Credentials approved by a state agency to be offered within that stateâs jurisdiction by postsecondary institutions."@en-US ;
	vs:term_status vs:unstable ;
	meta:changeHistory <http://credreg.net/ctdl/termhistory/collectionCategory/StateApprovedPostsecondary/json> .

compare:EQ a skos:Concept ;
	skos:prefLabel "Equal To"@en-US ;
	skos:definition "The value of the left is equal to the value of the right."@en-US ;
	vs:term_status vs:unstable ;
	meta:changeHistory <http://credreg.net/ctdl/termhistory/compare/EQ/json> ;
	owl:equivalentClass odrl2:eq .

compare:GT a skos:Concept ;
	skos:prefLabel "Greater Than"@en-US ;
	skos:definition "The value of the left is greater than the value of the right."@en-US ;
	vs:term_status vs:unstable ;
	meta:changeHistory <http://credreg.net/ctdl/termhistory/compare/GT/json> ;
	owl:equivalentClass odrl2:gt .

compare:GTEQ a skos:Concept ;
	skos:prefLabel "Greater Than or Equal To"@en-US ;
	skos:definition "The value of the left is greater than or equal to the value of the right."@en-US ;
	vs:term_status vs:unstable ;
	meta:changeHistory <http://credreg.net/ctdl/termhistory/compare/GTEQ/json> ;
	owl:equivalentClass odrl2:gteq .

compare:LT a skos:Concept ;
	skos:prefLabel "Less Than"@en-US ;
	skos:definition "The value of the left is less than the value of the right."@en-US ;
	vs:term_status vs:unstable ;
	meta:changeHistory <http://credreg.net/ctdl/termhistory/compare/LT/json> ;
	owl:equivalentClass odrl2:lt .

compare:LTEQ a skos:Concept ;
	skos:prefLabel "Less Than or Equal To"@en-US ;
	skos:definition "The value of the left is less than or equal to the value of the right."@en-US ;
	vs:term_status vs:unstable ;
	meta:changeHistory <http://credreg.net/ctdl/termhistory/compare/LTEQ/json> ;
	owl:equivalentClass odrl2:lteq .

compare:NEQ a skos:Concept ;
	skos:prefLabel "Not Equal To"@en-US ;
	skos:definition "The value of the left is not equal to the value of the right."@en-US ;
	vs:term_status vs:unstable ;
	meta:changeHistory <http://credreg.net/ctdl/termhistory/compare/NEQ/json> ;
	owl:equivalentClass odrl2:neq .

costType:AggregateCost a skos:Concept ;
	skos:prefLabel "Aggregate Cost"@en-US ;
	skos:definition "Sum of direct costs."@en-US ;
	vs:term_status vs:stable ;
	meta:changeHistory <http://credreg.net/ctdl/termhistory/costType/AggregateCost/json> .

costType:Application a skos:Concept ;
	skos:prefLabel "Application"@en-US ;
	skos:definition "Cost of applying for the resource being described."@en-US ;
	vs:term_status vs:stable ;
	meta:changeHistory <http://credreg.net/ctdl/termhistory/costType/Application/json> .

costType:BackgroundCheck a skos:Concept ;
	skos:prefLabel "Background Check"@en-US ;
	skos:definition "Cost for a background check."@en-US ;
	vs:term_status vs:stable ;
	meta:changeHistory <http://credreg.net/ctdl/termhistory/costType/BackgroundCheck/json> .

costType:EnrollmentFee a skos:Concept ;
	skos:prefLabel "Enrollment Fee"@en-US ;
	skos:definition "Cost to enroll in the learning opportunity being described."@en-US ;
	vs:term_status vs:stable ;
	meta:changeHistory <http://credreg.net/ctdl/termhistory/costType/EnrollmentFee/json> .

costType:GraduationFee a skos:Concept ;
	skos:prefLabel "Graduation Fee"@en-US ;
	skos:definition "Separate graduation fee."@en-US ;
	vs:term_status vs:stable ;
	meta:changeHistory <http://credreg.net/ctdl/termhistory/costType/GraduationFee/json> .

costType:LearningResource a skos:Concept ;
	skos:prefLabel "Learning Resource"@en-US ;
	skos:definition "Cost for one or more learning resources."@en-US ;
	dct:description "Examples include resources such as textbooks, workbooks, laboratory supplies, and other related supplies."@en-US ;
	vs:term_status vs:stable ;
	meta:changeHistory <http://credreg.net/ctdl/termhistory/costType/LearningResource/json> .

costType:Meals a skos:Concept ;
	skos:prefLabel "Meals"@en-US ;
	skos:definition "Cost for meals while participating in the learning opportunity."@en-US ;
	vs:term_status vs:stable ;
	meta:changeHistory <http://credreg.net/ctdl/termhistory/costType/Meals/json> .

costType:MixedFees a skos:Concept ;
	skos:prefLabel "Mixed Fees"@en-US ;
	skos:definition "The sum of fees that are not identified individually."@en-US ;
	vs:term_status vs:stable ;
	meta:changeHistory <http://credreg.net/ctdl/termhistory/costType/MixedFees/json> .

costType:OptionalCharges a skos:Concept ;
	skos:prefLabel "Optional Charges"@en-US ;
	skos:definition "Cost for additional fees, other services, equipment, or facilities that are not required."@en-US ;
	vs:term_status vs:stable ;
	meta:changeHistory <http://credreg.net/ctdl/termhistory/costType/OptionalCharges/json> .

costType:ProcessingFee a skos:Concept ;
	skos:prefLabel "Processing Fee"@en-US ;
	skos:definition "Cost for processing or expediting information related to the resource being described."@en-US ;
	vs:term_status vs:stable ;
	meta:changeHistory <http://credreg.net/ctdl/termhistory/costType/ProcessingFee/json> .

costType:ProgramSpecificFee a skos:Concept ;
	skos:prefLabel "Program Specific Fee"@en-US ;
	skos:definition "Additional cost for participation with a specific program or course of study such as engineering, business, and nursing."@en-US ;
	vs:term_status vs:stable ;
	meta:changeHistory <http://credreg.net/ctdl/termhistory/costType/ProgramSpecificFee/json> .

costType:ReexaminationFee a skos:Concept ;
	skos:prefLabel "Reexamination Fee"@en-US ;
	skos:definition "Cost for retaking an instance of the resource being described."@en-US ;
	vs:term_status vs:stable ;
	meta:changeHistory <http://credreg.net/ctdl/termhistory/costType/ReexaminationFee/json> .

costType:RenewalFee a skos:Concept ;
	skos:prefLabel "Maintenance Fee"@en-US ;
	skos:definition "Cost for maintenance or renewal of the resource being described."@en-US ;
	vs:term_status vs:stable ;
	meta:changeHistory <http://credreg.net/ctdl/termhistory/costType/RenewalFee/json> .

costType:ReschedulingFee a skos:Concept ;
	skos:prefLabel "Rescheduling Fee"@en-US ;
	skos:definition "Cost for rescheduling an instance of the resource being described."@en-US ;
	vs:term_status vs:stable ;
	meta:changeHistory <http://credreg.net/ctdl/termhistory/costType/ReschedulingFee/json> .

costType:RoomOrResidency a skos:Concept ;
	skos:prefLabel "Room or Residence"@en-US ;
	skos:definition "Cost for room, residence or boarding."@en-US ;
	vs:term_status vs:stable ;
	meta:changeHistory <http://credreg.net/ctdl/termhistory/costType/RoomOrResidency/json> .

costType:ScoringFee a skos:Concept ;
	skos:prefLabel "Scoring Fee"@en-US ;
	skos:definition "Cost for scoring the resource being described."@en-US ;
	vs:term_status vs:stable ;
	meta:changeHistory <http://credreg.net/ctdl/termhistory/costType/ScoringFee/json> .

costType:StandaloneAssessment a skos:Concept ;
	skos:prefLabel "Standalone/Extra Assessment"@en-US ;
	skos:definition "Cost for standalone assessments."@en-US ;
	vs:term_status vs:stable ;
	meta:changeHistory <http://credreg.net/ctdl/termhistory/costType/StandaloneAssessment/json> .

costType:StudentServicesFee a skos:Concept ;
	skos:prefLabel "Student Services Fee"@en-US ;
	skos:definition "Cost for student services related to the learning opportunity."@en-US ;
	vs:term_status vs:stable ;
	meta:changeHistory <http://credreg.net/ctdl/termhistory/costType/StudentServicesFee/json> .

costType:TechnologyFee a skos:Concept ;
	skos:prefLabel "Technology Fee"@en-US ;
	skos:definition "Cost for accessing technologies related to the learning opportunity or activity."@en-US ;
	vs:term_status vs:stable ;
	meta:changeHistory <http://credreg.net/ctdl/termhistory/costType/TechnologyFee/json> .

costType:Tuition a skos:Concept ;
	skos:prefLabel "Tuition"@en-US ;
	skos:definition "Cost for teaching and instruction."@en-US ;
	vs:term_status vs:stable ;
	meta:changeHistory <http://credreg.net/ctdl/termhistory/costType/Tuition/json> .

credentialStat:Active a skos:Concept ;
	skos:prefLabel "Active"@en-US ;
	skos:definition "Awards of the credential are ongoing."@en-US ;
	vs:term_status vs:stable ;
	meta:changeHistory <http://credreg.net/ctdl/termhistory/credentialStat/Active/json> .

credentialStat:Deprecated a skos:Concept ;
	skos:prefLabel "Deprecated"@en-US ;
	skos:definition "Awards of the credential have ceased."@en-US ;
	vs:term_status vs:stable ;
	meta:changeHistory <http://credreg.net/ctdl/termhistory/credentialStat/Deprecated/json> .

credentialStat:Probationary a skos:Concept ;
	skos:prefLabel "Probationary"@en-US ;
	skos:definition "Credential award is provisional or temporary; frequently pending further assessment of qualification."@en-US ;
	vs:term_status vs:stable ;
	meta:changeHistory <http://credreg.net/ctdl/termhistory/credentialStat/Probationary/json> .

credentialStat:Suspended a skos:Concept ;
	skos:prefLabel "Suspended"@en-US ;
	skos:definition "Awards of the credential are not available, but may resume."@en-US ;
	vs:term_status vs:stable ;
	meta:changeHistory <http://credreg.net/ctdl/termhistory/credentialStat/Suspended/json> .

credentialStat:TeachOut a skos:Concept ;
	skos:prefLabel "Teach Out"@en-US ;
	skos:definition "Arrangement by which an educational institution provides its current students with the opportunity to complete the credential when the program, institution or location offering access closes."@en-US ;
	vs:term_status vs:unstable ;
	meta:changeHistory <http://credreg.net/ctdl/termhistory/credentialStat/TeachOut/json> .

creditUnit:AcademicYear a skos:Concept ;
	skos:prefLabel "Academic Year"@en-US ;
	skos:definition "Credit that is issued or accepted as being related to one or more academic years."@en-US ;
	vs:term_status vs:stable ;
	meta:changeHistory <http://credreg.net/ctdl/termhistory/creditUnit/AcademicYear/json> ;
	skos:broader creditUnit:TimeBasedCredit .

creditUnit:CarnegieUnit a skos:Concept ;
	skos:prefLabel "Carnegie Unit"@en-US ;
	skos:definition "Credit that is based on 120 hours of contact time or class time with an instructor."@en-US ;
	vs:term_status vs:stable ;
	meta:changeHistory <http://credreg.net/ctdl/termhistory/creditUnit/CarnegieUnit/json> ;
	skos:broader creditUnit:TimeBasedCredit .

creditUnit:CertificateCredit a skos:Concept ;
	skos:prefLabel "Certificate Credit"@en-US ;
	skos:definition "Credit that is issued or accepted for certificates."@en-US ;
	dct:description "Includes credits earned while enrolled in a certificate program."@en-US ;
	vs:term_status vs:stable ;
	meta:changeHistory <http://credreg.net/ctdl/termhistory/creditUnit/CertificateCredit/json> ;
	skos:broader creditUnit:TypeBasedCredit .

creditUnit:ClockHour a skos:Concept ;
	skos:prefLabel "Clock Hour"@en-US ;
	skos:definition "Credit that is issued or accepted as being related to one or more temporal hours."@en-US ;
	vs:term_status vs:stable ;
	meta:changeHistory <http://credreg.net/ctdl/termhistory/creditUnit/ClockHour/json> ;
	skos:broader creditUnit:TimeBasedCredit .

creditUnit:CompetencyCredit a skos:Concept ;
	skos:prefLabel "Competency Credit"@en-US ;
	skos:definition "Credit that is issued or accepted for a particular competency or set of competencies."@en-US ;
	vs:term_status vs:stable ;
	meta:changeHistory <http://credreg.net/ctdl/termhistory/creditUnit/CompetencyCredit/json> ;
	skos:broader creditUnit:TypeBasedCredit .

creditUnit:ContactHour a skos:Concept ;
	skos:prefLabel "Contact Hour"@en-US ;
	skos:definition "Credit that is issued or accepted as being related to one or more temporal hours of instruction presented to students."@en-US ;
	vs:term_status vs:stable ;
	meta:changeHistory <http://credreg.net/ctdl/termhistory/creditUnit/ContactHour/json> ;
	skos:broader creditUnit:TimeBasedCredit .

creditUnit:ContinuingEducationUnit a skos:Concept ;
	skos:prefLabel "Continuing Education Unit"@en-US ;
	skos:definition "Credit that is issued or is accepted as education units for meeting professional development requirements."@en-US ;
	dct:description "Based on international standards, continuing education units are based on contact hours that may be converted to other units of measurement, such as professional development hours (PDH), continuing education credits (CEU), and continuing professional credits (CPC)."@en-US ;
	vs:term_status vs:stable ;
	meta:changeHistory <http://credreg.net/ctdl/termhistory/creditUnit/ContinuingEducationUnit/json> ;
	skos:broader creditUnit:TypeBasedCredit .

creditUnit:DegreeCredit a skos:Concept ;
	skos:prefLabel "Degree Credit"@en-US ;
	skos:definition "Credit that is issued or is accepted as credit for earning a college-level degree."@en-US ;
	dct:description "Includes credits earned while enrolled in a postsecondary program for a college-level degree."@en-US ;
	vs:term_status vs:stable ;
	meta:changeHistory <http://credreg.net/ctdl/termhistory/creditUnit/DegreeCredit/json> ;
	skos:broader creditUnit:TypeBasedCredit .

creditUnit:DualCredit a skos:Concept ;
	skos:prefLabel "Dual Credit"@en-US ;
	skos:definition "Credit that is applicable to two different educational levels."@en-US ;
	vs:term_status vs:stable ;
	meta:changeHistory <http://credreg.net/ctdl/termhistory/creditUnit/DualCredit/json> ;
	skos:broader creditUnit:TypeBasedCredit .

creditUnit:QuarterHour a skos:Concept ;
	skos:prefLabel "Quarter Hour"@en-US ;
	skos:definition "Credit that is issued or accepted at an academic quarter level."@en-US ;
	vs:term_status vs:stable ;
	meta:changeHistory <http://credreg.net/ctdl/termhistory/creditUnit/QuarterHour/json> ;
	skos:broader creditUnit:TimeBasedCredit .

creditUnit:RequirementCredit a skos:Concept ;
	skos:prefLabel "Requirement Credit"@en-US ;
	skos:definition "Credit that is issued or accepted for some type of requirement."@en-US ;
	vs:term_status vs:stable ;
	meta:changeHistory <http://credreg.net/ctdl/termhistory/creditUnit/RequirementCredit/json> ;
	skos:broader creditUnit:TypeBasedCredit .

creditUnit:SecondaryDiplomaCredit a skos:Concept ;
	skos:prefLabel "Secondary Diploma Credit"@en-US ;
	skos:definition "Credit that is issued or accepted for a secondary diploma."@en-US ;
	dct:description "Includes credits earned while enrolled in a secondary diploma program that meet graduation requirements."@en-US ;
	vs:term_status vs:stable ;
	meta:changeHistory <http://credreg.net/ctdl/termhistory/creditUnit/SecondaryDiplomaCredit/json> ;
	skos:broader creditUnit:TypeBasedCredit .

creditUnit:SemesterHour a skos:Concept ;
	skos:prefLabel "Semester Hour"@en-US ;
	skos:definition "Credit that is issued or accepted at a semester level."@en-US ;
	vs:term_status vs:stable ;
	meta:changeHistory <http://credreg.net/ctdl/termhistory/creditUnit/SemesterHour/json> ;
	skos:broader creditUnit:TimeBasedCredit .

creditUnit:TimeBasedCredit a skos:Concept ;
	skos:prefLabel "Time-Based Credit"@en-US ;
	skos:definition "Credit with a unit of measurement based on time, either figuratively or literally."@en-US ;
	vs:term_status vs:stable ;
	meta:changeHistory <http://credreg.net/ctdl/termhistory/creditUnit/TimeBasedCredit/json> ;
	skos:narrower creditUnit:AcademicYear, creditUnit:CarnegieUnit, creditUnit:ClockHour, creditUnit:ContactHour, creditUnit:QuarterHour, creditUnit:SemesterHour .

creditUnit:TypeBasedCredit a skos:Concept ;
	skos:prefLabel "Type-Based Credit"@en-US ;
	skos:definition "Credit with a unit of measurement based on the type of credit."@en-US ;
	vs:term_status vs:stable ;
	meta:changeHistory <http://credreg.net/ctdl/termhistory/creditUnit/TypeBasedCredit/json> ;
	skos:narrower creditUnit:CertificateCredit, creditUnit:CompetencyCredit, creditUnit:ContinuingEducationUnit, creditUnit:DegreeCredit, creditUnit:DualCredit, creditUnit:RequirementCredit, creditUnit:SecondaryDiplomaCredit .

deliveryType:BlendedDelivery a skos:Concept ;
	skos:prefLabel "Blended Delivery"@en-US ;
	skos:definition "Delivery includes significant levels of both in person and online."@en-US ;
	vs:term_status vs:stable ;
	meta:changeHistory <http://credreg.net/ctdl/termhistory/deliveryType/BlendedDelivery/json> .

deliveryType:InPerson a skos:Concept ;
	skos:prefLabel "In-Person Only"@en-US ;
	skos:definition "Delivery is only face-to-face."@en-US ;
	vs:term_status vs:stable ;
	meta:changeHistory <http://credreg.net/ctdl/termhistory/deliveryType/InPerson/json> .

deliveryType:OnlineOnly a skos:Concept ;
	skos:prefLabel "Online Only"@en-US ;
	skos:definition "Delivery is only via the Internet."@en-US ;
	vs:term_status vs:stable ;
	meta:changeHistory <http://credreg.net/ctdl/termhistory/deliveryType/OnlineOnly/json> .

financialAid:AcademicAssistantship a skos:Concept ;
	skos:prefLabel "Academic Assistantship"@en-US ;
	skos:definition "Paid employment in which students receive tuition or other reimbursement for the tasks they perform for faculty members, departments, and/or educational institutions."@en-US ;
	vs:term_status vs:stable ;
	meta:changeHistory <http://credreg.net/ctdl/termhistory/financialAid/AcademicAssistantship/json> ;
	skos:broader financialAid:WorkBased ;
	owl:equivalentClass <https://ceds.ed.gov/element/000113#Assistantships> .

financialAid:Apprenticeship a skos:Concept ;
	skos:prefLabel "Apprenticeship"@en-US ;
	skos:definition "Combination of on-the-job training and related instruction that meets standards in which workers learn the practical and theoretical aspects of a skilled occupation."@en-US ;
	vs:term_status vs:stable ;
	meta:changeHistory <http://credreg.net/ctdl/termhistory/financialAid/Apprenticeship/json> ;
	skos:broader financialAid:WorkBased .

financialAid:CoOperative a skos:Concept ;
	skos:prefLabel "Co-Operative"@en-US ;
	skos:definition "Paid work experience utilized by approved career and technical education programs to combine classroom and on-the-job training and education which provides academic credit for structured job experience."@en-US ;
	vs:term_status vs:stable ;
	meta:changeHistory <http://credreg.net/ctdl/termhistory/financialAid/CoOperative/json> ;
	skos:broader financialAid:WorkBased .

financialAid:DoDTuitionAssistance a skos:Concept ;
	skos:prefLabel "Department of Defense Tuition Assistance"@en-US ;
	skos:definition "Financial assistance provided to qualified active duty service members and their families for voluntary off-duty educational programs in support of professional and personal self-development goals."@en-US ;
	vs:term_status vs:stable ;
	meta:changeHistory <http://credreg.net/ctdl/termhistory/financialAid/DoDTuitionAssistance/json> ;
	skos:broader financialAid:Military ;
	owl:equivalentClass <https://ceds.ed.gov/element/001610#DODTuitionAssistance> .

financialAid:FederalGrant a skos:Concept ;
	skos:prefLabel "Federal Grant"@en-US ;
	skos:definition "Financial subsidy, which doesnât require repayment, based on meeting requirements determined by the Federal Government."@en-US ;
	vs:term_status vs:stable ;
	meta:changeHistory <http://credreg.net/ctdl/termhistory/financialAid/FederalGrant/json> ;
	skos:broader financialAid:Grant ;
	owl:equivalentClass <https://ceds.ed.gov/element/000113#OtherFederalGrants> .

financialAid:FederalScholarship a skos:Concept ;
	skos:prefLabel "Federal Scholarship"@en-US ;
	skos:definition "Financial aid award, which doesnât require repayment, from the Federal Government based on student achievement and other criteria for education."@en-US ;
	vs:term_status vs:stable ;
	meta:changeHistory <http://credreg.net/ctdl/termhistory/financialAid/FederalScholarship/json> ;
	skos:broader financialAid:Scholarship ;
	owl:equivalentClass <https://ceds.ed.gov/element/000113#FederalScholarships> .

financialAid:FederalSubsidizedLoan a skos:Concept ;
	skos:prefLabel "Federal Subsidized Loan"@en-US ;
	skos:definition "Loan from the Federal Government that is based on financial needs of the student and is intended to offset costs related to education, living, and resources."@en-US ;
	vs:term_status vs:stable ;
	meta:changeHistory <http://credreg.net/ctdl/termhistory/financialAid/FederalSubsidizedLoan/json> ;
	skos:broader financialAid:Loan ;
	owl:equivalentClass <https://ceds.ed.gov/element/000113#FederalSubsidizedLoans> .

financialAid:FederalUnsubsidizedLoan a skos:Concept ;
	skos:prefLabel "Federal Unsubsidized Loan"@en-US ;
	skos:definition "Loan from the Federal Government that does not require evidence of the financial needs of the student, and is intended to offset costs related to education, living, and resources."@en-US ;
	vs:term_status vs:stable ;
	meta:changeHistory <http://credreg.net/ctdl/termhistory/financialAid/FederalUnsubsidizedLoan/json> ;
	skos:broader financialAid:Loan ;
	owl:equivalentClass <https://ceds.ed.gov/element/000113#FederalUnsubsidizedLoans> .

financialAid:FederalWorkStudy a skos:Concept ;
	skos:prefLabel "Federal Work Study"@en-US ;
	skos:definition "Program funded by the Federal Government designed to provide part-time jobs for students to offset educational expenses."@en-US ;
	vs:term_status vs:stable ;
	meta:changeHistory <http://credreg.net/ctdl/termhistory/financialAid/FederalWorkStudy/json> ;
	skos:broader financialAid:WorkBased ;
	owl:equivalentClass <https://ceds.ed.gov/element/000113#FederalWorkStudy> .

financialAid:General a skos:Concept ;
	skos:prefLabel "General Financial Assistance"@en-US ;
	skos:definition "Types of financial assistance for students towards education, training, or related costs of pursuing a credential, program, or other resource."@en-US ;
	vs:term_status vs:stable ;
	meta:changeHistory <http://credreg.net/ctdl/termhistory/financialAid/General/json> ;
	owl:equivalentClass ceds:000113 ;
	skos:narrower financialAid:Grant, financialAid:Loan, financialAid:Scholarship, financialAid:WorkBased .

financialAid:Grant a skos:Concept ;
	skos:prefLabel "Grant"@en-US ;
	skos:definition "Financial subsidy, which doesnât require repayment, based on meeting requirements determined by the grantor."@en-US ;
	vs:term_status vs:stable ;
	meta:changeHistory <http://credreg.net/ctdl/termhistory/financialAid/Grant/json> ;
	skos:broader financialAid:General ;
	skos:narrower financialAid:FederalGrant, financialAid:InstitutionalGrant, financialAid:LoanForgivenessProgram, financialAid:OtherGrant, financialAid:PellGrant, financialAid:PrivateGrant, financialAid:PromiseProgram, financialAid:StateLocalGrant, financialAid:WIOA .

financialAid:InstitutionalGrant a skos:Concept ;
	skos:prefLabel "Institutional Grant"@en-US ;
	skos:definition "Financial subsidy, including free or discounted tuition or other fees, which doesnât require repayment, based on meeting requirements determined by an educational institution."@en-US ;
	vs:term_status vs:stable ;
	meta:changeHistory <http://credreg.net/ctdl/termhistory/financialAid/InstitutionalGrant/json> ;
	skos:broader financialAid:Grant ;
	owl:equivalentClass <https://ceds.ed.gov/element/000113#InstitutionalGrants> .

financialAid:InstitutionalLoan a skos:Concept ;
	skos:prefLabel "Institutional Loan"@en-US ;
	skos:definition "Loan from an educational institution that is intended to offset costs related to education, living, and resources."@en-US ;
	vs:term_status vs:stable ;
	meta:changeHistory <http://credreg.net/ctdl/termhistory/financialAid/InstitutionalLoan/json> ;
	skos:broader financialAid:Loan ;
	owl:equivalentClass <https://ceds.ed.gov/element/000113#InstitutionalLoans> .

financialAid:InstitutionalScholarship a skos:Concept ;
	skos:prefLabel "Institutional Scholarship"@en-US ;
	skos:definition "Financial aid award, which doesnât require repayment, from an educational institution based on student achievement and other criteria for education."@en-US ;
	vs:term_status vs:stable ;
	meta:changeHistory <http://credreg.net/ctdl/termhistory/financialAid/InstitutionalScholarship/json> ;
	skos:broader financialAid:Scholarship ;
	owl:equivalentClass <https://ceds.ed.gov/element/000113#InstitutionalScholarships> .

financialAid:Internship a skos:Concept ;
	skos:prefLabel "Internship"@en-US ;
	skos:definition "Time-limited work offered by an organization approved by a qualified institution to gain experience or satisfy requirements for another resource."@en-US ;
	vs:term_status vs:stable ;
	meta:changeHistory <http://credreg.net/ctdl/termhistory/financialAid/Internship/json> ;
	skos:broader financialAid:WorkBased .

financialAid:Loan a skos:Concept ;
	skos:prefLabel "Loan"@en-US ;
	skos:definition "Financial aid that requires repayment with terms determined by the entity providing the loan."@en-US ;
	vs:term_status vs:stable ;
	meta:changeHistory <http://credreg.net/ctdl/termhistory/financialAid/Loan/json> ;
	skos:broader financialAid:General ;
	skos:narrower financialAid:FederalSubsidizedLoan, financialAid:FederalUnsubsidizedLoan, financialAid:InstitutionalLoan, financialAid:OtherLoan, financialAid:ParentPLUSLoan, financialAid:PrivateLoan, financialAid:StateLocalLoan .

financialAid:LoanForgivenessProgram a skos:Concept ;
	skos:prefLabel "Loan Forgiveness Program"@en-US ;
	skos:definition "Program that forgives the remaining balance on a loan after meeting certain requirements."@en-US ;
	vs:term_status vs:stable ;
	meta:changeHistory <http://credreg.net/ctdl/termhistory/financialAid/LoanForgivenessProgram/json> ;
	skos:broader financialAid:Grant .

financialAid:Military a skos:Concept ;
	skos:prefLabel "Military"@en-US ;
	skos:definition "Financial aid available to active duty service members, veterans, and/or their qualified family members."@en-US ;
	vs:term_status vs:stable ;
	meta:changeHistory <http://credreg.net/ctdl/termhistory/financialAid/Military/json> ;
	owl:equivalentClass ceds:001610 ;
	skos:narrower financialAid:DoDTuitionAssistance, financialAid:Post911GIBill, financialAid:StateLocalMilitaryAssistance, financialAid:VEAP, financialAid:VocationalRehabilitation .

financialAid:OtherGrant a skos:Concept ;
	skos:prefLabel "Other Grant"@en-US ;
	skos:definition "Financial subsidy based on meeting requirements from one or more other sources."@en-US ;
	vs:term_status vs:stable ;
	meta:changeHistory <http://credreg.net/ctdl/termhistory/financialAid/OtherGrant/json> ;
	skos:broader financialAid:Grant ;
	owl:equivalentClass <https://ceds.ed.gov/element/000113#OtherGrants> .

financialAid:OtherLoan a skos:Concept ;
	skos:prefLabel "Other Loan"@en-US ;
	skos:definition "Loan from one or more other sources that is intended to offset costs related to education, living, and resources."@en-US ;
	vs:term_status vs:stable ;
	meta:changeHistory <http://credreg.net/ctdl/termhistory/financialAid/OtherLoan/json> ;
	skos:broader financialAid:Loan ;
	owl:equivalentClass <https://ceds.ed.gov/element/000113#OtherLoans> .

financialAid:OtherOnCampusWork a skos:Concept ;
	skos:prefLabel "Other On-Campus Work"@en-US ;
	skos:definition "Paid non-academic employment available for students on an educational institutionâs campus."@en-US ;
	vs:term_status vs:stable ;
	meta:changeHistory <http://credreg.net/ctdl/termhistory/financialAid/OtherOnCampusWork/json> ;
	skos:broader financialAid:WorkBased ;
	owl:equivalentClass <https://ceds.ed.gov/element/000113#OtherOnCampusWork> .

financialAid:OtherScholarship a skos:Concept ;
	skos:prefLabel "Other Scholarship"@en-US ;
	skos:definition "Financial aid award, which doesnât require repayment, from one or more other sources based on student achievement and other criteria."@en-US ;
	vs:term_status vs:stable ;
	meta:changeHistory <http://credreg.net/ctdl/termhistory/financialAid/OtherScholarship/json> ;
	skos:broader financialAid:Scholarship ;
	owl:equivalentClass <https://ceds.ed.gov/element/000113#OtherScholarships> .

financialAid:ParentPLUSLoan a skos:Concept ;
	skos:prefLabel "Parent PLUS Loan"@en-US ;
	skos:definition "Loan from the Federal Government available to the parents of dependent students."@en-US ;
	vs:term_status vs:stable ;
	meta:changeHistory <http://credreg.net/ctdl/termhistory/financialAid/ParentPLUSLoan/json> ;
	skos:broader financialAid:Loan ;
	owl:equivalentClass <https://ceds.ed.gov/element/000113#ParentPLUSLoans> .

financialAid:PellGrant a skos:Concept ;
	skos:prefLabel "Pell Grant"@en-US ;
	skos:definition "Financial subsidy, which doesnât require repayment, that the Federal Government provides based on the financial needs of the student."@en-US ;
	vs:term_status vs:stable ;
	meta:changeHistory <http://credreg.net/ctdl/termhistory/financialAid/PellGrant/json> ;
	skos:broader financialAid:Grant ;
	owl:equivalentClass <https://ceds.ed.gov/element/000113#PellGrants> .

financialAid:Post911GIBill a skos:Concept ;
	skos:prefLabel "Post 9-11 GI Bill"@en-US ;
	skos:definition "Financial assistance provided to qualified active duty service members, veterans, and qualified family members that is based on military service and intended to offset costs related to education, living, and resources."@en-US ;
	vs:term_status vs:stable ;
	meta:changeHistory <http://credreg.net/ctdl/termhistory/financialAid/Post911GIBill/json> ;
	skos:broader financialAid:Military ;
	owl:equivalentClass <https://ceds.ed.gov/element/001610#Post911GIBill> .

financialAid:PrivateGrant a skos:Concept ;
	skos:prefLabel "Private Grant"@en-US ;
	skos:definition "Financial subsidy, which doesnât require repayment, based on meeting requirements determined by a private entity, including employers."@en-US ;
	vs:term_status vs:stable ;
	meta:changeHistory <http://credreg.net/ctdl/termhistory/financialAid/PrivateGrant/json> ;
	skos:broader financialAid:Grant ;
	owl:equivalentClass <https://ceds.ed.gov/element/000113#PrivateGrants> .

financialAid:PrivateLoan a skos:Concept ;
	skos:prefLabel "Private Loan"@en-US ;
	skos:definition "Loan from a private entity, including employers, that is intended to offset costs related to education, living, and resources."@en-US ;
	vs:term_status vs:stable ;
	meta:changeHistory <http://credreg.net/ctdl/termhistory/financialAid/PrivateLoan/json> ;
	skos:broader financialAid:Loan ;
	owl:equivalentClass <https://ceds.ed.gov/element/000113#PrivateLoans> .

financialAid:PrivateScholarship a skos:Concept ;
	skos:prefLabel "Private Scholarship"@en-US ;
	skos:definition "Financial aid award, which doesnât require repayment, from a private entity, including employers, based on student achievement and other criteria for education."@en-US ;
	vs:term_status vs:stable ;
	meta:changeHistory <http://credreg.net/ctdl/termhistory/financialAid/PrivateScholarship/json> ;
	skos:broader financialAid:Scholarship ;
	owl:equivalentClass <https://ceds.ed.gov/element/000113#PrivateScholarships> .

financialAid:PromiseProgram a skos:Concept ;
	skos:prefLabel "Promise Program"@en-US ;
	skos:definition "Program for students in a given area, with minimal requirements, that pays for tuition without requiring repayment."@en-US ;
	vs:term_status vs:stable ;
	meta:changeHistory <http://credreg.net/ctdl/termhistory/financialAid/PromiseProgram/json> ;
	skos:broader financialAid:Grant .

financialAid:Scholarship a skos:Concept ;
	skos:prefLabel "Scholarship"@en-US ;
	skos:definition "Financial aid award based on student achievement and other criteria for education that doesnât require repayment."@en-US ;
	vs:term_status vs:stable ;
	meta:changeHistory <http://credreg.net/ctdl/termhistory/financialAid/Scholarship/json> ;
	skos:broader financialAid:General ;
	skos:narrower financialAid:FederalScholarship, financialAid:InstitutionalScholarship, financialAid:OtherScholarship, financialAid:PrivateScholarship, financialAid:StateLocalScholarship .

financialAid:StateLocalGrant a skos:Concept ;
	skos:prefLabel "State or Local Grant"@en-US ;
	skos:definition "Financial subsidy, which doesnât require repayment, based on meeting requirements determined by a state, province, region, and/or local government."@en-US ;
	vs:term_status vs:stable ;
	meta:changeHistory <http://credreg.net/ctdl/termhistory/financialAid/StateLocalGrant/json> ;
	skos:broader financialAid:Grant ;
	owl:equivalentClass <https://ceds.ed.gov/element/000113#StateAndLocalGrants> .

financialAid:StateLocalLoan a skos:Concept ;
	skos:prefLabel "State or Local Loan"@en-US ;
	skos:definition "Loan from a state, province, region, and/or local government that is intended to offset costs related to education, living, and resources."@en-US ;
	vs:term_status vs:stable ;
	meta:changeHistory <http://credreg.net/ctdl/termhistory/financialAid/StateLocalLoan/json> ;
	skos:broader financialAid:Loan ;
	owl:equivalentClass <https://ceds.ed.gov/element/000113#StateLoans> .

financialAid:StateLocalMilitaryAssistance a skos:Concept ;
	skos:prefLabel "State or Local Military Assistance"@en-US ;
	skos:definition "Financial aid provided by a state or local government to active duty service members, veterans, and/or qualified family members."@en-US ;
	vs:term_status vs:stable ;
	meta:changeHistory <http://credreg.net/ctdl/termhistory/financialAid/StateLocalMilitaryAssistance/json> ;
	skos:broader financialAid:Military .

financialAid:StateLocalScholarship a skos:Concept ;
	skos:prefLabel "State or Local Scholarship"@en-US ;
	skos:definition "Financial aid award, which doesnât require repayment, from a state, province, region, and/or local government based on student achievement and other criteria for education."@en-US ;
	vs:term_status vs:stable ;
	meta:changeHistory <http://credreg.net/ctdl/termhistory/financialAid/StateLocalScholarship/json> ;
	skos:broader financialAid:Scholarship ;
	owl:equivalentClass <https://ceds.ed.gov/element/000113#StateAndLocalScholarships> .

financialAid:StateLocalWork a skos:Concept ;
	skos:prefLabel "State or Local Work"@en-US ;
	skos:definition "Program funded by a state, province, region, and/or local government designed to provide work for students to offset educational expenses."@en-US ;
	vs:term_status vs:stable ;
	meta:changeHistory <http://credreg.net/ctdl/termhistory/financialAid/StateLocalWork/json> ;
	skos:broader financialAid:WorkBased ;
	owl:equivalentClass <https://ceds.ed.gov/element/000113#StateWork> .

financialAid:VEAP a skos:Concept ;
	skos:prefLabel "Veteran Educational Assistance Program"@en-US ;
	skos:definition "Financial assistance provided to qualified active duty service members and veterans as a matching program that is intended to offset educational expenses."@en-US ;
	vs:term_status vs:stable ;
	meta:changeHistory <http://credreg.net/ctdl/termhistory/financialAid/VEAP/json> ;
	skos:broader financialAid:Military .

financialAid:VocationalRehabilitation a skos:Concept ;
	skos:prefLabel "Vocational Rehabilitation"@en-US ;
	skos:definition "Financial for veterans with a qualifying service-connected disability rating for training or education related to pursuit of a career or career-related resource."@en-US ;
	vs:term_status vs:stable ;
	meta:changeHistory <http://credreg.net/ctdl/termhistory/financialAid/VocationalRehabilitation/json> ;
	skos:broader financialAid:Military .

financialAid:WIOA a skos:Concept ;
	skos:prefLabel "Workforce Investment Opportunity Act (WIOA)"@en-US ;
	skos:definition "Financial aid established on behalf of a qualified participant with a training provider that is on the state's Eligible Training Provider List (ETPL)."@en-US ;
	vs:term_status vs:stable ;
	meta:changeHistory <http://credreg.net/ctdl/termhistory/financialAid/WIOA/json> ;
	skos:broader financialAid:Grant .

financialAid:WorkBased a skos:Concept ;
	skos:prefLabel "Work-Based"@en-US ;
	skos:definition "Financial compensation for participating in work-based learning opportunities."@en-US ;
	vs:term_status vs:stable ;
	meta:changeHistory <http://credreg.net/ctdl/termhistory/financialAid/WorkBased/json> ;
	skos:broader financialAid:General ;
	skos:narrower financialAid:AcademicAssistantship, financialAid:Apprenticeship, financialAid:CoOperative, financialAid:FederalWorkStudy, financialAid:Internship, financialAid:OtherOnCampusWork, financialAid:StateLocalWork .

inputType:Associations a skos:Concept ;
	skos:prefLabel "Professional Associations"@en-US ;
	skos:definition "External stakeholder review, guidance or recommendations by professional associations."@en-US ;
	vs:term_status vs:stable ;
	meta:changeHistory <http://credreg.net/ctdl/termhistory/inputType/Associations/json> .

inputType:Business a skos:Concept ;
	skos:prefLabel "Business"@en-US ;
	skos:definition "External stakeholder review, guidance or recommendations by business."@en-US ;
	vs:term_status vs:stable ;
	meta:changeHistory <http://credreg.net/ctdl/termhistory/inputType/Business/json> .

inputType:BusinessAssociation a skos:Concept ;
	skos:prefLabel "Business or Industry Association"@en-US ;
	skos:definition "External stakeholder review, guidance or recommendations by business or industry association."@en-US ;
	vs:term_status vs:stable ;
	meta:changeHistory <http://credreg.net/ctdl/termhistory/inputType/BusinessAssociation/json> .

inputType:Consumers a skos:Concept ;
	skos:prefLabel "Consumers"@en-US ;
	skos:definition "External stakeholder review, guidance or recommendations by consumers."@en-US ;
	vs:term_status vs:stable ;
	meta:changeHistory <http://credreg.net/ctdl/termhistory/inputType/Consumers/json> .

inputType:EducationAdministrators a skos:Concept ;
	skos:prefLabel "Education Administrators"@en-US ;
	skos:definition "External stakeholder review, guidance or recommendations by education administrators."@en-US ;
	vs:term_status vs:stable ;
	meta:changeHistory <http://credreg.net/ctdl/termhistory/inputType/EducationAdministrators/json> .

inputType:Educators a skos:Concept ;
	skos:prefLabel "Educators"@en-US ;
	skos:definition "External stakeholder review, guidance or recommendations by education instructors or faculty."@en-US ;
	vs:term_status vs:stable ;
	meta:changeHistory <http://credreg.net/ctdl/termhistory/inputType/Educators/json> .

inputType:Experts a skos:Concept ;
	skos:prefLabel "Subject Matter Experts"@en-US ;
	skos:definition "External stakeholder review, guidance or recommendations by subject matter experts."@en-US ;
	vs:term_status vs:stable ;
	meta:changeHistory <http://credreg.net/ctdl/termhistory/inputType/Experts/json> .

inputType:Governments a skos:Concept ;
	skos:prefLabel "Governments"@en-US ;
	skos:definition "External stakeholder review, guidance or recommendations by government."@en-US ;
	dct:description "May include local, state or provincial, and federal or national government."@en-US ;
	vs:term_status vs:stable ;
	meta:changeHistory <http://credreg.net/ctdl/termhistory/inputType/Governments/json> .

inputType:Guardians a skos:Concept ;
	skos:prefLabel "Guardians"@en-US ;
	skos:definition "External stakeholder review, guidance or recommendations by parents or guardians."@en-US ;
	vs:term_status vs:stable ;
	meta:changeHistory <http://credreg.net/ctdl/termhistory/inputType/Guardians/json> .

inputType:InternationalBodies a skos:Concept ;
	skos:prefLabel "International Bodies"@en-US ;
	skos:definition "External stakeholder review, guidance or recommendations by international bodies."@en-US ;
	vs:term_status vs:stable ;
	meta:changeHistory <http://credreg.net/ctdl/termhistory/inputType/InternationalBodies/json> .

inputType:Practitioners a skos:Concept ;
	skos:prefLabel "Practitioners"@en-US ;
	skos:definition "External stakeholder review, guidance or recommendations by practitioners."@en-US ;
	vs:term_status vs:stable ;
	meta:changeHistory <http://credreg.net/ctdl/termhistory/inputType/Practitioners/json> .

inputType:Public a skos:Concept ;
	skos:prefLabel "Public"@en-US ;
	skos:definition "External stakeholder review, guidance or recommendations by community members and the general public."@en-US ;
	vs:term_status vs:stable ;
	meta:changeHistory <http://credreg.net/ctdl/termhistory/inputType/Public/json> .

inputType:Students a skos:Concept ;
	skos:prefLabel "Students"@en-US ;
	skos:definition "External stakeholder review, guidance or recommendations by all types of learners."@en-US ;
	vs:term_status vs:stable ;
	meta:changeHistory <http://credreg.net/ctdl/termhistory/inputType/Students/json> .

learnMethod:Applied a skos:Concept ;
	skos:prefLabel "Applied Instruction"@en-US ;
	skos:definition "Provides learning opportunities in the context of real world examples, cases, and applications."@en-US ;
	dct:description "Applies to methods such as contextual learning, applied academics, academic-technical integration, problem-based learning, project-based learning, and case methods."@en-US ;
	vs:term_status vs:stable ;
	meta:changeHistory <http://credreg.net/ctdl/termhistory/learnMethod/Applied/json> .

learnMethod:Gaming a skos:Concept ;
	skos:prefLabel "Gaming"@en-US ;
	skos:definition "Provides interactive educational experiences which demonstrate concepts in a way that promotes critical thinking, overcoming challenges within prescribed rule sets, problem solving, and in some cases, teamwork and/or competition."@en-US ;
	dct:description "Individual or group games that have cognitive, social, behavioral, and/or emotional dimensions which are related to educational objectives."@en-US ;
	vs:term_status vs:stable ;
	meta:changeHistory <http://credreg.net/ctdl/termhistory/learnMethod/Gaming/json> .

learnMethod:Laboratory a skos:Concept ;
	skos:prefLabel "Laboratory"@en-US ;
	skos:definition "Hands-on individual or group experiences for applied learning concepts and methods, procedures and protocols with equipment and technologies."@en-US ;
	dct:description "Applies to clinical practice and methods such as physical and/or virtual simulation or participation, whether direct or indirect."@en-US ;
	vs:term_status vs:stable ;
	meta:changeHistory <http://credreg.net/ctdl/termhistory/learnMethod/Laboratory/json> .

learnMethod:Lecture a skos:Concept ;
	skos:prefLabel "Lecture"@en-US ;
	skos:definition "Primary method is presentation by an instructor of learning material and may include student discussion."@en-US ;
	dct:description "Lecture courses may involve student questions and answers, but the role of the instructor is clearly differentiated from that of the students."@en-US ;
	vs:term_status vs:stable ;
	meta:changeHistory <http://credreg.net/ctdl/termhistory/learnMethod/Lecture/json> .

learnMethod:Prerecorded a skos:Concept ;
	skos:prefLabel "Prerecorded"@en-US ;
	skos:definition "Learning by using video, audio, or other prerecorded content."@en-US ;
	vs:term_status vs:stable ;
	meta:changeHistory <http://credreg.net/ctdl/termhistory/learnMethod/Prerecorded/json> .

learnMethod:SelfPaced a skos:Concept ;
	skos:prefLabel "Self Paced"@en-US ;
	skos:definition "Provides for personalization and flexibility in the timing and progression of learning for individual learners based on their preferences and needs, prior learning experiences, and ability to progress through learning opportunities."@en-US ;
	dct:description "Applies to methods such as competency-based education, open-entry/open exit, independent study, private study, and correspondence."@en-US ;
	vs:term_status vs:stable ;
	meta:changeHistory <http://credreg.net/ctdl/termhistory/learnMethod/SelfPaced/json> .

learnMethod:Seminar a skos:Concept ;
	skos:prefLabel "Seminar"@en-US ;
	skos:definition "Primary method is active student discussion leading to advancement of the topic and facilitated by an instructor."@en-US ;
	dct:description "Seminars typically involve small groups to facilitate equal opportunity with the instructor and colleagues to be engaged and occasionally may include students leading discussions."@en-US ;
	vs:term_status vs:stable ;
	meta:changeHistory <http://credreg.net/ctdl/termhistory/learnMethod/Seminar/json> .

learnMethod:WorkBased a skos:Concept ;
	skos:prefLabel "Work Based"@en-US ;
	skos:definition "Provides real-world work experiences that may be paid or unpaid and provided in group or individual formats normally outside the classroom."@en-US ;
	dct:description "Applies to methods such as apprenticeships, internships, externships, work study, clinical rotations, residencies, practicums, field study, team projects, and cooperative education."@en-US ;
	vs:term_status vs:stable ;
	meta:changeHistory <http://credreg.net/ctdl/termhistory/learnMethod/WorkBased/json> .

lifeCycle:Active a skos:Concept ;
	skos:prefLabel "Active"@en-US ;
	skos:definition "Resource is active, current, ongoing, offered, operational, or available."@en-US ;
	vs:term_status vs:unstable ;
	meta:changeHistory <http://credreg.net/ctdl/termhistory/lifeCycle/Active/json> .

lifeCycle:Ceased a skos:Concept ;
	skos:prefLabel "Ceased"@en-US ;
	skos:definition "Resource is permanently no longer active, current, ongoing, offered, operational, or available."@en-US ;
	vs:term_status vs:unstable ;
	meta:changeHistory <http://credreg.net/ctdl/termhistory/lifeCycle/Ceased/json> .

lifeCycle:Ceasing a skos:Concept ;
	skos:prefLabel "Ceasing"@en-US ;
	skos:definition "Resource is no longer active, current, ongoing, offered, operational, or available, except for participants who are already engaged with it."@en-US ;
	vs:term_status vs:unstable ;
	meta:changeHistory <http://credreg.net/ctdl/termhistory/lifeCycle/Ceasing/json> ;
	skos:narrower lifeCycle:TeachOut .

lifeCycle:Developing a skos:Concept ;
	skos:prefLabel "Developing"@en-US ;
	skos:definition "Resource is under development and may or may not become active, current, ongoing, offered, operational, or available."@en-US ;
	vs:term_status vs:unstable ;
	meta:changeHistory <http://credreg.net/ctdl/termhistory/lifeCycle/Developing/json> .

lifeCycle:Suspended a skos:Concept ;
	skos:prefLabel "Suspended"@en-US ;
	skos:definition "Resource is temporarily not active, current, ongoing, offered, operational, or available."@en-US ;
	vs:term_status vs:unstable ;
	meta:changeHistory <http://credreg.net/ctdl/termhistory/lifeCycle/Suspended/json> .

lifeCycle:TeachOut a skos:Concept ;
	skos:prefLabel "Teach Out"@en-US ;
	skos:definition "Arrangement by which an educational institution provides its current students with the opportunity to complete their course of study when the program, institution or location offering access closes."@en-US ;
	vs:term_status vs:unstable ;
	meta:changeHistory <http://credreg.net/ctdl/termhistory/lifeCycle/TeachOut/json> ;
	skos:broader lifeCycle:Ceasing .

logic:And a skos:Concept ;
	skos:prefLabel "And"@en-US ;
	skos:definition "Relation is satisfied when all of the conditions and constraints are satisfied."@en-US ;
	vann:usageNote "When used in a Component Condition, this applies to the combination of all immediately subordinate Component Conditions and Constraints."@en-US ;
	vs:term_status vs:unstable ;
	meta:changeHistory <http://credreg.net/ctdl/termhistory/logic/And/json> ;
	owl:equivalentClass odrl2:and .

logic:OnlyOne a skos:Concept ;
	skos:prefLabel "Only One"@en-US ;
	skos:definition "Relation is satisfied when exactly one, and not more, of the conditions or constraints is satisfied."@en-US ;
	vann:usageNote "When used in a Component Condition, this applies to the combination of all immediately subordinate Component Conditions and Constraints."@en-US ;
	vs:term_status vs:unstable ;
	meta:changeHistory <http://credreg.net/ctdl/termhistory/logic/OnlyOne/json> ;
	owl:equivalentClass odrl2:xone .

logic:Or a skos:Concept ;
	skos:prefLabel "Or"@en-US ;
	skos:definition "Relation is satisfied when at least one of the conditions or constraints is satisfied."@en-US ;
	vann:usageNote "When used in a Component Condition, this applies to the combination of all immediately subordinate Component Conditions and Constraints."@en-US ;
	vs:term_status vs:unstable ;
	meta:changeHistory <http://credreg.net/ctdl/termhistory/logic/Or/json> ;
	owl:equivalentClass odrl2:or .

orgType:AssessmentBody a skos:Concept ;
	skos:prefLabel "Assessment Body"@en-US ;
	skos:definition "Primarily offers assessments for credentials as a service."@en-US ;
	vs:term_status vs:stable ;
	meta:changeHistory <http://credreg.net/ctdl/termhistory/orgType/AssessmentBody/json> .

orgType:Business a skos:Concept ;
	skos:prefLabel "Business"@en-US ;
	skos:definition "Organization that primarily sells products or services and employs one or more individuals."@en-US ;
	vs:term_status vs:stable ;
	meta:changeHistory <http://credreg.net/ctdl/termhistory/orgType/Business/json> .

orgType:BusinessAssociation a skos:Concept ;
	skos:prefLabel "Business or Industry Association"@en-US ;
	skos:definition "Membership organization primarily engaged in promoting the interests of their business members and providing them with services that may involve the provision of education and credentialing services."@en-US ;
	vs:term_status vs:stable ;
	meta:changeHistory <http://credreg.net/ctdl/termhistory/orgType/BusinessAssociation/json> .

orgType:CertificationBody a skos:Concept ;
	skos:prefLabel "Certification Body"@en-US ;
	skos:definition "Independent, third-party organization that operates a certification program. A certification body may or may not be governmental, and may or may not have regulatory authority."@en-US ;
	vs:term_status vs:stable ;
	meta:changeHistory <http://credreg.net/ctdl/termhistory/orgType/CertificationBody/json> .

orgType:Collaborative a skos:Concept ;
	skos:prefLabel "Collaborative"@en-US ;
	skos:definition "Organized group of entities in the public, private, government sectors that collaborates to achieve a common set of goals."@en-US ;
	vs:term_status vs:stable ;
	meta:changeHistory <http://credreg.net/ctdl/termhistory/orgType/Collaborative/json> .

orgType:CoordinatingBody a skos:Concept ;
	skos:prefLabel "Coordinating Body"@en-US ;
	skos:definition "An organization that organizes multiple stakeholders around a common goal."@en-US ;
	vs:term_status vs:stable ;
	meta:changeHistory <http://credreg.net/ctdl/termhistory/orgType/CoordinatingBody/json> .

orgType:FourYear a skos:Concept ;
	skos:prefLabel "Four-Year College"@en-US ;
	skos:definition "Authorized postsecondary institution that primarily offers bachelor or higher degrees, but may also award associate degrees."@en-US ;
	dct:description "Includes free-standing medical, law or other first-professional schools, schools that offer postbaccalaureate certificates only, those that offer graduate programs only, etc."@en-US ;
	vs:term_status vs:stable ;
	meta:changeHistory <http://credreg.net/ctdl/termhistory/orgType/FourYear/json> ;
	skos:broader orgType:Postsecondary .

orgType:Government a skos:Concept ;
	skos:prefLabel "Government Agency"@en-US ;
	skos:definition "Organization in the public sector at the federal, state or local levels."@en-US ;
	dct:description "Includes quasi-governmental organizations, special districts (e.g., libraries), corrections organizations, etc., except college and school districts. Is also responsible for the oversight and administration of specific functions other than the military services."@en-US ;
	vs:term_status vs:stable ;
	meta:changeHistory <http://credreg.net/ctdl/termhistory/orgType/Government/json> .

orgType:HighSchool a skos:Concept ;
	skos:prefLabel "High School"@en-US ;
	skos:definition "Secondary school providing instruction and educational services that do not focus primarily on career and technical education or alternative education."@en-US ;
	vs:term_status vs:stable ;
	meta:changeHistory <http://credreg.net/ctdl/termhistory/orgType/HighSchool/json> ;
	skos:broader orgType:SecondarySchool .

orgType:LaborUnion a skos:Concept ;
	skos:prefLabel "Labor Union"@en-US ;
	skos:definition "Membership organization of workers formed for the purpose of advancing its members' interests in respect to wages, benefits, and working conditions."@en-US ;
	vs:term_status vs:stable ;
	meta:changeHistory <http://credreg.net/ctdl/termhistory/orgType/LaborUnion/json> .

orgType:Magnet a skos:Concept ;
	skos:prefLabel "Magnet/Competitive Admissions School"@en-US ;
	skos:definition "Public school offering special instruction and programs not available elsewhere, designed to attract a more diverse student body from throughout a school district."@en-US ;
	vs:term_status vs:stable ;
	meta:changeHistory <http://credreg.net/ctdl/termhistory/orgType/Magnet/json> ;
	skos:broader orgType:SecondarySchool .

orgType:Military a skos:Concept ;
	skos:prefLabel "Military"@en-US ;
	skos:definition "Armed services of a government entity."@en-US ;
	vs:term_status vs:stable ;
	meta:changeHistory <http://credreg.net/ctdl/termhistory/orgType/Military/json> .

orgType:NonTraditional a skos:Concept ;
	skos:prefLabel "Alternative/Non-Traditional School"@en-US ;
	skos:definition "Secondary (i.e., high school) that: 1) addresses needs of students which cannot typically be met in a regular school; 2) provides nontraditional education; 3) falls outside of the categories of regular, magnet/special program emphasis, or career and technical education."@en-US ;
	vs:term_status vs:stable ;
	meta:changeHistory <http://credreg.net/ctdl/termhistory/orgType/NonTraditional/json> ;
	skos:broader orgType:SecondarySchool .

orgType:Postsecondary a skos:Concept ;
	skos:prefLabel "Postsecondary Educational Institution"@en-US ;
	skos:definition "Organization such as a college or university."@en-US ;
	dct:description "Organization with the authority to award degrees, and whose primary purpose is to provide postsecondary (tertiary or non-tertiary) education including programs whose purpose is providing academic, vocational, and continuing professional education."@en-US ;
	vs:term_status vs:stable ;
	meta:changeHistory <http://credreg.net/ctdl/termhistory/orgType/Postsecondary/json> ;
	skos:narrower orgType:FourYear, orgType:TwoYear .

orgType:PrimarilyOnline a skos:Concept ;
	skos:prefLabel "Primarily Online"@en-US ;
	skos:definition "Organization that primarily operates online."@en-US ;
	vs:term_status vs:stable ;
	meta:changeHistory <http://credreg.net/ctdl/termhistory/orgType/PrimarilyOnline/json> .

orgType:ProfessionalAssociation a skos:Concept ;
	skos:prefLabel "Professional Association"@en-US ;
	skos:definition "Membership organization primarily engaged in promoting the interests of a particular profession, the interests of individuals engaged in that profession, and providing them with services that may involve the provision of education and credentialing services."@en-US ;
	vs:term_status vs:stable ;
	meta:changeHistory <http://credreg.net/ctdl/termhistory/orgType/ProfessionalAssociation/json> .

orgType:QualityAssurance a skos:Concept ;
	skos:prefLabel "Quality Assurance Body"@en-US ;
	skos:definition "External body that performs accreditation, endorsement, approval, and/or recognition of a credential issuer."@en-US ;
	vs:term_status vs:stable ;
	meta:changeHistory <http://credreg.net/ctdl/termhistory/orgType/QualityAssurance/json> .

orgType:SecondarySchool a skos:Concept ;
	skos:prefLabel "Secondary School"@en-US ;
	skos:definition "Secondary school primarily providing education to students at the ninth grade or higher."@en-US ;
	vs:term_status vs:stable ;
	meta:changeHistory <http://credreg.net/ctdl/termhistory/orgType/SecondarySchool/json> ;
	skos:narrower orgType:HighSchool, orgType:Magnet, orgType:NonTraditional, orgType:Technical .

orgType:Technical a skos:Concept ;
	skos:prefLabel "Career and Technical School"@en-US ;
	skos:definition "Secondary school that focuses primarily on providing formal preparation for skilled, technical or professional occupations or careers."@en-US ;
	vs:term_status vs:stable ;
	meta:changeHistory <http://credreg.net/ctdl/termhistory/orgType/Technical/json> ;
	skos:broader orgType:SecondarySchool .

orgType:TrainingProvider a skos:Concept ;
	skos:prefLabel "Education and Training Provider"@en-US ;
	skos:definition "Organization whose major purpose is to provide education and training services but is not a postsecondary education institution with the authority to award degrees."@en-US ;
	dct:description "Includes community-based organizations, non-degree granting proprietary schools which are education and training providers that are recognized by states as schools."@en-US ;
	vann:usageNote "In the U.S., use for Title IV eligible organizations that do not award degrees."@en-US ;
	vs:term_status vs:stable ;
	meta:changeHistory <http://credreg.net/ctdl/termhistory/orgType/TrainingProvider/json> .

orgType:TwoYear a skos:Concept ;
	skos:prefLabel "Two-Year College"@en-US ;
	skos:definition "Authorized postsecondary institution that primarily offers associate degrees and certificates, and, if authorized, may also award higher degrees."@en-US ;
	dct:description "Includes occupational and vocational schools with programs of at least 1800 hours, academic institutions with programs of less than 4 years, etc."@en-US ;
	vs:term_status vs:stable ;
	meta:changeHistory <http://credreg.net/ctdl/termhistory/orgType/TwoYear/json> ;
	skos:broader orgType:Postsecondary .

orgType:Vendor a skos:Concept ;
	skos:prefLabel "Vendor"@en-US ;
	skos:definition "Sells, maintains, and issues credentials for its own products and services for public access and use."@en-US ;
	vs:term_status vs:stable ;
	meta:changeHistory <http://credreg.net/ctdl/termhistory/orgType/Vendor/json> .

residency:InState a skos:Concept ;
	skos:prefLabel "In-State"@en-US ;
	skos:definition "Legal residency or domicile status of the agent is the state or province of the relevant activity."@en-US ;
	vs:term_status vs:stable ;
	meta:changeHistory <http://credreg.net/ctdl/termhistory/residency/InState/json> .

residency:International a skos:Concept ;
	skos:prefLabel "Foreign/International"@en-US ;
	skos:definition "Legal residency, domicile, or citizen status of the agent is as a foreign national."@en-US ;
	vs:term_status vs:stable ;
	meta:changeHistory <http://credreg.net/ctdl/termhistory/residency/International/json> .

residency:Local a skos:Concept ;
	skos:prefLabel "Local"@en-US ;
	skos:definition "Legal residency or domicile status of the agent is local."@en-US ;
	vs:term_status vs:stable ;
	meta:changeHistory <http://credreg.net/ctdl/termhistory/residency/Local/json> .

residency:OutOfState a skos:Concept ;
	skos:prefLabel "Out-of-State"@en-US ;
	skos:definition "Legal residency or domicile status of the agent is a state or province different from the state or provincial locus of the relevant activity."@en-US ;
	vs:term_status vs:stable ;
	meta:changeHistory <http://credreg.net/ctdl/termhistory/residency/OutOfState/json> .

residency:Regional a skos:Concept ;
	skos:prefLabel "Regional"@en-US ;
	skos:definition "Legal residency or domicile status of the agent is the same geographic or political region as that of the relevant activity."@en-US ;
	vs:term_status vs:stable ;
	meta:changeHistory <http://credreg.net/ctdl/termhistory/residency/Regional/json> .

scheduleFrequency:Annually a skos:Concept ;
	skos:prefLabel "Annually"@en-US ;
	skos:definition "Schedule is on an annual basis, typically occurring once per year."@en-US ;
	vs:term_status vs:unstable ;
	meta:changeHistory <http://credreg.net/ctdl/termhistory/scheduleFrequency/Annually/json> .

scheduleFrequency:BiMonthly a skos:Concept ;
	skos:prefLabel "Bi-Monthly"@en-US ;
	skos:definition "Schedule is on a bi-monthly basis, typically occurring every other month."@en-US ;
	vs:term_status vs:unstable ;
	meta:changeHistory <http://credreg.net/ctdl/termhistory/scheduleFrequency/BiMonthly/json> .

scheduleFrequency:EventBased a skos:Concept ;
	skos:prefLabel "Event-Based"@en-US ;
	skos:definition "Schedule is determined or triggered by other events, such as completion of activities, completion of the resource, events external to the resource, or other events; refer to the resource's information for details."@en-US ;
	vs:term_status vs:unstable ;
	meta:changeHistory <http://credreg.net/ctdl/termhistory/scheduleFrequency/EventBased/json> .

scheduleFrequency:Irregular a skos:Concept ;
	skos:prefLabel "Irregular"@en-US ;
	skos:definition "Schedule has no significant pattern."@en-US ;
	vs:term_status vs:unstable ;
	meta:changeHistory <http://credreg.net/ctdl/termhistory/scheduleFrequency/Irregular/json> .

scheduleFrequency:Monthly a skos:Concept ;
	skos:prefLabel "Monthly"@en-US ;
	skos:definition "Schedule is on a monthly basis, typically occurring once per month."@en-US ;
	vs:term_status vs:unstable ;
	meta:changeHistory <http://credreg.net/ctdl/termhistory/scheduleFrequency/Monthly/json> .

scheduleFrequency:MultiplePerWeek a skos:Concept ;
	skos:prefLabel "Multiple Per Week"@en-US ;
	skos:definition "Schedule is more frequent than a weekly basis."@en-US ;
	vs:term_status vs:unstable ;
	meta:changeHistory <http://credreg.net/ctdl/termhistory/scheduleFrequency/MultiplePerWeek/json> .

scheduleFrequency:OnDemand a skos:Concept ;
	skos:prefLabel "On-Demand"@en-US ;
	skos:definition "Schedule allows the participant to choose when the resource begins."@en-US ;
	vs:term_status vs:unstable ;
	meta:changeHistory <http://credreg.net/ctdl/termhistory/scheduleFrequency/OnDemand/json> .

scheduleFrequency:OpenEntryExit a skos:Concept ;
	skos:prefLabel "Open Entry/Exit"@en-US ;
	skos:definition "Schedule allows for the participant to enter, participate with, and complete the resource during any period of the resource's run time."@en-US ;
	vs:term_status vs:unstable ;
	meta:changeHistory <http://credreg.net/ctdl/termhistory/scheduleFrequency/OpenEntryExit/json> .

scheduleFrequency:Quarterly a skos:Concept ;
	skos:prefLabel "Quarterly"@en-US ;
	skos:definition "Schedule is on an quarterly basis, typically occurring three or four times per year."@en-US ;
	vs:term_status vs:unstable ;
	meta:changeHistory <http://credreg.net/ctdl/termhistory/scheduleFrequency/Quarterly/json> .

scheduleFrequency:SelfPaced a skos:Concept ;
	skos:prefLabel "Self-Paced"@en-US ;
	skos:definition "Schedule allows for participation at a self-determined pace, though some specific dates and deadlines may be involved."@en-US ;
	vs:term_status vs:unstable ;
	meta:changeHistory <http://credreg.net/ctdl/termhistory/scheduleFrequency/SelfPaced/json> .

scheduleFrequency:SemiAnnually a skos:Concept ;
	skos:prefLabel "Semi-Annually"@en-US ;
	skos:definition "Schedule is on an semi-annual basis, typically occurring twice per year."@en-US ;
	vs:term_status vs:unstable ;
	meta:changeHistory <http://credreg.net/ctdl/termhistory/scheduleFrequency/SemiAnnually/json> .

scheduleFrequency:SingleInstance a skos:Concept ;
	skos:prefLabel "Single Instance"@en-US ;
	skos:definition "Schedule is a single instance of this event."@en-US ;
	vs:term_status vs:unstable ;
	meta:changeHistory <http://credreg.net/ctdl/termhistory/scheduleFrequency/SingleInstance/json> .

scheduleFrequency:Weekly a skos:Concept ;
	skos:prefLabel "Weekly"@en-US ;
	skos:definition "Schedule is on a weekly basis, typically occurring once per week."@en-US ;
	vs:term_status vs:unstable ;
	meta:changeHistory <http://credreg.net/ctdl/termhistory/scheduleFrequency/Weekly/json> .

scheduleTiming:Daytime a skos:Concept ;
	skos:prefLabel "Daytime"@en-US ;
	skos:definition "Schedule is typically during daytime hours."@en-US ;
	vs:term_status vs:unstable ;
	meta:changeHistory <http://credreg.net/ctdl/termhistory/scheduleTiming/Daytime/json> .

scheduleTiming:Evening a skos:Concept ;
	skos:prefLabel "Evening"@en-US ;
	skos:definition "Schedule is typically during evening hours."@en-US ;
	vs:term_status vs:unstable ;
	meta:changeHistory <http://credreg.net/ctdl/termhistory/scheduleTiming/Evening/json> .

scheduleTiming:Weekdays a skos:Concept ;
	skos:prefLabel "Weekdays"@en-US ;
	skos:definition "Schedule is Monday through Friday, consecutively or non-consecutively."@en-US ;
	vs:term_status vs:unstable ;
	meta:changeHistory <http://credreg.net/ctdl/termhistory/scheduleTiming/Weekdays/json> .

scheduleTiming:Weekends a skos:Concept ;
	skos:prefLabel "Weekends"@en-US ;
	skos:definition "Schedule is on a weekly basis, Saturday and/or Sunday."@en-US ;
	vs:term_status vs:unstable ;
	meta:changeHistory <http://credreg.net/ctdl/termhistory/scheduleTiming/Weekends/json> .

score:CriterionReferenced a skos:Concept ;
	skos:prefLabel "Criterion-Referenced"@en-US ;
	skos:definition "Scored based on a comparison to defined criteria and levels of performance."@en-US ;
	vs:term_status vs:stable ;
	meta:changeHistory <http://credreg.net/ctdl/termhistory/score/CriterionReferenced/json> .

score:NormReferenced a skos:Concept ;
	skos:prefLabel "Norm-Referenced"@en-US ;
	skos:definition "Scored based on a comparison to a distribution of performance in a reference population."@en-US ;
	vs:term_status vs:stable ;
	meta:changeHistory <http://credreg.net/ctdl/termhistory/score/NormReferenced/json> .

serviceType:AccreditService a skos:Concept ;
	skos:prefLabel "Accredit Service"@en-US ;
	skos:definition "Agent service provides official authorization to, or approval of, a credential, organization or program based on prescribed standards or criteria."@en-US ;
	vs:term_status vs:stable ;
	meta:changeHistory <http://credreg.net/ctdl/termhistory/serviceType/AccreditService/json> .

serviceType:ApproveService a skos:Concept ;
	skos:prefLabel "Approve Service"@en-US ;
	skos:definition "Agent service official accepts a credential or authorizes an organization to act or operate."@en-US ;
	vs:term_status vs:stable ;
	meta:changeHistory <http://credreg.net/ctdl/termhistory/serviceType/ApproveService/json> .

serviceType:OfferService a skos:Concept ;
	skos:prefLabel "Offer Service"@en-US ;
	skos:definition "Agent service offers resources such as credentials, assessments, or learning opportunities."@en-US ;
	vs:term_status vs:stable ;
	meta:changeHistory <http://credreg.net/ctdl/termhistory/serviceType/OfferService/json> .

serviceType:RecognizeService a skos:Concept ;
	skos:prefLabel "Recognize Service"@en-US ;
	skos:definition "Agent service recommends, endorses, indicates preference for, or otherwise provides a positive judgment."@en-US ;
	vs:term_status vs:stable ;
	meta:changeHistory <http://credreg.net/ctdl/termhistory/serviceType/RecognizeService/json> .

serviceType:RegulateService a skos:Concept ;
	skos:prefLabel "Regulate Service"@en-US ;
	skos:definition "Agent service monitors and enforces legal requirements or standards."@en-US ;
	vs:term_status vs:stable ;
	meta:changeHistory <http://credreg.net/ctdl/termhistory/serviceType/RegulateService/json> .

serviceType:RenewService a skos:Concept ;
	skos:prefLabel "Renew Service"@en-US ;
	skos:definition "Agent provides service to extend (renew) the validity of a credential."@en-US ;
	vs:term_status vs:stable ;
	meta:changeHistory <http://credreg.net/ctdl/termhistory/serviceType/RenewService/json> .

serviceType:RevokeService a skos:Concept ;
	skos:prefLabel "Revoke Service"@en-US ;
	skos:definition "Agent provides service to end (revoke) the validity or operation of an awarded credential."@en-US ;
	vs:term_status vs:stable ;
	meta:changeHistory <http://credreg.net/ctdl/termhistory/serviceType/RevokeService/json> .

